# baseURI: https://unifiedcyberontology.org/ontology/uco/pattern
# imports: https://unifiedcyberontology.org/ontology/uco/core

@base <https://unifiedcyberontology.org/ontology/uco/pattern> .
@prefix action: <https://unifiedcyberontology.org/ontology/uco/action#> .
@prefix core: <https://unifiedcyberontology.org/ontology/uco/core#> .
@prefix identity: <https://unifiedcyberontology.org/ontology/uco/identity#> .
@prefix location: <https://unifiedcyberontology.org/ontology/uco/location#> .
@prefix marking: <https://unifiedcyberontology.org/ontology/uco/marking#> .
@prefix owl: <http://www.w3.org/2002/07/owl#> .
@prefix pattern: <https://unifiedcyberontology.org/ontology/uco/pattern#> .
@prefix rdf: <http://www.w3.org/1999/02/22-rdf-syntax-ns#> .
@prefix rdfs: <http://www.w3.org/2000/01/rdf-schema#> .
@prefix role: <https://unifiedcyberontology.org/ontology/uco/role#> .
@prefix sh: <http://www.w3.org/ns/shacl#> .
@prefix types: <https://unifiedcyberontology.org/ontology/uco/types#> .
@prefix xml: <http://www.w3.org/XML/1998/namespace> .
@prefix xsd: <http://www.w3.org/2001/XMLSchema#> .

<https://unifiedcyberontology.org/ontology/uco/pattern>
	a owl:Ontology ;
	rdfs:label "uco-pattern"@en ;
	owl:imports <https://unifiedcyberontology.org/ontology/uco/core> ;
	.

pattern:LogicalPattern
	a
		owl:Class ,
		sh:NodeShape
		;
	rdfs:subClassOf pattern:Pattern ;
	rdfs:label "LogicalPattern"@en ;
	rdfs:comment "A logical pattern is a grouping of characteristics unique to an informational pattern expressed via a structured pattern expression following the rules of logic."@en ;
	sh:property
		[
			sh:class core:ExternalReference ;
			sh:minCount "0"^^xsd:integer ;
			sh:path core:externalReference ;
		] ,
		[
			sh:class core:IdentityAbstraction ;
			sh:maxCount "1"^^xsd:integer ;
			sh:path core:createdBy ;
		] ,
		[
			sh:datatype xsd:dateTime ;
			sh:maxCount "1"^^xsd:integer ;
			sh:path core:objectCreatedTime ;
		] ,
		[
			sh:datatype xsd:string ;
			sh:maxCount "1"^^xsd:integer ;
			sh:path core:name ;
		] ,
		[
			sh:datatype xsd:string ;
			sh:maxCount "1"^^xsd:integer ;
			sh:path core:specVersion ;
		] ,
		[
			sh:datatype pattern:PatternExpression ;
			sh:maxCount "1"^^xsd:integer ;
			sh:path pattern:patternExpression ;
		] ,
		[
			sh:datatype types:Identifier ;
			sh:maxCount "1"^^xsd:integer ;
			sh:path core:id ;
		] ,
		[
			sh:path core:description ;
		] ,
		[
			sh:path core:hasFacet ;
		] ,
		[
			sh:path core:modifiedTime ;
		] ,
		[
			sh:path core:objectMarking ;
		] ,
		[
			sh:path core:tag ;
		] ,
		[
			sh:path core:type ;
		]
		;
	sh:targetClass pattern:LogicalPattern ;
	.

pattern:Pattern
	a
		owl:Class ,
		sh:NodeShape
		;
	rdfs:subClassOf core:UcoObject ;
	rdfs:label "Pattern"@en ;
	rdfs:comment "A pattern is a combination of properties, acts, tendencies, etc., forming a consistent or characteristic arrangement."@en ;
	sh:property
		[
			sh:class core:ExternalReference ;
			sh:minCount "0"^^xsd:integer ;
			sh:path core:externalReference ;
		] ,
		[
			sh:class core:IdentityAbstraction ;
			sh:maxCount "1"^^xsd:integer ;
			sh:path core:createdBy ;
		] ,
		[
			sh:datatype xsd:dateTime ;
			sh:maxCount "1"^^xsd:integer ;
			sh:path core:objectCreatedTime ;
		] ,
		[
			sh:datatype xsd:string ;
			sh:maxCount "1"^^xsd:integer ;
			sh:path core:name ;
		] ,
		[
			sh:datatype xsd:string ;
			sh:maxCount "1"^^xsd:integer ;
			sh:path core:specVersion ;
		] ,
		[
			sh:datatype types:Identifier ;
			sh:maxCount "1"^^xsd:integer ;
			sh:path core:id ;
		] ,
		[
			sh:path core:description ;
		] ,
		[
			sh:path core:hasFacet ;
		] ,
		[
			sh:path core:modifiedTime ;
		] ,
		[
			sh:path core:objectMarking ;
		] ,
		[
			sh:path core:tag ;
		] ,
		[
			sh:path core:type ;
		]
		;
	sh:targetClass pattern:Pattern ;
	.

pattern:PatternExpression
	a
		owl:Class ,
		sh:NodeShape
		;
	rdfs:label "PatternExpression"@en ;
	rdfs:comment "A pattern expression is a grouping of characteristics unique to an explicit logical expression defining a pattern (e.g., regular expression, SQL Select expression, etc.)."@en ;
	sh:targetClass pattern:PatternExpression ;
	.

pattern:patternExpression
	a owl:DatatypeProperty ;
	rdfs:label "patternExpression"@en ;
	rdfs:comment "An explicit logical pattern expression."@en ;
	rdfs:range pattern:PatternExpression ;
	.

