# imports: https://ontology.unifiedcyberontology.org/co/1.3.0
# imports: https://ontology.unifiedcyberontology.org/uco/core/1.3.0
# imports: https://ontology.unifiedcyberontology.org/uco/vocabulary/1.3.0

@prefix co: <http://purl.org/co/> .
@prefix core: <https://ontology.unifiedcyberontology.org/uco/core/> .
@prefix owl: <http://www.w3.org/2002/07/owl#> .
@prefix rdf: <http://www.w3.org/1999/02/22-rdf-syntax-ns#> .
@prefix rdfs: <http://www.w3.org/2000/01/rdf-schema#> .
@prefix sh: <http://www.w3.org/ns/shacl#> .
@prefix types: <https://ontology.unifiedcyberontology.org/uco/types/> .
@prefix uco-co: <https://ontology.unifiedcyberontology.org/co/> .
@prefix vocabulary: <https://ontology.unifiedcyberontology.org/uco/vocabulary/> .
@prefix xsd: <http://www.w3.org/2001/XMLSchema#> .

<https://ontology.unifiedcyberontology.org/uco/types>
	a owl:Ontology ;
	rdfs:label "uco-types"@en ;
	owl:backwardCompatibleWith types:1.2.0 ;
	owl:imports
		uco-co:1.3.0 ,
		core:1.3.0 ,
		vocabulary:1.3.0
		;
	owl:priorVersion types:1.2.0 ;
	owl:versionIRI types:1.3.0 ;
	.

types:ControlledDictionary
	a
		owl:Class ,
		sh:NodeShape
		;
	rdfs:subClassOf types:Dictionary ;
	rdfs:label "ControlledDictionary"@en ;
	rdfs:comment "A controlled dictionary is a list of (term/key, value) pairs where each term/key exists no more than once and is constrained to an explicitly defined set of values."@en ;
	sh:property [
		sh:class types:ControlledDictionaryEntry ;
		sh:path types:entry ;
	] ;
	sh:targetClass types:ControlledDictionary ;
	.

types:ControlledDictionaryEntry
	a
		owl:Class ,
		sh:NodeShape
		;
	rdfs:subClassOf types:DictionaryEntry ;
	rdfs:label "ControlledDictionaryEntry"@en ;
	rdfs:comment "A controlled dictionary entry is a single (term/key, value) pair where the term/key is constrained to an explicitly defined set of values."@en ;
	sh:targetClass types:ControlledDictionaryEntry ;
	.

types:Dictionary
	a
		owl:Class ,
		sh:NodeShape
		;
	rdfs:subClassOf core:UcoInherentCharacterizationThing ;
	rdfs:label "Dictionary"@en ;
	rdfs:comment "A dictionary is list of (term/key, value) pairs with each term/key having an expectation to exist no more than once.  types:Dictionary alone does not validate this expectation, but validation is available.  For use cases where this expectation must be validated, the subclass types:ProperDictionary should be used instead of types:Dictionary.  For instances where this expectation has been found to be violated, the subclass types:ImproperDictionary should be used instead of types:Dictionary."@en ;
	sh:property [
		sh:class types:DictionaryEntry ;
		sh:nodeKind sh:IRI ;
		sh:path types:entry ;
	] ;
	sh:targetClass types:Dictionary ;
	.

types:Dictionary-keyUniqueness-shape
	a sh:NodeShape ;
	sh:description "This shape is separated from the types:Dictionary class-shape in order to associate a warning-severity SPARQL-based shape."@en ;
	sh:severity sh:Warning ;
	sh:sparql [
		a sh:SPARQLConstraint ;
		sh:message "A key in a dictionary should appear no more than once.  The value literal does.  Please consider using the types:ImproperDictionary class and types:repeatsKey property."@en ;
		sh:select """
			PREFIX types: <https://ontology.unifiedcyberontology.org/uco/types/>
			SELECT $this ?value
			WHERE {
				$this
					types:entry/types:key ?value ;
					.
				FILTER NOT EXISTS {
					$this
						a types:ImproperDictionary ;
						.
				}
				FILTER NOT EXISTS {
					$this
						a types:ProperDictionary ;
						.
				}
			}
			GROUP BY ?value
			HAVING (COUNT(?value) > 1)
			""" ;
	] ;
	sh:targetClass types:Dictionary ;
	.

types:DictionaryEntry
	a
		owl:Class ,
		sh:NodeShape
		;
	rdfs:subClassOf core:UcoInherentCharacterizationThing ;
	rdfs:label "DictionaryEntry"@en ;
	rdfs:comment "A dictionary entry is a single (term/key, value) pair."@en ;
	sh:property
		[
			sh:datatype xsd:string ;
			sh:maxCount "1"^^xsd:integer ;
			sh:minCount "1"^^xsd:integer ;
			sh:nodeKind sh:Literal ;
			sh:path types:key ;
		] ,
		[
			sh:datatype xsd:string ;
			sh:maxCount "1"^^xsd:integer ;
			sh:minCount "1"^^xsd:integer ;
			sh:nodeKind sh:Literal ;
			sh:path types:value ;
		]
		;
	sh:targetClass types:DictionaryEntry ;
	.

types:Hash
	a
		owl:Class ,
		sh:NodeShape
		;
	rdfs:subClassOf core:UcoInherentCharacterizationThing ;
	rdfs:label "Hash"@en ;
	rdfs:comment "A hash is a grouping of characteristics unique to the result of applying a mathematical algorithm that maps data of arbitrary size to a bit string (the 'hash') and is a one-way function, that is, a function which is practically infeasible to invert. This is commonly used for integrity checking of data. [based on https://en.wikipedia.org/wiki/Cryptographic_hash_function]"@en ;
	sh:property
		[
			sh:datatype xsd:hexBinary ;
			sh:maxCount "1"^^xsd:integer ;
			sh:minCount "1"^^xsd:integer ;
			sh:nodeKind sh:Literal ;
			sh:path types:hashValue ;
		] ,
		[
			sh:datatype vocabulary:HashNameVocab ;
			sh:message "Value is outside the default vocabulary HashNameVocab." ;
			sh:path types:hashMethod ;
			sh:severity sh:Info ;
		] ,
		[
			sh:maxCount "1"^^xsd:integer ;
			sh:minCount "1"^^xsd:integer ;
			sh:nodeKind sh:Literal ;
			sh:or (
				[
					sh:datatype vocabulary:HashNameVocab ;
				]
				[
					sh:datatype xsd:string ;
				]
			) ;
			sh:path types:hashMethod ;
		] ,
		[
			sh:message "Value is not member of the vocabulary HashNameVocab." ;
			sh:or (
				[
					sh:datatype vocabulary:HashNameVocab ;
					sh:in (
						"MD5"^^vocabulary:HashNameVocab
						"MD6"^^vocabulary:HashNameVocab
						"SHA1"^^vocabulary:HashNameVocab
						"SHA224"^^vocabulary:HashNameVocab
						"SHA256"^^vocabulary:HashNameVocab
						"SHA3-224"^^vocabulary:HashNameVocab
						"SHA3-256"^^vocabulary:HashNameVocab
						"SHA3-384"^^vocabulary:HashNameVocab
						"SHA3-512"^^vocabulary:HashNameVocab
						"SHA384"^^vocabulary:HashNameVocab
						"SHA512"^^vocabulary:HashNameVocab
						"SSDEEP"^^vocabulary:HashNameVocab
					) ;
				]
				[
					sh:datatype xsd:string ;
				]
			) ;
			sh:path types:hashMethod ;
		]
		;
	sh:targetClass types:Hash ;
	.

types:Identifier
	a rdfs:Datatype ;
	rdfs:comment "An identifier is a string conformant to the specified UUID-based format for UCO object identifiers."@en ;
	.

types:ImproperDictionary
	a
		owl:Class ,
		sh:NodeShape
		;
	rdfs:subClassOf types:Dictionary ;
	rdfs:label "ImproperDictionary"@en ;
	owl:disjointWith types:ProperDictionary ;
	sh:property [
		sh:datatype xsd:string ;
		sh:nodeKind sh:Literal ;
		sh:path types:repeatsKey ;
	] ;
	sh:targetClass types:ImproperDictionary ;
	.

types:ImproperDictionary-disjointWith-ProperDictionary-shape
	a sh:NodeShape ;
	sh:message "types:ImproperDictionary and types:ProperDictionary are disjoint classes."@en ;
	sh:not [
		a sh:NodeShape ;
		sh:class types:ProperDictionary ;
	] ;
	sh:targetClass types:ImproperDictionary ;
	.

types:NativeFormatString
	a rdfs:Datatype ;
	rdfs:comment "Specifies data in its native format of some external language. The data may be encoded in Base64 per [RFC4648]. Data encoded in Base64 must be denoted as such using the encoded property."@en ;
	.

types:ProperDictionary
	a
		owl:Class ,
		sh:NodeShape
		;
	rdfs:subClassOf types:Dictionary ;
	rdfs:label "ProperDictionary"@en ;
	rdfs:comment "A proper dictionary is list of (term/key, value) pairs with each term/key existing no more than once."@en ;
	owl:disjointWith types:ImproperDictionary ;
	sh:sparql [
		a sh:SPARQLConstraint ;
		sh:message "A key in a proper dictionary can appear no more than once."@en ;
		sh:select """
			PREFIX types: <https://ontology.unifiedcyberontology.org/uco/types/>
			SELECT $this ?value
			WHERE {
				$this
					types:entry/types:key ?value ;
					.
			}
			GROUP BY ?value
			HAVING (COUNT(?value) > 1)
		""" ;
	] ;
	sh:targetClass types:ProperDictionary ;
	.

types:StructuredText
	a rdfs:Datatype ;
	rdfs:comment "Expresses string-based data in some information structuring format (e.g., HTML5)."@en ;
	.

types:Thread
	a
		owl:Class ,
		sh:NodeShape
		;
	rdfs:subClassOf
		co:Bag ,
		core:UcoInherentCharacterizationThing
		;
	rdfs:label "Thread"@en ;
	rdfs:comment "A semi-ordered array of items, that can be present in multiple copies.  Implemetation of a UCO Thread is similar to a Collections Ontology List, except a Thread may fork and merge - that is, one of its members may have two or more direct successors, and two or more direct predecessors."@en ;
	owl:disjointWith co:List ;
	sh:property [
		sh:class types:ThreadItem ;
		sh:path co:item ;
	] ;
	.

types:Thread-disjointWith-co-List-shape
	a sh:NodeShape ;
	sh:message "types:Thread and co:List are disjoint classes."@en ;
	sh:not [
		a sh:NodeShape ;
		sh:class co:List ;
	] ;
	sh:targetClass types:Thread ;
	.

types:ThreadItem
	a
		owl:Class ,
		sh:NodeShape
		;
	rdfs:subClassOf
		co:Item ,
		core:UcoInherentCharacterizationThing
		;
	rdfs:label "ThreadItem"@en ;
	rdfs:comment "A ThreadItem is a member of a thread."@en ;
	owl:disjointWith co:ListItem ;
	sh:property [
		sh:class core:UcoObject ;
		sh:path co:itemContent ;
	] ;
	.

types:ThreadItem-disjointWith-co-ListItem-shape
	a sh:NodeShape ;
	sh:message "types:ThreadItem and co:ListItem are disjoint classes."@en ;
	sh:not [
		a sh:NodeShape ;
		sh:class co:ListItem ;
	] ;
	sh:targetClass types:ThreadItem ;
	.

types:entry
	a owl:ObjectProperty ;
	rdfs:label "entry"@en ;
	rdfs:comment "A dictionary entry."@en ;
	rdfs:range types:DictionaryEntry ;
	.

types:hashMethod
	a owl:DatatypeProperty ;
	rdfs:label "hashMethod"@en ;
	rdfs:comment "A particular cryptographic hashing method (e.g., MD5)."@en ;
	rdfs:range [
		a rdfs:Datatype ;
		owl:unionOf (
			vocabulary:HashNameVocab
			xsd:string
		) ;
	] ;
	.

types:hashValue
	a owl:DatatypeProperty ;
	rdfs:label "hashValue"@en ;
	rdfs:comment "A cryptographic hash value."@en ;
	rdfs:range xsd:hexBinary ;
	.

types:key
	a owl:DatatypeProperty ;
	rdfs:label "key"@en ;
	rdfs:comment "A key property of a single dictionary entry."@en ;
	rdfs:range xsd:string ;
	.

types:repeatsKey
	a owl:DatatypeProperty ;
	rdfs:label "repeatsKey"@en ;
	rdfs:comment "A key found to be repeated in multiple dictionary entries within one dictionary."@en ;
	rdfs:domain types:ImproperDictionary ;
	rdfs:range xsd:string ;
	.

types:repeatsKey-subjects-shape
	a sh:NodeShape ;
	sh:class types:ImproperDictionary ;
	sh:targetSubjectsOf types:repeatsKey ;
	.

types:threadNextItem
	a owl:ObjectProperty ;
	rdfs:subPropertyOf types:threadSuccessor ;
	rdfs:label "threadNextItem"@en ;
	rdfs:comment "The link to a next item in a thread."@en ;
	rdfs:seeAlso co:nextItem ;
	.

types:threadNextItem-subjects-shape
	a sh:PropertyShape ;
	sh:class types:ThreadItem ;
	sh:nodeKind sh:IRI ;
	sh:path types:threadNextItem ;
	sh:targetSubjectsOf types:threadNextItem ;
	.

types:threadOriginItem
	a owl:ObjectProperty ;
	rdfs:subPropertyOf co:item ;
	rdfs:label "threadOriginItem"@en ;
	rdfs:comment "A link to an item of the thread known to have no predecessor."@en ;
	rdfs:domain types:Thread ;
	rdfs:range [
		a owl:Class ;
		owl:intersectionOf (
			types:ThreadItem
			[
				a owl:Restriction ;
				owl:onProperty types:threadPreviousItem ;
				owl:cardinality "0"^^xsd:nonNegativeInteger ;
			]
		) ;
	] ;
	rdfs:seeAlso co:firstItem ;
	.

types:threadOriginItem-subjects-shape
	a sh:PropertyShape ;
	sh:class types:ThreadItem ;
	sh:nodeKind sh:IRI ;
	sh:path types:threadOriginItem ;
	sh:targetSubjectsOf types:threadOriginItem ;
	.

types:threadOriginItem-subjects-threadPredecessor-shape
	a sh:PropertyShape ;
	sh:description "An origin item in a thread must not have a predecessor."@en ;
	sh:maxCount "0"^^xsd:integer ;
	sh:nodeKind sh:IRI ;
	sh:path (
		types:threadOriginItem
		types:threadPredecessor
	) ;
	sh:targetSubjectsOf types:threadOriginItem ;
	.

types:threadOriginItem-subjects-threadPreviousItem-shape
	a sh:PropertyShape ;
	sh:description "An origin item in a thread must not have a previous item."@en ;
	sh:maxCount "0"^^xsd:integer ;
	sh:nodeKind sh:IRI ;
	sh:path (
		types:threadOriginItem
		types:threadPreviousItem
	) ;
	sh:targetSubjectsOf types:threadOriginItem ;
	.

types:threadPredecessor
	a
		owl:ObjectProperty ,
		owl:TransitiveProperty
		;
	rdfs:label "threadPredecessor"@en ;
	rdfs:comment "The link to the preceding item in a thread."@en ;
	rdfs:domain types:ThreadItem ;
	rdfs:range types:ThreadItem ;
	rdfs:seeAlso co:precededBy ;
	owl:inverseOf types:threadSuccessor ;
	.

types:threadPredecessor-subjects-shape
	a sh:PropertyShape ;
	sh:class types:ThreadItem ;
	sh:nodeKind sh:IRI ;
	sh:path types:threadPredecessor ;
	sh:targetSubjectsOf types:threadPredecessor ;
	.

types:threadPreviousItem
	a owl:ObjectProperty ;
	rdfs:subPropertyOf types:threadPredecessor ;
	rdfs:label "threadPreviousItem"@en ;
	rdfs:comment "A direct link to a previous item in a thread."@en ;
	rdfs:seeAlso co:previousItem ;
	owl:inverseOf types:threadNextItem ;
	.

types:threadPreviousItem-subjects-shape
	a sh:PropertyShape ;
	sh:class types:ThreadItem ;
	sh:nodeKind sh:IRI ;
	sh:path types:threadPreviousItem ;
	sh:targetSubjectsOf types:threadPreviousItem ;
	.

types:threadSuccessor
	a
		owl:ObjectProperty ,
		owl:TransitiveProperty
		;
	rdfs:label "threadSuccessor"@en ;
	rdfs:comment "A link to a following item in a thread."@en ;
	rdfs:domain types:ThreadItem ;
	rdfs:range types:ThreadItem ;
	rdfs:seeAlso co:followedBy ;
	.

types:threadSuccessor-subjects-shape
	a sh:PropertyShape ;
	sh:class types:ThreadItem ;
	sh:nodeKind sh:IRI ;
	sh:path types:threadSuccessor ;
	sh:targetSubjectsOf types:threadSuccessor ;
	.

types:threadTerminalItem
	a owl:ObjectProperty ;
	rdfs:subPropertyOf co:item ;
	rdfs:label "threadTerminalItem"@en ;
	rdfs:comment "A link to an item of the thread known to have no successor."@en ;
	rdfs:domain types:Thread ;
	rdfs:range [
		a owl:Class ;
		owl:intersectionOf (
			types:ThreadItem
			[
				a owl:Restriction ;
				owl:onProperty types:threadNextItem ;
				owl:cardinality "0"^^xsd:nonNegativeInteger ;
			]
		) ;
	] ;
	rdfs:seeAlso co:lastItem ;
	.

types:threadTerminalItem-subjects-shape
	a sh:PropertyShape ;
	sh:class types:ThreadItem ;
	sh:nodeKind sh:IRI ;
	sh:path types:threadTerminalItem ;
	sh:targetSubjectsOf types:threadTerminalItem ;
	.

types:threadTerminalItem-subjects-threadNextItem-shape
	a sh:PropertyShape ;
	sh:description "A terminal item in a thread must not have a next item."@en ;
	sh:maxCount "0"^^xsd:integer ;
	sh:nodeKind sh:IRI ;
	sh:path (
		types:threadTerminalItem
		types:threadNextItem
	) ;
	sh:targetSubjectsOf types:threadTerminalItem ;
	.

types:threadTerminalItem-subjects-threadSuccessor-shape
	a sh:PropertyShape ;
	sh:description "A terminal item in a thread must not have a successor."@en ;
	sh:maxCount "0"^^xsd:integer ;
	sh:nodeKind sh:IRI ;
	sh:path (
		types:threadTerminalItem
		types:threadSuccessor
	) ;
	sh:targetSubjectsOf types:threadTerminalItem ;
	.

types:value
	a owl:DatatypeProperty ;
	rdfs:label "value"@en ;
	rdfs:comment "A specific property value."@en ;
	rdfs:range xsd:string ;
	.

