{
    "@context": {
        "observable": "https://unifiedcyberontology.org/ontology/uco/observable/",
        "owl": "http://www.w3.org/2002/07/owl#",
        "rdfs": "http://www.w3.org/2000/01/rdf-schema#",
        "sh": "http://www.w3.org/ns/shacl#",
        "xsd": "http://www.w3.org/2001/XMLSchema#"
    },
    "@graph": [
        {
            "@id": "observable:ActionTicket",
            "@type": "owl:Class",
            "rdfs:subClassOf": {
                "@id": "observable:Observable"
            },
            "rdfs:label": "Action Ticket",
            "rdfs:comment": "A record in a ticketing system representing a work request or issue.",
            "sh:property": [
                {
                    "sh:path": {
                        "@id": "observable:title"
                    }
                },
                {
                    "sh:path": {
                        "@id": "observable:description"
                    }
                },
                {
                    "sh:path": {
                        "@id": "observable:type"
                    }
                },
                {
                    "sh:path": {
                        "@id": "observable:priority"
                    }
                },
                {
                    "sh:path": {
                        "@id": "observable:status"
                    }
                },
                {
                    "sh:path": {
                        "@id": "observable:assignee"
                    }
                },
                {
                    "sh:path": {
                        "@id": "observable:reporter"
                    }
                },
                {
                    "sh:path": {
                        "@id": "observable:requestor"
                    }
                },
                {
                    "sh:path": {
                        "@id": "observable:ticketID"
                    }
                },
                {
                    "sh:path": {
                        "@id": "observable:created"
                    }
                },
                {
                    "sh:path": {
                        "@id": "observable:updated"
                    }
                },
                {
                    "sh:path": {
                        "@id": "observable:createdVia"
                    }
                },
                {
                    "sh:path": {
                        "@id": "observable:organization"
                    }
                },
                {
                    "sh:path": {
                        "@id": "observable:interestedIn"
                    }
                },
                {
                    "sh:path": {
                        "@id": "observable:tags"
                    }
                }
            ]
        },
        {
            "@id": "observable:title",
            "@type": "owl:DatatypeProperty",
            "rdfs:label": "Title",
            "rdfs:comment": "A brief description of the issue or request.",
            "rdfs:range": {
                "@id": "xsd:string"
            }
        },
        {
            "@id": "observable:description",
            "@type": "owl:DatatypeProperty",
            "rdfs:label": "Description",
            "rdfs:comment": "A detailed explanation of the issue or request.",
            "rdfs:range": {
                "@id": "xsd:string"
            }
        },
        {
            "@id": "observable:type",
            "@type": "owl:DatatypeProperty",
            "rdfs:label": "Type",
            "rdfs:comment": "The nature of the ticket, e.g., Bug, Feature Request, Task.",
            "rdfs:range": {
                "@id": "xsd:string"
            }
        },
        {
            "@id": "observable:priority",
            "@type": "owl:DatatypeProperty",
            "rdfs:label": "Priority",
            "rdfs:comment": "The level of urgency or importance, categorized as low, normal, high, or urgent.",
            "rdfs:range": {
                "@id": "xsd:string"
            }
        },
        {
            "@id": "observable:status",
            "@type": "owl:DatatypeProperty",
            "rdfs:label": "Status",
            "rdfs:comment": "The current state of the ticket, e.g., Open, In Progress, Resolved.",
            "rdfs:range": {
                "@id": "xsd:string"
            }
        },
        {
            "@id": "observable:assignee",
            "@type": "owl:DatatypeProperty",
            "rdfs:label": "Assignee",
            "rdfs:comment": "A URL to the name record of the assigned person responsible for actioning the ticket.",
            "rdfs:range": {
                "@id": "xsd:anyURI"
            }
        },
        {
            "@id": "observable:reporter",
            "@type": "owl:DatatypeProperty",
            "rdfs:label": "Reporter",
            "rdfs:comment": "The individual or entity that reported the issue or made the request.",
            "rdfs:range": {
                "@id": "xsd:string"
            }
        },
        {
            "@id": "observable:requestor",
            "@type": "owl:DatatypeProperty",
            "rdfs:label": "Requestor",
            "rdfs:comment": "A URL to the name record of the submitter of the ticket.",
            "rdfs:range": {
                "@id": "xsd:anyURI"
            }
        },
        {
            "@id": "observable:ticketID",
            "@type": "owl:DatatypeProperty",
            "rdfs:label": "Ticket ID",
            "rdfs:comment": "A unique identifier for the ticket, represented as an integer.",
            "rdfs:range": {
                "@id": "xsd:integer"
            }
        },
        {
            "@id": "observable:created",
            "@type": "owl:DatatypeProperty",
            "rdfs:label": "Created",
            "rdfs:comment": "The date and time when the ticket was created.",
            "rdfs:range": {
                "@id": "xsd:dateTime"
            }
        },
        {
            "@id": "observable:updated",
            "@type": "owl:DatatypeProperty",
            "rdfs:label": "Updated",
            "rdfs:comment": "The date and time when the ticket was last updated.",
            "rdfs:range": {
                "@id": "xsd:dateTime"
            }
        },
        {
            "@id": "observable:createdVia",
            "@type": "owl:DatatypeProperty",
            "rdfs:label": "Created via",
            "rdfs:comment": "The medium through which the ticket was created, e.g., web, email.",
            "rdfs:range": {
                "@id": "xsd:string"
            }
        },
        {
            "@id": "observable:organization",
            "@type": "owl:DatatypeProperty",
            "rdfs:label": "Organization",
            "rdfs:comment": "The name of the organization of the requestor.",
            "rdfs:range": {
                "@id": "xsd:string"
            }
        },
        {
            "@id": "observable:interestedIn",
            "@type": "owl:DatatypeProperty",
            "rdfs:label": "I am interested in",
            "rdfs:comment": "Classification assigned by the assignee from a list unique to the organization.",
            "rdfs:range": {
                "@id": "xsd:string"
            }
        },
        {
            "@id": "observable:tags",
            "@type": "owl:DatatypeProperty",
            "rdfs:label": "Tags",
            "rdfs:comment": "One or more tags assigned by the assignee to further classify the ticket.",
            "rdfs:range": {
                "@id": "xsd:string"
            }
        }
    ]
}
