# baseURI: https://unifiedcyberontology.org/ontology/uco/observable
# imports: https://unifiedcyberontology.org/ontology/uco/action
# imports: https://unifiedcyberontology.org/ontology/uco/core
# imports: https://unifiedcyberontology.org/ontology/uco/identity
# imports: https://unifiedcyberontology.org/ontology/uco/location
# imports: https://unifiedcyberontology.org/ontology/uco/types
# imports: https://unifiedcyberontology.org/ontology/uco/vocabulary

@base <https://unifiedcyberontology.org/ontology/uco/observable> .
@prefix identity: <https://unifiedcyberontology.org/ontology/uco/identity#> .
@prefix observable: <https://unifiedcyberontology.org/ontology/uco/observable#> .
@prefix owl: <http://www.w3.org/2002/07/owl#> .
@prefix rdf: <http://www.w3.org/1999/02/22-rdf-syntax-ns#> .
@prefix rdfs: <http://www.w3.org/2000/01/rdf-schema#> .
@prefix vocabulary: <https://unifiedcyberontology.org/ontology/uco/vocabulary#> .
@prefix xml: <http://www.w3.org/XML/1998/namespace> .
@prefix xsd: <http://www.w3.org/2001/XMLSchema#> .

<https://unifiedcyberontology.org/ontology/uco/observable>
	a owl:Ontology ;
	rdfs:label "uco-observable"@en ;
	owl:imports
		<https://unifiedcyberontology.org/ontology/uco/action> ,
		<https://unifiedcyberontology.org/ontology/uco/core> ,
		<https://unifiedcyberontology.org/ontology/uco/identity> ,
		<https://unifiedcyberontology.org/ontology/uco/location> ,
		<https://unifiedcyberontology.org/ontology/uco/types> ,
		<https://unifiedcyberontology.org/ontology/uco/vocabulary>
		;
	.

observable:API
	a owl:Class ;
	rdfs:subClassOf observable:ObservableObject ;
	rdfs:label "API"@en ;
	rdfs:comment "An API (application programming interface) is a computing interface that defines interactions between multiple software or mixed hardware-software intermediaries. It defines the kinds of calls or requests that can be made, how to make them, the data formats that should be used, the conventions to follow, etc. [based on https://en.wikipedia.org/wiki/API]"@en ;
	.

observable:ARPCache
	a owl:Class ;
	rdfs:subClassOf observable:ObservableObject ;
	rdfs:label "ARPCache"@en ;
	rdfs:comment "An ARP cache is a collection of Address Resolution Protocol (ARP) entries (mostly dynamic) that are created when an IP address is resolved to a MAC address (so the computer can effectively communicate with the IP address). [based on https://en.wikipedia.org/wiki/ARP_cache]"@en ;
	.

observable:ARPCacheEntry
	a owl:Class ;
	rdfs:subClassOf observable:ObservableObject ;
	rdfs:label "ARPCacheEntry"@en ;
	rdfs:comment "An ARP cache entry is a single Address Resolution Protocol (ARP) response record that is created when an IP address is resolved to a MAC address (so the computer can effectively communicate with the IP address). [based on https://en.wikipedia.org/wiki/ARP_cache]"@en ;
	.

observable:Account
	a owl:Class ;
	rdfs:subClassOf observable:ObservableObject ;
	rdfs:label "Account"@en ;
	rdfs:comment "An account is an arrangement with an entity to enable and control the provision of some capability or service."@en ;
	.

observable:AccountAuthenticationFacet
	a owl:Class ;
	rdfs:subClassOf
		<https://unifiedcyberontology.org/ontology/uco/core#Facet> ,
		[
			a owl:Restriction ;
			owl:onProperty observable:passwordLastChanged ;
			owl:maxCardinality "1"^^xsd:nonNegativeInteger ;
		] ,
		[
			a owl:Restriction ;
			owl:onProperty observable:password ;
			owl:maxQualifiedCardinality "1"^^xsd:nonNegativeInteger ;
			owl:onDataRange xsd:string ;
		] ,
		[
			a owl:Restriction ;
			owl:onProperty observable:passwordType ;
			owl:maxQualifiedCardinality "1"^^xsd:nonNegativeInteger ;
			owl:onDataRange xsd:string ;
		]
		;
	rdfs:label "AccountAuthenticationFacet"@en ;
	rdfs:comment "An account authentication facet is a grouping of characteristics unique to the mechanism of accessing an account."@en ;
	.

observable:AccountFacet
	a owl:Class ;
	rdfs:subClassOf
		<https://unifiedcyberontology.org/ontology/uco/core#Facet> ,
		[
			a owl:Restriction ;
			owl:onProperty observable:accountIssuer ;
			owl:maxCardinality "1"^^xsd:nonNegativeInteger ;
		] ,
		[
			a owl:Restriction ;
			owl:onProperty observable:accountType ;
			owl:maxCardinality "1"^^xsd:nonNegativeInteger ;
		] ,
		[
			a owl:Restriction ;
			owl:onProperty observable:expirationTime ;
			owl:maxCardinality "1"^^xsd:nonNegativeInteger ;
		] ,
		[
			a owl:Restriction ;
			owl:onProperty observable:modifiedTime ;
			owl:maxCardinality "1"^^xsd:nonNegativeInteger ;
		] ,
		[
			a owl:Restriction ;
			owl:onProperty observable:observableCreatedTime ;
			owl:maxCardinality "1"^^xsd:nonNegativeInteger ;
		] ,
		[
			a owl:Restriction ;
			owl:onProperty observable:owner ;
			owl:maxCardinality "1"^^xsd:nonNegativeInteger ;
		] ,
		[
			a owl:Restriction ;
			owl:onProperty observable:isActive ;
			owl:maxQualifiedCardinality "1"^^xsd:nonNegativeInteger ;
			owl:onDataRange xsd:boolean ;
		] ,
		[
			a owl:Restriction ;
			owl:onProperty observable:accountIdentifier ;
			owl:onDataRange xsd:string ;
			owl:qualifiedCardinality "1"^^xsd:nonNegativeInteger ;
		]
		;
	rdfs:label "AccountFacet"@en ;
	rdfs:comment "An account facet is a grouping of characteristics unique to an arrangement with an entity to enable and control the provision of some capability or service."@en ;
	.

observable:Address
	a owl:Class ;
	rdfs:subClassOf observable:ObservableObject ;
	rdfs:label "Address"@en ;
	rdfs:comment "An address is an identifier assigned to enable routing and management of information."@en ;
	.

observable:AlternateDataStream
	a owl:Class ;
	rdfs:subClassOf
		[
			a owl:Restriction ;
			owl:onProperty observable:hashes ;
			owl:maxCardinality "1"^^xsd:nonNegativeInteger ;
		] ,
		[
			a owl:Restriction ;
			owl:onProperty observable:size ;
			owl:maxQualifiedCardinality "1"^^xsd:nonNegativeInteger ;
			owl:onDataRange xsd:integer ;
		] ,
		[
			a owl:Restriction ;
			owl:onProperty <https://unifiedcyberontology.org/ontology/uco/core#name> ;
			owl:onDataRange xsd:string ;
			owl:qualifiedCardinality "1"^^xsd:nonNegativeInteger ;
		]
		;
	rdfs:label "AlternateDataStream"@en ;
	rdfs:comment "An alternate data stream is data content stored within an NTFS file that is independent of the standard content stream of the file and is hidden from access by default NTFS file viewing mechanisms."@en ;
	.

observable:Appliance
	a owl:Class ;
	rdfs:subClassOf observable:Device ;
	rdfs:label "Appliance"@en ;
	rdfs:comment "An appliance is a purpose-built computer with software or firmware that is designed to provide a specific computing capability or resource. [based on https://en.wikipedia.org/wiki/Computer_appliance]"@en ;
	.

observable:Application
	a owl:Class ;
	rdfs:subClassOf observable:ObservableObject ;
	rdfs:label "Application"@en ;
	rdfs:comment "An application is a particular software program designed for end users."@en ;
	.

observable:ApplicationAccount
	a owl:Class ;
	rdfs:subClassOf observable:DigitalAccount ;
	rdfs:label "ApplicationAccount"@en ;
	rdfs:comment "An application account is an account within a particular software program designed for end users."@en ;
	.

observable:ApplicationAccountFacet
	a owl:Class ;
	rdfs:subClassOf
		<https://unifiedcyberontology.org/ontology/uco/core#Facet> ,
		[
			a owl:Restriction ;
			owl:onProperty observable:application ;
			owl:onClass observable:ObservableObject ;
			owl:qualifiedCardinality "1"^^xsd:nonNegativeInteger ;
		]
		;
	rdfs:label "ApplicationAccountFacet"@en ;
	rdfs:comment "An application account facet is a grouping of characteristics unique to an account within a particular software program designed for end users."@en ;
	.

observable:ApplicationFacet
	a owl:Class ;
	rdfs:subClassOf
		<https://unifiedcyberontology.org/ontology/uco/core#Facet> ,
		[
			a owl:Restriction ;
			owl:onProperty observable:operatingSystem ;
			owl:onClass observable:ObservableObject ;
			owl:maxQualifiedCardinality "1"^^xsd:nonNegativeInteger ;
		] ,
		[
			a owl:Restriction ;
			owl:onProperty observable:numberOfLaunches ;
			owl:maxQualifiedCardinality "1"^^xsd:nonNegativeInteger ;
			owl:onDataRange xsd:integer ;
		] ,
		[
			a owl:Restriction ;
			owl:onProperty observable:applicationIdentifier ;
			owl:maxQualifiedCardinality "1"^^xsd:nonNegativeInteger ;
			owl:onDataRange xsd:string ;
		] ,
		[
			a owl:Restriction ;
			owl:onProperty observable:version ;
			owl:maxQualifiedCardinality "1"^^xsd:nonNegativeInteger ;
			owl:onDataRange xsd:string ;
		]
		;
	rdfs:label "ApplicationFacet"@en ;
	rdfs:comment "An application facet is a grouping of characteristics unique to a particular software program designed for ends users."@en ;
	.

observable:ArchiveFile
	a owl:Class ;
	rdfs:subClassOf observable:File ;
	rdfs:label "ArchiveFile"@en ;
	rdfs:comment "An archive file is a file that is composed of one or more computer files along with metadata."@en ;
	.

observable:ArchiveFileFacet
	a owl:Class ;
	rdfs:subClassOf
		<https://unifiedcyberontology.org/ontology/uco/core#Facet> ,
		[
			a owl:Restriction ;
			owl:onProperty observable:archiveType ;
			owl:maxQualifiedCardinality "1"^^xsd:nonNegativeInteger ;
			owl:onDataRange xsd:string ;
		] ,
		[
			a owl:Restriction ;
			owl:onProperty observable:comment ;
			owl:maxQualifiedCardinality "1"^^xsd:nonNegativeInteger ;
			owl:onDataRange xsd:string ;
		] ,
		[
			a owl:Restriction ;
			owl:onProperty observable:version ;
			owl:maxQualifiedCardinality "1"^^xsd:nonNegativeInteger ;
			owl:onDataRange xsd:string ;
		]
		;
	rdfs:label "ArchiveFileFacet"@en ;
	rdfs:comment "An archive file facet is a grouping of characteristics unique to a file that is composed of one or more computer files along with metadata."@en ;
	.

observable:AttachmentFacet
	a owl:Class ;
	rdfs:subClassOf <https://unifiedcyberontology.org/ontology/uco/core#Facet> ;
	rdfs:label "AttachmentFacet"@en ;
	rdfs:comment "An attachment facet is a grouping of characteristics unique to the inclusion of an associated object as part of a message."@en ;
	.

observable:Audio
	a owl:Class ;
	rdfs:subClassOf observable:ObservableObject ;
	rdfs:label "Audio"@en ;
	rdfs:comment "Audio is a digital representation of sound."@en ;
	.

observable:AudioFacet
	a owl:Class ;
	rdfs:subClassOf
		<https://unifiedcyberontology.org/ontology/uco/core#Facet> ,
		[
			a owl:Restriction ;
			owl:onProperty observable:bitRate ;
			owl:maxQualifiedCardinality "1"^^xsd:nonNegativeInteger ;
			owl:onDataRange xsd:integer ;
		] ,
		[
			a owl:Restriction ;
			owl:onProperty observable:duration ;
			owl:maxQualifiedCardinality "1"^^xsd:nonNegativeInteger ;
			owl:onDataRange xsd:integer ;
		] ,
		[
			a owl:Restriction ;
			owl:onProperty observable:audioType ;
			owl:maxQualifiedCardinality "1"^^xsd:nonNegativeInteger ;
			owl:onDataRange xsd:string ;
		] ,
		[
			a owl:Restriction ;
			owl:onProperty observable:format ;
			owl:maxQualifiedCardinality "1"^^xsd:nonNegativeInteger ;
			owl:onDataRange xsd:string ;
		]
		;
	rdfs:label "AudioFacet"@en ;
	rdfs:comment "An audio facet is a grouping of characteristics unique to a digital representation of sound."@en ;
	.

observable:AutonomousSystem
	a owl:Class ;
	rdfs:subClassOf observable:ObservableObject ;
	rdfs:label "AutonomousSystem"@en ;
	rdfs:comment "An autonomous system is a collection of connected Internet Protocol (IP) routing prefixes under the control of one or more network operators on behalf of a single administrative entity or domain that presents a common, clearly defined routing policy to the Internet. [based on https://en.wikipedia.org/wiki/Autonomous_system_(Internet)]"@en ;
	.

observable:AutonomousSystemFacet
	a owl:Class ;
	rdfs:subClassOf
		<https://unifiedcyberontology.org/ontology/uco/core#Facet> ,
		[
			a owl:Restriction ;
			owl:onProperty observable:regionalInternetRegistry ;
			owl:maxCardinality "1"^^xsd:nonNegativeInteger ;
		] ,
		[
			a owl:Restriction ;
			owl:onProperty observable:asHandle ;
			owl:maxQualifiedCardinality "1"^^xsd:nonNegativeInteger ;
			owl:onDataRange xsd:string ;
		] ,
		[
			a owl:Restriction ;
			owl:onProperty observable:number ;
			owl:onDataRange xsd:integer ;
			owl:qualifiedCardinality "1"^^xsd:nonNegativeInteger ;
		]
		;
	rdfs:label "AutonomousSystemFacet"@en ;
	rdfs:comment "An autonomous system facet is a grouping of characteristics unique to a collection of connected Internet Protocol (IP) routing prefixes under the control of one or more network operators on behalf of a single administrative entity or domain that presents a common, clearly defined routing policy to the Internet. [based on https://en.wikipedia.org/wiki/Autonomous_system_(Internet)]"@en ;
	.

observable:BlockDeviceNode
	a owl:Class ;
	rdfs:subClassOf observable:FileSystemObject ;
	rdfs:label "BlockDeviceNode"@en ;
	rdfs:comment "A block device node is a UNIX filesystem special file that serves as a conduit to communicate with devices, providing buffered randomly accesible input and output. Block device nodes are used to apply access rights to the devices and to direct operations on the files to the appropriate device drivers. [based on https://en.wikipedia.org/wiki/Unix_file_types]"@en ;
	.

observable:BluetoothAddress
	a owl:Class ;
	rdfs:subClassOf observable:MACAddress ;
	rdfs:label "BluetoothAddress"@en ;
	rdfs:comment "A Bluetooth address is a Bluetooth standard conformant identifier assigned to a Bluetooth device to enable routing and management of Bluetooth standards conformant communication to or from that device."@en ;
	.

observable:BluetoothAddressFacet
	a owl:Class ;
	rdfs:subClassOf
		<https://unifiedcyberontology.org/ontology/uco/core#MACAddressFacet> ,
		[
			a owl:Restriction ;
			owl:onProperty observable:addressValue ;
			owl:maxQualifiedCardinality "1"^^xsd:nonNegativeInteger ;
			owl:onDataRange xsd:string ;
		]
		;
	rdfs:label "BluetoothAddressFacet"@en ;
	rdfs:comment "A Bluetooth address facet is a grouping of characteristics unique to a Bluetooth standard conformant identifier assigned to a Bluetooth device to enable routing and management of Bluetooth standards conformant communication to or from that device."@en ;
	.

observable:BotConfiguration
	a owl:Class ;
	rdfs:subClassOf observable:ObservableObject ;
	rdfs:label "BotConfiguration"@en ;
	rdfs:comment "A bot configuration is a set of contextual settings for a software application that runs automated tasks (scripts) over the Internet at a much higher rate than would be possible for a human alone."@en ;
	.

observable:BrowserBookmark
	a owl:Class ;
	rdfs:subClassOf observable:ObservableObject ;
	rdfs:label "BrowserBookmark"@en ;
	rdfs:comment "A browser bookmark is a saved shortcut that directs a WWW (World Wide Web) browser software program to a particular WWW accessible resource. [based on https://techterms.com/definition/bookmark]"@en ;
	.

observable:BrowserBookmarkFacet
	a owl:Class ;
	rdfs:subClassOf
		<https://unifiedcyberontology.org/ontology/uco/core#Facet> ,
		[
			a owl:Restriction ;
			owl:onProperty observable:accessedTime ;
			owl:maxCardinality "1"^^xsd:nonNegativeInteger ;
		] ,
		[
			a owl:Restriction ;
			owl:onProperty observable:modifiedTime ;
			owl:maxCardinality "1"^^xsd:nonNegativeInteger ;
		] ,
		[
			a owl:Restriction ;
			owl:onProperty observable:observableCreatedTime ;
			owl:maxCardinality "1"^^xsd:nonNegativeInteger ;
		] ,
		[
			a owl:Restriction ;
			owl:onProperty observable:application ;
			owl:onClass observable:ObservableObject ;
			owl:maxQualifiedCardinality "1"^^xsd:nonNegativeInteger ;
		] ,
		[
			a owl:Restriction ;
			owl:onProperty observable:visitCount ;
			owl:maxQualifiedCardinality "1"^^xsd:nonNegativeInteger ;
			owl:onDataRange xsd:integer ;
		] ,
		[
			a owl:Restriction ;
			owl:onProperty observable:bookmarkPath ;
			owl:maxQualifiedCardinality "1"^^xsd:nonNegativeInteger ;
			owl:onDataRange xsd:string ;
		]
		;
	rdfs:label "BrowserBookmarkFacet"@en ;
	rdfs:comment "A browser bookmark facet is a grouping of characteristics unique to a saved shortcut that directs a WWW (World Wide Web) browser software program to a particular WWW accessible resource. [based on https://techterms.com/definition/bookmark]"@en ;
	.

observable:BrowserCookie
	a owl:Class ;
	rdfs:subClassOf observable:ObservableObject ;
	rdfs:label "BrowserCookie"@en ;
	rdfs:comment "A browser cookie is a piece of of data sent from a website and stored on the user's computer by the user's web browser while the user is browsing. [based on https://en.wikipedia.org/wiki/HTTP_cookie]"@en ;
	.

observable:BrowserCookieFacet
	a owl:Class ;
	rdfs:subClassOf
		<https://unifiedcyberontology.org/ontology/uco/core#Facet> ,
		[
			a owl:Restriction ;
			owl:onProperty observable:accessedTime ;
			owl:maxCardinality "1"^^xsd:nonNegativeInteger ;
		] ,
		[
			a owl:Restriction ;
			owl:onProperty observable:expirationTime ;
			owl:maxCardinality "1"^^xsd:nonNegativeInteger ;
		] ,
		[
			a owl:Restriction ;
			owl:onProperty observable:observableCreatedTime ;
			owl:maxCardinality "1"^^xsd:nonNegativeInteger ;
		] ,
		[
			a owl:Restriction ;
			owl:onProperty observable:application ;
			owl:onClass observable:ObservableObject ;
			owl:maxQualifiedCardinality "1"^^xsd:nonNegativeInteger ;
		] ,
		[
			a owl:Restriction ;
			owl:onProperty observable:cookieDomain ;
			owl:onClass observable:ObservableObject ;
			owl:maxQualifiedCardinality "1"^^xsd:nonNegativeInteger ;
		] ,
		[
			a owl:Restriction ;
			owl:onProperty observable:isSecure ;
			owl:maxQualifiedCardinality "1"^^xsd:nonNegativeInteger ;
			owl:onDataRange xsd:boolean ;
		] ,
		[
			a owl:Restriction ;
			owl:onProperty observable:cookieName ;
			owl:maxQualifiedCardinality "1"^^xsd:nonNegativeInteger ;
			owl:onDataRange xsd:string ;
		] ,
		[
			a owl:Restriction ;
			owl:onProperty observable:cookiePath ;
			owl:maxQualifiedCardinality "1"^^xsd:nonNegativeInteger ;
			owl:onDataRange xsd:string ;
		]
		;
	rdfs:label "BrowserCookieFacet"@en ;
	rdfs:comment "A browser cookie facet is a grouping of characteristics unique to a piece of data sent from a website and stored on the user's computer by the user's web browser while the user is browsing. [based on https://en.wikipedia.org/wiki/HTTP_cookie]"@en ;
	.

observable:Calendar
	a owl:Class ;
	rdfs:subClassOf observable:ObservableObject ;
	rdfs:label "Calendar"@en ;
	rdfs:comment "A calendar is a collection of appointments, meetings, and events."@en ;
	.

observable:CalendarEntry
	a owl:Class ;
	rdfs:subClassOf observable:ObservableObject ;
	rdfs:label "CalendarEntry"@en ;
	rdfs:comment "A calendar entry is an appointment, meeting or event within a collection of appointments, meetings and events."@en ;
	.

observable:CalendarEntryFacet
	a owl:Class ;
	rdfs:subClassOf
		<https://unifiedcyberontology.org/ontology/uco/core#Facet> ,
		[
			a owl:Restriction ;
			owl:onProperty observable:endTime ;
			owl:maxCardinality "1"^^xsd:nonNegativeInteger ;
		] ,
		[
			a owl:Restriction ;
			owl:onProperty observable:location ;
			owl:maxCardinality "1"^^xsd:nonNegativeInteger ;
		] ,
		[
			a owl:Restriction ;
			owl:onProperty observable:modifiedTime ;
			owl:maxCardinality "1"^^xsd:nonNegativeInteger ;
		] ,
		[
			a owl:Restriction ;
			owl:onProperty observable:observableCreatedTime ;
			owl:maxCardinality "1"^^xsd:nonNegativeInteger ;
		] ,
		[
			a owl:Restriction ;
			owl:onProperty observable:owner ;
			owl:maxCardinality "1"^^xsd:nonNegativeInteger ;
		] ,
		[
			a owl:Restriction ;
			owl:onProperty observable:remindTime ;
			owl:maxCardinality "1"^^xsd:nonNegativeInteger ;
		] ,
		[
			a owl:Restriction ;
			owl:onProperty observable:startTime ;
			owl:maxCardinality "1"^^xsd:nonNegativeInteger ;
		] ,
		[
			a owl:Restriction ;
			owl:onProperty observable:application ;
			owl:onClass observable:ObservableObject ;
			owl:maxQualifiedCardinality "1"^^xsd:nonNegativeInteger ;
		] ,
		[
			a owl:Restriction ;
			owl:onProperty observable:isPrivate ;
			owl:maxQualifiedCardinality "1"^^xsd:nonNegativeInteger ;
			owl:onDataRange xsd:boolean ;
		] ,
		[
			a owl:Restriction ;
			owl:onProperty observable:duration ;
			owl:maxQualifiedCardinality "1"^^xsd:nonNegativeInteger ;
			owl:onDataRange xsd:integer ;
		] ,
		[
			a owl:Restriction ;
			owl:onProperty observable:eventStatus ;
			owl:maxQualifiedCardinality "1"^^xsd:nonNegativeInteger ;
			owl:onDataRange xsd:string ;
		] ,
		[
			a owl:Restriction ;
			owl:onProperty observable:eventType ;
			owl:maxQualifiedCardinality "1"^^xsd:nonNegativeInteger ;
			owl:onDataRange xsd:string ;
		] ,
		[
			a owl:Restriction ;
			owl:onProperty observable:recurrence ;
			owl:maxQualifiedCardinality "1"^^xsd:nonNegativeInteger ;
			owl:onDataRange xsd:string ;
		] ,
		[
			a owl:Restriction ;
			owl:onProperty observable:subject ;
			owl:maxQualifiedCardinality "1"^^xsd:nonNegativeInteger ;
			owl:onDataRange xsd:string ;
		]
		;
	rdfs:label "CalendarEntryFacet"@en ;
	rdfs:comment "A calendar entry facet is a grouping of characteristics unique to an appointment, meeting, or event within a collection of appointments, meetings, and events."@en ;
	.

observable:CalendarFacet
	a owl:Class ;
	rdfs:subClassOf
		<https://unifiedcyberontology.org/ontology/uco/core#Facet> ,
		[
			a owl:Restriction ;
			owl:onProperty observable:application ;
			owl:onClass observable:ObservableObject ;
			owl:maxQualifiedCardinality "1"^^xsd:nonNegativeInteger ;
		] ,
		[
			a owl:Restriction ;
			owl:onProperty observable:owner ;
			owl:onClass observable:ObservableObject ;
			owl:maxQualifiedCardinality "1"^^xsd:nonNegativeInteger ;
		]
		;
	rdfs:label "CalendarFacet"@en ;
	rdfs:comment "A calendar facet is a grouping of characteristics unique to a collection of appointments, meetings, and events."@en ;
	.

observable:CharacterDeviceNode
	a owl:Class ;
	rdfs:subClassOf observable:FileSystemObject ;
	rdfs:label "CharacterDeviceNode"@en ;
	rdfs:comment "A character device node is a UNIX filesystem special file that serves as a conduit to communicate with devices, providing only a serial stream of input or accepting a serial stream of output. Character device nodes are used to apply access rights to the devices and to direct operations on the files to the appropriate device drivers. [based on https://en.wikipedia.org/wiki/Unix_file_types]"@en ;
	.

observable:Code
	a owl:Class ;
	rdfs:subClassOf observable:ObservableObject ;
	rdfs:label "Code"@en ;
	rdfs:comment "Code is a direct representation (source, byte or binary) of a collection of computer instructions that form software which tell a computer how to work. [based on https://en.wikipedia.org/wiki/Software]"@en ;
	.

observable:CompressedStreamFacet
	a owl:Class ;
	rdfs:subClassOf
		<https://unifiedcyberontology.org/ontology/uco/core#Facet> ,
		[
			a owl:Restriction ;
			owl:onProperty observable:compressionRatio ;
			owl:maxQualifiedCardinality "1"^^xsd:nonNegativeInteger ;
			owl:onDataRange xsd:double ;
		] ,
		[
			a owl:Restriction ;
			owl:onProperty observable:compressionMethod ;
			owl:maxQualifiedCardinality "1"^^xsd:nonNegativeInteger ;
			owl:onDataRange xsd:string ;
		]
		;
	rdfs:label "CompressedStreamFacet"@en ;
	rdfs:comment "A compressed stream facet is a grouping of characteristics unique to the application of a size-reduction process to a body of data content."@en ;
	.

observable:ComputerSpecification
	a owl:Class ;
	rdfs:subClassOf observable:ObservableObject ;
	rdfs:label "ComputerSpecification"@en ;
	rdfs:comment "A computer specification is the hardware and software of a programmable electronic device that can store, retrieve, and process data. {based on merriam-webster.com/dictionary/computer]"@en ;
	.

observable:ComputerSpecificationFacet
	a owl:Class ;
	rdfs:subClassOf
		<https://unifiedcyberontology.org/ontology/uco/core#Facet> ,
		[
			a owl:Restriction ;
			owl:onProperty observable:biosDate ;
			owl:maxCardinality "1"^^xsd:nonNegativeInteger ;
		] ,
		[
			a owl:Restriction ;
			owl:onProperty observable:biosReleaseDate ;
			owl:maxCardinality "1"^^xsd:nonNegativeInteger ;
		] ,
		[
			a owl:Restriction ;
			owl:onProperty observable:localTime ;
			owl:maxCardinality "1"^^xsd:nonNegativeInteger ;
		] ,
		[
			a owl:Restriction ;
			owl:onProperty observable:systemTime ;
			owl:maxCardinality "1"^^xsd:nonNegativeInteger ;
		] ,
		[
			a owl:Restriction ;
			owl:onProperty observable:currentSystemDate ;
			owl:maxQualifiedCardinality "1"^^xsd:nonNegativeInteger ;
			owl:onDataRange xsd:dateTime ;
		] ,
		[
			a owl:Restriction ;
			owl:onProperty observable:availableRam ;
			owl:maxQualifiedCardinality "1"^^xsd:nonNegativeInteger ;
			owl:onDataRange xsd:integer ;
		] ,
		[
			a owl:Restriction ;
			owl:onProperty observable:totalRam ;
			owl:maxQualifiedCardinality "1"^^xsd:nonNegativeInteger ;
			owl:onDataRange xsd:integer ;
		] ,
		[
			a owl:Restriction ;
			owl:onProperty observable:biosManufacturer ;
			owl:maxQualifiedCardinality "1"^^xsd:nonNegativeInteger ;
			owl:onDataRange xsd:string ;
		] ,
		[
			a owl:Restriction ;
			owl:onProperty observable:biosSerialNumber ;
			owl:maxQualifiedCardinality "1"^^xsd:nonNegativeInteger ;
			owl:onDataRange xsd:string ;
		] ,
		[
			a owl:Restriction ;
			owl:onProperty observable:biosVersion ;
			owl:maxQualifiedCardinality "1"^^xsd:nonNegativeInteger ;
			owl:onDataRange xsd:string ;
		] ,
		[
			a owl:Restriction ;
			owl:onProperty observable:cpu ;
			owl:maxQualifiedCardinality "1"^^xsd:nonNegativeInteger ;
			owl:onDataRange xsd:string ;
		] ,
		[
			a owl:Restriction ;
			owl:onProperty observable:cpuFamily ;
			owl:maxQualifiedCardinality "1"^^xsd:nonNegativeInteger ;
			owl:onDataRange xsd:string ;
		] ,
		[
			a owl:Restriction ;
			owl:onProperty observable:gpu ;
			owl:maxQualifiedCardinality "1"^^xsd:nonNegativeInteger ;
			owl:onDataRange xsd:string ;
		] ,
		[
			a owl:Restriction ;
			owl:onProperty observable:gpuFamily ;
			owl:maxQualifiedCardinality "1"^^xsd:nonNegativeInteger ;
			owl:onDataRange xsd:string ;
		] ,
		[
			a owl:Restriction ;
			owl:onProperty observable:hostname ;
			owl:maxQualifiedCardinality "1"^^xsd:nonNegativeInteger ;
			owl:onDataRange xsd:string ;
		] ,
		[
			a owl:Restriction ;
			owl:onProperty observable:processorArchitecture ;
			owl:maxQualifiedCardinality "1"^^xsd:nonNegativeInteger ;
			owl:onDataRange xsd:string ;
		] ,
		[
			a owl:Restriction ;
			owl:onProperty observable:timezoneDST ;
			owl:maxQualifiedCardinality "1"^^xsd:nonNegativeInteger ;
			owl:onDataRange xsd:string ;
		] ,
		[
			a owl:Restriction ;
			owl:onProperty observable:timezoneStandard ;
			owl:maxQualifiedCardinality "1"^^xsd:nonNegativeInteger ;
			owl:onDataRange xsd:string ;
		] ,
		[
			a owl:Restriction ;
			owl:onProperty observable:uptime ;
			owl:maxQualifiedCardinality "1"^^xsd:nonNegativeInteger ;
			owl:onDataRange xsd:string ;
		]
		;
	rdfs:label "ComputerSpecificationFacet"@en ;
	rdfs:comment "A computer specificaiton facet is a grouping of characteristics unique to the hardware and software of a programmable electronic device that can store, retrieve, and process data. [based on merriam-webster.com/dictionary/computer]"@en ;
	.

observable:Contact
	a owl:Class ;
	rdfs:subClassOf observable:ObservableObject ;
	rdfs:label "Contact"@en ;
	rdfs:comment "A contact is a set of identification and communication related details for a single entity."@en ;
	.

observable:ContactAddress
	a owl:Class ;
	rdfs:subClassOf
		[
			a owl:Restriction ;
			owl:onProperty observable:observable:geolocationAddress ;
			owl:maxQualifiedCardinality "1"^^xsd:nonNegativeInteger ;
			owl:onDataRange <https://unifiedcyberontology.org/ontology/uco/location#Location> ;
		] ,
		[
			a owl:Restriction ;
			owl:onProperty observable:contactAddressScope ;
			owl:maxQualifiedCardinality "1"^^xsd:nonNegativeInteger ;
			owl:onDataRange [
				a rdfs:Datatype ;
				owl:unionOf (
					xsd:string
					vocabulary:ContactAddressScopeVocab
				) ;
			] ;
		]
		;
	rdfs:label "ContactAddress"@en ;
	rdfs:comment "A contact address is a grouping of characteristics unique to a geolocation address of a contact entity."@en ;
	.

observable:ContactAffiliation
	a owl:Class ;
	rdfs:subClassOf
		[
			a owl:Restriction ;
			owl:onProperty observable:observable:organizationDepartment ;
			owl:maxQualifiedCardinality "1"^^xsd:nonNegativeInteger ;
			owl:onDataRange xsd:string ;
		] ,
		[
			a owl:Restriction ;
			owl:onProperty observable:observable:organizationPosition ;
			owl:maxQualifiedCardinality "1"^^xsd:nonNegativeInteger ;
			owl:onDataRange xsd:string ;
		] ,
		[
			a owl:Restriction ;
			owl:onProperty observable:observable:organizationLocation ;
			owl:minQualifiedCardinality "0"^^xsd:nonNegativeInteger ;
			owl:onDataRange observable:ContactAddress ;
		] ,
		[
			a owl:Restriction ;
			owl:onProperty observable:observable:contactEmail ;
			owl:minQualifiedCardinality "0"^^xsd:nonNegativeInteger ;
			owl:onDataRange observable:ContactEmail ;
		] ,
		[
			a owl:Restriction ;
			owl:onProperty observable:observable:contactMessaging ;
			owl:minQualifiedCardinality "0"^^xsd:nonNegativeInteger ;
			owl:onDataRange observable:ContactMessaging ;
		] ,
		[
			a owl:Restriction ;
			owl:onProperty observable:observable:contactPhone ;
			owl:minQualifiedCardinality "0"^^xsd:nonNegativeInteger ;
			owl:onDataRange observable:ContactPhone ;
		] ,
		[
			a owl:Restriction ;
			owl:onProperty observable:observable:contactProfile ;
			owl:minQualifiedCardinality "0"^^xsd:nonNegativeInteger ;
			owl:onDataRange observable:ContactProfile ;
		] ,
		[
			a owl:Restriction ;
			owl:onProperty observable:observable:contactURL ;
			owl:minQualifiedCardinality "0"^^xsd:nonNegativeInteger ;
			owl:onDataRange observable:ContactURL ;
		] ,
		[
			a owl:Restriction ;
			owl:onProperty observable:contactOrganization ;
			owl:onDataRange identity:Organization ;
			owl:qualifiedCardinality "1"^^xsd:nonNegativeInteger ;
		]
		;
	rdfs:label "ContactListAffiliation"@en ;
	rdfs:comment "A contact affiliation is a grouping of characteristics unique to details of an organizational affiliation for a single contact entity."@en ;
	.

observable:ContactEmail
	a owl:Class ;
	rdfs:subClassOf
		[
			a owl:Restriction ;
			owl:onProperty observable:observable:emailAddress ;
			owl:maxQualifiedCardinality "1"^^xsd:nonNegativeInteger ;
			owl:onDataRange observable:ObservableObject ;
		] ,
		[
			a owl:Restriction ;
			owl:onProperty observable:contactEmailScope ;
			owl:maxQualifiedCardinality "1"^^xsd:nonNegativeInteger ;
			owl:onDataRange [
				a rdfs:Datatype ;
				owl:unionOf (
					xsd:string
					vocabulary:ContactEmailScopeVocab
				) ;
			] ;
		]
		;
	rdfs:label "ContactEmail"@en ;
	rdfs:comment "A contact email is a grouping of characteristics unique to details for contacting a contact entity by email."@en ;
	.

observable:ContactFacet
	a owl:Class ;
	rdfs:subClassOf
		<https://unifiedcyberontology.org/ontology/uco/core#Facet> ,
		[
			a owl:Restriction ;
			owl:onProperty observable:sourceApplication ;
			owl:onClass observable:ObservableObject ;
			owl:maxQualifiedCardinality "1"^^xsd:nonNegativeInteger ;
		] ,
		[
			a owl:Restriction ;
			owl:onProperty identity:birthdate ;
			owl:maxQualifiedCardinality "1"^^xsd:nonNegativeInteger ;
			owl:onDataRange xsd:dateTime ;
		] ,
		[
			a owl:Restriction ;
			owl:onProperty observable:lastTimeContacted ;
			owl:maxQualifiedCardinality "1"^^xsd:nonNegativeInteger ;
			owl:onDataRange xsd:dateTime ;
		] ,
		[
			a owl:Restriction ;
			owl:onProperty observable:numberTimesContacted ;
			owl:maxQualifiedCardinality "1"^^xsd:nonNegativeInteger ;
			owl:onDataRange xsd:integer ;
		] ,
		[
			a owl:Restriction ;
			owl:onProperty observable:contactID ;
			owl:maxQualifiedCardinality "1"^^xsd:nonNegativeInteger ;
			owl:onDataRange xsd:string ;
		] ,
		[
			a owl:Restriction ;
			owl:onProperty observable:displayName ;
			owl:maxQualifiedCardinality "1"^^xsd:nonNegativeInteger ;
			owl:onDataRange xsd:string ;
		] ,
		[
			a owl:Restriction ;
			owl:onProperty observable:firstName ;
			owl:maxQualifiedCardinality "1"^^xsd:nonNegativeInteger ;
			owl:onDataRange xsd:string ;
		] ,
		[
			a owl:Restriction ;
			owl:onProperty observable:lastName ;
			owl:maxQualifiedCardinality "1"^^xsd:nonNegativeInteger ;
			owl:onDataRange xsd:string ;
		] ,
		[
			a owl:Restriction ;
			owl:onProperty observable:middleName ;
			owl:maxQualifiedCardinality "1"^^xsd:nonNegativeInteger ;
			owl:onDataRange xsd:string ;
		] ,
		[
			a owl:Restriction ;
			owl:onProperty observable:namePhonetic ;
			owl:maxQualifiedCardinality "1"^^xsd:nonNegativeInteger ;
			owl:onDataRange xsd:string ;
		] ,
		[
			a owl:Restriction ;
			owl:onProperty observable:namePrefix ;
			owl:maxQualifiedCardinality "1"^^xsd:nonNegativeInteger ;
			owl:onDataRange xsd:string ;
		] ,
		[
			a owl:Restriction ;
			owl:onProperty observable:nameSuffix ;
			owl:maxQualifiedCardinality "1"^^xsd:nonNegativeInteger ;
			owl:onDataRange xsd:string ;
		] ,
		[
			a owl:Restriction ;
			owl:onProperty observable:contactGroup ;
			owl:minQualifiedCardinality "0"^^xsd:nonNegativeInteger ;
			owl:onDataRange xsd:string ;
		] ,
		[
			a owl:Restriction ;
			owl:onProperty observable:contactNote ;
			owl:minQualifiedCardinality "0"^^xsd:nonNegativeInteger ;
			owl:onDataRange xsd:string ;
		] ,
		[
			a owl:Restriction ;
			owl:onProperty observable:nickname ;
			owl:minQualifiedCardinality "0"^^xsd:nonNegativeInteger ;
			owl:onDataRange xsd:string ;
		] ,
		[
			a owl:Restriction ;
			owl:onProperty observable:contactAddress ;
			owl:minQualifiedCardinality "0"^^xsd:nonNegativeInteger ;
			owl:onDataRange observable:ContactAddress ;
		] ,
		[
			a owl:Restriction ;
			owl:onProperty observable:contactAffiliation ;
			owl:minQualifiedCardinality "0"^^xsd:nonNegativeInteger ;
			owl:onDataRange observable:ContactAffiliation ;
		] ,
		[
			a owl:Restriction ;
			owl:onProperty observable:contactEmail ;
			owl:minQualifiedCardinality "0"^^xsd:nonNegativeInteger ;
			owl:onDataRange observable:ContactEmail ;
		] ,
		[
			a owl:Restriction ;
			owl:onProperty observable:contactMessaging ;
			owl:minQualifiedCardinality "0"^^xsd:nonNegativeInteger ;
			owl:onDataRange observable:ContactMessaging ;
		] ,
		[
			a owl:Restriction ;
			owl:onProperty observable:contactPhone ;
			owl:minQualifiedCardinality "0"^^xsd:nonNegativeInteger ;
			owl:onDataRange observable:ContactPhone ;
		] ,
		[
			a owl:Restriction ;
			owl:onProperty observable:contactProfile ;
			owl:minQualifiedCardinality "0"^^xsd:nonNegativeInteger ;
			owl:onDataRange observable:ContactProfile ;
		] ,
		[
			a owl:Restriction ;
			owl:onProperty observable:contactSIP ;
			owl:minQualifiedCardinality "0"^^xsd:nonNegativeInteger ;
			owl:onDataRange observable:ContactSIP ;
		] ,
		[
			a owl:Restriction ;
			owl:onProperty observable:contactURL ;
			owl:minQualifiedCardinality "0"^^xsd:nonNegativeInteger ;
			owl:onDataRange observable:ContactURL ;
		]
		;
	rdfs:label "ContactFacet"@en ;
	rdfs:comment "A contact facet is a grouping of characteristics unique to a set of identification and communication related details for a single entity."@en ;
	.

observable:ContactList
	a owl:Class ;
	rdfs:subClassOf observable:ObservableObject ;
	rdfs:label "ContactList"@en ;
	rdfs:comment "A contact list is a set of multiple individual contacts such as that found in a digital address book."@en ;
	.

observable:ContactListFacet
	a owl:Class ;
	rdfs:subClassOf
		<https://unifiedcyberontology.org/ontology/uco/core#Facet> ,
		[
			a owl:Restriction ;
			owl:onProperty observable:observable:sourceApplication ;
			owl:maxQualifiedCardinality "1"^^xsd:nonNegativeInteger ;
			owl:onDataRange observable:ObservableObject ;
		] ,
		[
			a owl:Restriction ;
			owl:onProperty observable:contact ;
			owl:minQualifiedCardinality "1"^^xsd:nonNegativeInteger ;
			owl:onDataRange observable:ObservableObject ;
		]
		;
	rdfs:label "ContactListFacet"@en ;
	rdfs:comment "A contact list facet is a grouping of characteristics unique to a set of multiple individual contacts such as that found in a digital address book."@en ;
	.

observable:ContactMessaging
	a owl:Class ;
	rdfs:subClassOf
		[
			a owl:Restriction ;
			owl:onProperty observable:observable:contactAddress ;
			owl:maxQualifiedCardinality "1"^^xsd:nonNegativeInteger ;
			owl:onDataRange observable:ObservableObject ;
		] ,
		[
			a owl:Restriction ;
			owl:onProperty observable:observable:contactMessagingPlatform ;
			owl:maxQualifiedCardinality "1"^^xsd:nonNegativeInteger ;
			owl:onDataRange observable:ObservableObject ;
		]
		;
	rdfs:label "ContactMessaging"@en ;
	rdfs:comment "A contact messaging is a grouping of characteristics unique to details for contacting a contact entity by digital messaging."@en ;
	.

observable:ContactPhone
	a owl:Class ;
	rdfs:subClassOf
		[
			a owl:Restriction ;
			owl:onProperty observable:observable:contactPhoneNumber ;
			owl:maxQualifiedCardinality "1"^^xsd:nonNegativeInteger ;
			owl:onDataRange observable:ObservableObject ;
		] ,
		[
			a owl:Restriction ;
			owl:onProperty observable:contactPhoneScope ;
			owl:maxQualifiedCardinality "1"^^xsd:nonNegativeInteger ;
			owl:onDataRange [
				a rdfs:Datatype ;
				owl:unionOf (
					xsd:string
					vocabulary:ContactPhoneScopeVocab
				) ;
			] ;
		]
		;
	rdfs:label "ContactPhone"@en ;
	rdfs:comment "A contact phone is a grouping of characteristics unique to details for contacting a contact entity by telephone."@en ;
	.

observable:ContactProfile
	a owl:Class ;
	rdfs:subClassOf
		[
			a owl:Restriction ;
			owl:onProperty observable:contactProfilePlatform ;
			owl:maxQualifiedCardinality "1"^^xsd:nonNegativeInteger ;
			owl:onDataRange observable:ObservableObject ;
		] ,
		[
			a owl:Restriction ;
			owl:onProperty observable:profile ;
			owl:maxQualifiedCardinality "1"^^xsd:nonNegativeInteger ;
			owl:onDataRange observable:ObservableObject ;
		]
		;
	rdfs:label "ContactProfile"@en ;
	rdfs:comment "A contact profile is a grouping of characteristics unique to details for contacting a contact entity by online service."@en ;
	.

observable:ContactSIP
	a owl:Class ;
	rdfs:subClassOf
		[
			a owl:Restriction ;
			owl:onProperty observable:observable:sipAddress ;
			owl:maxQualifiedCardinality "1"^^xsd:nonNegativeInteger ;
			owl:onDataRange observable:ObservableObject ;
		] ,
		[
			a owl:Restriction ;
			owl:onProperty observable:contactSIPScope ;
			owl:maxQualifiedCardinality "1"^^xsd:nonNegativeInteger ;
			owl:onDataRange [
				a rdfs:Datatype ;
				owl:unionOf (
					xsd:string
					vocabulary:ContactSIPScopeVocab
				) ;
			] ;
		]
		;
	rdfs:label "ContactSIP"@en ;
	rdfs:comment "A contact SIP is a grouping of characteristics unique to details for contacting a contact entity by Session Initiation Protocol (SIP)."@en ;
	.

observable:ContactURL
	a owl:Class ;
	rdfs:subClassOf
		[
			a owl:Restriction ;
			owl:onProperty observable:observable:url ;
			owl:maxQualifiedCardinality "1"^^xsd:nonNegativeInteger ;
			owl:onDataRange observable:ObservableObject ;
		] ,
		[
			a owl:Restriction ;
			owl:onProperty observable:contactURLScope ;
			owl:maxQualifiedCardinality "1"^^xsd:nonNegativeInteger ;
			owl:onDataRange [
				a rdfs:Datatype ;
				owl:unionOf (
					xsd:string
					vocabulary:ContactURLScopeVocab
				) ;
			] ;
		]
		;
	rdfs:label "ContactURL"@en ;
	rdfs:comment "A contact URL is a grouping of characteristics unique to details for contacting a contact entity by Uniform Resource Locator (URL)."@en ;
	.

observable:ContentData
	a owl:Class ;
	rdfs:subClassOf observable:ObservableObject ;
	rdfs:label "ContentData"@en ;
	rdfs:comment "Content data is a block of digital data."@en ;
	.

observable:ContentDataFacet
	a owl:Class ;
	rdfs:subClassOf
		<https://unifiedcyberontology.org/ontology/uco/core#Facet> ,
		[
			a owl:Restriction ;
			owl:onProperty observable:byteOrder ;
			owl:maxCardinality "1"^^xsd:nonNegativeInteger ;
		] ,
		[
			a owl:Restriction ;
			owl:onProperty observable:dataPayloadReferenceURL ;
			owl:onClass observable:ObservableObject ;
			owl:maxQualifiedCardinality "1"^^xsd:nonNegativeInteger ;
		] ,
		[
			a owl:Restriction ;
			owl:onProperty observable:isEncrypted ;
			owl:maxQualifiedCardinality "1"^^xsd:nonNegativeInteger ;
			owl:onDataRange xsd:boolean ;
		] ,
		[
			a owl:Restriction ;
			owl:onProperty observable:entropy ;
			owl:maxQualifiedCardinality "1"^^xsd:nonNegativeInteger ;
			owl:onDataRange xsd:double ;
		] ,
		[
			a owl:Restriction ;
			owl:onProperty observable:sizeInBytes ;
			owl:maxQualifiedCardinality "1"^^xsd:nonNegativeInteger ;
			owl:onDataRange xsd:integer ;
		] ,
		[
			a owl:Restriction ;
			owl:onProperty observable:dataPayload ;
			owl:maxQualifiedCardinality "1"^^xsd:nonNegativeInteger ;
			owl:onDataRange xsd:string ;
		] ,
		[
			a owl:Restriction ;
			owl:onProperty observable:magicNumber ;
			owl:maxQualifiedCardinality "1"^^xsd:nonNegativeInteger ;
			owl:onDataRange xsd:string ;
		] ,
		[
			a owl:Restriction ;
			owl:onProperty observable:mimeClass ;
			owl:maxQualifiedCardinality "1"^^xsd:nonNegativeInteger ;
			owl:onDataRange xsd:string ;
		] ,
		[
			a owl:Restriction ;
			owl:onProperty observable:mimeType ;
			owl:maxQualifiedCardinality "1"^^xsd:nonNegativeInteger ;
			owl:onDataRange xsd:string ;
		]
		;
	rdfs:label "ContentDataFacet"@en ;
	rdfs:comment "A content data facet is a grouping of characteristics unique to a block of digital data."@en ;
	.

observable:CookieHistory
	a owl:Class ;
	rdfs:subClassOf observable:ObservableObject ;
	rdfs:label "CookieHistory"@en ;
	rdfs:comment "A cookie history is the stored web cookie history for a particular web browser."@en ;
	.

observable:Credential
	a owl:Class ;
	rdfs:subClassOf observable:ObservableObject ;
	rdfs:label "Credential"@en ;
	rdfs:comment "A credential is a single specific login and password combination for authorization of access to a digital account or system."@en ;
	.

observable:CredentialDump
	a owl:Class ;
	rdfs:subClassOf observable:ObservableObject ;
	rdfs:label "CredentialDump"@en ;
	rdfs:comment "A credential dump is a collection (typically forcibly extracted from a system) of specific login and password combinations for authorization of access to a digital account or system."@en ;
	.

observable:DNSCache
	a owl:Class ;
	rdfs:subClassOf observable:ObservableObject ;
	rdfs:label "DNSCache"@en ;
	rdfs:comment "An DNS cache is a temporary locally stored collection of previous Domain Name System (DNS) query results (created when an domain name is resolved to a IP address) for a particular computer."@en ;
	.

observable:DNSRecord
	a owl:Class ;
	rdfs:subClassOf observable:ObservableObject ;
	rdfs:label "DNSRecord"@en ;
	rdfs:comment "A DNS record is a single Domain Name System (DNS) artifact specifying information of a particular type (routing, authority, responsibility, security, etc.) for a specific Internet domain name."@en ;
	.

observable:DataRangeFacet
	a owl:Class ;
	rdfs:subClassOf
		<https://unifiedcyberontology.org/ontology/uco/core#Facet> ,
		[
			a owl:Restriction ;
			owl:onProperty observable:rangeOffset ;
			owl:maxQualifiedCardinality "1"^^xsd:nonNegativeInteger ;
			owl:onDataRange xsd:integer ;
		] ,
		[
			a owl:Restriction ;
			owl:onProperty observable:rangeSize ;
			owl:maxQualifiedCardinality "1"^^xsd:nonNegativeInteger ;
			owl:onDataRange xsd:integer ;
		] ,
		[
			a owl:Restriction ;
			owl:onProperty observable:rangeOffsetType ;
			owl:maxQualifiedCardinality "1"^^xsd:nonNegativeInteger ;
			owl:onDataRange xsd:string ;
		]
		;
	rdfs:label "DataRangeFacet"@en ;
	rdfs:comment "A data range facet is a grouping of characteristics unique to a particular contiguous scope within a block of digital data."@en ;
	.

observable:DefinedEffectFacet
	a owl:Class ;
	rdfs:subClassOf <https://unifiedcyberontology.org/ontology/uco/core#Facet> ;
	rdfs:label "DefinedEffectFacet"@en ;
	rdfs:comment "A defined effect facet is a grouping of characteristics unique to the effect of an observable action in relation to one or more observable objects."@en ;
	.

observable:Device
	a owl:Class ;
	rdfs:subClassOf observable:ObservableObject ;
	rdfs:label "Device"@en ;
	rdfs:comment "A device is a piece of equipment or a mechanism designed to serve a special purpose or perform a special function. [based on https://www.merriam-webster.com/dictionary/device]"@en ;
	.

observable:DeviceFacet
	a owl:Class ;
	rdfs:subClassOf
		<https://unifiedcyberontology.org/ontology/uco/core#Facet> ,
		[
			a owl:Restriction ;
			owl:onProperty observable:deviceType ;
			owl:maxCardinality "1"^^xsd:nonNegativeInteger ;
		] ,
		[
			a owl:Restriction ;
			owl:onProperty observable:manufacturer ;
			owl:maxQualifiedCardinality "1"^^xsd:nonNegativeInteger ;
			owl:onDataRange xsd:string ;
		] ,
		[
			a owl:Restriction ;
			owl:onProperty observable:model ;
			owl:maxQualifiedCardinality "1"^^xsd:nonNegativeInteger ;
			owl:onDataRange xsd:string ;
		] ,
		[
			a owl:Restriction ;
			owl:onProperty observable:serialNumber ;
			owl:maxQualifiedCardinality "1"^^xsd:nonNegativeInteger ;
			owl:onDataRange xsd:string ;
		]
		;
	rdfs:label "DeviceFacet"@en ;
	rdfs:comment "A device facet is a grouping of characteristics unique to a piece of equipment or a mechanism designed to serve a special purpose or perform a special function. [based on https://www.merriam-webster.com/dictionary/device]"@en ;
	.

observable:DigitalAccount
	a owl:Class ;
	rdfs:subClassOf observable:Account ;
	rdfs:label "DigitalAccount"@en ;
	rdfs:comment "A digital account is an arrangement with an entity to enable and control the provision of some capability or service within the digital domain."@en ;
	.

observable:DigitalAccountFacet
	a owl:Class ;
	rdfs:subClassOf
		<https://unifiedcyberontology.org/ontology/uco/core#Facet> ,
		[
			a owl:Restriction ;
			owl:onProperty observable:firstLoginTime ;
			owl:maxCardinality "1"^^xsd:nonNegativeInteger ;
		] ,
		[
			a owl:Restriction ;
			owl:onProperty observable:lastLoginTime ;
			owl:maxCardinality "1"^^xsd:nonNegativeInteger ;
		] ,
		[
			a owl:Restriction ;
			owl:onProperty observable:isDisabled ;
			owl:maxQualifiedCardinality "1"^^xsd:nonNegativeInteger ;
			owl:onDataRange xsd:boolean ;
		] ,
		[
			a owl:Restriction ;
			owl:onProperty observable:displayName ;
			owl:maxQualifiedCardinality "1"^^xsd:nonNegativeInteger ;
			owl:onDataRange xsd:string ;
		]
		;
	rdfs:label "DigitalAccountFacet"@en ;
	rdfs:comment "A digital account facet is a grouping of characteristics unique to an arrangement with an entity to enable and control the provision of some capability or service within the digital domain."@en ;
	.

observable:DigitalAddress
	a owl:Class ;
	rdfs:subClassOf observable:Address ;
	rdfs:label "DigitalAddress"@en ;
	rdfs:comment "A digital address is an identifier assigned to enable routing and management of digital communication."@en ;
	.

observable:DigitalAddressFacet
	a owl:Class ;
	rdfs:subClassOf
		<https://unifiedcyberontology.org/ontology/uco/core#Facet> ,
		[
			a owl:Restriction ;
			owl:onProperty observable:addressValue ;
			owl:cardinality "1"^^xsd:nonNegativeInteger ;
			owl:onDataRange xsd:string ;
		] ,
		[
			a owl:Restriction ;
			owl:onProperty observable:displayName ;
			owl:maxQualifiedCardinality "1"^^xsd:nonNegativeInteger ;
			owl:onDataRange xsd:string ;
		]
		;
	rdfs:label "DigitalAddressFacet"@en ;
	rdfs:comment "A digital address facet is a grouping of characteristics unique to an identifier assigned to enable routing and management of digital communication."@en ;
	.

observable:DigitalSignatureInfo
	a owl:Class ;
	rdfs:subClassOf observable:ObservableObject ;
	rdfs:label "DigitalSignatureInfo"@en ;
	rdfs:comment "A digital signature info is a value calculated via a mathematical scheme for demonstrating the authenticity of an electronic message or document."@en ;
	.

observable:DigitalSignatureInfoFacet
	a owl:Class ;
	rdfs:subClassOf
		<https://unifiedcyberontology.org/ontology/uco/core#Facet> ,
		[
			a owl:Restriction ;
			owl:onProperty observable:certificateIssuer ;
			owl:maxCardinality "1"^^xsd:nonNegativeInteger ;
		] ,
		[
			a owl:Restriction ;
			owl:onProperty observable:certificateSubject ;
			owl:maxCardinality "1"^^xsd:nonNegativeInteger ;
		] ,
		[
			a owl:Restriction ;
			owl:onProperty observable:signatureDescription ;
			owl:maxQualifiedCardinality "1"^^xsd:nonNegativeInteger ;
			owl:onDataRange xsd:string ;
		] ,
		[
			a owl:Restriction ;
			owl:onProperty observable:signatureExists ;
			owl:onDataRange xsd:boolean ;
			owl:qualifiedCardinality "1"^^xsd:nonNegativeInteger ;
		] ,
		[
			a owl:Restriction ;
			owl:onProperty observable:signatureVerified ;
			owl:onDataRange xsd:boolean ;
			owl:qualifiedCardinality "1"^^xsd:nonNegativeInteger ;
		]
		;
	rdfs:label "DigitalSignatureInfoFacet"@en ;
	rdfs:comment "A digital signature info facet is a grouping of characteristics unique to a value calculated via a mathematical scheme for demonstrating the authenticity of an electronic message or document."@en ;
	.

observable:Directory
	a owl:Class ;
	rdfs:subClassOf observable:FileSystemObject ;
	rdfs:label "Directory"@en ;
	rdfs:comment "A directory is a file system cataloging structure which contains references to other computer files, and possibly other directories. On many computers, directories are known as folders, or drawers, analogous to a workbench or the traditional office filing cabinet. In UNIX a directory is implemented as a special file. [based on https://en.wikipedia.org/wiki/Directory_(computing)]"@en ;
	.

observable:Disk
	a owl:Class ;
	rdfs:subClassOf observable:ObservableObject ;
	rdfs:label "Disk"@en ;
	rdfs:comment "A disk is a storage mechanism where data is recorded by various electronic, magnetic, optical, or mechanical changes to a surface layer of one or more rotating disks."@en ;
	.

observable:DiskFacet
	a owl:Class ;
	rdfs:subClassOf
		<https://unifiedcyberontology.org/ontology/uco/core#Facet> ,
		[
			a owl:Restriction ;
			owl:onProperty observable:diskType ;
			owl:maxCardinality "1"^^xsd:nonNegativeInteger ;
		] ,
		[
			a owl:Restriction ;
			owl:onProperty observable:diskSize ;
			owl:maxQualifiedCardinality "1"^^xsd:nonNegativeInteger ;
			owl:onDataRange xsd:integer ;
		] ,
		[
			a owl:Restriction ;
			owl:onProperty observable:freeSpace ;
			owl:maxQualifiedCardinality "1"^^xsd:nonNegativeInteger ;
			owl:onDataRange xsd:integer ;
		]
		;
	rdfs:label "DiskFacet"@en ;
	rdfs:comment "A disk facet is a grouping of characteristics unique to a storage mechanism where data is recorded by various electronic, magnetic, optical, or mechanical changes to a surface layer of one or more rotating disks."@en ;
	.

observable:DiskPartition
	a owl:Class ;
	rdfs:subClassOf observable:ObservableObject ;
	rdfs:label "DiskPartition"@en ;
	rdfs:comment "A disk partition is a particular managed region on a storage mechanism where data is recorded by various electronic, magnetic, optical, or mechanical changes to a surface layer of one or more rotating disks. [based on https://en.wikipedia.org/wiki/Disk_storage]"@en ;
	.

observable:DiskPartitionFacet
	a owl:Class ;
	rdfs:subClassOf
		<https://unifiedcyberontology.org/ontology/uco/core#Facet> ,
		[
			a owl:Restriction ;
			owl:onProperty observable:diskPartitionType ;
			owl:maxCardinality "1"^^xsd:nonNegativeInteger ;
		] ,
		[
			a owl:Restriction ;
			owl:onProperty observable:observableCreatedTime ;
			owl:maxCardinality "1"^^xsd:nonNegativeInteger ;
		] ,
		[
			a owl:Restriction ;
			owl:onProperty observable:partitionID ;
			owl:maxQualifiedCardinality "1"^^xsd:nonNegativeInteger ;
			owl:onDataRange xsd:integer ;
		] ,
		[
			a owl:Restriction ;
			owl:onProperty observable:partitionLength ;
			owl:maxQualifiedCardinality "1"^^xsd:nonNegativeInteger ;
			owl:onDataRange xsd:integer ;
		] ,
		[
			a owl:Restriction ;
			owl:onProperty observable:partitionOffset ;
			owl:maxQualifiedCardinality "1"^^xsd:nonNegativeInteger ;
			owl:onDataRange xsd:integer ;
		] ,
		[
			a owl:Restriction ;
			owl:onProperty observable:spaceLeft ;
			owl:maxQualifiedCardinality "1"^^xsd:nonNegativeInteger ;
			owl:onDataRange xsd:integer ;
		] ,
		[
			a owl:Restriction ;
			owl:onProperty observable:spaceUsed ;
			owl:maxQualifiedCardinality "1"^^xsd:nonNegativeInteger ;
			owl:onDataRange xsd:integer ;
		] ,
		[
			a owl:Restriction ;
			owl:onProperty observable:totalSpace ;
			owl:maxQualifiedCardinality "1"^^xsd:nonNegativeInteger ;
			owl:onDataRange xsd:integer ;
		] ,
		[
			a owl:Restriction ;
			owl:onProperty observable:mountPoint ;
			owl:maxQualifiedCardinality "1"^^xsd:nonNegativeInteger ;
			owl:onDataRange xsd:string ;
		]
		;
	rdfs:label "DiskPartitionFacet"@en ;
	rdfs:comment "A disk partition facet is a grouping of characteristics unique to a particular managed region on a storage mechanism."@en ;
	.

observable:DomainName
	a owl:Class ;
	rdfs:subClassOf observable:ObservableObject ;
	rdfs:label "DomainName"@en ;
	rdfs:comment "A domain name is an identification string that defines a realm of administrative autonomy, authority or control within the Internet. [based on https://en.wikipedia.org/wiki/Domain_name]"@en ;
	.

observable:DomainNameFacet
	a owl:Class ;
	rdfs:subClassOf
		<https://unifiedcyberontology.org/ontology/uco/core#Facet> ,
		[
			a owl:Restriction ;
			owl:onProperty observable:isTLD ;
			owl:maxQualifiedCardinality "1"^^xsd:nonNegativeInteger ;
			owl:onDataRange xsd:boolean ;
		] ,
		[
			a owl:Restriction ;
			owl:onProperty observable:value ;
			owl:onDataRange xsd:string ;
			owl:qualifiedCardinality "1"^^xsd:nonNegativeInteger ;
		]
		;
	rdfs:label "DomainNameFacet"@en ;
	rdfs:comment "A domain name facet is a grouping of characteristics unique to an identification string that defines a realm of administrative autonomy, authority or control within the Internet. [based on https://en.wikipedia.org/wiki/Domain_name]"@en ;
	.

observable:ESN
	a owl:DatatypeProperty ;
	rdfs:label "ESN"@en ;
	rdfs:comment "Electronic Serial Number ."@en ;
	rdfs:range xsd:string ;
	.

observable:EXIFFacet
	a owl:Class ;
	rdfs:subClassOf
		<https://unifiedcyberontology.org/ontology/uco/core#Facet> ,
		[
			a owl:Restriction ;
			owl:onProperty observable:exifData ;
			owl:minCardinality "1"^^xsd:nonNegativeInteger ;
		]
		;
	rdfs:label "EXIFFacet"@en ;
	rdfs:comment "An EXIF (exchangeable image file format) facet is a grouping of characteristics unique to the formats for images, sound, and ancillary tags used by digital cameras (including smartphones), scanners and other systems handling image and sound files recorded by digital cameras conformant to JEIDA/JEITA/CIPA specifications. [based on https://en.wikipedia.org/wiki/Exif]"@en ;
	.

observable:EmailAccount
	a owl:Class ;
	rdfs:subClassOf observable:DigitalAccount ;
	rdfs:label "EmailAccount"@en ;
	rdfs:comment "An email account is an arrangement with an entity to enable and control the provision of electronic mail (email) capabilities or services."@en ;
	.

observable:EmailAccountFacet
	a owl:Class ;
	rdfs:subClassOf
		<https://unifiedcyberontology.org/ontology/uco/core#Facet> ,
		[
			a owl:Restriction ;
			owl:onProperty observable:emailAddress ;
			owl:onClass observable:ObservableObject ;
			owl:qualifiedCardinality "1"^^xsd:nonNegativeInteger ;
		]
		;
	rdfs:label "EmailAccountFacet"@en ;
	rdfs:comment "An email account facet is a grouping of characteristics unique to an arrangement with an entity to enable and control the provision of electronic mail (email) capabilities or services."@en ;
	.

observable:EmailAddress
	a owl:Class ;
	rdfs:subClassOf observable:DigitalAddress ;
	rdfs:label "EmailAddress"@en ;
	rdfs:comment "An email address is an identifier for an electronic mailbox to which electronic mail messages (conformant to the Simple Mail Transfer Protocol (SMTP)) are sent from and delivered to."@en ;
	.

observable:EmailAddressFacet
	a owl:Class ;
	rdfs:subClassOf
		<https://unifiedcyberontology.org/ontology/uco/core#DigitalAddressFacet> ,
		[
			a owl:Restriction ;
			owl:onProperty observable:displayName ;
			owl:maxQualifiedCardinality "1"^^xsd:nonNegativeInteger ;
			owl:onDataRange xsd:string ;
		] ,
		[
			a owl:Restriction ;
			owl:onProperty observable:addressValue ;
			owl:onDataRange xsd:string ;
			owl:qualifiedCardinality "1"^^xsd:nonNegativeInteger ;
		]
		;
	rdfs:label "EmailAddressFacet"@en ;
	rdfs:comment "An email address facet is a grouping of characteristics unique to an identifier for an electronic mailbox to which electronic mail messages (conformant to the Simple Mail Transfer Protocol (SMTP)) are sent from and delivered to."@en ;
	.

observable:EmailMessage
	a owl:Class ;
	rdfs:subClassOf observable:Message ;
	rdfs:label "EmailMessage"@en ;
	rdfs:comment "An email message is a message that is an instance of an electronic mail correspondence conformant to the internet message format described in RFC 5322 and related RFCs."@en ;
	.

observable:EmailMessageFacet
	a owl:Class ;
	rdfs:subClassOf
		<https://unifiedcyberontology.org/ontology/uco/core#Facet> ,
		[
			a owl:Restriction ;
			owl:onProperty observable:modifiedTime ;
			owl:maxCardinality "1"^^xsd:nonNegativeInteger ;
		] ,
		[
			a owl:Restriction ;
			owl:onProperty observable:otherHeaders ;
			owl:maxCardinality "1"^^xsd:nonNegativeInteger ;
		] ,
		[
			a owl:Restriction ;
			owl:onProperty observable:receivedTime ;
			owl:maxCardinality "1"^^xsd:nonNegativeInteger ;
		] ,
		[
			a owl:Restriction ;
			owl:onProperty observable:sentTime ;
			owl:maxCardinality "1"^^xsd:nonNegativeInteger ;
		] ,
		[
			a owl:Restriction ;
			owl:onProperty observable:application ;
			owl:onClass observable:ObservableObject ;
			owl:maxQualifiedCardinality "1"^^xsd:nonNegativeInteger ;
		] ,
		[
			a owl:Restriction ;
			owl:onProperty observable:bodyRaw ;
			owl:onClass observable:ObservableObject ;
			owl:maxQualifiedCardinality "1"^^xsd:nonNegativeInteger ;
		] ,
		[
			a owl:Restriction ;
			owl:onProperty observable:from ;
			owl:onClass observable:ObservableObject ;
			owl:maxQualifiedCardinality "1"^^xsd:nonNegativeInteger ;
		] ,
		[
			a owl:Restriction ;
			owl:onProperty observable:headerRaw ;
			owl:onClass observable:ObservableObject ;
			owl:maxQualifiedCardinality "1"^^xsd:nonNegativeInteger ;
		] ,
		[
			a owl:Restriction ;
			owl:onProperty observable:inReplyTo ;
			owl:onClass observable:ObservableObject ;
			owl:maxQualifiedCardinality "1"^^xsd:nonNegativeInteger ;
		] ,
		[
			a owl:Restriction ;
			owl:onProperty observable:sender ;
			owl:onClass observable:ObservableObject ;
			owl:maxQualifiedCardinality "1"^^xsd:nonNegativeInteger ;
		] ,
		[
			a owl:Restriction ;
			owl:onProperty observable:xOriginatingIP ;
			owl:onClass observable:ObservableObject ;
			owl:maxQualifiedCardinality "1"^^xsd:nonNegativeInteger ;
		] ,
		[
			a owl:Restriction ;
			owl:onProperty observable:isRead ;
			owl:maxQualifiedCardinality "1"^^xsd:nonNegativeInteger ;
			owl:onDataRange xsd:boolean ;
		] ,
		[
			a owl:Restriction ;
			owl:onProperty observable:body ;
			owl:maxQualifiedCardinality "1"^^xsd:nonNegativeInteger ;
			owl:onDataRange xsd:string ;
		] ,
		[
			a owl:Restriction ;
			owl:onProperty observable:contentDisposition ;
			owl:maxQualifiedCardinality "1"^^xsd:nonNegativeInteger ;
			owl:onDataRange xsd:string ;
		] ,
		[
			a owl:Restriction ;
			owl:onProperty observable:contentType ;
			owl:maxQualifiedCardinality "1"^^xsd:nonNegativeInteger ;
			owl:onDataRange xsd:string ;
		] ,
		[
			a owl:Restriction ;
			owl:onProperty observable:messageID ;
			owl:maxQualifiedCardinality "1"^^xsd:nonNegativeInteger ;
			owl:onDataRange xsd:string ;
		] ,
		[
			a owl:Restriction ;
			owl:onProperty observable:priority ;
			owl:maxQualifiedCardinality "1"^^xsd:nonNegativeInteger ;
			owl:onDataRange xsd:string ;
		] ,
		[
			a owl:Restriction ;
			owl:onProperty observable:subject ;
			owl:maxQualifiedCardinality "1"^^xsd:nonNegativeInteger ;
			owl:onDataRange xsd:string ;
		] ,
		[
			a owl:Restriction ;
			owl:onProperty observable:xMailer ;
			owl:maxQualifiedCardinality "1"^^xsd:nonNegativeInteger ;
			owl:onDataRange xsd:string ;
		] ,
		[
			a owl:Restriction ;
			owl:onProperty observable:isMimeEncoded ;
			owl:onDataRange xsd:boolean ;
			owl:qualifiedCardinality "1"^^xsd:nonNegativeInteger ;
		] ,
		[
			a owl:Restriction ;
			owl:onProperty observable:isMultipart ;
			owl:onDataRange xsd:boolean ;
			owl:qualifiedCardinality "1"^^xsd:nonNegativeInteger ;
		]
		;
	rdfs:label "EmailMessageFacet"@en ;
	rdfs:comment "An email message facet is a grouping of characteristics unique to a message that is an instance of an electronic mail correspondence conformant to the internet message format described in RFC 5322 and related RFCs."@en ;
	.

observable:EncodedStreamFacet
	a owl:Class ;
	rdfs:subClassOf
		<https://unifiedcyberontology.org/ontology/uco/core#Facet> ,
		[
			a owl:Restriction ;
			owl:onProperty observable:encodingMethod ;
			owl:maxQualifiedCardinality "1"^^xsd:nonNegativeInteger ;
			owl:onDataRange xsd:string ;
		]
		;
	rdfs:label "EncodedStreamFacet"@en ;
	rdfs:comment "An encoded stream facet is a grouping of characteristics unique to the conversion of a body of data content from one form to another form."@en ;
	.

observable:EncryptedStreamFacet
	a owl:Class ;
	rdfs:subClassOf
		<https://unifiedcyberontology.org/ontology/uco/core#Facet> ,
		[
			a owl:Restriction ;
			owl:onProperty observable:encryptionMethod ;
			owl:maxCardinality "1"^^xsd:nonNegativeInteger ;
		] ,
		[
			a owl:Restriction ;
			owl:onProperty observable:encryptionMode ;
			owl:maxCardinality "1"^^xsd:nonNegativeInteger ;
		]
		;
	rdfs:label "EncryptedStreamFacet"@en ;
	rdfs:comment "An encrypted stream facet is a grouping of characteristics unique to the conversion of a body of data content from one form to another obfuscated form in such a way that reversing the conversion to obtain the original data form can only be accomplished through possession and use of a specific key."@en ;
	.

observable:EnvironmentVariable
	a owl:Class ;
	rdfs:subClassOf
		[
			a owl:Restriction ;
			owl:onProperty observable:value ;
			owl:maxQualifiedCardinality "1"^^xsd:nonNegativeInteger ;
			owl:onDataRange xsd:string ;
		] ,
		[
			a owl:Restriction ;
			owl:onProperty <https://unifiedcyberontology.org/ontology/uco/core#name> ;
			owl:onDataRange xsd:string ;
			owl:qualifiedCardinality "1"^^xsd:nonNegativeInteger ;
		]
		;
	rdfs:label "EnvironmentVariable"@en ;
	rdfs:comment "An environment variable is a grouping of characteristics unique to a dynamic-named value that can affect the way running processes will behave on a computer. [based on https://en.wikipedia.org/wiki/Environment_variable]"@en ;
	.

observable:Event
	a owl:Class ;
	rdfs:subClassOf observable:ObservableObject ;
	rdfs:label "Event"@en ;
	rdfs:comment "An event is something that happens in a digital context (e.g., operating system events)."@en ;
	.

observable:EventFacet
	a owl:Class ;
	rdfs:subClassOf
		<https://unifiedcyberontology.org/ontology/uco/core#Facet> ,
		[
			a owl:Restriction ;
			owl:onProperty observable:observableCreatedTime ;
			owl:maxCardinality "1"^^xsd:nonNegativeInteger ;
		] ,
		[
			a owl:Restriction ;
			owl:onProperty observable:cyberAction ;
			owl:onClass observable:ObservableAction ;
			owl:maxQualifiedCardinality "1"^^xsd:nonNegativeInteger ;
		] ,
		[
			a owl:Restriction ;
			owl:onProperty observable:computerName ;
			owl:maxQualifiedCardinality "1"^^xsd:nonNegativeInteger ;
			owl:onDataRange xsd:string ;
		] ,
		[
			a owl:Restriction ;
			owl:onProperty observable:eventID ;
			owl:maxQualifiedCardinality "1"^^xsd:nonNegativeInteger ;
			owl:onDataRange xsd:string ;
		] ,
		[
			a owl:Restriction ;
			owl:onProperty observable:eventText ;
			owl:maxQualifiedCardinality "1"^^xsd:nonNegativeInteger ;
			owl:onDataRange xsd:string ;
		] ,
		[
			a owl:Restriction ;
			owl:onProperty observable:eventType ;
			owl:maxQualifiedCardinality "1"^^xsd:nonNegativeInteger ;
			owl:onDataRange xsd:string ;
		] ,
		[
			a owl:Restriction ;
			owl:onProperty observable:application ;
			owl:onClass observable:ObservableObject ;
			owl:qualifiedCardinality "1"^^xsd:nonNegativeInteger ;
		]
		;
	rdfs:label "EventFacet"@en ;
	rdfs:comment "An event facet is a grouping of characteristics unique to something that happens in a digital context (e.g., operating system events)."@en ;
	.

observable:EventLog
	a owl:Class ;
	rdfs:subClassOf observable:ObservableObject ;
	rdfs:label "EventLog"@en ;
	rdfs:comment "An event log is a recorded collection of events."@en ;
	.

observable:ExtInodeFacet
	a owl:Class ;
	rdfs:subClassOf
		<https://unifiedcyberontology.org/ontology/uco/core#Facet> ,
		[
			a owl:Restriction ;
			owl:onProperty observable:extDeletionTime ;
			owl:maxCardinality "1"^^xsd:nonNegativeInteger ;
		] ,
		[
			a owl:Restriction ;
			owl:onProperty observable:extInodeChangeTime ;
			owl:maxCardinality "1"^^xsd:nonNegativeInteger ;
		] ,
		[
			a owl:Restriction ;
			owl:onProperty observable:extFileType ;
			owl:maxQualifiedCardinality "1"^^xsd:nonNegativeInteger ;
			owl:onDataRange xsd:integer ;
		] ,
		[
			a owl:Restriction ;
			owl:onProperty observable:extFlags ;
			owl:maxQualifiedCardinality "1"^^xsd:nonNegativeInteger ;
			owl:onDataRange xsd:integer ;
		] ,
		[
			a owl:Restriction ;
			owl:onProperty observable:extHardLinkCount ;
			owl:maxQualifiedCardinality "1"^^xsd:nonNegativeInteger ;
			owl:onDataRange xsd:integer ;
		] ,
		[
			a owl:Restriction ;
			owl:onProperty observable:extInodeID ;
			owl:maxQualifiedCardinality "1"^^xsd:nonNegativeInteger ;
			owl:onDataRange xsd:integer ;
		] ,
		[
			a owl:Restriction ;
			owl:onProperty observable:extPermissions ;
			owl:maxQualifiedCardinality "1"^^xsd:nonNegativeInteger ;
			owl:onDataRange xsd:integer ;
		] ,
		[
			a owl:Restriction ;
			owl:onProperty observable:extSGID ;
			owl:maxQualifiedCardinality "1"^^xsd:nonNegativeInteger ;
			owl:onDataRange xsd:integer ;
		] ,
		[
			a owl:Restriction ;
			owl:onProperty observable:extSUID ;
			owl:maxQualifiedCardinality "1"^^xsd:nonNegativeInteger ;
			owl:onDataRange xsd:integer ;
		]
		;
	rdfs:label "ExtInodeFacet"@en ;
	rdfs:comment "An extInode facet is a grouping of characteristics unique to a file system object (file, directory, etc.) conformant to the extended file system (EXT or related derivations) specification."@en ;
	.

observable:ExtractedString
	a owl:Class ;
	rdfs:subClassOf
		[
			a owl:Restriction ;
			owl:onProperty observable:byteStringValue ;
			owl:maxCardinality "1"^^xsd:nonNegativeInteger ;
		] ,
		[
			a owl:Restriction ;
			owl:onProperty observable:encoding ;
			owl:maxCardinality "1"^^xsd:nonNegativeInteger ;
		] ,
		[
			a owl:Restriction ;
			owl:onProperty observable:language ;
			owl:maxCardinality "1"^^xsd:nonNegativeInteger ;
		] ,
		[
			a owl:Restriction ;
			owl:onProperty observable:length ;
			owl:maxQualifiedCardinality "1"^^xsd:nonNegativeInteger ;
			owl:onDataRange xsd:integer ;
		] ,
		[
			a owl:Restriction ;
			owl:onProperty observable:englishTranslation ;
			owl:maxQualifiedCardinality "1"^^xsd:nonNegativeInteger ;
			owl:onDataRange xsd:string ;
		] ,
		[
			a owl:Restriction ;
			owl:onProperty observable:stringValue ;
			owl:maxQualifiedCardinality "1"^^xsd:nonNegativeInteger ;
			owl:onDataRange xsd:string ;
		]
		;
	rdfs:label "ExtractedString"@en ;
	rdfs:comment "An extracted string is a grouping of characteristics unique to a series of characters pulled from an observable object."@en ;
	.

observable:ExtractedStringsFacet
	a owl:Class ;
	rdfs:subClassOf <https://unifiedcyberontology.org/ontology/uco/core#Facet> ;
	rdfs:label "ExtractedStringsFacet"@en ;
	rdfs:comment "An extracted strings facet is a grouping of characteristics unique to one or more sequences of characters pulled from an observable object."@en ;
	.

observable:File
	a owl:Class ;
	rdfs:subClassOf observable:FileSystemObject ;
	rdfs:label "File"@en ;
	rdfs:comment "A file is a computer resource for recording data discretely on a computer storage device."@en ;
	.

observable:FileFacet
	a owl:Class ;
	rdfs:subClassOf
		<https://unifiedcyberontology.org/ontology/uco/core#Facet> ,
		[
			a owl:Restriction ;
			owl:onProperty observable:accessedTime ;
			owl:maxCardinality "1"^^xsd:nonNegativeInteger ;
		] ,
		[
			a owl:Restriction ;
			owl:onProperty observable:fileSystemType ;
			owl:maxCardinality "1"^^xsd:nonNegativeInteger ;
		] ,
		[
			a owl:Restriction ;
			owl:onProperty observable:metadataChangeTime ;
			owl:maxCardinality "1"^^xsd:nonNegativeInteger ;
		] ,
		[
			a owl:Restriction ;
			owl:onProperty observable:modifiedTime ;
			owl:maxCardinality "1"^^xsd:nonNegativeInteger ;
		] ,
		[
			a owl:Restriction ;
			owl:onProperty observable:observableCreatedTime ;
			owl:maxCardinality "1"^^xsd:nonNegativeInteger ;
		] ,
		[
			a owl:Restriction ;
			owl:onProperty observable:sizeInBytes ;
			owl:maxQualifiedCardinality "1"^^xsd:nonNegativeInteger ;
			owl:onDataRange xsd:integer ;
		] ,
		[
			a owl:Restriction ;
			owl:onProperty observable:allocationStatus ;
			owl:maxQualifiedCardinality "1"^^xsd:nonNegativeInteger ;
			owl:onDataRange xsd:string ;
		] ,
		[
			a owl:Restriction ;
			owl:onProperty observable:extension ;
			owl:maxQualifiedCardinality "1"^^xsd:nonNegativeInteger ;
			owl:onDataRange xsd:string ;
		]
		;
	rdfs:label "FileFacet"@en ;
	rdfs:comment "A file facet is a grouping of characteristics unique to the storage of a file (computer resource for recording data discretely in a computer storage device) on a file system (process that manages how and where data on a storage device is stored, accessed and managed). [based on https://en.wikipedia.org/Computer_file and https://www.techopedia.com/definition/5510/file-system]"@en ;
	.

observable:FilePermissionsFacet
	a owl:Class ;
	rdfs:subClassOf
		<https://unifiedcyberontology.org/ontology/uco/core#Facet> ,
		[
			a owl:Restriction ;
			owl:onProperty observable:owner ;
			owl:onClass observable:ObservableObject ;
			owl:maxQualifiedCardinality "1"^^xsd:nonNegativeInteger ;
		]
		;
	rdfs:label "FilePermissionsFacet"@en ;
	rdfs:comment "A file permissions facet is a grouping of characteristics unique to the access rights (e.g., view, change, navigate, execute) of a file on a file system."@en ;
	.

observable:FileSystem
	a owl:Class ;
	rdfs:subClassOf observable:ObservableObject ;
	rdfs:label "FileSystem"@en ;
	rdfs:commenet "A file system is the process that manages how and where data on a storage medium is stored, accessed and managed. [based on https://www.techopedia.com/definition/5510/file-system]"@en ;
	.

observable:FileSystemFacet
	a owl:Class ;
	rdfs:subClassOf
		<https://unifiedcyberontology.org/ontology/uco/core#Facet> ,
		[
			a owl:Restriction ;
			owl:onProperty observable:fileSystemType ;
			owl:maxCardinality "1"^^xsd:nonNegativeInteger ;
		] ,
		[
			a owl:Restriction ;
			owl:onProperty observable:clusterSize ;
			owl:maxQualifiedCardinality "1"^^xsd:nonNegativeInteger ;
			owl:onDataRange xsd:integer ;
		]
		;
	rdfs:label "FileSystemFacet"@en ;
	rdfs:comment "A file system facet is a grouping of characteristics unique to the process that manages how and where data on a storage medium is stored, accessed and managed. [based on https://www.techopedia.com/definition/5510/file-system]"@en ;
	.

observable:FileSystemObject
	a owl:Class ;
	rdfs:subClassOf observable:ObservableObject ;
	rdfs:label "FileSystemObject"@en ;
	rdfs:comment "A file system object is an informational object represented and managed within a file system."@en ;
	.

observable:ForumPost
	a owl:Class ;
	rdfs:subClassOf observable:Message ;
	rdfs:label "ForumPost"@en ;
	rdfs:comment "A forum post is message submitted by a user account to an online forum where the message content (and typically metadata including who posted it and when) is viewable by any party with viewing permissions on the forum."@en ;
	.

observable:ForumPrivateMessage
	a owl:Class ;
	rdfs:subClassOf observable:Message ;
	rdfs:label "ForumPrivateMessage"@en ;
	rdfs:comment "A forum private message (aka PM or DM (direct message)) is a one-to-one message from one specific user account to another specific user account on an online form where transmission is managed by the online forum platform and the message is only viewable by the parties directly involved."@en ;
	.

observable:FragmentFacet
	a owl:Class ;
	rdfs:subClassOf <https://unifiedcyberontology.org/ontology/uco/core#Facet> ;
	rdfs:label "FragmentFacet"@en ;
	rdfs:comment "A fragment facet is a grouping of characteristics unique to an individual piece of the content of a file."@en ;
	.

observable:GUI
	a owl:Class ;
	rdfs:subClassOf observable:ObservableObject ;
	rdfs:label "GUI"@en ;
	rdfs:comment "A GUI is a graphical user interface that allows users to interact with electronic devices through graphical icons and audio indicators such as primary notation, instead of text-based user interfaces, typed command labels or text navigation. [based on https://en.wikipedia.org/wiki/Graphical_user_interface]"@en ;
	.

observable:GenericObservableObject
	a owl:Class ;
	rdfs:subClassOf observable:ObservableObject ;
	rdfs:label "GenericObservableObject"@en ;
	rdfs:comment "A generic observable object is an article or unit within the digital domain."@en ;
	.

observable:GeoLocationEntry
	a owl:Class ;
	rdfs:label "GeoLocationEntry"@en ;
	rdfs:comment "A geolocation entry is a single application-specific geolocation entry."@en ;
	rdfs:subCassOf observable:ObservableObject ;
	.

observable:GeoLocationEntryFacet
	a owl:Class ;
	rdfs:subClassOf
		<https://unifiedcyberontology.org/ontology/uco/core#Facet> ,
		[
			a owl:Restriction ;
			owl:onProperty observable:location ;
			owl:maxCardinality "1"^^xsd:nonNegativeInteger ;
		] ,
		[
			a owl:Restriction ;
			owl:onProperty observable:observableCreatedTime ;
			owl:maxCardinality "1"^^xsd:nonNegativeInteger ;
		] ,
		[
			a owl:Restriction ;
			owl:onProperty observable:application ;
			owl:onClass observable:ObservableObject ;
			owl:qualifiedCardinality "1"^^xsd:nonNegativeInteger ;
		]
		;
	rdfs:label "GeoLocationEntryFacet"@en ;
	rdfs:comment "A geolocation entry facet is a grouping of characteristics unique to a single application-specific geolocation entry."@en ;
	.

observable:GeoLocationLog
	a owl:Class ;
	rdfs:subClassOf observable:ObservableObject ;
	rdfs:label "GeoLocationLog"@en ;
	rdfs:comment "A geolocation log is a record containing geolocation tracks and/or geolocation entries."@en ;
	.

observable:GeoLocationLogFacet
	a owl:Class ;
	rdfs:subClassOf
		<https://unifiedcyberontology.org/ontology/uco/core#Facet> ,
		[
			a owl:Restriction ;
			owl:onProperty observable:observableCreatedTime ;
			owl:maxCardinality "1"^^xsd:nonNegativeInteger ;
		] ,
		[
			a owl:Restriction ;
			owl:onProperty observable:application ;
			owl:onClass observable:ObservableObject ;
			owl:qualifiedCardinality "1"^^xsd:nonNegativeInteger ;
		]
		;
	rdfs:label "GeoLocationLogFacet"@en ;
	rdfs:comment "A geolocation log facet is a grouping of characteristics unique to a record containing geolocation tracks and/or geolocation entries."@en ;
	.

observable:GeoLocationTrack
	a owl:Class ;
	rdfs:subClassOf observable:ObservableObject ;
	rdfs:label "GeoLocationTrack"@en ;
	rdfs:comment "A geolocation track is a set of contiguous geolocation entries representing a path/track taken."@en ;
	.

observable:GeoLocationTrackFacet
	a owl:Class ;
	rdfs:subClassOf
		<https://unifiedcyberontology.org/ontology/uco/core#Facet> ,
		[
			a owl:Restriction ;
			owl:onProperty observable:endTime ;
			owl:maxCardinality "1"^^xsd:nonNegativeInteger ;
		] ,
		[
			a owl:Restriction ;
			owl:onProperty observable:startTime ;
			owl:maxCardinality "1"^^xsd:nonNegativeInteger ;
		] ,
		[
			a owl:Restriction ;
			owl:onProperty observable:application ;
			owl:onClass observable:ObservableObject ;
			owl:qualifiedCardinality "1"^^xsd:nonNegativeInteger ;
		]
		;
	rdfs:label "GeoLocationTrackFacet"@en ;
	rdfs:comment "A geolocation track facet is a grouping of characteristics unique to a set of contiguous geolocation entries representing a path/track taken."@en ;
	.

observable:GlobalFlagType
	a owl:Class ;
	rdfs:subClassOf
		[
			a owl:Restriction ;
			owl:onProperty observable:abbreviation ;
			owl:maxQualifiedCardinality "1"^^xsd:nonNegativeInteger ;
			owl:onDataRange xsd:string ;
		] ,
		[
			a owl:Restriction ;
			owl:onProperty observable:destination ;
			owl:maxQualifiedCardinality "1"^^xsd:nonNegativeInteger ;
			owl:onDataRange xsd:string ;
		] ,
		[
			a owl:Restriction ;
			owl:onProperty observable:symbolicName ;
			owl:maxQualifiedCardinality "1"^^xsd:nonNegativeInteger ;
			owl:onDataRange xsd:string ;
		]
		;
	rdfs:label "GlobalFlagType"@en ;
	rdfs:comment 'A global flag type is a grouping of characteristics unique to the Windows systemwide global variable named NtGlobalFlag that enables various internal debugging, tracing, and validation support in the operating system. [based on "Windows Global Flags, Chapter 3: System Mechanisms of Windows Internals by Solomon, Russinovich, and Ionescu]'@en ;
	.

observable:HTTPConnection
	a owl:Class ;
	rdfs:subClassOf observable:NetworkConnection ;
	rdfs:label "HTTPConnection"@en ;
	rdfs:comment "An HTTP connection is network connection that is conformant to the Hypertext Transfer Protocol (HTTP) standard."@en ;
	.

observable:HTTPConnectionFacet
	a owl:Class ;
	rdfs:subClassOf
		<https://unifiedcyberontology.org/ontology/uco/core#Facet> ,
		[
			a owl:Restriction ;
			owl:onProperty observable:httpRequestHeader ;
			owl:maxCardinality "1"^^xsd:nonNegativeInteger ;
		] ,
		[
			a owl:Restriction ;
			owl:onProperty observable:httpMessageBodyData ;
			owl:onClass observable:ObservableObject ;
			owl:maxQualifiedCardinality "1"^^xsd:nonNegativeInteger ;
		] ,
		[
			a owl:Restriction ;
			owl:onProperty observable:httpMesageBodyLength ;
			owl:maxQualifiedCardinality "1"^^xsd:nonNegativeInteger ;
			owl:onDataRange xsd:integer ;
		] ,
		[
			a owl:Restriction ;
			owl:onProperty observable:requestVersion ;
			owl:maxQualifiedCardinality "1"^^xsd:nonNegativeInteger ;
			owl:onDataRange xsd:string ;
		] ,
		[
			a owl:Restriction ;
			owl:onProperty observable:requestMethod ;
			owl:onDataRange xsd:string ;
			owl:qualifiedCardinality "1"^^xsd:nonNegativeInteger ;
		] ,
		[
			a owl:Restriction ;
			owl:onProperty observable:requestValue ;
			owl:onDataRange xsd:string ;
			owl:qualifiedCardinality "1"^^xsd:nonNegativeInteger ;
		]
		;
	rdfs:label "HTTPConnectionFacet"@en ;
	rdfs:comment "An HTTP connection facet is a grouping of characteristics unique to portions of a network connection that are conformant to the Hypertext Transfer Protocol (HTTP) standard."@en ;
	.

observable:Hostname
	a owl:Class ;
	rdfs:subClassOf observable:ObservableObject ;
	rdfs:label "Hostname"@en ;
	rdfs:comment "A hostname is a label that is assigned to a device connected to a computer network and that is used to identify the device in various forms of electronic communication, such as the World Wide Web. A hostname may be a domain name, if it is properly organized into the domain name system. A domain name may be a hostname if it has been assigned to an Internet host and associated with the host's IP address. [based on https://en.wikipedia.org/wiki/Hostname]"@en ;
	.

observable:ICCID
	a owl:DatatypeProperty ;
	rdfs:label "ICCID"@en ;
	rdfs:comment "Integrated circuit card identifier (http://www.itu.int/)."@en ;
	rdfs:range xsd:string ;
	.

observable:ICMPConnection
	a owl:Class ;
	rdfs:subClassOf observable:NetworkConnection ;
	rdfs:label "ICMPConnection"@en ;
	rdfs:comment "An ICMP connection is a network connection that is conformant to the Internet Control Message Protocol (ICMP) standard."@en ;
	.

observable:ICMPConnectionFacet
	a owl:Class ;
	rdfs:subClassOf <https://unifiedcyberontology.org/ontology/uco/core#Facet> ;
	rdfs:label "ICMPConnectionFacet"@en ;
	rdfs:comment "An ICMP connection facet is a grouping of characteristics unique to portions of a network connection that are conformant to the Internet Control Message Protocol (ICMP) standard."@en ;
	.

observable:IComHandlerActionType
	a owl:Class ;
	rdfs:subClassOf
		[
			a owl:Restriction ;
			owl:onProperty observable:comClassID ;
			owl:maxQualifiedCardinality "1"^^xsd:nonNegativeInteger ;
			owl:onDataRange xsd:string ;
		] ,
		[
			a owl:Restriction ;
			owl:onProperty observable:comData ;
			owl:maxQualifiedCardinality "1"^^xsd:nonNegativeInteger ;
			owl:onDataRange xsd:string ;
		]
		;
	rdfs:label "IComHandlerActionType"@en ;
	rdfs:comment "An IComHandler action type is a grouping of characteristics unique to a Windows Task-related action that fires a Windows COM handler (smart code in the client address space that can optimize calls between a client and server). [based on https://docs.microsoft.com/en-us/windows/win32/taskschd/comhandleraction]"@en ;
	.

observable:IExecActionType
	a owl:Class ;
	rdfs:subClassOf
		[
			a owl:Restriction ;
			owl:onProperty observable:execArguments ;
			owl:maxQualifiedCardinality "1"^^xsd:nonNegativeInteger ;
			owl:onDataRange xsd:string ;
		] ,
		[
			a owl:Restriction ;
			owl:onProperty observable:execProgramPath ;
			owl:maxQualifiedCardinality "1"^^xsd:nonNegativeInteger ;
			owl:onDataRange xsd:string ;
		] ,
		[
			a owl:Restriction ;
			owl:onProperty observable:execWorkingDirectory ;
			owl:maxQualifiedCardinality "1"^^xsd:nonNegativeInteger ;
			owl:onDataRange xsd:string ;
		]
		;
	rdfs:label "IExecActionType"@en ;
	rdfs:comment "An IExec action type is a grouping of characteristics unique to an action that executes a command-line operation on a Windows operating system. [based on https://docs.microsoft.com/en-us/windows/win32/api/taskschd/nn-taskschd-iexecaction?redirectedfrom=MSDN]"@en ;
	.

observable:IMEI
	a owl:DatatypeProperty ;
	rdfs:label "IMEI"@en ;
	rdfs:comment "International Mobile Equipment Identity (IMEI)."@en ;
	rdfs:range xsd:string ;
	.

observable:IMSI
	a owl:DatatypeProperty ;
	rdfs:label "IMSI"@en ;
	rdfs:comment "An International Mobile Subscriber Identity (IMSI) is a unique identification associated with all GSM and UMTS network mobile phone users. It is stored as a 64-bit field in the SIM inside the phone and is sent by the phone to the network."@en ;
	rdfs:range xsd:string ;
	.

observable:IPAddress
	a owl:Class ;
	rdfs:subClassOf observable:DigitalAddress ;
	rdfs:label "IPAddress"@en ;
	rdfs:comment "An IP address is an Internet Protocol (IP) standards conformant identifier assigned to a device to enable routing and management of IP standards conformant communication to or from that device."@en ;
	.

observable:IPAddressFacet
	a owl:Class ;
	rdfs:subClassOf
		<https://unifiedcyberontology.org/ontology/uco/core#DigitalAddressFacet> ,
		[
			a owl:Restriction ;
			owl:onProperty observable:addressValue ;
			owl:cardinality "1"^^xsd:nonNegativeInteger ;
			owl:onDataRange xsd:string ;
		] ,
		[
			a owl:Restriction ;
			owl:onProperty observable:displayName ;
			owl:maxQualifiedCardinality "1"^^xsd:nonNegativeInteger ;
			owl:onDataRange xsd:string ;
		]
		;
	rdfs:label "IPAddressFacet"@en ;
	rdfs:comment "An IP address facet is a grouping of characteristics unique to an Internet Protocol (IP) standards conformant identifier assigned to a device to enable routing and management of IP standards conformant communication to or from that device."@en ;
	.

observable:IPNetmask
	a owl:Class ;
	rdfs:subClassOf observable:ObservableObject ;
	rdfs:label "IPNetmask"@en ;
	rdfs:comment "An IP netmask is a 32-bit \"mask\" used to divide an IP address into subnets and specify the network's available hosts."@en ;
	.

observable:IPv4Address
	a owl:Class ;
	rdfs:subClassOf observable:IPAddress ;
	rdfs:label "IPv4Address"@en ;
	rdfs:comment "An IPv4 (Internet Protocol version 4) address is an IPv4 standards conformant identifier assigned to a device to enable routing and management of IPv4 standards conformant communication to or from that device."@en ;
	.

observable:IPv4AddressFacet
	a owl:Class ;
	rdfs:subClassOf
		<https://unifiedcyberontology.org/ontology/uco/core#IPAddressFacet> ,
		[
			a owl:Restriction ;
			owl:onProperty observable:addressValue ;
			owl:onDataRange xsd:string ;
			owl:qualifiedCardinality "1"^^xsd:nonNegativeInteger ;
		]
		;
	rdfs:label "IPv4AddressFacet"@en ;
	rdfs:comment "An IPv4 (Internet Protocol version 4) address facet is a grouping of characteristics unique to an IPv4 standards conformant identifier assigned to a device to enable routing and management of IPv4 standards conformant communication to or from that device."@en ;
	.

observable:IPv6Address
	a owl:Class ;
	rdfs:subClassOf observable:IPAddress ;
	rdfs:label "IPv6Address"@en ;
	rdfs:comment "An IPv6 (Internet Protocol version 6) address is an IPv6 standards conformant identifier assigned to a device to enable routing and management of IPv6 standards conformant communication to or from that device."@en ;
	.

observable:IPv6AddressFacet
	a owl:Class ;
	rdfs:subClassOf
		<https://unifiedcyberontology.org/ontology/uco/core#IPAddressFacet> ,
		[
			a owl:Restriction ;
			owl:onProperty observable:addressValue ;
			owl:onDataRange xsd:string ;
			owl:qualifiedCardinality "1"^^xsd:nonNegativeInteger ;
		]
		;
	rdfs:label "IPv6AddressFacet"@en ;
	rdfs:comment "An IPv6 (Internet Protocol version 6) address facet is a grouping of characteristics unique to an IPv6 standards conformant identifier assigned to a device to enable routing and management of IPv6 standards conformant communication to or from that device."@en ;
	.

observable:IShowMessageActionType
	a owl:Class ;
	rdfs:subClassOf
		[
			a owl:Restriction ;
			owl:onProperty observable:showMessageBody ;
			owl:maxQualifiedCardinality "1"^^xsd:nonNegativeInteger ;
			owl:onDataRange xsd:string ;
		] ,
		[
			a owl:Restriction ;
			owl:onProperty observable:showMessageTitle ;
			owl:maxQualifiedCardinality "1"^^xsd:nonNegativeInteger ;
			owl:onDataRange xsd:string ;
		]
		;
	rdfs:label "IShowMessageActionType"@en ;
	rdfs:comment "An IShow message action type is a grouping of characteristics unique to an action that shows a message box when a task is activate. [based on https://docs.microsoft.com/en-us/windows/win32/api/taskschd/nn-taskschd-ishowmessageaction?redirectedfrom=MSDN]"@en ;
	.

observable:Image
	a owl:Class ;
	rdfs:subClassOf observable:ObservableObject ;
	rdfs:label "Image"@en ;
	rdfs:comment "An image is a complete copy of a hard disk, memory, or other digital media."@en ;
	.

observable:ImageFacet
	a owl:Class ;
	rdfs:subClassOf
		<https://unifiedcyberontology.org/ontology/uco/core#Facet> ,
		[
			a owl:Restriction ;
			owl:onProperty observable:imageType ;
			owl:maxQualifiedCardinality "1"^^xsd:nonNegativeInteger ;
			owl:onDataRange xsd:string ;
		]
		;
	rdfs:label "ImageFacet"@en ;
	rdfs:comment "An image facet is a grouping of characteristics unique to a complete copy of a hard disk, memory, or other digital media."@en ;
	.

observable:InstantMessagingAddress
	a owl:Class ;
	rdfs:subClassOf observable:DigitalAddress ;
	rdfs:label "InstantMessagingAddress"@en ;
	rdfs:comment ""@en ;
	.

observable:InstantMessagingAddressFacet
	a owl:Class ;
	rdfs:subClassOf
		<https://unifiedcyberontology.org/ontology/uco/core#DigitalAddressFacet> ,
		[
			a owl:Restriction ;
			owl:onProperty observable:addressValue ;
			owl:cardinality "1"^^xsd:nonNegativeInteger ;
			owl:onDataRange xsd:string ;
		] ,
		[
			a owl:Restriction ;
			owl:onProperty observable:displayName ;
			owl:maxQualifiedCardinality "1"^^xsd:nonNegativeInteger ;
			owl:onDataRange xsd:string ;
		]
		;
	rdfs:label "InstantMessagingAddressFacet"@en ;
	rdfs:comment "An instant messaging address facet is a grouping of characteristics unique to an identifier assigned to enable routing and management of instant messaging digital communication."@en ;
	.

observable:Junction
	a owl:Class ;
	rdfs:subClassOf observable:FileSystemObject ;
	rdfs:label "Junction"@en ;
	rdfs:comment "A junction is a specific NTFS (New Technology File System) reparse point to redirect a directory access to another directory which can be on the same volume or another volume. A junction is similar to a directory symbolic link but may differ on whether they are processed on the local system or on the remote file server. [based on https://jp-andre.pagesperso-orange.fr/junctions.html]"@en ;
	.

observable:Library
	a owl:Class ;
	rdfs:subClassOf observable:ObservableObject ;
	rdfs:label "Library"@en ;
	rdfs:comment "A library is a suite of data and programming code that is used to develop software programs and applications. [based on https://www.techopedia.com/definition/3828/software-library]"@en ;
	.

observable:LibraryFacet
	a owl:Class ;
	rdfs:subClassOf
		<https://unifiedcyberontology.org/ontology/uco/core#Facet> ,
		[
			a owl:Restriction ;
			owl:onProperty observable:libraryType ;
			owl:maxCardinality "1"^^xsd:nonNegativeInteger ;
		]
		;
	rdfs:label "LibraryFacet"@en ;
	rdfs:comment "A library facet is a grouping of characteristics unique to a suite of data and programming code that is used to develop software programs and applications. [based on https://www.techopedia.com/definition/3828/software-library]"@en ;
	.

observable:MACAddress
	a owl:Class ;
	rdfs:subClassOf observable:DigitalAddress ;
	rdfs:label "MACAddress"@en ;
	rdfs:comment "A MAC address is a media access control standards conformant identifier assigned to a network interface to enable routing and management of communications at the data link layer of a network segment."@en ;
	.

observable:MACAddressFacet
	a owl:Class ;
	rdfs:subClassOf
		<https://unifiedcyberontology.org/ontology/uco/core#DigitalAddressFacet> ,
		[
			a owl:Restriction ;
			owl:onProperty observable:addressValue ;
			owl:onDataRange xsd:string ;
			owl:qualifiedCardinality "1"^^xsd:nonNegativeInteger ;
		]
		;
	rdfs:label "MACAddressFacet"@en ;
	rdfs:comment "A MAC address facet is a grouping of characteristics unique to a media access control standards conformant identifier assigned to a network interface to enable routing and management of communications at the data link layer of a network segment."@en ;
	.

observable:MSISDN
	a owl:DatatypeProperty ;
	rdfs:label "MSISDN"@en ;
	rdfs:comment "Mobile Station International Subscriber Directory Number (MSISDN) is a number used to identify a mobile phone number internationally. MSISDN is defined by the E.164 numbering plan. This number includes a country code and a National Destination Code which identifies the subscriber's operator."@en ;
	rdfs:range xsd:string ;
	.

observable:MSISDNType
	a owl:DatatypeProperty ;
	rdfs:label "MSISDNType"@en ;
	rdfs:comment "???."@en ;
	rdfs:range xsd:string ;
	.

observable:Memory
	a owl:Class ;
	rdfs:subClassOf observable:ObservableObject ;
	rdfs:label "Memory"@en ;
	rdfs:comment "Memory is a particular region of temporary information storage (e.g., RAM (random access memory), ROM (read only memory)) on a digital device."@en ;
	.

observable:MemoryFacet
	a owl:Class ;
	rdfs:subClassOf
		<https://unifiedcyberontology.org/ontology/uco/core#Facet> ,
		[
			a owl:Restriction ;
			owl:onProperty observable:regionSize ;
			owl:maxCardinality "1"^^xsd:nonNegativeInteger ;
		] ,
		[
			a owl:Restriction ;
			owl:onProperty observable:blockType ;
			owl:maxQualifiedCardinality "1"^^xsd:nonNegativeInteger ;
			owl:onDataRange vocabulary:MemoryBlockTypeVocab ;
		] ,
		[
			a owl:Restriction ;
			owl:onProperty observable:isInjected ;
			owl:onDataRange xsd:boolean ;
			owl:qualifiedCardinality "1"^^xsd:nonNegativeInteger ;
		] ,
		[
			a owl:Restriction ;
			owl:onProperty observable:isMapped ;
			owl:onDataRange xsd:boolean ;
			owl:qualifiedCardinality "1"^^xsd:nonNegativeInteger ;
		] ,
		[
			a owl:Restriction ;
			owl:onProperty observable:isProtected ;
			owl:onDataRange xsd:boolean ;
			owl:qualifiedCardinality "1"^^xsd:nonNegativeInteger ;
		] ,
		[
			a owl:Restriction ;
			owl:onProperty observable:isVolatile ;
			owl:onDataRange xsd:boolean ;
			owl:qualifiedCardinality "1"^^xsd:nonNegativeInteger ;
		]
		;
	rdfs:label "MemoryFacet"@en ;
	rdfs:comment "A memory facet is a grouping of characteristics unique to a particular region of temporary information storage (e.g., RAM (random access memory), ROM (read only memory)) on a digital device."@en ;
	.

observable:Message
	a owl:Class ;
	rdfs:subClassOf observable:ObservableObject ;
	rdfs:label "Message"@en ;
	rdfs:comment "A message is a discrete unit of electronic communication intended by the source for consumption by some recipient or group of recipients. [based on https://en.wikipedia.org/wiki/Message]"@en ;
	.

observable:MessageFacet
	a owl:Class ;
	rdfs:subClassOf
		<https://unifiedcyberontology.org/ontology/uco/core#Facet> ,
		[
			a owl:Restriction ;
			owl:onProperty observable:sentTime ;
			owl:maxCardinality "1"^^xsd:nonNegativeInteger ;
		] ,
		[
			a owl:Restriction ;
			owl:onProperty observable:application ;
			owl:onClass observable:ObservableObject ;
			owl:maxQualifiedCardinality "1"^^xsd:nonNegativeInteger ;
		] ,
		[
			a owl:Restriction ;
			owl:onProperty observable:from ;
			owl:onClass observable:ObservableObject ;
			owl:maxQualifiedCardinality "1"^^xsd:nonNegativeInteger ;
		] ,
		[
			a owl:Restriction ;
			owl:onProperty observable:messageID ;
			owl:maxQualifiedCardinality "1"^^xsd:nonNegativeInteger ;
			owl:onDataRange xsd:string ;
		] ,
		[
			a owl:Restriction ;
			owl:onProperty observable:messageText ;
			owl:maxQualifiedCardinality "1"^^xsd:nonNegativeInteger ;
			owl:onDataRange xsd:string ;
		] ,
		[
			a owl:Restriction ;
			owl:onProperty observable:messageType ;
			owl:maxQualifiedCardinality "1"^^xsd:nonNegativeInteger ;
			owl:onDataRange xsd:string ;
		] ,
		[
			a owl:Restriction ;
			owl:onProperty observable:sessionID ;
			owl:maxQualifiedCardinality "1"^^xsd:nonNegativeInteger ;
			owl:onDataRange xsd:string ;
		]
		;
	rdfs:label "MessageFacet"@en ;
	rdfs:comment "A message facet is a grouping of characteristics unique to a discrete unit of electronic communication intended by the source for consumption by some recipient or group of recipients. [based on https://en.wikipedia.org/wiki/Message]"@en ;
	.

observable:MessageThread
	a owl:Class ;
	rdfs:subClassOf observable:ObservableObject ;
	rdfs:label "MessageTread"@en ;
	rdfs:comment "A message thread is a running commentary of electronic messages pertaining to one topic or question."@en ;
	.

observable:MessageThreadFacet
	a owl:Class ;
	rdfs:subClassOf
		<https://unifiedcyberontology.org/ontology/uco/core#Facet> ,
		[
			a owl:Restriction ;
			owl:onProperty observable:visibility ;
			owl:maxQualifiedCardinality "1"^^xsd:nonNegativeInteger ;
			owl:onDataRange xsd:boolean ;
		] ,
		[
			a owl:Restriction ;
			owl:onProperty observable:message ;
			owl:onClass observable:ObservableObject ;
			owl:minQualifiedCardinality "1"^^xsd:nonNegativeInteger ;
		]
		;
	rdfs:label "MessageThreadFacet"@en ;
	rdfs:comment "A message thread facet is a grouping of characteristics unique to a running commentary of electronic messages pertaining to one topic or question."@en ;
	.

observable:MftRecordFacet
	a owl:Class ;
	rdfs:subClassOf
		<https://unifiedcyberontology.org/ontology/uco/core#Facet> ,
		[
			a owl:Restriction ;
			owl:onProperty observable:mftFileNameAccessedTime ;
			owl:maxCardinality "1"^^xsd:nonNegativeInteger ;
		] ,
		[
			a owl:Restriction ;
			owl:onProperty observable:mftFileNameCreatedTime ;
			owl:maxCardinality "1"^^xsd:nonNegativeInteger ;
		] ,
		[
			a owl:Restriction ;
			owl:onProperty observable:mftFileNameModifiedTime ;
			owl:maxCardinality "1"^^xsd:nonNegativeInteger ;
		] ,
		[
			a owl:Restriction ;
			owl:onProperty observable:mftFileNameRecordChangeTime ;
			owl:maxCardinality "1"^^xsd:nonNegativeInteger ;
		] ,
		[
			a owl:Restriction ;
			owl:onProperty observable:mftRecordChangeTime ;
			owl:maxCardinality "1"^^xsd:nonNegativeInteger ;
		] ,
		[
			a owl:Restriction ;
			owl:onProperty observable:mftFileID ;
			owl:maxQualifiedCardinality "1"^^xsd:nonNegativeInteger ;
			owl:onDataRange xsd:integer ;
		] ,
		[
			a owl:Restriction ;
			owl:onProperty observable:mftFileNameLength ;
			owl:maxQualifiedCardinality "1"^^xsd:nonNegativeInteger ;
			owl:onDataRange xsd:integer ;
		] ,
		[
			a owl:Restriction ;
			owl:onProperty observable:mftFlags ;
			owl:maxQualifiedCardinality "1"^^xsd:nonNegativeInteger ;
			owl:onDataRange xsd:integer ;
		] ,
		[
			a owl:Restriction ;
			owl:onProperty observable:mftParentID ;
			owl:maxQualifiedCardinality "1"^^xsd:nonNegativeInteger ;
			owl:onDataRange xsd:integer ;
		] ,
		[
			a owl:Restriction ;
			owl:onProperty observable:ntfsHardLinkCount ;
			owl:maxQualifiedCardinality "1"^^xsd:nonNegativeInteger ;
			owl:onDataRange xsd:integer ;
		] ,
		[
			a owl:Restriction ;
			owl:onProperty observable:ntfsOwnerID ;
			owl:maxQualifiedCardinality "1"^^xsd:nonNegativeInteger ;
			owl:onDataRange xsd:string ;
		] ,
		[
			a owl:Restriction ;
			owl:onProperty observable:ntfsOwnerSID ;
			owl:maxQualifiedCardinality "1"^^xsd:nonNegativeInteger ;
			owl:onDataRange xsd:string ;
		]
		;
	rdfs:label "MftRecordFacet"@en ;
	rdfs:comment "An MFT record facet is a grouping of characteristics unique to the details of a single file as managed in an NTFS (new technology filesystem) master file table (which is a collection of information about all files on an NTFS filesystem). [based on https://docs.microsoft.com/en-us/windows/win32/devnotes/master-file-table]"@en ;
	.

observable:MimePartType
	a owl:Class ;
	rdfs:subClassOf
		[
			a owl:Restriction ;
			owl:onProperty observable:bodyRaw ;
			owl:onClass observable:ObservableObject ;
			owl:maxQualifiedCardinality "1"^^xsd:nonNegativeInteger ;
		] ,
		[
			a owl:Restriction ;
			owl:onProperty observable:body ;
			owl:maxQualifiedCardinality "1"^^xsd:nonNegativeInteger ;
			owl:onDataRange xsd:string ;
		] ,
		[
			a owl:Restriction ;
			owl:onProperty observable:contentDisposition ;
			owl:maxQualifiedCardinality "1"^^xsd:nonNegativeInteger ;
			owl:onDataRange xsd:string ;
		] ,
		[
			a owl:Restriction ;
			owl:onProperty observable:contentType ;
			owl:maxQualifiedCardinality "1"^^xsd:nonNegativeInteger ;
			owl:onDataRange xsd:string ;
		]
		;
	rdfs:label "MimePartType"@en ;
	rdfs:comment "A mime part type is a grouping of characteristics unique to a component of a multi-part email body."@en ;
	.

observable:MobileAccount
	a owl:Class ;
	rdfs:subClassOf observable:DigitalAccount ;
	rdfs:label "MobileAccount"@en ;
	rdfs:comment "A mobile account is an arrangement with an entity to enable and control the provision of some capability or service on a portable computing device. [based on https://www.lexico.com/definition/mobile_device]"@en ;
	.

observable:MobileAccountFacet
	a owl:Class ;
	rdfs:subClassOf
		<https://unifiedcyberontology.org/ontology/uco/core#Facet> ,
		[
			a owl:Restriction ;
			owl:onProperty observable:IMSI ;
			owl:maxQualifiedCardinality "1"^^xsd:nonNegativeInteger ;
			owl:onDataRange xsd:string ;
		] ,
		[
			a owl:Restriction ;
			owl:onProperty observable:MSISDN ;
			owl:maxQualifiedCardinality "1"^^xsd:nonNegativeInteger ;
			owl:onDataRange xsd:string ;
		] ,
		[
			a owl:Restriction ;
			owl:onProperty observable:MSISDNType ;
			owl:maxQualifiedCardinality "1"^^xsd:nonNegativeInteger ;
			owl:onDataRange xsd:string ;
		]
		;
	rdfs:label "MobileAccountFacet"@en ;
	rdfs:comment "A mobile account facet is a grouping of characteristics unique to an arrangement with an entity to enable and control the provision of some capability or service on a portable computing device. [based on https://www.lexico.com/definition/mobile_device]"@en ;
	.

observable:MobileDevice
	a owl:Class ;
	rdfs:subClassOf observable:Device ;
	rdfs:label "MobileDevice"@en ;
	rdfs:comment "A mobile device is a portable computing device. [based on https://www.lexico.com.definition/mobile_device]"@en ;
	.

observable:MobileDeviceFacet
	a owl:Class ;
	rdfs:subClassOf
		<https://unifiedcyberontology.org/ontology/uco/core#Facet> ,
		[
			a owl:Restriction ;
			owl:onProperty observable:storageCapacityInBytes ;
			owl:maxQualifiedCardinality "1"^^xsd:nonNegativeInteger ;
			owl:onDataRange xsd:integer ;
		] ,
		[
			a owl:Restriction ;
			owl:onProperty observable:ESN ;
			owl:maxQualifiedCardinality "1"^^xsd:nonNegativeInteger ;
			owl:onDataRange xsd:string ;
		] ,
		[
			a owl:Restriction ;
			owl:onProperty observable:IMEI ;
			owl:maxQualifiedCardinality "1"^^xsd:nonNegativeInteger ;
			owl:onDataRange xsd:string ;
		] ,
		[
			a owl:Restriction ;
			owl:onProperty observable:bluetoothDeviceName ;
			owl:maxQualifiedCardinality "1"^^xsd:nonNegativeInteger ;
			owl:onDataRange xsd:string ;
		] ,
		[
			a owl:Restriction ;
			owl:onProperty observable:clockSetting ;
			owl:maxQualifiedCardinality "1"^^xsd:nonNegativeInteger ;
			owl:onDataRange xsd:string ;
		] ,
		[
			a owl:Restriction ;
			owl:onProperty observable:keypadUnlockCode ;
			owl:maxQualifiedCardinality "1"^^xsd:nonNegativeInteger ;
			owl:onDataRange xsd:string ;
		] ,
		[
			a owl:Restriction ;
			owl:onProperty observable:mockLocationsAllowed ;
			owl:maxQualifiedCardinality "1"^^xsd:nonNegativeInteger ;
			owl:onDataRange xsd:string ;
		] ,
		[
			a owl:Restriction ;
			owl:onProperty observable:network ;
			owl:maxQualifiedCardinality "1"^^xsd:nonNegativeInteger ;
			owl:onDataRange xsd:string ;
		] ,
		[
			a owl:Restriction ;
			owl:onProperty observable:phoneActivationTime ;
			owl:maxQualifiedCardinality "1"^^xsd:nonNegativeInteger ;
			owl:onDataRange xsd:string ;
		]
		;
	rdfs:label "MobileDeviceFacet"@en ;
	rdfs:comment "A mobile device facet is a grouping of characteristics unique to a portable computing device. [based on https://www.lexico.com/definition/mobile_device]"@en ;
	.

observable:Mutex
	a owl:Class ;
	rdfs:subClassOf observable:ObservableObject ;
	rdfs:label "Mutex"@en ;
	rdfs:comment "A mutex is a mechanism that enforces limits on access to a resource when there are many threads of execution. A mutex is designed to enforce a mutual exclusion concurrency control policy, and with a variety of possible methods there exists multiple unique implementations for different applications. [based on https://en.wikipedia.org/wiki/Lock_(computer_science)]"@en ;
	.

observable:MutexFacet
	a owl:Class ;
	rdfs:subClassOf
		<https://unifiedcyberontology.org/ontology/uco/core#Facet> ,
		[
			a owl:Restriction ;
			owl:onProperty observable:isNamed ;
			owl:onDataRange xsd:boolean ;
			owl:qualifiedCardinality "1"^^xsd:nonNegativeInteger ;
		]
		;
	rdfs:label "MutexFacet"@en ;
	rdfs:comment "A mutex facet is a grouping of characteristics unique to a mechanism that enforces limits on access to a resource when there are many threads of execution. A mutex is designed to enforce a mutual exclusion concurrency control policy, and with a variety of possible methods there exists multiple unique implementations for different applications. [based on https://en.wikipedia.org/wiki/Lock_(computer_science)]"@en ;
	.

observable:NTFSFile
	a owl:Class ;
	rdfs:subClassOf observable:File ;
	rdfs:label "NTFSFile"@en ;
	rdfs:comment "An NTFS file is a New Technology File System (NTFS) file."@en ;
	.

observable:NTFSFilePermissionsFacet
	a owl:Class ;
	rdfs:subClassOf <https://unifiedcyberontology.org/ontology/uco/core#Facet> ;
	rdfs:label "NTFSFilePermissionsFacet"@en ;
	rdfs:comment "An NTFS file permissions facet is a grouping of characteristics unique to the access rights (e.g., view, change, navigate, execute) of a file on an NTFS (new technology filesystem) file system."@en ;
	.

observable:NTFSFileSystemFacet
	a owl:Class ;
	rdfs:subClassOf
		<https://unifiedcyberontology.org/ontology/uco/core#Facet> ,
		[
			a owl:Restriction ;
			owl:onProperty observable:entryID ;
			owl:maxQualifiedCardinality "1"^^xsd:nonNegativeInteger ;
			owl:onDataRange xsd:integer ;
		] ,
		[
			a owl:Restriction ;
			owl:onProperty observable:sid ;
			owl:maxQualifiedCardinality "1"^^xsd:nonNegativeInteger ;
			owl:onDataRange xsd:string ;
		]
		;
	rdfs:label "NTFSFileSystemFacet"@en ;
	rdfs:comment "An NTFS file system facet is a grouping of characteristics unique to a file on an NTFS (new technology filesystem) file system."@en ;
	.

observable:NamedPipe
	a owl:Class ;
	rdfs:subClassOf observable:FileSystemObject ;
	rdfs:label "NamedPipe"@en ;
	rdfs:comment "A named pipe is a mechanism for FIFO (first-in-first-out) inter-process communication. It is persisted as a filesystem object (that can be deleted like any other file), can be written to or read from by any process and exists beyond the lifespan of any process interacting with it (unlike simple anonymous pipes). [based on https://en.wikipedia.org/wiki/Named_pipe]"@en ;
	.

observable:NetworkAppliance
	a owl:Class ;
	rdfs:subClassOf observable:Appliance ;
	rdfs:label "NetworkAppliance"@en ;
	rdfs:comment "A network appliance is a purpose-built computer with software or firmware that is designed to provide a specific network management function."@en ;
	.

observable:NetworkConnectionFacet
	a owl:Class ;
	rdfs:subClassOf
		<https://unifiedcyberontology.org/ontology/uco/core#Facet> ,
		[
			a owl:Restriction ;
			owl:onProperty observable:endTime ;
			owl:maxCardinality "1"^^xsd:nonNegativeInteger ;
		] ,
		[
			a owl:Restriction ;
			owl:onProperty observable:protocols ;
			owl:maxCardinality "1"^^xsd:nonNegativeInteger ;
		] ,
		[
			a owl:Restriction ;
			owl:onProperty observable:startTime ;
			owl:maxCardinality "1"^^xsd:nonNegativeInteger ;
		] ,
		[
			a owl:Restriction ;
			owl:onProperty observable:isActive ;
			owl:maxQualifiedCardinality "1"^^xsd:nonNegativeInteger ;
			owl:onDataRange xsd:boolean ;
		] ,
		[
			a owl:Restriction ;
			owl:onProperty observable:destinationPort ;
			owl:maxQualifiedCardinality "1"^^xsd:nonNegativeInteger ;
			owl:onDataRange xsd:integer ;
		] ,
		[
			a owl:Restriction ;
			owl:onProperty observable:sourcePort ;
			owl:maxQualifiedCardinality "1"^^xsd:nonNegativeInteger ;
			owl:onDataRange xsd:integer ;
		]
		;
	rdfs:label "NetworkConnectionFacet"@en ;
	rdfs:comment "A network connection facet is a grouping of characteristics unique to a connection (complete or attempted) accross a digital network (a group of two or more computer systems linked together). [based on https://www.webopedia.com/TERM/N/network.html]"@en ;
	.

observable:NetworkConnetion
	a owl:Class ;
	rdfs:subClassOf observable:ObservableObject ;
	rdfs:label "NetworkConnection"@en ;
	rdfs:comment "A network connection is a connection (completed or attempted) across a digital network (a group of two or more computer systems linked together). [based on https://www.webopedia.com/TERM/N/network.html]"@en ;
	.

observable:NetworkFlow
	a owl:Class ;
	rdfs:subClassOf observable:ObservableObject ;
	rdfs:label "NetworkFlow"@en ;
	rdfs:comment "A network flow is a sequence of data transiting one or more digital network (a group or two or more computer systems linked together) connections. [based on https://www.webopedia.com/TERM/N/network.html]"@en ;
	.

observable:NetworkFlowFacet
	a owl:Class ;
	rdfs:subClassOf
		<https://unifiedcyberontology.org/ontology/uco/core#Facet> ,
		[
			a owl:Restriction ;
			owl:onProperty observable:ipfix ;
			owl:maxCardinality "1"^^xsd:nonNegativeInteger ;
		] ,
		[
			a owl:Restriction ;
			owl:onProperty observable:dstPayload ;
			owl:onClass observable:ObservableObject ;
			owl:maxQualifiedCardinality "1"^^xsd:nonNegativeInteger ;
		] ,
		[
			a owl:Restriction ;
			owl:onProperty observable:srcPayload ;
			owl:onClass observable:ObservableObject ;
			owl:maxQualifiedCardinality "1"^^xsd:nonNegativeInteger ;
		] ,
		[
			a owl:Restriction ;
			owl:onProperty observable:dstBytes ;
			owl:maxQualifiedCardinality "1"^^xsd:nonNegativeInteger ;
			owl:onDataRange xsd:integer ;
		] ,
		[
			a owl:Restriction ;
			owl:onProperty observable:dstPackets ;
			owl:maxQualifiedCardinality "1"^^xsd:nonNegativeInteger ;
			owl:onDataRange xsd:integer ;
		] ,
		[
			a owl:Restriction ;
			owl:onProperty observable:srcBytes ;
			owl:maxQualifiedCardinality "1"^^xsd:nonNegativeInteger ;
			owl:onDataRange xsd:integer ;
		] ,
		[
			a owl:Restriction ;
			owl:onProperty observable:srcPackets ;
			owl:maxQualifiedCardinality "1"^^xsd:nonNegativeInteger ;
			owl:onDataRange xsd:integer ;
		]
		;
	rdfs:label "NetworkFlowFacet"@en ;
	rdfs:comment "A network flow facet is a grouping of characteristics unique to a sequence of data transiting one or more digital network (a group of two or more computer systems linked together) connections. [based on https://www.webopedia.com/TERM/N/network.html]"@en ;
	.

observable:NetworkInterface
	a owl:Class ;
	rdfs:subClassOf observable:ObservableObject ;
	rdfs:label "NetworkInterface"@en ;
	rdfs:comment "A network interface is a software or hardware interface between two pieces of equipment or protocol layers in a computer network."@en ;
	.

observable:NetworkInterfaceFacet
	a owl:Class ;
	rdfs:subClassOf
		<https://unifiedcyberontology.org/ontology/uco/core#Facet> ,
		[
			a owl:Restriction ;
			owl:onProperty observable:dhcpLeaseExpires ;
			owl:maxCardinality "1"^^xsd:nonNegativeInteger ;
		] ,
		[
			a owl:Restriction ;
			owl:onProperty observable:dhcpLeaseObtained ;
			owl:maxCardinality "1"^^xsd:nonNegativeInteger ;
		] ,
		[
			a owl:Restriction ;
			owl:onProperty observable:macAddress ;
			owl:onClass observable:ObservableObject ;
			owl:maxQualifiedCardinality "1"^^xsd:nonNegativeInteger ;
		] ,
		[
			a owl:Restriction ;
			owl:onProperty observable:adapterName ;
			owl:maxQualifiedCardinality "1"^^xsd:nonNegativeInteger ;
			owl:onDataRange xsd:string ;
		]
		;
	rdfs:label "NetworkInterfaceFacet"@en ;
	rdfs:comment "A network interface facet is a grouping of characteristics unique to a software or hardware interface between two pieces of equipment or protocol layers in a computer network."@en ;
	.

observable:NetworkProtocol
	a owl:Class ;
	rdfs:subClassOf observable:ObservableObject ;
	rdfs:label "NetworkProtocol"@en ;
	rdfs:comment "A network protocol is an established set of structured rules that determine how data is transmitted between different devices in the same network. Essentially, it allows connected devices to communicate with each other, regardless of any differences in their internal processes, structure or design. [based on https://www.comptia.org/content/guides/what-is-a-network-protocol]"@en ;
	.

observable:NetworkRoute
	a owl:Class ;
	rdfs:subClassOf observable:ObservableObject ;
	rdfs:label "NetworkRoute"@en ;
	rdfs:comment "A network route is a specific path (of specific network nodes, connections and protocols) for traffic in a network or between or across multiple networks."@en ;
	.

observable:NetworkSocketAddressFamily
	a rdfs:Datatype ;
	owl:equivalentClass [
		a rdfs:Datatype ;
		owl:oneOf [
			a rdf:List ;
			rdf:first "af_appletalk" ;
			rdf:rest [
				a rdf:List ;
				rdf:first "af_bth" ;
				rdf:rest [
					a rdf:List ;
					rdf:first "af_inet" ;
					rdf:rest [
						a rdf:List ;
						rdf:first "af_inet6" ;
						rdf:rest [
							a rdf:List ;
							rdf:first "af_ipx" ;
							rdf:rest [
								a rdf:List ;
								rdf:first "af_irda" ;
								rdf:rest [
									a rdf:List ;
									rdf:first "af_netbios" ;
									rdf:rest [
										a rdf:List ;
										rdf:first "af_unspec" ;
										rdf:rest rdf:nil ;
									] ;
								] ;
							] ;
						] ;
					] ;
				] ;
			] ;
		] ;
	] ;
	.

observable:NetworkSocketProtocolFamily
	a rdfs:Datatype ;
	owl:equivalentClass [
		a rdfs:Datatype ;
		owl:oneOf [
			a rdf:List ;
			rdf:first "pf_appletalk" ;
			rdf:rest [
				a rdf:List ;
				rdf:first "pf_ash" ;
				rdf:rest [
					a rdf:List ;
					rdf:first "pf_atmpvc" ;
					rdf:rest [
						a rdf:List ;
						rdf:first "pf_atmsvc" ;
						rdf:rest [
							a rdf:List ;
							rdf:first "pf_ax25" ;
							rdf:rest [
								a rdf:List ;
								rdf:first "pf_bluetooth" ;
								rdf:rest [
									a rdf:List ;
									rdf:first "pf_bridge" ;
									rdf:rest [
										a rdf:List ;
										rdf:first "pf_decnet" ;
										rdf:rest [
											a rdf:List ;
											rdf:first "pf_econet" ;
											rdf:rest [
												a rdf:List ;
												rdf:first "pf_inet" ;
												rdf:rest [
													a rdf:List ;
													rdf:first "pf_inet6" ;
													rdf:rest [
														a rdf:List ;
														rdf:first "pf_ipx" ;
														rdf:rest [
															a rdf:List ;
															rdf:first "pf_irda" ;
															rdf:rest [
																a rdf:List ;
																rdf:first "pf_key" ;
																rdf:rest [
																	a rdf:List ;
																	rdf:first "pf_netbeui" ;
																	rdf:rest [
																		a rdf:List ;
																		rdf:first "pf_netlink" ;
																		rdf:rest [
																			a rdf:List ;
																			rdf:first "pf_netrom" ;
																			rdf:rest [
																				a rdf:List ;
																				rdf:first "pf_packet" ;
																				rdf:rest [
																					a rdf:List ;
																					rdf:first "pf_pppox" ;
																					rdf:rest [
																						a rdf:List ;
																						rdf:first "pf_rose" ;
																						rdf:rest [
																							a rdf:List ;
																							rdf:first "pf_route" ;
																							rdf:rest [
																								a rdf:List ;
																								rdf:first "pf_security" ;
																								rdf:rest [
																									a rdf:List ;
																									rdf:first "pf_sna" ;
																									rdf:rest [
																										a rdf:List ;
																										rdf:first "pf_wanpipe" ;
																										rdf:rest [
																											a rdf:List ;
																											rdf:first "pf_x25" ;
																											rdf:rest rdf:nil ;
																										] ;
																									] ;
																								] ;
																							] ;
																						] ;
																					] ;
																				] ;
																			] ;
																		] ;
																	] ;
																] ;
															] ;
														] ;
													] ;
												] ;
											] ;
										] ;
									] ;
								] ;
							] ;
						] ;
					] ;
				] ;
			] ;
		] ;
	] ;
	.

observable:NetworkSocketType
	a rdfs:Datatype ;
	owl:equivalentClass [
		a rdfs:Datatype ;
		owl:oneOf [
			a rdf:List ;
			rdf:first "sock_dgram" ;
			rdf:rest [
				a rdf:List ;
				rdf:first "sock_raw" ;
				rdf:rest [
					a rdf:List ;
					rdf:first "sock_rdm" ;
					rdf:rest [
						a rdf:List ;
						rdf:first "sock_seqpacket" ;
						rdf:rest [
							a rdf:List ;
							rdf:first "sock_stream" ;
							rdf:rest rdf:nil ;
						] ;
					] ;
				] ;
			] ;
		] ;
	] ;
	.

observable:NetworkSubnet
	a owl:Class ;
	rdfs:subClassOf observable:ObservableObject ;
	rdfs:label "NetworkSubnet"@en ;
	rdfs:comment "A network subnet is a logical subdivision of an IP network. [based on https://en.wikipedia.org/wiki/Subnetwork]"@en ;
	.

observable:Note
	a owl:Class ;
	rdfs:subClassOf observable:ObservableObject ;
	rdfs:label "Note"@en ;
	rdfs:comment "A note is a brief textual record."@en ;
	.

observable:NoteFacet
	a owl:Class ;
	rdfs:subClassOf
		<https://unifiedcyberontology.org/ontology/uco/core#Facet> ,
		[
			a owl:Restriction ;
			owl:onProperty observable:modifiedTime ;
			owl:maxCardinality "1"^^xsd:nonNegativeInteger ;
		] ,
		[
			a owl:Restriction ;
			owl:onProperty observable:observableCreatedTime ;
			owl:maxCardinality "1"^^xsd:nonNegativeInteger ;
		] ,
		[
			a owl:Restriction ;
			owl:onProperty observable:text ;
			owl:maxQualifiedCardinality "1"^^xsd:nonNegativeInteger ;
			owl:onDataRange xsd:string ;
		] ,
		[
			a owl:Restriction ;
			owl:onProperty observable:application ;
			owl:onClass observable:ObservableObject ;
			owl:qualifiedCardinality "1"^^xsd:nonNegativeInteger ;
		]
		;
	rdfs:label "NoteFacet"@en ;
	rdfs:comment "A note facet is a grouping of characteristics unique to a brief textual record."@en ;
	.

observable:Observable
	a owl:Class ;
	rdfs:subClassOf <https://unifiedcyberontology.org/ontology/uco/core#UcoObject> ;
	rdfs:label "Observable"@en ;
	rdfs:comment "An observable is a characterizable item or action within the digital domain."@en ;
	.

observable:ObservableAction
	a owl:Class ;
	rdfs:subClassOf
		<https://unifiedcyberontology.org/ontology/uco/action#Action> ,
		observable:Observable
		;
	rdfs:label "ObservableAction"@en ;
	rdfs:comment "An observable action is a grouping of characteristics unique to something that may be done or performed within the digital domain."@en ;
	.

observable:ObservableObject
	a owl:Class ;
	rdfs:subClassOf
		<https://unifiedcyberontology.org/ontology/uco/core#Item> ,
		observable:Observable ,
		[
			a owl:Restriction ;
			owl:onProperty observable:state ;
			owl:maxCardinality "1"^^xsd:nonNegativeInteger ;
		] ,
		[
			a owl:Restriction ;
			owl:onProperty observable:hasChanged ;
			owl:onDataRange xsd:boolean ;
			owl:qualifiedCardinality "1"^^xsd:nonNegativeInteger ;
		]
		;
	rdfs:label "ObservableObject"@en ;
	rdfs:comment "An observable object is a grouping of characteristics unique to a distinct article or unit within the digital domain."@en ;
	.

observable:ObservablePattern
	a owl:Class ;
	rdfs:subClassOf observable:Observable ;
	rdfs:label "ObservablePattern"@en ;
	rdfs:comment "An observable pattern is a grouping of characteristics unique to a logical pattern composed of observable object and observable action properties."@en ;
	.

observable:ObservableRelationship
	a owl:Class ;
	rdfs:subClassOf
		<https://unifiedcyberontology.org/ontology/uco/core#Relationship> ,
		observable:Observable
		;
	rdfs:label "ObservableRelationship"@en ;
	rdfs:comment "An observable relationship is a grouping of characteristics unique to an assertion of an association between two observable objects."@en ;
	.

observable:Observation
	a owl:Class ;
	rdfs:subClassOf
		<https://unifiedcyberontology.org/ontology/uco/action#Action> ,
		[
			a owl:Restriction ;
			owl:onProperty <https://unifiedcyberontology.org/ontology/uco/core#name> ;
			owl:cardinality "1"^^xsd:nonNegativeInteger ;
		] ,
		[
			a owl:Restriction ;
			owl:onProperty <https://unifiedcyberontology.org/ontology/uco/core#name> ;
			owl:hasValue "observe" ;
		]
		;
	rdfs:label "Observation"@en ;
	rdfs:comment "An observation is a temporal perception of an observable."@en ;
	.

observable:OnlineService
	a owl:Class ;
	rdfs:label "OnlineService"@en ;
	rdfs:comment "An online service is a particular provision mechanism of information access, distribution or manipulation over the Internet."@en ;
	rdfs:subClasOf observable:ObservableObject ;
	.

observable:OnlineServiceFacet
	a owl:Class ;
	rdfs:subClassOf
		<https://unifiedcyberontology/ontology/uco/core#Facet> ,
		[
			a owl:Restriction ;
			owl:onProperty <https://unifiedcyberontology/ontology/uco/core#name> ;
			owl:cardinality "1"^^xsd:nonNegativeInteger ;
		] ,
		[
			a owl:Restriction ;
			owl:onProperty <https://unifiedcyberontology/ontology/uco/observable#inetLocation> ;
			owl:minCardinality "0"^^xsd:nonNegativeInteger ;
		] ,
		[
			a owl:Restriction ;
			owl:onProperty <https://unifiedcyberontology/ontology/uco/observable#location> ;
			owl:minCardinality "0"^^xsd:nonNegativeInteger ;
		]
		;
	rdfs:label "OnlineServiceFacet"@en-US ;
	rdfs:comment "An online service facet is a grouping of characteristics unique to a particular provision mechanism of information access, distribution or manipulation over the Internet."@en-US ;
	.

observable:OperatingSystem
	a owl:Class ;
	rdfs:subClassOf observable:ObservableObject ;
	rdfs:label "OperatingSystem"@en ;
	rdfs:comment "An operating system is the software that manages computer hardware, software resources, and provides common services for computer programs. [based on https://en.wikipedia.org/wiki/Operating_system]"@en ;
	.

observable:OperatingSystemFacet
	a owl:Class ;
	rdfs:subClassOf
		<https://unifiedcyberontology.org/ontology/uco/core#Facet> ,
		[
			a owl:Restriction ;
			owl:onProperty observable:bitness ;
			owl:maxCardinality "1"^^xsd:nonNegativeInteger ;
		] ,
		[
			a owl:Restriction ;
			owl:onProperty observable:environmentVariables ;
			owl:maxCardinality "1"^^xsd:nonNegativeInteger ;
		] ,
		[
			a owl:Restriction ;
			owl:onProperty observable:installDate ;
			owl:maxCardinality "1"^^xsd:nonNegativeInteger ;
		] ,
		[
			a owl:Restriction ;
			owl:onProperty observable:manufacturer ;
			owl:maxQualifiedCardinality "1"^^xsd:nonNegativeInteger ;
			owl:onDataRange xsd:string ;
		] ,
		[
			a owl:Restriction ;
			owl:onProperty observable:version ;
			owl:maxQualifiedCardinality "1"^^xsd:nonNegativeInteger ;
			owl:onDataRange xsd:string ;
		]
		;
	rdfs:label "OperatingSystemFacet"@en ;
	rdfs:comment "An operating system facet is a grouping of characteristics unique to the software that manages computer hardware, software resources, and provides common services for computer programs. [based on https://en.wikipedia.org/wiki/Operating_system]"@en ;
	.

observable:PDFFile
	a owl:Class ;
	rdfs:subClassOf observable:File ;
	rdfs:label "PDFFile"@en ;
	rdfs:comment "A PDF file is a Portable Document Format (PDF) file."@en ;
	.

observable:PDFFileFacet
	a owl:Class ;
	rdfs:subClassOf
		<https://unifiedcyberontology.org/ontology/uco/core#Facet> ,
		[
			a owl:Restriction ;
			owl:onProperty observable:documentInformationDictionary ;
			owl:maxCardinality "1"^^xsd:nonNegativeInteger ;
		] ,
		[
			a owl:Restriction ;
			owl:onProperty observable:isOptimized ;
			owl:maxQualifiedCardinality "1"^^xsd:nonNegativeInteger ;
			owl:onDataRange xsd:boolean ;
		] ,
		[
			a owl:Restriction ;
			owl:onProperty observable:pdfId1 ;
			owl:maxQualifiedCardinality "1"^^xsd:nonNegativeInteger ;
			owl:onDataRange xsd:string ;
		] ,
		[
			a owl:Restriction ;
			owl:onProperty observable:version ;
			owl:maxQualifiedCardinality "1"^^xsd:nonNegativeInteger ;
			owl:onDataRange xsd:string ;
		]
		;
	rdfs:label "PDFFileFacet"@en ;
	rdfs:comment "A PDF file facet is a grouping of characteristics unique to a PDF (Portable Document Format) file."@en ;
	.

observable:PIN
	a owl:DatatypeProperty ;
	rdfs:label "PIN"@en ;
	rdfs:comment "Personal Identification Number (PIN)."@en ;
	rdfs:range xsd:string ;
	.

observable:PUK
	a owl:DatatypeProperty ;
	rdfs:label "PUK"@en ;
	rdfs:comment "Personal Unlocking Key (PUK) to unlock the SIM card."@en ;
	rdfs:range xsd:string ;
	.

observable:PathRelationFacet
	a owl:Class ;
	rdfs:subClassOf <https://unifiedcyberontology.org/ontology/uco/core#Facet> ;
	rdfs:label "PathRelationFacet"@en ;
	rdfs:comment "A path relation facet is a grouping of characteristics unique to the location of one object within another containing object."@en ;
	.

observable:PaymentCard
	a owl:Class ;
	rdfs:subClassOf observable:ObservableObject ;
	rdfs:label "PaymentCard"@en ;
	rdfs:comment "A payment card is a physical token that is part of a payment system issued by financial institutions, such as a bank, to a customer that enables its owner (the cardholder) to access the funds in the customer's designated bank accounts, or through a credit account and make payments by electronic funds transfer and access automated teller machines (ATMs). [based on https://en.wikipedia.org/wiki/Payment_card]"@en ;
	.

observable:PhoneAccount
	a owl:Class ;
	rdfs:subClassOf observable:DigitalAccount ;
	rdfs:label "PhoneAccount"@en ;
	rdfs:comment "A phone account is an arrangement with an entity to enable and control the provision of a telephony capability or service."@en ;
	.

observable:PhoneAccountFacet
	a owl:Class ;
	rdfs:subClassOf
		<https://unifiedcyberontology.org/ontology/uco/core#Facet> ,
		[
			a owl:Restriction ;
			owl:onProperty observable:phoneNumber ;
			owl:onDataRange xsd:string ;
			owl:qualifiedCardinality "1"^^xsd:nonNegativeInteger ;
		]
		;
	rdfs:label "PhoneAccountFacet"@en ;
	rdfs:comment "A phone account facet is a grouping of characteristics unique to an arrangement with an entity to enable and control the provision of a telephony capability or service."@en ;
	.

observable:PhoneCall
	a owl:Class ;
	rdfs:subClassOf observable:ObservableObject ;
	rdfs:label "PhoneCall"@en ;
	rdfs:comment "A phone call is a connection over a telephone network between the called party and the calling party. [based on https://en.wikipedia.org/wiki/Telephone_call]"@en ;
	.

observable:PhoneCallFacet
	a owl:Class ;
	rdfs:subClassOf
		<https://unifiedcyberontology.org/ontology/uco/core#Facet> ,
		[
			a owl:Restriction ;
			owl:onProperty observable:endTime ;
			owl:maxCardinality "1"^^xsd:nonNegativeInteger ;
		] ,
		[
			a owl:Restriction ;
			owl:onProperty observable:startTime ;
			owl:maxCardinality "1"^^xsd:nonNegativeInteger ;
		] ,
		[
			a owl:Restriction ;
			owl:onProperty observable:from ;
			owl:onClass observable:ObservableObject ;
			owl:maxQualifiedCardinality "1"^^xsd:nonNegativeInteger ;
		] ,
		[
			a owl:Restriction ;
			owl:onProperty observable:to ;
			owl:onClass observable:ObservableObject ;
			owl:maxQualifiedCardinality "1"^^xsd:nonNegativeInteger ;
		] ,
		[
			a owl:Restriction ;
			owl:onProperty observable:duration ;
			owl:maxQualifiedCardinality "1"^^xsd:nonNegativeInteger ;
			owl:onDataRange xsd:integer ;
		] ,
		[
			a owl:Restriction ;
			owl:onProperty observable:callType ;
			owl:maxQualifiedCardinality "1"^^xsd:nonNegativeInteger ;
			owl:onDataRange xsd:string ;
		] ,
		[
			a owl:Restriction ;
			owl:onProperty observable:application ;
			owl:onClass observable:ObservableObject ;
			owl:qualifiedCardinality "1"^^xsd:nonNegativeInteger ;
		]
		;
	rdfs:label "PhoneCallFacet"@en ;
	rdfs:comment "A phone call facet is a grouping of characteristics unique to a connection over a telephone network between the called party and the calling party. [based on https://en.wikipedia.org/wiki/Telephone_call]"@en ;
	.

observable:Pipe
	a owl:Class ;
	rdfs:subClassOf observable:ObservableObject ;
	rdfs:label "Pipe"@en ;
	rdfs:comment "A pipe is a mechanism for one-way inter-process communication using message passing where data written by one process is buffered by the operating system until it is read by the next process, and this uni-directional channel disappears when the processes are completed. [based on https://en.wikipedia.org/wiki/Pipeline_(Unix) ; https://en.wikipedia.org/wiki/Anonymous_pipe]"@en ;
	.

observable:Post
	a owl:Class ;
	rdfs:subClassOf observable:Message ;
	rdfs:label "Post"@en ;
	rdfs:comment "A post is message submitted to an online discussion/publishing site (forum, blog, etc.)."@en ;
	.

observable:Process
	a owl:Class ;
	rdfs:subClassOf observable:ObservableObject ;
	rdfs:label "Process"@en ;
	rdfs:comment "A process is an instance of a computer program executed on an operating system."@en ;
	.

observable:ProcessFacet
	a owl:Class ;
	rdfs:subClassOf
		<https://unifiedcyberontology.org/ontology/uco/core#Facet> ,
		[
			a owl:Restriction ;
			owl:onProperty observable:environmentVariables ;
			owl:maxCardinality "1"^^xsd:nonNegativeInteger ;
		] ,
		[
			a owl:Restriction ;
			owl:onProperty observable:exitTime ;
			owl:maxCardinality "1"^^xsd:nonNegativeInteger ;
		] ,
		[
			a owl:Restriction ;
			owl:onProperty observable:observableCreatedTime ;
			owl:maxCardinality "1"^^xsd:nonNegativeInteger ;
		] ,
		[
			a owl:Restriction ;
			owl:onProperty observable:binary ;
			owl:onClass observable:ObservableObject ;
			owl:maxQualifiedCardinality "1"^^xsd:nonNegativeInteger ;
		] ,
		[
			a owl:Restriction ;
			owl:onProperty observable:creatorUser ;
			owl:onClass observable:ObservableObject ;
			owl:maxQualifiedCardinality "1"^^xsd:nonNegativeInteger ;
		] ,
		[
			a owl:Restriction ;
			owl:onProperty observable:parent ;
			owl:onClass observable:ObservableObject ;
			owl:maxQualifiedCardinality "1"^^xsd:nonNegativeInteger ;
		] ,
		[
			a owl:Restriction ;
			owl:onProperty observable:isHidden ;
			owl:maxQualifiedCardinality "1"^^xsd:nonNegativeInteger ;
			owl:onDataRange xsd:boolean ;
		] ,
		[
			a owl:Restriction ;
			owl:onProperty observable:exitStatus ;
			owl:maxQualifiedCardinality "1"^^xsd:nonNegativeInteger ;
			owl:onDataRange xsd:integer ;
		] ,
		[
			a owl:Restriction ;
			owl:onProperty observable:pid ;
			owl:maxQualifiedCardinality "1"^^xsd:nonNegativeInteger ;
			owl:onDataRange xsd:integer ;
		] ,
		[
			a owl:Restriction ;
			owl:onProperty observable:currentWorkingDirectory ;
			owl:maxQualifiedCardinality "1"^^xsd:nonNegativeInteger ;
			owl:onDataRange xsd:string ;
		] ,
		[
			a owl:Restriction ;
			owl:onProperty observable:status ;
			owl:maxQualifiedCardinality "1"^^xsd:nonNegativeInteger ;
			owl:onDataRange xsd:string ;
		]
		;
	rdfs:label "ProcessFacet"@en ;
	rdfs:comment "A process facet is a grouping of characteristics unique to an instance of a computer program executed on an operating system."@en ;
	.

observable:Profile
	a owl:Class ;
	rdfs:subClassOf observable:ObservableObject ;
	rdfs:label "Profile"@en ;
	rdfs:comment "A profile is an explicit digital representation of identity and characteristics of the owner of a single user account associated with an online service or application. [based on https://en.wikipedia.org/wiki/User_profile]"@en ;
	.

observable:ProfileFacet
	a owl:Class ;
	rdfs:subClassOf
		<https://unifiedcyberontology.org/ontology/uco/core#Facet> ,
		[
			a owl:Restriction ;
			owl:onProperty <https://unifiedcyberontology.org/ontology/uco/core#name> ;
			owl:maxCardinality "1"^^xsd:nonNegativeInteger ;
		] ,
		[
			a owl:Restriction ;
			owl:onProperty observable:contactAddress ;
			owl:maxCardinality "1"^^xsd:nonNegativeInteger ;
		] ,
		[
			a owl:Restriction ;
			owl:onProperty observable:contactEmail ;
			owl:maxCardinality "1"^^xsd:nonNegativeInteger ;
		] ,
		[
			a owl:Restriction ;
			owl:onProperty observable:contactMessaging ;
			owl:maxCardinality "1"^^xsd:nonNegativeInteger ;
		] ,
		[
			a owl:Restriction ;
			owl:onProperty observable:contactPhone ;
			owl:maxCardinality "1"^^xsd:nonNegativeInteger ;
		] ,
		[
			a owl:Restriction ;
			owl:onProperty observable:contactURL ;
			owl:maxCardinality "1"^^xsd:nonNegativeInteger ;
		] ,
		[
			a owl:Restriction ;
			owl:onProperty observable:displayName ;
			owl:maxCardinality "1"^^xsd:nonNegativeInteger ;
		] ,
		[
			a owl:Restriction ;
			owl:onProperty observable:profileAccount ;
			owl:maxCardinality "1"^^xsd:nonNegativeInteger ;
		] ,
		[
			a owl:Restriction ;
			owl:onProperty observable:profileCreated ;
			owl:maxCardinality "1"^^xsd:nonNegativeInteger ;
		] ,
		[
			a owl:Restriction ;
			owl:onProperty observable:profileIdentity ;
			owl:maxCardinality "1"^^xsd:nonNegativeInteger ;
		] ,
		[
			a owl:Restriction ;
			owl:onProperty observable:profileService ;
			owl:maxCardinality "1"^^xsd:nonNegativeInteger ;
		] ,
		[
			a owl:Restriction ;
			owl:onProperty observable:profileLanguage ;
			owl:minCardinality "0"^^xsd:nonNegativeInteger ;
		]
		;
	rdfs:label "ProfileFacet"@en-US ;
	rdfs:comment "A profile facet is a grouping of characteristics unique to an explicit digital representation of identity and characteristics of the owner of a single user account associated with an online service or application. [based on https://en.wikipedia.org/wiki/User_profile]"@en-US ;
	.

observable:PropertiesEnumeratedEffectFacet
	a owl:Class ;
	rdfs:subClassOf
		<https://unifiedcyberontology.org/ontology/uco/core#Facet> ,
		observable:DefinedEffectFacet ,
		[
			a owl:Restriction ;
			owl:onProperty observable:properties ;
			owl:onDataRange xsd:string ;
			owl:qualifiedCardinality "1"^^xsd:nonNegativeInteger ;
		]
		;
	rdfs:label "PropertiesEnumeratedEffectFacet"@en ;
	rdfs:comment "A properties enumerated effect facet is a grouping of characteristics unique to the effects of actions upon observable objects where a characteristic of the observable object is enumerated. An example of this would be startup parameters for a process."@en ;
	.

observable:PropertyReadEffectFacet
	a owl:Class ;
	rdfs:subClassOf
		<https://unifiedcyberontology.org/ontology/uco/core#Facet> ,
		observable:DefinedEffectFacet ,
		[
			a owl:Restriction ;
			owl:onProperty observable:propertyName ;
			owl:maxQualifiedCardinality "1"^^xsd:nonNegativeInteger ;
			owl:onDataRange xsd:string ;
		] ,
		[
			a owl:Restriction ;
			owl:onProperty observable:value ;
			owl:maxQualifiedCardinality "1"^^xsd:nonNegativeInteger ;
			owl:onDataRange xsd:string ;
		]
		;
	rdfs:label "PropertyReadEffectFacet"@en ;
	rdfs:comment "A properties read effect facet is a grouping of characteristics unique to the effects of actions upon observable objects where a characteristic is read from an observable object. An example of this would be the current running state of a process."@en ;
	.

observable:RasterPicture
	a owl:Class ;
	rdfs:subClassOf observable:File ;
	rdfs:label "RasterPicture"@en ;
	rdfs:comment "A raster picture is a raster (or bitmap) image."@en ;
	.

observable:RasterPictureFacet
	a owl:Class ;
	rdfs:subClassOf
		<https://unifiedcyberontology.org/ontology/uco/core#Facet> ,
		[
			a owl:Restriction ;
			owl:onProperty observable:camera ;
			owl:onClass observable:ObservableObject ;
			owl:maxQualifiedCardinality "1"^^xsd:nonNegativeInteger ;
		] ,
		[
			a owl:Restriction ;
			owl:onProperty observable:bitsPerPixel ;
			owl:maxQualifiedCardinality "1"^^xsd:nonNegativeInteger ;
			owl:onDataRange xsd:integer ;
		] ,
		[
			a owl:Restriction ;
			owl:onProperty observable:pictureHeight ;
			owl:maxQualifiedCardinality "1"^^xsd:nonNegativeInteger ;
			owl:onDataRange xsd:integer ;
		] ,
		[
			a owl:Restriction ;
			owl:onProperty observable:pictureWidth ;
			owl:maxQualifiedCardinality "1"^^xsd:nonNegativeInteger ;
			owl:onDataRange xsd:integer ;
		] ,
		[
			a owl:Restriction ;
			owl:onProperty observable:imageCompressionMethod ;
			owl:maxQualifiedCardinality "1"^^xsd:nonNegativeInteger ;
			owl:onDataRange xsd:string ;
		] ,
		[
			a owl:Restriction ;
			owl:onProperty observable:pictureType ;
			owl:maxQualifiedCardinality "1"^^xsd:nonNegativeInteger ;
			owl:onDataRange xsd:string ;
		]
		;
	rdfs:label "RasterPictureFacet"@en ;
	rdfs:comment "A raster picture facet is a grouping of characteristics unique to a raster (or bitmap) image."@en ;
	.

observable:RegistryDatatype
	a rdfs:Datatype ;
	owl:equivalentClass [
		a rdfs:Datatype ;
		owl:oneOf [
			a rdf:List ;
			rdf:first "reg_binary" ;
			rdf:rest [
				a rdf:List ;
				rdf:first "reg_dword" ;
				rdf:rest [
					a rdf:List ;
					rdf:first "reg_dword_big_endian" ;
					rdf:rest [
						a rdf:List ;
						rdf:first "reg_expand_sz" ;
						rdf:rest [
							a rdf:List ;
							rdf:first "reg_full_resource_descriptor" ;
							rdf:rest [
								a rdf:List ;
								rdf:first "reg_invalid_type" ;
								rdf:rest [
									a rdf:List ;
									rdf:first "reg_link" ;
									rdf:rest [
										a rdf:List ;
										rdf:first "reg_multi_sz" ;
										rdf:rest [
											a rdf:List ;
											rdf:first "reg_none" ;
											rdf:rest [
												a rdf:List ;
												rdf:first "reg_qword" ;
												rdf:rest [
													a rdf:List ;
													rdf:first "reg_resource_list" ;
													rdf:rest [
														a rdf:List ;
														rdf:first "reg_resource_requirements_list" ;
														rdf:rest [
															a rdf:List ;
															rdf:first "reg_sz" ;
															rdf:rest rdf:nil ;
														] ;
													] ;
												] ;
											] ;
										] ;
									] ;
								] ;
							] ;
						] ;
					] ;
				] ;
			] ;
		] ;
	] ;
	.

observable:ReparsePoint
	a owl:Class ;
	rdfs:subClassOf observable:FileSystemObject ;
	rdfs:label "ReparsePoint"@en ;
	rdfs:comment "A reparse point is a type of NTFS (New Technology File System) object which is an optional attribute of files and directories meant to define some sort of preprocessing before accessing the said file or directory. For instance reparse points can be used to redirect access to files which have been moved to long term storage so that some application would retrieve them and make them directly accessible. A reparse point contains a reparse tag and data that are interpreted by a filesystem filter identified by the tag. [based on https://jp-andre.pagesperso-orange.fr/junctions.html ; https://en.wikipedia.org/wiki/NTFS_reparse_point]"@en ;
	.

observable:SIMCard
	a owl:Class ;
	rdfs:subClassOf observable:Device ;
	rdfs:label "SIMCard" ;
	rdfs:comment "A SIM card is a subscriber identification module card intended to securely store the international mobile subscriber identity (IMSI) number and its related key, which are used to identify and authenticate subscribers on mobile telephony. [based on https://en.wikipedia.org/wiki/SIM_card]"@en ;
	.

observable:SIMCardFacet
	a owl:Class ;
	rdfs:subClassOf
		<https://unifiedcyberontology.org/ontology/uco/core#Facet> ,
		[
			a owl:Restriction ;
			owl:onProperty observable:carrier ;
			owl:onClass identity:Identity ;
			owl:maxQualifiedCardinality "1"^^xsd:nonNegativeInteger ;
		] ,
		[
			a owl:Restriction ;
			owl:onProperty observable:storageCapacityInBytes ;
			owl:maxQualifiedCardinality "1"^^xsd:nonNegativeInteger ;
			owl:onDataRange xsd:integer ;
		] ,
		[
			a owl:Restriction ;
			owl:onProperty observable:ICCID ;
			owl:maxQualifiedCardinality "1"^^xsd:nonNegativeInteger ;
			owl:onDataRange xsd:string ;
		] ,
		[
			a owl:Restriction ;
			owl:onProperty observable:IMSI ;
			owl:maxQualifiedCardinality "1"^^xsd:nonNegativeInteger ;
			owl:onDataRange xsd:string ;
		] ,
		[
			a owl:Restriction ;
			owl:onProperty observable:PIN ;
			owl:maxQualifiedCardinality "1"^^xsd:nonNegativeInteger ;
			owl:onDataRange xsd:string ;
		] ,
		[
			a owl:Restriction ;
			owl:onProperty observable:PUK ;
			owl:maxQualifiedCardinality "1"^^xsd:nonNegativeInteger ;
			owl:onDataRange xsd:string ;
		] ,
		[
			a owl:Restriction ;
			owl:onProperty observable:SIMForm ;
			owl:maxQualifiedCardinality "1"^^xsd:nonNegativeInteger ;
			owl:onDataRange xsd:string ;
		] ,
		[
			a owl:Restriction ;
			owl:onProperty observable:SIMType ;
			owl:maxQualifiedCardinality "1"^^xsd:nonNegativeInteger ;
			owl:onDataRange xsd:string ;
		]
		;
	rdfs:label "SIMCardFacet"@en ;
	rdfs:comment "A SIM card facet is a grouping of characteristics unique to a subscriber identification module card intended to securely store the international mobile subscriber identity (IMSI) number and its related key, which are used to identify and authenticate subscribers on mobile telephony devices (such as mobile phones and computers). [based on https://en.wikipedia.org/wiki/SIM_card]"@en ;
	.

observable:SIMForm
	a owl:DatatypeProperty ;
	rdfs:label "SIMForm"@en ;
	rdfs:comment "The form of SIM card such as SIM, Micro SIM, Nano SIM."@en ;
	rdfs:range xsd:string ;
	.

observable:SIMType
	a owl:DatatypeProperty ;
	rdfs:label "SIMType"@en ;
	rdfs:comment "The type of SIM card such as SIM, USIM, UICC."@en ;
	rdfs:range xsd:string ;
	.

observable:SIPAddress
	a owl:Class ;
	rdfs:subClassOf observable:DigitalAddress ;
	rdfs:label "SIPAddress"@en ;
	rdfs:comment "A SIP address is an identifier for Session Initiation Protocol (SIP) communication."@en ;
	.

observable:SIPAddressFacet
	a owl:Class ;
	rdfs:subClassOf
		<https://unifiedcyberontology.org/ontology/uco/core#DigitalAddressFacet> ,
		[
			a owl:Restriction ;
			owl:onProperty observable:addressValue ;
			owl:cardinality "1"^^xsd:nonNegativeInteger ;
			owl:onDataRange xsd:string ;
		] ,
		[
			a owl:Restriction ;
			owl:onProperty observable:displayName ;
			owl:maxQualifiedCardinality "1"^^xsd:nonNegativeInteger ;
			owl:onDataRange xsd:string ;
		]
		;
	rdfs:label "SIPAddressFacet"@en ;
	rdfs:comment "A SIP address facet is a grouping of characteristics unique to a Session Initiation Protocol (SIP) standards conformant identifier assigned to a user to enable routing and management of SIP standards conformant communication to or from that user loosely coupled from any particular devices."@en ;
	.

observable:SMSMessage
	a owl:Class ;
	rdfs:subClassOf observable:Message ;
	rdfs:label "SMSMessage"@en ;
	rdfs:comment "An SMS message is a message conformant to the short message service (SMS) communication protocol standards."@en ;
	.

observable:SMSMessageFacet
	a owl:Class ;
	rdfs:subClassOf
		<https://unifiedcyberontology.org/ontology/uco/core#Facet> ,
		[
			a owl:Restriction ;
			owl:onProperty observable:isRead ;
			owl:maxQualifiedCardinality "1"^^xsd:nonNegativeInteger ;
			owl:onDataRange xsd:boolean ;
		]
		;
	rdfs:label "SMSMessageFacet"@en ;
	rdfs:comment "A SMS message facet is a grouping of characteristics unique to a message conformant to the short message service (SMS) communication protocol standards."@en ;
	.

observable:SQLiteBlob
	a owl:Class ;
	rdfs:subClassOf observable:ObservableObject ;
	rdfs:label "SQLiteBlob"@en ;
	rdfs:comment "An SQLite blob is a blob (binary large object) of data within an SQLite database. [based on https://en.wikipedia.org/wiki/SQLite]"@en ;
	.

observable:SQLiteBlobFacet
	a owl:Class ;
	rdfs:subClassOf
		<https://unifiedcyberontology.org/ontology/uco/core#Facet> ,
		[
			a owl:Restriction ;
			owl:onProperty observable:columnName ;
			owl:maxQualifiedCardinality "1"^^xsd:nonNegativeInteger ;
			owl:onDataRange xsd:string ;
		] ,
		[
			a owl:Restriction ;
			owl:onProperty observable:rowCondition ;
			owl:maxQualifiedCardinality "1"^^xsd:nonNegativeInteger ;
			owl:onDataRange xsd:string ;
		] ,
		[
			a owl:Restriction ;
			owl:onProperty observable:tableName ;
			owl:maxQualifiedCardinality "1"^^xsd:nonNegativeInteger ;
			owl:onDataRange xsd:string ;
		]
		;
	rdfs:label "SQLiteBlobFacet"@en ;
	rdfs:comment "An SQLite blob facet is a grouping of characteristics unique to a blob (binary large object) of data within an SQLite database. [based on https://en.wikipedia.org/wiki/SQLite]"@en ;
	.

observable:SecurityAppliance
	a owl:Class ;
	rdfs:subClassOf observable:Appliance ;
	rdfs:label "SecurityAppliance"@en ;
	rdfs:comment "A security appliance is a purpose-built computer with software or firmware that is designed to provide a specific security function to protect computer networks."@en ;
	.

observable:Semaphore
	a owl:Class ;
	rdfs:subClassOf observable:ObservableObject ;
	rdfs:label "Semaphore"@en ;
	rdfs:comment "A semaphore is a variable or abstract data type used to control access to a common resource by multiple processes and avoid critical section problems in a concurrent system such as a multitasking operating system. [based on https://en.wikipedia.org/wiki/Semaphore_(programming)]"@en ;
	.

observable:SendControlCodeEffectFacet
	a owl:Class ;
	rdfs:subClassOf
		<https://unifiedcyberontology.org/ontology/uco/core#Facet> ,
		observable:DefinedEffectFacet ,
		[
			a owl:Restriction ;
			owl:onProperty observable:controlCode ;
			owl:onDataRange xsd:string ;
			owl:qualifiedCardinality "1"^^xsd:nonNegativeInteger ;
		]
		;
	rdfs:label "SendControlCodeEffectFacet"@en ;
	rdfs:comment "A send control code effect facet is a grouping of characteristics unique to the effects of actions upon observable objects where a control code, or other control-oriented communication signal, is sent to the observable object. An example of this would be an action sending a control code changing the running state of a process."@en ;
	.

observable:ShopListing
	a owl:Class ;
	rdfs:subClassOf observable:ObservableObject ;
	rdfs:label "ShopListing"@en ;
	rdfs:comment "A shop listing is a listing of offered products on an online marketplace/shop."@en ;
	.

observable:Snapshot
	a owl:Class ;
	rdfs:label "Snapshot"@en ;
	rdfs:comment "A snapshot is a file system object representing a snapshot of the contents of a part of a file system at a point in time."@en ;
	rdfs:subClasOf observable:FileSystemObject ;
	.

observable:Socket
	a owl:Class ;
	rdfs:subClassOf observable:FileSystemObject ;
	rdfs:label "Socket"@en ;
	rdfs:comment "A socket is a special file used for inter-process communication, which enables communication between two processes. In addition to sending data, processes can send file descriptors across a Unix domain socket connection using the sendmsg() and recvmsg() system calls. Unlike named pipes which allow only unidirectional data flow, sockets are fully duplex-capable. [based on https://en.wikipedia.org/wiki/Unix_file_types]"@en ;
	.

observable:SocketAddress
	a owl:Class ;
	rdfs:subClassOf observable:Address ;
	rdfs:label "SocketAddress"@en ;
	rdfs:comment "A socket address (combining and IP address and a port number) is a composite identifier for a network socket endpoint supporting internet protocol communications."@en ;
	.

observable:Software
	a owl:Class ;
	rdfs:subClassOf observable:ObservableObject ;
	rdfs:label "Software"@en ;
	rdfs:comment "Software is a definitely scoped instance of a collection of data or computer instructions that tell the computer how to work. [based on https://en.wikipedia.org/wiki/Software]"@en ;
	.

observable:SoftwareFacet
	a owl:Class ;
	rdfs:subClassOf
		<https://unifiedcyberontology.org/ontology/uco/core#Facet> ,
		[
			a owl:Restriction ;
			owl:onProperty observable:cpeid ;
			owl:maxQualifiedCardinality "1"^^xsd:nonNegativeInteger ;
			owl:onDataRange xsd:string ;
		] ,
		[
			a owl:Restriction ;
			owl:onProperty observable:language ;
			owl:maxQualifiedCardinality "1"^^xsd:nonNegativeInteger ;
			owl:onDataRange xsd:string ;
		] ,
		[
			a owl:Restriction ;
			owl:onProperty observable:manufacturer ;
			owl:maxQualifiedCardinality "1"^^xsd:nonNegativeInteger ;
			owl:onDataRange xsd:string ;
		] ,
		[
			a owl:Restriction ;
			owl:onProperty observable:swid ;
			owl:maxQualifiedCardinality "1"^^xsd:nonNegativeInteger ;
			owl:onDataRange xsd:string ;
		] ,
		[
			a owl:Restriction ;
			owl:onProperty observable:version ;
			owl:maxQualifiedCardinality "1"^^xsd:nonNegativeInteger ;
			owl:onDataRange xsd:string ;
		]
		;
	rdfs:label "SoftwareFacet"@en ;
	rdfs:comment "A software facet is a grouping of characteristics unique to a software program (a definitively scoped instance of a collection of data or computer instructions that tell the computer how to work). [based on https://en.wikipedia.org/wiki/Software]"@en ;
	.

observable:StateChangeEffectFacet
	a owl:Class ;
	rdfs:subClassOf
		<https://unifiedcyberontology.org/ontology/uco/core#Facet> ,
		observable:DefinedEffectFacet ,
		[
			a owl:Restriction ;
			owl:onProperty observable:oldObject ;
			owl:onClass observable:ObservableObject ;
			owl:maxQualifiedCardinality "1"^^xsd:nonNegativeInteger ;
		] ,
		[
			a owl:Restriction ;
			owl:onProperty observable:newObject ;
			owl:onClass observable:ObservableObject ;
			owl:qualifiedCardinality "1"^^xsd:nonNegativeInteger ;
		]
		;
	rdfs:label "StateChangeEffectFacet"@en ;
	rdfs:comment "A state change effect facet is a grouping of characteristics unique to the effects of actions upon observable objects where a state of the observable object is changed."@en ;
	.

observable:SymbolicLink
	a owl:Class ;
	rdfs:subClassOf <https://unifedcyberontology.org/ontology/uco/observable#FileSystemObject> ;
	rdfs:label "SymbolicLink"@en ;
	rdfs:comment "A symbolic link is a file that contains a reference to another file or directory in the form of an absolute or relative path and that affects pathname resolution. [based on https://en.wikipedia.org/wiki/Symbolic_link]"@en ;
	.

observable:SymbolicLinkFacet
	a owl:Class ;
	rdfs:subClassOf
		<https://unifiedcyberontology.org/ontology/uco/core#Facet> ,
		[
			a owl:Restriction ;
			owl:onProperty observable:targetFile ;
			owl:onClass observable:ObservableObject ;
			owl:qualifiedCardinality "1"^^xsd:nonNegativeInteger ;
		]
		;
	rdfs:label "SymbolicLinkFacet"@en ;
	rdfs:comment "A symbolic link facet is a grouping of characteristics unique to a file that contains a reference to another file or directory in the form of an absolute or relative path and that affects pathname resolution. [based on https://en.wikipedia.org/wiki/Symbolic_link]"@en ;
	.

observable:TCPConnection
	a owl:Class ;
	rdfs:subClassOf observable:NetworkConnection ;
	rdfs:label "TCPConnection"@en ;
	rdfs:comment "A TCP connection is a network connection that is conformant to the Transfer "@en ;
	.

observable:TCPConnectionFacet
	a owl:Class ;
	rdfs:subClassOf <https://unifiedcyberontology.org/ontology/uco/core#Facet> ;
	rdfs:label "TCPConnectionFacet"@en ;
	rdfs:comment "A TCP connection facet is a grouping of characteristics unique to portions of a network connection that are conformant to the Transmission Control Protocl (TCP) standard."@en ;
	.

observable:TaskActionType
	a owl:Class ;
	rdfs:subClassOf
		[
			a owl:Restriction ;
			owl:onProperty observable:iComHandlerAction ;
			owl:onClass observable:IComHandlerActionType ;
			owl:maxQualifiedCardinality "1"^^xsd:nonNegativeInteger ;
		] ,
		[
			a owl:Restriction ;
			owl:onProperty observable:iExecAction ;
			owl:onClass observable:IExecActionType ;
			owl:maxQualifiedCardinality "1"^^xsd:nonNegativeInteger ;
		] ,
		[
			a owl:Restriction ;
			owl:onProperty observable:iShowMessageAction ;
			owl:onClass observable:IShowMessageActionType ;
			owl:maxQualifiedCardinality "1"^^xsd:nonNegativeInteger ;
		] ,
		[
			a owl:Restriction ;
			owl:onProperty observable:iEmailAction ;
			owl:onClass observable:ObservableObject ;
			owl:maxQualifiedCardinality "1"^^xsd:nonNegativeInteger ;
		] ,
		[
			a owl:Restriction ;
			owl:onProperty observable:actionID ;
			owl:maxQualifiedCardinality "1"^^xsd:nonNegativeInteger ;
			owl:onDataRange xsd:string ;
		] ,
		[
			a owl:Restriction ;
			owl:onProperty observable:actionType ;
			owl:maxQualifiedCardinality "1"^^xsd:nonNegativeInteger ;
			owl:onDataRange vocabulary:TaskActionTypeVocab ;
		]
		;
	rdfs:label "TaskActionType"@en ;
	rdfs:comment "A task action type is a grouping of characteristics for a scheduled action to be completed."@en ;
	.

observable:Thread
	a owl:Class ;
	rdfs:subClassOf observable:ObservableObject ;
	rdfs:label "Thread"@en ;
	rdfs:comment "A thread is the smallest sequence of programmed instructions that can be managed independently by a scheduler on a computer, which is typically a part of the operating system. It is a component of a process. Multiple threads can exist within one process, executing concurrently and sharing resources such as memory, while different processes do not share these resources. In particular, the threads of a process share its executable code and the values of its dynamically allocated variables and non-thread-local global variables at any given time. [based on https://en.wikipedia.org/wiki/Thread_(computing)]"@en ;
	.

observable:TriggerType
	a owl:Class ;
	rdfs:subClassOf
		[
			a owl:Restriction ;
			owl:onProperty observable:triggerBeginTime ;
			owl:maxCardinality "1"^^xsd:nonNegativeInteger ;
		] ,
		[
			a owl:Restriction ;
			owl:onProperty observable:triggerEndTime ;
			owl:maxCardinality "1"^^xsd:nonNegativeInteger ;
		] ,
		[
			a owl:Restriction ;
			owl:onProperty observable:isEnabled ;
			owl:maxQualifiedCardinality "1"^^xsd:nonNegativeInteger ;
			owl:onDataRange xsd:boolean ;
		] ,
		[
			a owl:Restriction ;
			owl:onProperty observable:triggerDelay ;
			owl:maxQualifiedCardinality "1"^^xsd:nonNegativeInteger ;
			owl:onDataRange xsd:string ;
		] ,
		[
			a owl:Restriction ;
			owl:onProperty observable:triggerMaxRunTime ;
			owl:maxQualifiedCardinality "1"^^xsd:nonNegativeInteger ;
			owl:onDataRange xsd:string ;
		] ,
		[
			a owl:Restriction ;
			owl:onProperty observable:triggerSessionChangeType ;
			owl:maxQualifiedCardinality "1"^^xsd:nonNegativeInteger ;
			owl:onDataRange xsd:string ;
		] ,
		[
			a owl:Restriction ;
			owl:onProperty observable:triggerFrequency ;
			owl:maxQualifiedCardinality "1"^^xsd:nonNegativeInteger ;
			owl:onDataRange vocabulary:TriggerFrequencyVocab ;
		] ,
		[
			a owl:Restriction ;
			owl:onProperty observable:triggerType ;
			owl:maxQualifiedCardinality "1"^^xsd:nonNegativeInteger ;
			owl:onDataRange vocabulary:TriggerTypeVocab ;
		]
		;
	rdfs:label "TriggerType"@en ;
	rdfs:comment "A trigger type is a grouping of characterizes unique to a set of criteria that, when met, starts the execution of a task within a Windows operating system. [based on https://docs.microsoft.com/en-us/windows/win32/taskschd/task-triggers]"@en ;
	.

observable:Tweet
	a owl:Class ;
	rdfs:subClassOf observable:Message ;
	rdfs:label "Tweet"@en ;
	rdfs:comment "A tweet is message submitted by a Twitter user account to the Twitter microblogging platform."@en ;
	.

observable:TwitterProfileFacet
	a owl:Class ;
	rdfs:subClassOf
		<https://unifiedcyberontology.org/ontology/uco/core#Facet> ,
		[
			a owl:Restriction ;
			owl:onProperty observable:twitterId ;
			owl:cardinality "1"^^xsd:nonNegativeInteger ;
		] ,
		[
			a owl:Restriction ;
			owl:onProperty observable:favoritesCount ;
			owl:maxCardinality "1"^^xsd:nonNegativeInteger ;
		] ,
		[
			a owl:Restriction ;
			owl:onProperty observable:followersCount ;
			owl:maxCardinality "1"^^xsd:nonNegativeInteger ;
		] ,
		[
			a owl:Restriction ;
			owl:onProperty observable:friendsCount ;
			owl:maxCardinality "1"^^xsd:nonNegativeInteger ;
		] ,
		[
			a owl:Restriction ;
			owl:onProperty observable:listedCount ;
			owl:maxCardinality "1"^^xsd:nonNegativeInteger ;
		] ,
		[
			a owl:Restriction ;
			owl:onProperty observable:profileBackgroundLocation ;
			owl:maxCardinality "1"^^xsd:nonNegativeInteger ;
		] ,
		[
			a owl:Restriction ;
			owl:onProperty observable:profileBannerLocation ;
			owl:maxCardinality "1"^^xsd:nonNegativeInteger ;
		] ,
		[
			a owl:Restriction ;
			owl:onProperty observable:profileImageLocation ;
			owl:maxCardinality "1"^^xsd:nonNegativeInteger ;
		] ,
		[
			a owl:Restriction ;
			owl:onProperty observable:profileIsProtected ;
			owl:maxCardinality "1"^^xsd:nonNegativeInteger ;
		] ,
		[
			a owl:Restriction ;
			owl:onProperty observable:profileIsVerified ;
			owl:maxCardinality "1"^^xsd:nonNegativeInteger ;
		] ,
		[
			a owl:Restriction ;
			owl:onProperty observable:statusesCount ;
			owl:maxCardinality "1"^^xsd:nonNegativeInteger ;
		] ,
		[
			a owl:Restriction ;
			owl:onProperty observable:twitterHandle ;
			owl:maxCardinality "1"^^xsd:nonNegativeInteger ;
		] ,
		[
			a owl:Restriction ;
			owl:onProperty observable:userLocationString ;
			owl:maxCardinality "1"^^xsd:nonNegativeInteger ;
		] ,
		[
			a owl:Restriction ;
			owl:onProperty observable:profileBackgroundHash ;
			owl:minCardinality "0"^^xsd:nonNegativeInteger ;
		] ,
		[
			a owl:Restriction ;
			owl:onProperty observable:profileBannerHash ;
			owl:minCardinality "0"^^xsd:nonNegativeInteger ;
		] ,
		[
			a owl:Restriction ;
			owl:onProperty observable:profileImageHash ;
			owl:minCardinality "0"^^xsd:nonNegativeInteger ;
		]
		;
	rdfs:label "TwitterProfileFacet" ;
	rdfs:comment "A twitter profile facet is a grouping of characteristics unique to an explicit digital representation of identity and characteristics of the owner of a single Twitter user account. [based on https://en.wikipedia.org/wiki/User_profile]" ;
	.

observable:UNIXAccount
	a owl:Class ;
	rdfs:subClassOf observable:DigitalAccount ;
	rdfs:label "UNIXAccount"@en ;
	rdfs:comment "A UNIX account is an account on a UNIX operating system."@en ;
	.

observable:UNIXAccountFacet
	a owl:Class ;
	rdfs:subClassOf
		<https://unifiedcyberontology.org/ontology/uco/core#Facet> ,
		[
			a owl:Restriction ;
			owl:onProperty observable:gid ;
			owl:maxQualifiedCardinality "1"^^xsd:nonNegativeInteger ;
			owl:onDataRange xsd:integer ;
		] ,
		[
			a owl:Restriction ;
			owl:onProperty observable:shell ;
			owl:maxQualifiedCardinality "1"^^xsd:nonNegativeInteger ;
			owl:onDataRange xsd:string ;
		]
		;
	rdfs:label "UNIXAccountFacet"@en ;
	rdfs:comment "A UNIX account facet is a grouping of characteristics unique to an account on a UNIX operating system."@en ;
	.

observable:UNIXFile
	a owl:Class ;
	rdfs:subClassOf observable:File ;
	rdfs:label "UNIXFile"@en ;
	rdfs:comment "A UNIX file is a file pertaining to the UNIX operating system."@en ;
	.

observable:UNIXFilePermissionsFacet
	a owl:Class ;
	rdfs:subClassOf <https://unifiedcyberontology.org/ontology/uco/core#Facet> ;
	rdfs:label "UNIXFilePermissionsFacet"@en ;
	rdfs:comment "A UNIX file permissions facet is a grouping of characteristics unique to the access rights (e.g., view, change, navigate, execute) of a file on a UNIX file system."@en ;
	.

observable:UNIXProcess
	a owl:Class ;
	rdfs:subClassOf observable:Process ;
	rdfs:label "UNIXProcess"@en ;
	rdfs:comment "A UNIX process is an instance of a computer program executed on a UNIX operating system."@en ;
	.

observable:UNIXProcessFacet
	a owl:Class ;
	rdfs:subClassOf <https://unifiedcyberontology.org/ontology/uco/core#Facet> ;
	rdfs:label "UNIXProcessFacet"@en ;
	rdfs:comment "A UNIX process facet is a grouping of characteristics unique to an instance of a computer program executed on a UNIX operating system."@en ;
	.

observable:UNIXVolumeFacet
	a owl:Class ;
	rdfs:subClassOf
		<https://unifiedcyberontology.org/ontology/uco/core#Facet> ,
		[
			a owl:Restriction ;
			owl:onProperty observable:mountPoint ;
			owl:maxQualifiedCardinality "1"^^xsd:nonNegativeInteger ;
			owl:onDataRange xsd:string ;
		] ,
		[
			a owl:Restriction ;
			owl:onProperty observable:options ;
			owl:maxQualifiedCardinality "1"^^xsd:nonNegativeInteger ;
			owl:onDataRange xsd:string ;
		]
		;
	rdfs:label "UNIXVolumeFacet"@en ;
	rdfs:comment "A UNIX volume facet is a grouping of characteristics unique to a single accessible storage area (volume) with a single UNIX file system. [based on https://en.wikipedia.org/wiki/Volume_(computing)]"@en ;
	.

observable:URL
	a owl:Class ;
	rdfs:subClassOf observable:ObservableObject ;
	rdfs:label "URL"@en ;
	rdfs:comment "A URL is a uniform resource locator (URL) acting as a resolvable address to a particular WWW (World Wide Web) accessible resource."@en ;
	.

observable:URLFacet
	a owl:Class ;
	rdfs:subClassOf
		<https://unifiedcyberontology.org/ontology/uco/core#Facet> ,
		[
			a owl:Restriction ;
			owl:onProperty observable:host ;
			owl:onClass observable:ObservableObject ;
			owl:maxQualifiedCardinality "1"^^xsd:nonNegativeInteger ;
		] ,
		[
			a owl:Restriction ;
			owl:onProperty observable:userName ;
			owl:onClass observable:ObservableObject ;
			owl:maxQualifiedCardinality "1"^^xsd:nonNegativeInteger ;
		] ,
		[
			a owl:Restriction ;
			owl:onProperty observable:port ;
			owl:maxQualifiedCardinality "1"^^xsd:nonNegativeInteger ;
			owl:onDataRange xsd:integer ;
		] ,
		[
			a owl:Restriction ;
			owl:onProperty observable:fragment ;
			owl:maxQualifiedCardinality "1"^^xsd:nonNegativeInteger ;
			owl:onDataRange xsd:string ;
		] ,
		[
			a owl:Restriction ;
			owl:onProperty observable:password ;
			owl:maxQualifiedCardinality "1"^^xsd:nonNegativeInteger ;
			owl:onDataRange xsd:string ;
		] ,
		[
			a owl:Restriction ;
			owl:onProperty observable:path ;
			owl:maxQualifiedCardinality "1"^^xsd:nonNegativeInteger ;
			owl:onDataRange xsd:string ;
		] ,
		[
			a owl:Restriction ;
			owl:onProperty observable:query ;
			owl:maxQualifiedCardinality "1"^^xsd:nonNegativeInteger ;
			owl:onDataRange xsd:string ;
		] ,
		[
			a owl:Restriction ;
			owl:onProperty observable:scheme ;
			owl:maxQualifiedCardinality "1"^^xsd:nonNegativeInteger ;
			owl:onDataRange xsd:string ;
		] ,
		[
			a owl:Restriction ;
			owl:onProperty observable:fullValue ;
			owl:onDataRange xsd:string ;
			owl:qualifiedCardinality "1"^^xsd:nonNegativeInteger ;
		]
		;
	rdfs:label "URLFacet"@en ;
	rdfs:comment "A URL facet is a grouping of characteristics unique to a uniform resource locator (URL) acting as a resolvable address to a particular WWW (World Wide Web) accessible resource."@en ;
	.

observable:URLHistory
	a owl:Class ;
	rdfs:subClassOf observable:ObservableObject ;
	rdfs:label "URLHistory"@en ;
	rdfs:comment "A URL history characterizes the stored URL history for a particular web browser"@en ;
	.

observable:URLHistoryEntry
	a owl:Class ;
	rdfs:subClassOf
		[
			a owl:Restriction ;
			owl:onProperty observable:browserUserProfile ;
			owl:maxCardinality "1"^^xsd:nonNegativeInteger ;
		] ,
		[
			a owl:Restriction ;
			owl:onProperty observable:expirationTime ;
			owl:maxCardinality "1"^^xsd:nonNegativeInteger ;
		] ,
		[
			a owl:Restriction ;
			owl:onProperty observable:firstVisit ;
			owl:maxCardinality "1"^^xsd:nonNegativeInteger ;
		] ,
		[
			a owl:Restriction ;
			owl:onProperty observable:hostname ;
			owl:maxCardinality "1"^^xsd:nonNegativeInteger ;
		] ,
		[
			a owl:Restriction ;
			owl:onProperty observable:lastVisit ;
			owl:maxCardinality "1"^^xsd:nonNegativeInteger ;
		] ,
		[
			a owl:Restriction ;
			owl:onProperty observable:manuallyEnteredCount ;
			owl:maxCardinality "1"^^xsd:nonNegativeInteger ;
		] ,
		[
			a owl:Restriction ;
			owl:onProperty observable:pageTitle ;
			owl:maxCardinality "1"^^xsd:nonNegativeInteger ;
		] ,
		[
			a owl:Restriction ;
			owl:onProperty observable:url ;
			owl:maxCardinality "1"^^xsd:nonNegativeInteger ;
		] ,
		[
			a owl:Restriction ;
			owl:onProperty observable:visitCount ;
			owl:maxCardinality "1"^^xsd:nonNegativeInteger ;
		] ,
		[
			a owl:Restriction ;
			owl:onProperty observable:keywordSearchTerm ;
			owl:minCardinality "0"^^xsd:nonNegativeInteger ;
		] ,
		[
			a owl:Restriction ;
			owl:onProperty observable:referrerUrl ;
			owl:minCardinality "0"^^xsd:nonNegativeInteger ;
		]
		;
	rdfs:label "URL History Entry"@en-US ;
	rdfs:comment "A URL history entry is a grouping of characteristics unique to the properties of a single URL history entry for a particular browser."@en-US ;
	.

observable:URLHistoryFacet
	a owl:Class ;
	rdfs:subClassOf
		<https://unifiedcyberontology.org/ontology/uco/core#Facet> ,
		[
			a owl:Restriction ;
			owl:onProperty observable:browserInformation ;
			owl:maxCardinality "1"^^xsd:nonNegativeInteger ;
		] ,
		[
			a owl:Restriction ;
			owl:onProperty observable:urlHistoryEntry ;
			owl:minCardinality "1"^^xsd:nonNegativeInteger ;
		]
		;
	rdfs:label "URLHistoryFacet"@en-US ;
	rdfs:comment "A URL history facet is a grouping of characteristics unique to the stored URL history for a particular web browser"@en-US ;
	.

observable:URLVisit
	a owl:Class ;
	rdfs:subClassOf observable:ObservableObject ;
	rdfs:label "URLVisit"@en ;
	rdfs:comment "A URL visit characterizes the properties of a visit of a URL within a particular browser."@en ;
	.

observable:URLVisitFacet
	a owl:Class ;
	rdfs:subClassOf
		<https://unifiedcyberontology.org/ontology/uco/core#Facet> ,
		[
			a owl:Restriction ;
			owl:onProperty observable:browserInformation ;
			owl:maxCardinality "1"^^xsd:nonNegativeInteger ;
		] ,
		[
			a owl:Restriction ;
			owl:onProperty observable:fromURLVisit ;
			owl:maxCardinality "1"^^xsd:nonNegativeInteger ;
		] ,
		[
			a owl:Restriction ;
			owl:onProperty observable:url ;
			owl:maxCardinality "1"^^xsd:nonNegativeInteger ;
		] ,
		[
			a owl:Restriction ;
			owl:onProperty observable:urlTransitionType ;
			owl:maxCardinality "1"^^xsd:nonNegativeInteger ;
		] ,
		[
			a owl:Restriction ;
			owl:onProperty observable:visitDuration ;
			owl:maxCardinality "1"^^xsd:nonNegativeInteger ;
		] ,
		[
			a owl:Restriction ;
			owl:onProperty observable:visitTime ;
			owl:maxCardinality "1"^^xsd:nonNegativeInteger ;
		]
		;
	rdfs:label "URLVisitFacet"@en ;
	rdfs:comment "A URL visit facet is a grouping of characteristics unique to the properties of a visit of a URL within a particular browser."@en ;
	.

observable:UserAccount
	a owl:Class ;
	rdfs:subClassOf observable:DigitalAccount ;
	rdfs:label "UserAccount"@en ;
	rdfs:comment "A user account is an account controlling a user's access to a network, system or platform."@en ;
	.

observable:UserAccountFacet
	a owl:Class ;
	rdfs:subClassOf
		<https://unifiedcyberontology.org/ontology/uco/core#Facet> ,
		[
			a owl:Restriction ;
			owl:onProperty observable:canEscalatePrivs ;
			owl:maxQualifiedCardinality "1"^^xsd:nonNegativeInteger ;
			owl:onDataRange xsd:boolean ;
		] ,
		[
			a owl:Restriction ;
			owl:onProperty observable:isPrivileged ;
			owl:maxQualifiedCardinality "1"^^xsd:nonNegativeInteger ;
			owl:onDataRange xsd:boolean ;
		] ,
		[
			a owl:Restriction ;
			owl:onProperty observable:isServiceAccount ;
			owl:maxQualifiedCardinality "1"^^xsd:nonNegativeInteger ;
			owl:onDataRange xsd:boolean ;
		] ,
		[
			a owl:Restriction ;
			owl:onProperty observable:homeDirectory ;
			owl:maxQualifiedCardinality "1"^^xsd:nonNegativeInteger ;
			owl:onDataRange xsd:string ;
		]
		;
	rdfs:label "UserAccountFacet"@en ;
	rdfs:comment "A user account facet is a grouping of characteristics unique to an account controlling a user's access to a network, system, or platform."@en ;
	.

observable:UserSession
	a owl:Class ;
	rdfs:subClassOf observable:ObservableObject ;
	rdfs:label "UserSession"@en ;
	rdfs:comment "A user session is a temporary and interactive information interchange between two or more communicating devices within the managed scope of a single user. [based on https://en.wikipedia.org/wiki/Session_(computer_science)]"@en ;
	.

observable:UserSessionFacet
	a owl:Class ;
	rdfs:subClassOf
		<https://unifiedcyberontology.org/ontology/uco/core#Facet> ,
		[
			a owl:Restriction ;
			owl:onProperty observable:loginTime ;
			owl:maxCardinality "1"^^xsd:nonNegativeInteger ;
		] ,
		[
			a owl:Restriction ;
			owl:onProperty observable:logoutTime ;
			owl:maxCardinality "1"^^xsd:nonNegativeInteger ;
		] ,
		[
			a owl:Restriction ;
			owl:onProperty observable:effectiveUser ;
			owl:onClass observable:ObservableObject ;
			owl:maxQualifiedCardinality "1"^^xsd:nonNegativeInteger ;
		] ,
		[
			a owl:Restriction ;
			owl:onProperty observable:effectiveGroup ;
			owl:maxQualifiedCardinality "1"^^xsd:nonNegativeInteger ;
			owl:onDataRange xsd:string ;
		] ,
		[
			a owl:Restriction ;
			owl:onProperty observable:effectiveGroupID ;
			owl:maxQualifiedCardinality "1"^^xsd:nonNegativeInteger ;
			owl:onDataRange xsd:string ;
		]
		;
	rdfs:label "UserSessionFacet"@en ;
	rdfs:comment "A user session facet is a grouping of characteristics unique to a temporary and interactive information interchange between two or more communicating devices within the managed scope of a single user. [based on https://en.wikipedia.org/wiki/Session_(computer_science)]"@en ;
	.

observable:ValuesEnumeratedEffectFacet
	a owl:Class ;
	rdfs:subClassOf
		<https://unifiedcyberontology.org/ontology/uco/core#Facet> ,
		observable:DefinedEffectFacet ,
		[
			a owl:Restriction ;
			owl:onProperty observable:values ;
			owl:onDataRange xsd:string ;
			owl:qualifiedCardinality "1"^^xsd:nonNegativeInteger ;
		]
		;
	rdfs:label "ValuesEnumeratedEffectFacet"@en ;
	rdfs:comment "A values enumerated effect facet is a grouping of characteristics unique to the effects of actions upon observable objects where a value of the observable object is enumerated. An example of this would be the values of a registry key."@en ;
	.

observable:Volume
	a owl:Class ;
	rdfs:subClassOf observable:ObservableObject ;
	rdfs:label "Volume"@en ;
	rdfs:comment "A volume is a single accessible storage area (volume) with a single file system. [based on https://en.wikipedia.org/wiki/Volume_(computing)]"@en ;
	.

observable:VolumeFacet
	a owl:Class ;
	rdfs:subClassOf
		<https://unifiedcyberontology.org/ontology/uco/core#Facet> ,
		[
			a owl:Restriction ;
			owl:onProperty observable:sectorSize ;
			owl:maxQualifiedCardinality "1"^^xsd:nonNegativeInteger ;
			owl:onDataRange xsd:integer ;
		] ,
		[
			a owl:Restriction ;
			owl:onProperty observable:volumeID ;
			owl:maxQualifiedCardinality "1"^^xsd:nonNegativeInteger ;
			owl:onDataRange xsd:string ;
		]
		;
	rdfs:label "VolumeFacet"@en ;
	rdfs:comment "A volume facet is a grouping of characteristics unique to a single accessible storage area (volume) with a single file system. [based on https://en.wikipedia.org/wiki/Volume_(computing)]"@en ;
	.

observable:WebPage
	a owl:Class ;
	rdfs:subClassOf observable:ObservableObject ;
	rdfs:label "WebPage"@en ;
	rdfs:comment "A web page is a specific collection of information provided by a website and displayed to a user in a web browser. A website typically consists of many web pages linked together in a coherent fashion. [based on https://en.wikipedia.org/wiki/Web_page]"@en ;
	.

observable:WhoIs
	a owl:Class ;
	rdfs:subClassOf observable:ObservableObject ;
	rdfs:label "WhoIs"@en ;
	rdfs:comment "WhoIs is a response record conformant to the WHOIS protocol standard (RFC 3912). [based on https://en.wikipedia.org/wiki/WHOIS]"@en ;
	.

observable:WhoIsFacet
	a owl:Class ;
	rdfs:subClassOf
		<https://unifiedcyberontology.org/ontology/uco/core#Facet> ,
		[
			a owl:Restriction ;
			owl:onProperty observable:creationDate ;
			owl:maxCardinality "1"^^xsd:nonNegativeInteger ;
		] ,
		[
			a owl:Restriction ;
			owl:onProperty observable:expirationDate ;
			owl:maxCardinality "1"^^xsd:nonNegativeInteger ;
		] ,
		[
			a owl:Restriction ;
			owl:onProperty observable:lookupDate ;
			owl:maxCardinality "1"^^xsd:nonNegativeInteger ;
		] ,
		[
			a owl:Restriction ;
			owl:onProperty observable:updatedDate ;
			owl:maxCardinality "1"^^xsd:nonNegativeInteger ;
		] ,
		[
			a owl:Restriction ;
			owl:onProperty observable:domainName ;
			owl:onClass observable:ObservableObject ;
			owl:maxQualifiedCardinality "1"^^xsd:nonNegativeInteger ;
		] ,
		[
			a owl:Restriction ;
			owl:onProperty observable:ipAddress ;
			owl:onClass observable:ObservableObject ;
			owl:maxQualifiedCardinality "1"^^xsd:nonNegativeInteger ;
		] ,
		[
			a owl:Restriction ;
			owl:onProperty observable:registrantContactInfo ;
			owl:onClass observable:ObservableObject ;
			owl:maxQualifiedCardinality "1"^^xsd:nonNegativeInteger ;
		] ,
		[
			a owl:Restriction ;
			owl:onProperty observable:serverName ;
			owl:onClass observable:ObservableObject ;
			owl:maxQualifiedCardinality "1"^^xsd:nonNegativeInteger ;
		] ,
		[
			a owl:Restriction ;
			owl:onProperty observable:registrarInfo ;
			owl:onClass observable:WhoisRegistrarInfoType ;
			owl:maxQualifiedCardinality "1"^^xsd:nonNegativeInteger ;
		] ,
		[
			a owl:Restriction ;
			owl:onProperty observable:domainID ;
			owl:maxQualifiedCardinality "1"^^xsd:nonNegativeInteger ;
			owl:onDataRange xsd:string ;
		] ,
		[
			a owl:Restriction ;
			owl:onProperty observable:remarks ;
			owl:maxQualifiedCardinality "1"^^xsd:nonNegativeInteger ;
			owl:onDataRange xsd:string ;
		] ,
		[
			a owl:Restriction ;
			owl:onProperty observable:sponsoringRegistrar ;
			owl:maxQualifiedCardinality "1"^^xsd:nonNegativeInteger ;
			owl:onDataRange xsd:string ;
		] ,
		[
			a owl:Restriction ;
			owl:onProperty observable:regionalInternetRegistry ;
			owl:maxQualifiedCardinality "1"^^xsd:nonNegativeInteger ;
			owl:onDataRange vocabulary:RegionalRegistryTypeVocab ;
		] ,
		[
			a owl:Restriction ;
			owl:onProperty observable:dnssec ;
			owl:maxQualifiedCardinality "1"^^xsd:nonNegativeInteger ;
			owl:onDataRange vocabulary:WhoisDNSSECTypeVocab ;
		] ,
		[
			a owl:Restriction ;
			owl:onProperty observable:status ;
			owl:maxQualifiedCardinality "1"^^xsd:nonNegativeInteger ;
			owl:onDataRange vocabulary:WhoisStatusTypeVocab ;
		]
		;
	rdfs:label "WhoIsFacet"@en ;
	rdfs:comment "A whois facet is a grouping of characteristics unique to a response record conformant to the WHOIS protocol standard (RFC 3912). [based on https://en.wikipedia.org/wiki/WHOIS]"@en ;
	.

observable:WhoisContactFacet
	a owl:Class ;
	rdfs:subClassOf
		observable:ContactFacet ,
		[
			a owl:Restriction ;
			owl:onProperty observable:whoisContactType ;
			owl:maxQualifiedCardinality "1"^^xsd:nonNegativeInteger ;
			owl:onDataRange [
				a rdfs:Datatype ;
				owl:unionOf (
					xsd:string
					observable:WhoisContactTypeVocab
				) ;
			] ;
		]
		;
	rdfs:label "WhoIsContactFacet"@en ;
	rdfs:comment "A Whois contact type is a grouping of characteristics unique to contact-related information present in a response record conformant to the WHOIS protocol standard (RFC 3912). [based on https://en.wikipedia.org/wiki/WHOIS]"@en ;
	.

observable:WhoisRegistrarInfoType
	a owl:Class ;
	rdfs:subClassOf
		[
			a owl:Restriction ;
			owl:onProperty observable:geolocationAddress ;
			owl:maxCardinality "1"^^xsd:nonNegativeInteger ;
		] ,
		[
			a owl:Restriction ;
			owl:onProperty observable:contactPhoneNumber ;
			owl:onClass observable:ObservableObject ;
			owl:maxQualifiedCardinality "1"^^xsd:nonNegativeInteger ;
		] ,
		[
			a owl:Restriction ;
			owl:onProperty observable:emailAddress ;
			owl:onClass observable:ObservableObject ;
			owl:maxQualifiedCardinality "1"^^xsd:nonNegativeInteger ;
		] ,
		[
			a owl:Restriction ;
			owl:onProperty observable:referralURL ;
			owl:onClass observable:ObservableObject ;
			owl:maxQualifiedCardinality "1"^^xsd:nonNegativeInteger ;
		] ,
		[
			a owl:Restriction ;
			owl:onProperty observable:whoisServer ;
			owl:onClass observable:ObservableObject ;
			owl:maxQualifiedCardinality "1"^^xsd:nonNegativeInteger ;
		] ,
		[
			a owl:Restriction ;
			owl:onProperty observable:registrarGUID ;
			owl:maxQualifiedCardinality "1"^^xsd:nonNegativeInteger ;
			owl:onDataRange xsd:string ;
		] ,
		[
			a owl:Restriction ;
			owl:onProperty observable:registrarID ;
			owl:maxQualifiedCardinality "1"^^xsd:nonNegativeInteger ;
			owl:onDataRange xsd:string ;
		] ,
		[
			a owl:Restriction ;
			owl:onProperty observable:registrarName ;
			owl:maxQualifiedCardinality "1"^^xsd:nonNegativeInteger ;
			owl:onDataRange xsd:string ;
		]
		;
	rdfs:label "WhoisRegistrarInfoType"@en ;
	rdfs:comment "A Whois registrar info type is a grouping of characteristics unique to registrar-related information present in a response record conformant to the WHOIS protocol standard (RFC 3912). [based on https://en.wikipedia.org/wiki/WHOIS]"@en ;
	.

observable:WifiAddress
	a owl:Class ;
	rdfs:subClassOf observable:MACAddress ;
	rdfs:label "WifiAddress"@en ;
	rdfs:comment "A Wi-Fi address is a media access control (MAC) standards-conformant identifier assigned to a device network interface to enable routing and management of IEEE 802.11 standards-conformant communications to and from that device."@en ;
	.

observable:WifiAddressFacet
	a owl:Class ;
	rdfs:subClassOf
		<https://unifiedcyberontology.org/ontology/uco/core#MACAddressFacet> ,
		[
			a owl:Restriction ;
			owl:onProperty observable:addressValue ;
			owl:maxQualifiedCardinality "1"^^xsd:nonNegativeInteger ;
			owl:onDataRange xsd:string ;
		]
		;
	rdfs:label "WifiAddressFacet"@en ;
	rdfs:comment "A Wi-Fi address facet is a grouping of characteristics unique to a media access control (MAC) standards conformant identifier assigned to a device network interface to enable routing and management of IEEE 802.11 standards-conformant communications to and from that device."@en ;
	.

observable:Wiki
	a owl:Class ;
	rdfs:subClassOf observable:ObservableObject ;
	rdfs:label "Wiki"@en ;
	rdfs:comment "A wiki is an online hypertext publication collaboratively edited and managed by its own audience directly using a web browser. A typical wiki contains multiple pages/articles for the subjects or scope of the project and could be either open to the public or limited to use within an organization for maintaining its internal knowledge base. [based on https://en.wikipedia.org/wiki/Wiki]"@en ;
	.

observable:WikiArticle
	a owl:Class ;
	rdfs:subClassOf observable:ObservableObject ;
	rdfs:label "WikiArticle"@en ;
	rdfs:comment "A wiki article is one or more pages in a wiki focused on characterizing a particular topic."@en ;
	.

observable:WindowsAccount
	a owl:Class ;
	rdfs:subClassOf observable:DigitalAccount ;
	rdfs:label "WindowsAccount"@en ;
	rdfs:comment "A Windows account is a user account on a Windows operating system."@en ;
	.

observable:WindowsAccountFacet
	a owl:Class ;
	rdfs:subClassOf <https://unifiedcyberontology.org/ontology/uco/core#Facet> ;
	rdfs:label "WindowsAccountFacet"@en ;
	rdfs:comment "A Windows account facet is a grouping of characteristics unique to a user account on a Windows operating system."@en ;
	.

observable:WindowsActiveDirectoryAccount
	a owl:Class ;
	rdfs:subClassOf observable:DigitalAccount ;
	rdfs:label "WindowsActiveDirectoryAccount"@en ;
	rdfs:comment "A Windows Active Directory account is an account managed by directory-based identity-related services of a Windows operating system."@en ;
	.

observable:WindowsActiveDirectoryAccountFacet
	a owl:Class ;
	rdfs:subClassOf
		<https://unifiedcyberontology.org/ontology/uco/core#Facet> ,
		[
			a owl:Restriction ;
			owl:onProperty observable:objectGUID ;
			owl:onDataRange xsd:string ;
			owl:qualifiedCardinality "1"^^xsd:nonNegativeInteger ;
		]
		;
	rdfs:label "WindowsActiveDirectoryAccountFacet"@en ;
	rdfs:comment "A Windows Active Directory account facet is a grouping of characteristics unique to an account managed by directory-based identity-related services of a Windows operating system."@en ;
	.

observable:WindowsComputerSpecification
	a owl:Class ;
	rdfs:subClassOf observable:ObservableObject ;
	rdfs:label "WindowsComputerSpecification"@en ;
	rdfs:comment "A Windows computer specification is the hardware ans software of a programmable electronic device that can store, retrieve, and process data running a Microsoft Windows operating system. [based on merriam-webster.com/dictionary/computer]"@en ;
	.

observable:WindowsComputerSpecificationFacet
	a owl:Class ;
	rdfs:subClassOf
		<https://unifiedcyberontology.org/ontology/uco/core#Facet> ,
		[
			a owl:Restriction ;
			owl:onProperty observable:registeredOrganization ;
			owl:maxCardinality "1"^^xsd:nonNegativeInteger ;
		] ,
		[
			a owl:Restriction ;
			owl:onProperty observable:registeredOwner ;
			owl:maxCardinality "1"^^xsd:nonNegativeInteger ;
		] ,
		[
			a owl:Restriction ;
			owl:onProperty observable:windowsDirectory ;
			owl:onClass observable:ObservableObject ;
			owl:maxQualifiedCardinality "1"^^xsd:nonNegativeInteger ;
		] ,
		[
			a owl:Restriction ;
			owl:onProperty observable:windowsSystemDirectory ;
			owl:onClass observable:ObservableObject ;
			owl:maxQualifiedCardinality "1"^^xsd:nonNegativeInteger ;
		] ,
		[
			a owl:Restriction ;
			owl:onProperty observable:windowsTempDirectory ;
			owl:onClass observable:ObservableObject ;
			owl:maxQualifiedCardinality "1"^^xsd:nonNegativeInteger ;
		] ,
		[
			a owl:Restriction ;
			owl:onProperty observable:msProductID ;
			owl:maxQualifiedCardinality "1"^^xsd:nonNegativeInteger ;
			owl:onDataRange xsd:string ;
		] ,
		[
			a owl:Restriction ;
			owl:onProperty observable:msProductName ;
			owl:maxQualifiedCardinality "1"^^xsd:nonNegativeInteger ;
			owl:onDataRange xsd:string ;
		] ,
		[
			a owl:Restriction ;
			owl:onProperty observable:netBIOSName ;
			owl:maxQualifiedCardinality "1"^^xsd:nonNegativeInteger ;
			owl:onDataRange xsd:string ;
		]
		;
	rdfs:label "WindowsComputerSpecificationFacet"@en ;
	rdfs:comment "A Windows computer specification facet is a grouping of characteristics unique to the hardware and software of a programmable electronic device that can store, retrieve, and process data running a Microsoft Windows operating system. [based on merriam-webster.com/dictionary/computer]"@en ;
	.

observable:WindowsCriticalSection
	a owl:Class ;
	rdfs:subClassOf observable:ObservableObject ;
	rdfs:label "WindowsCriticalSection"@en ;
	rdfs:comment "A Windows critical section is a Windows object that provides synchronization similar to that provided by a mutex object, except that a critical section can be used only by the threads of a single process. Critical section objects cannot be shared across processes. Event, mutex, and semaphore objects can also be used in a single-process application, but critical section objects provide a slightly faster, more efficient mechanism for mutual-exclusion synchronization (a processor-specific test and set instruction). Like a mutex object, a critical section object can be owned by only one thread at a time, which makes it useful for protecting a shared resource from simultaneous access. Unlike a mutex object, there is no way to tell whether a critical section has been abandoned. [based on https://docs.microsoft.com/en-us/windows/win32/sync/critical-section-objects]"@en ;
	.

observable:WindowsEvent
	a owl:Class ;
	rdfs:subClassOf observable:ObservableObject ;
	rdfs:label "WindowsEvent"@en ;
	rdfs:comment "A Windows event is a notification record of an occurance of interest (system, security, application, etc.) on a Windows operating system."@en ;
	.

observable:WindowsFilemapping
	a owl:Class ;
	rdfs:subClassOf observable:ObservableObject ;
	rdfs:label "WindowsFilemapping"@en ;
	rdfs:comment "A Windows file mapping is the association of a file's contents with a portion of the virtual address space of a process within a Windows operating system. The system creates a file mapping object (also known as a section object) to maintain this association. A file view is the portion of virtual address space that a process uses to access the file's contents. File mapping allows the process to use both random input and output (I/O) and sequential I/O. It also allows the process to work efficiently with a large data file, such as a database, without having to map the whole file into memory. Multiple processes can also use memory-mapped files to share data. Processes read from and write to the file view using pointers, just as they would with dynamically allocated memory. The use of file mapping improves efficiency because the file resides on disk, but the file view resides in memory.[based on https://docs.microsoft.com/en-us/windows/win32/memory/file-mapping]"@en ;
	.

observable:WindowsHandle
	a owl:Class ;
	rdfs:subClassOf observable:ObservableObject ;
	rdfs:label "WindowsHandle"@en ;
	rdfs:comment "A Windows handle is an abstract reference to a resource within the Windows operating system, such as a window, memory, an open file or a pipe. It is the mechanism by which applications interact with such resources in the Windows operating system."@en ;
	.

observable:WindowsHook
	a owl:Class ;
	rdfs:subClassOf observable:ObservableObject ;
	rdfs:label "WindowsHook"@en ;
	rdfs:comment "A Windows hook is a mechanism by which an application can intercept events, such as messages, mouse actions, and keystrokes within the Windows operating system. A function that intercepts a particular type of event is known as a hook procedure. A hook procedure can act on each event it receives, and then modify or discard the event. [based on https://docs.microsoft.com/en-us/windows/win32/winmsg/about-hooks]"@en ;
	.

observable:WindowsMailslot
	a owl:Class ;
	rdfs:subClassOf observable:ObservableObject ;
	rdfs:label "WindowsMailslot"@en ;
	rdfs:comment "A Windows mailslot is is a pseudofile that resides in memory, and may be accessed using standard file functions. The data in a mailslot message can be in any form, but cannot be larger than 424 bytes when sent between computers. Unlike disk files, mailslots are temporary. When all handles to a mailslot are closed, the mailslot and all the data it contains are deleted. [based on https://docs.microsoft.com/en-us/windows/win32/ipc/about-mailslots]"@en ;
	.

observable:WindowsNetworkShare
	a owl:Class ;
	rdfs:subClassOf observable:ObservableObject ;
	rdfs:label "WindowsNetworkShare"@en ;
	rdfs:comment "A Windows network share is a Windows computer resource made available from one host to other hosts on a computer network. It is a device or piece of information on a computer that can be remotely accessed from another computer transparently as if it were a resource in the local machine. Network sharing is made possible by inter-process communication over the network. [based on https://en.wikipedia.org/wiki/Shared_resource]"@en ;
	.

observable:WindowsPEBinaryFile
	a owl:Class ;
	rdfs:subClassOf observable:File ;
	rdfs:label "WindowsPEBinaryFile"@en ;
	rdfs:comment "A Windows PE binary file is a Windows portable executable (PE) file."@en ;
	.

observable:WindowsPEBinaryFileFacet
	a owl:Class ;
	rdfs:subClassOf
		<https://unifiedcyberontology.org/ontology/uco/core#Facet> ,
		[
			a owl:Restriction ;
			owl:onProperty observable:peType ;
			owl:maxCardinality "1"^^xsd:nonNegativeInteger ;
		] ,
		[
			a owl:Restriction ;
			owl:onProperty observable:timeDateStamp ;
			owl:maxCardinality "1"^^xsd:nonNegativeInteger ;
		] ,
		[
			a owl:Restriction ;
			owl:onProperty observable:optionalHeader ;
			owl:onClass observable:WindowsPEOptionalHeader ;
			owl:maxQualifiedCardinality "1"^^xsd:nonNegativeInteger ;
		] ,
		[
			a owl:Restriction ;
			owl:onProperty observable:numberOfSections ;
			owl:maxQualifiedCardinality "1"^^xsd:nonNegativeInteger ;
			owl:onDataRange xsd:integer ;
		] ,
		[
			a owl:Restriction ;
			owl:onProperty observable:numberOfSymbols ;
			owl:maxQualifiedCardinality "1"^^xsd:nonNegativeInteger ;
			owl:onDataRange xsd:integer ;
		] ,
		[
			a owl:Restriction ;
			owl:onProperty observable:sizeOfOptionalHeader ;
			owl:maxQualifiedCardinality "1"^^xsd:nonNegativeInteger ;
			owl:onDataRange xsd:integer ;
		] ,
		[
			a owl:Restriction ;
			owl:onProperty observable:impHash ;
			owl:maxQualifiedCardinality "1"^^xsd:nonNegativeInteger ;
			owl:onDataRange xsd:string ;
		]
		;
	rdfs:label "WindowsPEBinaryFileFacet"@en ;
	rdfs:comment "A Windows PE binary file facet is a grouping of characteristics unique to a Windows portable executable (PE) file."@en ;
	.

observable:WindowsPEBinaryType
	a rdfs:Datatype ;
	owl:equivalentClass [
		a rdfs:Datatype ;
		owl:oneOf [
			a rdf:List ;
			rdf:first "dll" ;
			rdf:rest [
				a rdf:List ;
				rdf:first "exe" ;
				rdf:rest [
					a rdf:List ;
					rdf:first "sys" ;
					rdf:rest rdf:nil ;
				] ;
			] ;
		] ;
	] ;
	.

observable:WindowsPEFileHeader
	a owl:Class ;
	rdfs:subClassOf [
		a owl:Restriction ;
		owl:onProperty observable:timeDateStamp ;
		owl:maxCardinality "1"^^xsd:nonNegativeInteger ;
	] ;
	rdfs:label "WindowsPEFileHeader"@en ;
	rdfs:comment "A Windows PE file header is a grouping of characteristics unique to the 'header' of a Windows PE (Portable Executable) file, consisting of a collection of metadata about the overall nature and structure of the file."@en ;
	.

observable:WindowsPEOptionalHeader
	a owl:Class ;
	rdfs:label "WindowsPEOptionalHeader"@en ;
	rdfs:comment "A Windows PE optional header is a grouping of characteristics unique to the 'optional header' of a Windows PE (Portable Executable) file, consisting of a collection of metadata about the executable code structure of the file."@en ;
	.

observable:WindowsPESection
	a owl:Class ;
	rdfs:subClassOf
		[
			a owl:Restriction ;
			owl:onProperty observable:entropy ;
			owl:maxQualifiedCardinality "1"^^xsd:nonNegativeInteger ;
			owl:onDataRange xsd:float ;
		] ,
		[
			a owl:Restriction ;
			owl:onProperty observable:size ;
			owl:maxQualifiedCardinality "1"^^xsd:nonNegativeInteger ;
			owl:onDataRange xsd:integer ;
		] ,
		[
			a owl:Restriction ;
			owl:onProperty <https://unifiedcyberontology.org/ontology/uco/core#name> ;
			owl:onDataRange xsd:string ;
			owl:qualifiedCardinality "1"^^xsd:nonNegativeInteger ;
		]
		;
	rdfs:label "WindowsPESection"@en ;
	rdfs:comment "A Windows PE section is a grouping of characteristics unique to a specific default or custom-defined region of a Windows PE (Portable Executable) file, consisting of an individual portion of the actual executable content of the file delineated according to unique purpose and memory protection requirements."@en ;
	.

observable:WindowsPrefetch
	a owl:Class ;
	rdfs:subClassOf observable:ObservableObject ;
	rdfs:label "WindowsPrefetch"@en ;
	rdfs:comment "The Windows prefetch contains entries in a Windows prefetch file (used to speed up application startup starting with Windows XP)."@en ;
	.

observable:WindowsPrefetchFacet
	a owl:Class ;
	rdfs:subClassOf
		<https://unifiedcyberontology.org/ontology/uco/core#Facet> ,
		[
			a owl:Restriction ;
			owl:onProperty observable:firstRun ;
			owl:maxCardinality "1"^^xsd:nonNegativeInteger ;
		] ,
		[
			a owl:Restriction ;
			owl:onProperty observable:lastRun ;
			owl:maxCardinality "1"^^xsd:nonNegativeInteger ;
		] ,
		[
			a owl:Restriction ;
			owl:onProperty observable:volume ;
			owl:onClass observable:ObservableObject ;
			owl:maxQualifiedCardinality "1"^^xsd:nonNegativeInteger ;
		] ,
		[
			a owl:Restriction ;
			owl:onProperty observable:timesExecuted ;
			owl:maxQualifiedCardinality "1"^^xsd:nonNegativeInteger ;
			owl:onDataRange xsd:integer ;
		] ,
		[
			a owl:Restriction ;
			owl:onProperty observable:applicationFileName ;
			owl:maxQualifiedCardinality "1"^^xsd:nonNegativeInteger ;
			owl:onDataRange xsd:string ;
		] ,
		[
			a owl:Restriction ;
			owl:onProperty observable:prefetchHash ;
			owl:maxQualifiedCardinality "1"^^xsd:nonNegativeInteger ;
			owl:onDataRange xsd:string ;
		]
		;
	rdfs:label "WindowsPrefetchFacet"@en ;
	rdfs:comment "A Windows prefetch facet is a grouping of characteristics unique to entries in the Windows prefetch file (used to speed up application startup starting with Windows XP)."@en ;
	.

observable:WindowsProcess
	a owl:Class ;
	rdfs:subClassOf observable:Process ;
	rdfs:label "WindowsProcess"@en ;
	rdfs:comment "A Windows process is a program running on a Windows operating system."@en ;
	.

observable:WindowsProcessFacet
	a owl:Class ;
	rdfs:subClassOf
		<https://unifiedcyberontology.org/ontology/uco/core#Facet> ,
		[
			a owl:Restriction ;
			owl:onProperty observable:startupInfo ;
			owl:maxCardinality "1"^^xsd:nonNegativeInteger ;
		] ,
		[
			a owl:Restriction ;
			owl:onProperty observable:aslrEnabled ;
			owl:maxQualifiedCardinality "1"^^xsd:nonNegativeInteger ;
			owl:onDataRange xsd:boolean ;
		] ,
		[
			a owl:Restriction ;
			owl:onProperty observable:depEnabled ;
			owl:maxQualifiedCardinality "1"^^xsd:nonNegativeInteger ;
			owl:onDataRange xsd:boolean ;
		] ,
		[
			a owl:Restriction ;
			owl:onProperty observable:ownerSID ;
			owl:maxQualifiedCardinality "1"^^xsd:nonNegativeInteger ;
			owl:onDataRange xsd:string ;
		] ,
		[
			a owl:Restriction ;
			owl:onProperty observable:priority ;
			owl:maxQualifiedCardinality "1"^^xsd:nonNegativeInteger ;
			owl:onDataRange xsd:string ;
		] ,
		[
			a owl:Restriction ;
			owl:onProperty observable:windowTitle ;
			owl:maxQualifiedCardinality "1"^^xsd:nonNegativeInteger ;
			owl:onDataRange xsd:string ;
		]
		;
	rdfs:label "WindowsProcessFacet"@en ;
	rdfs:comment "A Windows process facet is a grouping of characteristics unique to a program running on a Windows operating system."@en ;
	.

observable:WindowsRegistryHive
	a owl:Class ;
	rdfs:subClassOf observable:ObservableObject ;
	rdfs:label "WindowsRegistryHive"@en ;
	rdfs:comment "The Windows registry hive is a particular logical group of keys, subkeys, and values in a Windows registry (a hierarchical database that stores low-level settings for the Microsoft Windows operating system and for applications that opt to use the registry). [based on https://en.wikipedia.org/wiki/Windows_Registry]"@en ;
	.

observable:WindowsRegistryHiveFacet
	a owl:Class ;
	rdfs:subClassOf
		<https://unifiedcyberontology.org/ontology/uco/core#Facet> ,
		[
			a owl:Restriction ;
			owl:onProperty observable:hiveType ;
			owl:maxQualifiedCardinality "1"^^xsd:nonNegativeInteger ;
			owl:onDataRange xsd:string ;
		]
		;
	rdfs:label "WindowsRegistryHiveFacet"@en ;
	rdfs:comment "A Windows registry hive facet is a grouping of characteristics unique to a particular logical group of keys, subkeys, and values in a Windows registry (a hierarchical database that stores low-level settings for the Microsoft Windows operating system and for applications that opt to use the registry). [based on https://en.wikipedia.org/wiki/Windows_Registry]"@en ;
	.

observable:WindowsRegistryKey
	a owl:Class ;
	rdfs:subClassOf observable:ObservableObject ;
	rdfs:label "WindowsRegistryKey"@en ;
	rdfs:comment "A Windows registry key is a particular key within a Windows registry (a hierarchical database that stores low-level settings for the Microsoft Windows operating system and for applications that opt to use the registry). [based on https://en.wikipedia.org/wiki/Windows_Registry]"@en ;
	.

observable:WindowsRegistryKeyFacet
	a owl:Class ;
	rdfs:subClassOf
		<https://unifiedcyberontology.org/ontology/uco/core#Facet> ,
		[
			a owl:Restriction ;
			owl:onProperty observable:modifiedTime ;
			owl:maxCardinality "1"^^xsd:nonNegativeInteger ;
		] ,
		[
			a owl:Restriction ;
			owl:onProperty observable:creator ;
			owl:onClass observable:ObservableObject ;
			owl:maxQualifiedCardinality "1"^^xsd:nonNegativeInteger ;
		] ,
		[
			a owl:Restriction ;
			owl:onProperty observable:numberOfSubkeys ;
			owl:maxQualifiedCardinality "1"^^xsd:nonNegativeInteger ;
			owl:onDataRange xsd:integer ;
		] ,
		[
			a owl:Restriction ;
			owl:onProperty observable:key ;
			owl:onDataRange xsd:string ;
			owl:qualifiedCardinality "1"^^xsd:nonNegativeInteger ;
		]
		;
	rdfs:label "WindowsRegistryKeyFacet"@en ;
	rdfs:comment "A Windows registry key facet is a grouping of characteristics unique to a particular key within a Windows registry (A hierarchical database that stores low-level settings for the Microsoft Windows operating system and for applications that opt to use the registry). [based on https://en.wikipedia.org/wiki/Windows_Registry]"@en ;
	.

observable:WindowsRegistryValue
	a owl:Class ;
	rdfs:subClassOf
		[
			a owl:Restriction ;
			owl:onProperty observable:dataType ;
			owl:maxCardinality "1"^^xsd:nonNegativeInteger ;
		] ,
		[
			a owl:Restriction ;
			owl:onProperty observable:data ;
			owl:maxQualifiedCardinality "1"^^xsd:nonNegativeInteger ;
			owl:onDataRange xsd:string ;
		] ,
		[
			a owl:Restriction ;
			owl:onProperty <https://unifiedcyberontology.org/ontology/uco/core#name> ;
			owl:onDataRange xsd:string ;
			owl:qualifiedCardinality "1"^^xsd:nonNegativeInteger ;
		]
		;
	rdfs:label "WindowsRegistryValue"@en ;
	rdfs:comment "A Windows registry value is a grouping of characteristics unique to a particular value within a Windows registry (a hierarchical database that stores low-level settings for the Microsoft Windows operating system and for applications that opt to use the registry. [based on https://en.wikipedia.org/wiki/Windows_Registry]"@en ;
	.

observable:WindowsService
	a owl:Class ;
	rdfs:subClassOf observable:ObservableObject ;
	rdfs:label "WindowsService"@en ;
	rdfs:comment "A Windows service is a specific Windows service (a computer program that operates in the background of a Windows operating system, similar to the way a UNIX daemon runs on UNIX). [based on https://en.wikipedia.org/wiki/Windows_service]"@en ;
	.

observable:WindowsServiceFacet
	a owl:Class ;
	rdfs:subClassOf
		<https://unifiedcyberontology.org/ontology/uco/core#Facet> ,
		[
			a owl:Restriction ;
			owl:onProperty observable:serviceStatus ;
			owl:maxCardinality "1"^^xsd:nonNegativeInteger ;
		] ,
		[
			a owl:Restriction ;
			owl:onProperty observable:serviceType ;
			owl:maxCardinality "1"^^xsd:nonNegativeInteger ;
		] ,
		[
			a owl:Restriction ;
			owl:onProperty observable:startType ;
			owl:maxCardinality "1"^^xsd:nonNegativeInteger ;
		] ,
		[
			a owl:Restriction ;
			owl:onProperty observable:displayName ;
			owl:maxQualifiedCardinality "1"^^xsd:nonNegativeInteger ;
			owl:onDataRange xsd:string ;
		] ,
		[
			a owl:Restriction ;
			owl:onProperty observable:groupName ;
			owl:maxQualifiedCardinality "1"^^xsd:nonNegativeInteger ;
			owl:onDataRange xsd:string ;
		] ,
		[
			a owl:Restriction ;
			owl:onProperty observable:startCommandLine ;
			owl:maxQualifiedCardinality "1"^^xsd:nonNegativeInteger ;
			owl:onDataRange xsd:string ;
		] ,
		[
			a owl:Restriction ;
			owl:onProperty observable:serviceName ;
			owl:onDataRange xsd:string ;
			owl:qualifiedCardinality "1"^^xsd:nonNegativeInteger ;
		]
		;
	rdfs:label "WindowsServiceFacet"@en ;
	rdfs:comment "A Windows service facet is a grouping of characteristics unique to a specific Windows service (a computer program that operates in the background of a Windows operating system, similar to the way a UNIX daemon runs on UNIX). [based on https://en.wikipedia.org/wiki/Windows_service]"@en ;
	.

observable:WindowsServiceStartType
	a rdfs:Datatype ;
	owl:equivalentClass [
		a rdfs:Datatype ;
		owl:oneOf [
			a rdf:List ;
			rdf:first "service_auto_start" ;
			rdf:rest [
				a rdf:List ;
				rdf:first "service_boot_start" ;
				rdf:rest [
					a rdf:List ;
					rdf:first "service_demand_start" ;
					rdf:rest [
						a rdf:List ;
						rdf:first "service_disabled" ;
						rdf:rest [
							a rdf:List ;
							rdf:first "service_system_alert" ;
							rdf:rest rdf:nil ;
						] ;
					] ;
				] ;
			] ;
		] ;
	] ;
	.

observable:WindowsServiceStatus
	a rdfs:Datatype ;
	owl:equivalentClass [
		a rdfs:Datatype ;
		owl:oneOf [
			a rdf:List ;
			rdf:first "service_continue_pending" ;
			rdf:rest [
				a rdf:List ;
				rdf:first "service_pause_pending" ;
				rdf:rest [
					a rdf:List ;
					rdf:first "service_paused" ;
					rdf:rest [
						a rdf:List ;
						rdf:first "service_running" ;
						rdf:rest [
							a rdf:List ;
							rdf:first "service_start_pending" ;
							rdf:rest [
								a rdf:List ;
								rdf:first "service_stop_pending" ;
								rdf:rest [
									a rdf:List ;
									rdf:first "service_stopped" ;
									rdf:rest rdf:nil ;
								] ;
							] ;
						] ;
					] ;
				] ;
			] ;
		] ;
	] ;
	.

observable:WindowsServiceType
	a rdfs:Datatype ;
	owl:equivalentClass [
		a rdfs:Datatype ;
		owl:oneOf [
			a rdf:List ;
			rdf:first "service_file_system_driver" ;
			rdf:rest [
				a rdf:List ;
				rdf:first "service_kernel_driver" ;
				rdf:rest [
					a rdf:List ;
					rdf:first "service_win32_own_process" ;
					rdf:rest [
						a rdf:List ;
						rdf:first "service_win32_share_process" ;
						rdf:rest rdf:nil ;
					] ;
				] ;
			] ;
		] ;
	] ;
	.

observable:WindowsSystemRestore
	a owl:Class ;
	rdfs:subClassOf observable:ObservableObject ;
	rdfs:label "WindowsSystemRestore"@en ;
	rdfs:comment "A Windows system restore is a capture of a Windows computer's state (including system files, installed applications, Windows Registry, and system settings) at a particular point in time such that the computer can be reverted to that state in the event of system malfunctions or other problems. [based on https://en.wikipedia.org/wiki/System_Restore]"@en ;
	.

observable:WindowsTask
	a owl:Class ;
	rdfs:subClassOf observable:ObservableObject ;
	rdfs:label "WindowsTask"@en ;
	rdfs:comment "A Windows task is a process that is scheduled to execute on a Windows operating system by the Windows Task Scheduler. [based on http://msdn.microsoft.com/en-us/library/windows/desktop/aa381311(v=vs.85).aspx]"@en ;
	.

observable:WindowsTaskFacet
	a owl:Class ;
	rdfs:subClassOf
		<https://unifiedcyberontology.org/ontology/uco/core#Facet> ,
		[
			a owl:Restriction ;
			owl:onProperty observable:mostRecentRunTime ;
			owl:maxCardinality "1"^^xsd:nonNegativeInteger ;
		] ,
		[
			a owl:Restriction ;
			owl:onProperty observable:nextRunTime ;
			owl:maxCardinality "1"^^xsd:nonNegativeInteger ;
		] ,
		[
			a owl:Restriction ;
			owl:onProperty observable:observableCreatedTime ;
			owl:maxCardinality "1"^^xsd:nonNegativeInteger ;
		] ,
		[
			a owl:Restriction ;
			owl:onProperty observable:account ;
			owl:onClass observable:ObservableObject ;
			owl:maxQualifiedCardinality "1"^^xsd:nonNegativeInteger ;
		] ,
		[
			a owl:Restriction ;
			owl:onProperty observable:application ;
			owl:onClass observable:ObservableObject ;
			owl:maxQualifiedCardinality "1"^^xsd:nonNegativeInteger ;
		] ,
		[
			a owl:Restriction ;
			owl:onProperty observable:workItemData ;
			owl:onClass observable:ObservableObject ;
			owl:maxQualifiedCardinality "1"^^xsd:nonNegativeInteger ;
		] ,
		[
			a owl:Restriction ;
			owl:onProperty observable:workingDirectory ;
			owl:onClass observable:ObservableObject ;
			owl:maxQualifiedCardinality "1"^^xsd:nonNegativeInteger ;
		] ,
		[
			a owl:Restriction ;
			owl:onProperty observable:exitCode ;
			owl:maxQualifiedCardinality "1"^^xsd:nonNegativeInteger ;
			owl:onDataRange xsd:integer ;
		] ,
		[
			a owl:Restriction ;
			owl:onProperty observable:maxRunTime ;
			owl:maxQualifiedCardinality "1"^^xsd:nonNegativeInteger ;
			owl:onDataRange xsd:integer ;
		] ,
		[
			a owl:Restriction ;
			owl:onProperty observable:accountLogonType ;
			owl:maxQualifiedCardinality "1"^^xsd:nonNegativeInteger ;
			owl:onDataRange xsd:string ;
		] ,
		[
			a owl:Restriction ;
			owl:onProperty observable:accountRunLevel ;
			owl:maxQualifiedCardinality "1"^^xsd:nonNegativeInteger ;
			owl:onDataRange xsd:string ;
		] ,
		[
			a owl:Restriction ;
			owl:onProperty observable:imageName ;
			owl:maxQualifiedCardinality "1"^^xsd:nonNegativeInteger ;
			owl:onDataRange xsd:string ;
		] ,
		[
			a owl:Restriction ;
			owl:onProperty observable:parameters ;
			owl:maxQualifiedCardinality "1"^^xsd:nonNegativeInteger ;
			owl:onDataRange xsd:string ;
		] ,
		[
			a owl:Restriction ;
			owl:onProperty observable:taskComment ;
			owl:maxQualifiedCardinality "1"^^xsd:nonNegativeInteger ;
			owl:onDataRange xsd:string ;
		] ,
		[
			a owl:Restriction ;
			owl:onProperty observable:taskCreator ;
			owl:maxQualifiedCardinality "1"^^xsd:nonNegativeInteger ;
			owl:onDataRange xsd:string ;
		] ,
		[
			a owl:Restriction ;
			owl:onProperty observable:priority ;
			owl:maxQualifiedCardinality "1"^^xsd:nonNegativeInteger ;
			owl:onDataRange vocabulary:TaskPriorityVocab ;
		] ,
		[
			a owl:Restriction ;
			owl:onProperty observable:status ;
			owl:maxQualifiedCardinality "1"^^xsd:nonNegativeInteger ;
			owl:onDataRange vocabulary:TaskStatusVocab ;
		]
		;
	rdfs:label "WindowsTaskFacet"@en ;
	rdfs:comment "A Windows Task facet is a grouping of characteristics unique to a Windows Task (a process that is scheduled to execute on a Windows operating system by the Windows Task Scheduler). [based on http://msdn.microsoft.com/en-us/library/windows/desktop/aa381311(v=vs.85).aspx]"@en ;
	.

observable:WindowsThread
	a owl:Class ;
	rdfs:subClassOf observable:Thread ;
	rdfs:label "WindowsThread"@en ;
	rdfs:comment "A Windows thread is a single thread of execution within a Windows process."@en ;
	.

observable:WindowsThreadFacet
	a owl:Class ;
	rdfs:subClassOf
		<https://unifiedcyberontology.org/ontology/uco/core#Facet> ,
		[
			a owl:Restriction ;
			owl:onProperty observable:creationTime ;
			owl:maxCardinality "1"^^xsd:nonNegativeInteger ;
		] ,
		[
			a owl:Restriction ;
			owl:onProperty observable:runningStatus ;
			owl:maxCardinality "1"^^xsd:nonNegativeInteger ;
		] ,
		[
			a owl:Restriction ;
			owl:onProperty observable:priority ;
			owl:maxQualifiedCardinality "1"^^xsd:nonNegativeInteger ;
			owl:onDataRange xsd:integer ;
		] ,
		[
			a owl:Restriction ;
			owl:onProperty observable:context ;
			owl:maxQualifiedCardinality "1"^^xsd:nonNegativeInteger ;
			owl:onDataRange xsd:string ;
		] ,
		[
			a owl:Restriction ;
			owl:onProperty observable:securityAttributes ;
			owl:maxQualifiedCardinality "1"^^xsd:nonNegativeInteger ;
			owl:onDataRange xsd:string ;
		]
		;
	rdfs:label "WindowsThreadFacet"@en ;
	rdfs:comment "A Windows thread facet is a grouping os characteristics unique to a single thread of execution within a Windows process."@en ;
	.

observable:WindowsVolumeFacet
	a owl:Class ;
	rdfs:subClassOf
		<https://unifiedcyberontology.org/ontology/uco/core#Facet> ,
		[
			a owl:Restriction ;
			owl:onProperty observable:driveLetter ;
			owl:maxQualifiedCardinality "1"^^xsd:nonNegativeInteger ;
			owl:onDataRange xsd:string ;
		] ,
		[
			a owl:Restriction ;
			owl:onProperty observable:driveType ;
			owl:maxQualifiedCardinality "1"^^xsd:nonNegativeInteger ;
			owl:onDataRange vocabulary:WindowsDriveTypeVocab ;
		] ,
		[
			a owl:Restriction ;
			owl:onProperty observable:windowsVolumeAttributes ;
			owl:maxQualifiedCardinality "4"^^xsd:nonNegativeInteger ;
			owl:onDataRange vocabulary:WindowsVolumeAttributeVocab ;
		]
		;
	rdfs:label "WindowsVolumeFacet"@en ;
	rdfs:comment "A Windows volume facet is a grouping of characteristics unique to a single accessible storage area (volume) with a single Windows file system. [based on https://en.wikipedia.org/wiki/Volume_(computing)]"@en ;
	.

observable:WindowsWaitableTime
	a owl:Class ;
	rdfs:subClassOf observable:ObservableObject ;
	rdfs:label "WindowsWaitableTime"@en ;
	rdfs:comment "A Windows waitable timer is a synchronization object within the Windows operating system whose state is set to signaled when a specified due time arrives. There are two types of waitable timers that can be created: manual-reset and synchronization. A timer of either type can also be a periodic timer. [based on https://docs.microsoft.com/en-us/windows/win32/sync/waitable-timer-objects]"@en ;
	.

observable:WirelessNetworkConnection
	a owl:Class ;
	rdfs:subClassOf observable:NetworkConnection ;
	rdfs:label "WirelessNetworkConnection"@en ;
	rdfs:comment "A wireless network connection is a connection (completed or attempted) across an IEEE 802.11 standards-confromant digital network (a group of two or more computer systems linked together). [based on https://www.webopedia.com/TERM/N/network.html]"@en ;
	.

observable:WirelessNetworkConnectionFacet
	a owl:Class ;
	rdfs:subClassOf
		<https://unifiedcyberontology.org/ontology/uco/core#Facet> ,
		[
			a owl:Restriction ;
			owl:onProperty observable:baseStation ;
			owl:maxQualifiedCardinality "1"^^xsd:nonNegativeInteger ;
			owl:onDataRange xsd:string ;
		] ,
		[
			a owl:Restriction ;
			owl:onProperty observable:ssid ;
			owl:maxQualifiedCardinality "1"^^xsd:nonNegativeInteger ;
			owl:onDataRange xsd:string ;
		]
		;
	rdfs:label "WirelessNetworkConnectionFacet"@en ;
	rdfs:comment "A wireless network connection facet is a grouping of characteristics unique to a connection (completed or attempted) across an IEEE 802.11 standards-conformant digital network (a group of two or more computer systems linked together). [based on https://www.webopedia.com/TERM/N/network.html]"@en ;
	.

observable:X509Certificate
	a owl:Class ;
	rdfs:subClassOf observable:ObservableObject ;
	rdfs:label "X509Certificate"@en ;
	rdfs:comment "A X.509 certificate is a public key digital identity certificate conformant to the X.509 PKI (Public Key Infrastructure) standard."@en ;
	.

observable:X509CertificateFacet
	a owl:Class ;
	rdfs:subClassOf
		<https://unifiedcyberontology.org/ontology/uco/core#Facet> ,
		[
			a owl:Restriction ;
			owl:onProperty observable:issuerHash ;
			owl:maxCardinality "1"^^xsd:nonNegativeInteger ;
		] ,
		[
			a owl:Restriction ;
			owl:onProperty observable:subjectHash ;
			owl:maxCardinality "1"^^xsd:nonNegativeInteger ;
		] ,
		[
			a owl:Restriction ;
			owl:onProperty observable:thumbprintHash ;
			owl:maxCardinality "1"^^xsd:nonNegativeInteger ;
		] ,
		[
			a owl:Restriction ;
			owl:onProperty observable:validityNotAfter ;
			owl:maxCardinality "1"^^xsd:nonNegativeInteger ;
		] ,
		[
			a owl:Restriction ;
			owl:onProperty observable:validityNotBefore ;
			owl:maxCardinality "1"^^xsd:nonNegativeInteger ;
		] ,
		[
			a owl:Restriction ;
			owl:onProperty observable:x509v3extensions ;
			owl:onClass observable:X509V3ExtensionsFacet ;
			owl:maxQualifiedCardinality "1"^^xsd:nonNegativeInteger ;
		] ,
		[
			a owl:Restriction ;
			owl:onProperty observable:isSelfSigned ;
			owl:maxQualifiedCardinality "1"^^xsd:nonNegativeInteger ;
			owl:onDataRange xsd:boolean ;
		] ,
		[
			a owl:Restriction ;
			owl:onProperty observable:subjectPublicKeyExponent ;
			owl:maxQualifiedCardinality "1"^^xsd:nonNegativeInteger ;
			owl:onDataRange xsd:integer ;
		] ,
		[
			a owl:Restriction ;
			owl:onProperty observable:issuer ;
			owl:maxQualifiedCardinality "1"^^xsd:nonNegativeInteger ;
			owl:onDataRange xsd:string ;
		] ,
		[
			a owl:Restriction ;
			owl:onProperty observable:serialNumber ;
			owl:maxQualifiedCardinality "1"^^xsd:nonNegativeInteger ;
			owl:onDataRange xsd:string ;
		] ,
		[
			a owl:Restriction ;
			owl:onProperty observable:signature ;
			owl:maxQualifiedCardinality "1"^^xsd:nonNegativeInteger ;
			owl:onDataRange xsd:string ;
		] ,
		[
			a owl:Restriction ;
			owl:onProperty observable:signatureAlgorithm ;
			owl:maxQualifiedCardinality "1"^^xsd:nonNegativeInteger ;
			owl:onDataRange xsd:string ;
		] ,
		[
			a owl:Restriction ;
			owl:onProperty observable:subject ;
			owl:maxQualifiedCardinality "1"^^xsd:nonNegativeInteger ;
			owl:onDataRange xsd:string ;
		] ,
		[
			a owl:Restriction ;
			owl:onProperty observable:subjectPublicKeyAlgorithm ;
			owl:maxQualifiedCardinality "1"^^xsd:nonNegativeInteger ;
			owl:onDataRange xsd:string ;
		] ,
		[
			a owl:Restriction ;
			owl:onProperty observable:subjectPublicKeyModulus ;
			owl:maxQualifiedCardinality "1"^^xsd:nonNegativeInteger ;
			owl:onDataRange xsd:string ;
		] ,
		[
			a owl:Restriction ;
			owl:onProperty observable:version ;
			owl:maxQualifiedCardinality "1"^^xsd:nonNegativeInteger ;
			owl:onDataRange xsd:string ;
		]
		;
	rdfs:label "X509CertificateFacet"@en ;
	rdfs:comment "A X.509 certificate facet is a grouping of characteristics unique to a public key digital identity certificate conformant to the X.509 PKI (Public Key Infrastructure) standard. "@en ;
	.

observable:X509V3Certificate
	a owl:Class ;
	rdfs:subClassOf observable:ObservableObject ;
	rdfs:label "X509V3Certificate"@en ;
	rdfs:comment "An X.509 v3 certificate is a public key digital identity certificate conformant to the X.509 v3 PKI (Public Key Infrastructure) standard. "@en ;
	.

observable:X509V3ExtensionsFacet
	a owl:Class ;
	rdfs:subClassOf
		<https://unifiedcyberontology.org/ontology/uco/core#Facet> ,
		[
			a owl:Restriction ;
			owl:onProperty observable:privateKeyUsagePeriodNotAfter ;
			owl:maxCardinality "1"^^xsd:nonNegativeInteger ;
		] ,
		[
			a owl:Restriction ;
			owl:onProperty observable:privateKeyUsagePeriodNotBefore ;
			owl:maxCardinality "1"^^xsd:nonNegativeInteger ;
		] ,
		[
			a owl:Restriction ;
			owl:onProperty observable:authorityKeyIdentifier ;
			owl:maxQualifiedCardinality "1"^^xsd:nonNegativeInteger ;
			owl:onDataRange xsd:string ;
		] ,
		[
			a owl:Restriction ;
			owl:onProperty observable:basicConstraints ;
			owl:maxQualifiedCardinality "1"^^xsd:nonNegativeInteger ;
			owl:onDataRange xsd:string ;
		] ,
		[
			a owl:Restriction ;
			owl:onProperty observable:certificatePolicies ;
			owl:maxQualifiedCardinality "1"^^xsd:nonNegativeInteger ;
			owl:onDataRange xsd:string ;
		] ,
		[
			a owl:Restriction ;
			owl:onProperty observable:crlDistributionPoints ;
			owl:maxQualifiedCardinality "1"^^xsd:nonNegativeInteger ;
			owl:onDataRange xsd:string ;
		] ,
		[
			a owl:Restriction ;
			owl:onProperty observable:extendedKeyUsage ;
			owl:maxQualifiedCardinality "1"^^xsd:nonNegativeInteger ;
			owl:onDataRange xsd:string ;
		] ,
		[
			a owl:Restriction ;
			owl:onProperty observable:inhibitAnyPolicy ;
			owl:maxQualifiedCardinality "1"^^xsd:nonNegativeInteger ;
			owl:onDataRange xsd:string ;
		] ,
		[
			a owl:Restriction ;
			owl:onProperty observable:issuerAlternativeName ;
			owl:maxQualifiedCardinality "1"^^xsd:nonNegativeInteger ;
			owl:onDataRange xsd:string ;
		] ,
		[
			a owl:Restriction ;
			owl:onProperty observable:keyUsage ;
			owl:maxQualifiedCardinality "1"^^xsd:nonNegativeInteger ;
			owl:onDataRange xsd:string ;
		] ,
		[
			a owl:Restriction ;
			owl:onProperty observable:nameConstraints ;
			owl:maxQualifiedCardinality "1"^^xsd:nonNegativeInteger ;
			owl:onDataRange xsd:string ;
		] ,
		[
			a owl:Restriction ;
			owl:onProperty observable:policyConstraints ;
			owl:maxQualifiedCardinality "1"^^xsd:nonNegativeInteger ;
			owl:onDataRange xsd:string ;
		] ,
		[
			a owl:Restriction ;
			owl:onProperty observable:policyMappings ;
			owl:maxQualifiedCardinality "1"^^xsd:nonNegativeInteger ;
			owl:onDataRange xsd:string ;
		] ,
		[
			a owl:Restriction ;
			owl:onProperty observable:subjectAlternativeName ;
			owl:maxQualifiedCardinality "1"^^xsd:nonNegativeInteger ;
			owl:onDataRange xsd:string ;
		] ,
		[
			a owl:Restriction ;
			owl:onProperty observable:subjectDirectoryAttributes ;
			owl:maxQualifiedCardinality "1"^^xsd:nonNegativeInteger ;
			owl:onDataRange xsd:string ;
		] ,
		[
			a owl:Restriction ;
			owl:onProperty observable:subjectKeyIdentifier ;
			owl:maxQualifiedCardinality "1"^^xsd:nonNegativeInteger ;
			owl:onDataRange xsd:string ;
		]
		;
	rdfs:label "X509V3ExtensionsFacet"@en ;
	rdfs:comment "An X.509 v3 certificate extensions facet is a grouping of characteristics unique to a public key digital identity certificate conformant to the X.509 v3 PKI (Public Key Infrastructure) standard."@en ;
	.

observable:abbreviation
	a owl:DatatypeProperty ;
	rdfs:label "abbreviation"@en ;
	rdfs:comment "The abbreviation of a global flag. See also: http://msdn.microsoft.com/en-us/library/windows/hardware/ff549646(v=vs.85).aspx."@en ;
	rdfs:range xsd:string ;
	.

observable:accessedDirectory
	a owl:ObjectProperty ;
	rdfs:label "accessedDirectory"@en ;
	rdfs:comment "Directories accessed by the prefetch application during startup."@en ;
	rdfs:range observable:ObservableObject ;
	.

observable:accessedFile
	a owl:ObjectProperty ;
	rdfs:label "accessedFile"@en ;
	rdfs:comment "Files (e.g., DLLs and other support files) used by the application during startup."@en ;
	rdfs:range observable:ObservableObject ;
	.

observable:accessedTime
	a owl:DatatypeProperty ;
	rdfs:label "accessedTime"@en ;
	rdfs:comment "The date and time at which the Object was accessed."@en ;
	rdfs:range xsd:dateTime ;
	.

observable:account
	a owl:ObjectProperty ;
	rdfs:label "account"@en ;
	rdfs:comment "Specifies the account used to run the scheduled task. See also: http://msdn.microsoft.com/en-us/library/windows/desktop/aa381228(v=vs.85).aspx."@en ;
	rdfs:range observable:ObservableObject ;
	.

observable:accountIdentifier
	a owl:DatatypeProperty ;
	rdfs:label "accountIdentifier"@en ;
	rdfs:comment "The unique identifier for the account."@en ;
	rdfs:range xsd:string ;
	.

observable:accountIssuer
	a owl:ObjectProperty ;
	rdfs:label "accountIssuer"@en ;
	rdfs:comment "The issuer of this account."@en ;
	rdfs:range <https://unifiedcyberontology.org/ontology/uco/core#UcoObject> ;
	.

observable:accountLogin
	a owl:DatatypeProperty ;
	rdfs:label "accountLogin"@en ;
	rdfs:comment "The login identifier for the digital account."@en ;
	rdfs:range xsd:string ;
	.

observable:accountLogonType
	a owl:DatatypeProperty ;
	rdfs:label "accountLogonType"@en ;
	rdfs:comment "Specifies the security logon method required to run the tasks associated with the account. See also: http://msdn.microsoft.com/en-us/library/windows/desktop/aa383013(v=vs.85).aspx."@en ;
	rdfs:range xsd:string ;
	.

observable:accountRunLevel
	a owl:DatatypeProperty ;
	rdfs:label "accountRunLevel"@en ;
	rdfs:comment "Specifies the permission level of the account that the task will be run at."@en ;
	rdfs:range xsd:string ;
	.

observable:accountType
	a owl:DatatypeProperty ;
	rdfs:label "accountType"@en ;
	rdfs:comment "The type of account, for instance bank, phone, application, service, etc."@en ;
	rdfs:range vocabulary:AccountTypeVocab ;
	.

observable:actionID
	a owl:DatatypeProperty ;
	rdfs:label "actionID"@en ;
	rdfs:comment "Specifies the user-defined identifier for the action. This identifier is used by the Task Scheduler for logging purposes. See also: http://msdn.microsoft.com/en-us/library/windows/desktop/aa380590(v=vs.85).aspx."@en ;
	rdfs:range xsd:string ;
	.

observable:actionList
	a owl:ObjectProperty ;
	rdfs:label "actionList"@en ;
	rdfs:comment "Specifies a list of actions to be performed by the scheduled task."@en ;
	rdfs:range observable:TaskActionType ;
	.

observable:actionType
	a owl:DatatypeProperty ;
	rdfs:label "actionType"@en ;
	rdfs:comment "Specifies the type of the action. See also: http://msdn.microsoft.com/en-us/library/windows/desktop/aa380596(v=vs.85).aspx."@en ;
	rdfs:range vocabulary:TaskActionTypeVocab ;
	.

observable:activeDirectoryGroups
	a owl:DatatypeProperty ;
	rdfs:label "activeDirectoryGroups"@en ;
	rdfs:range xsd:string ;
	.

observable:adapterName
	a owl:DatatypeProperty ;
	rdfs:label "adapterName"@en ;
	rdfs:comment "Specifies the name of the network adapter used by the network interface."@en ;
	rdfs:range xsd:string ;
	.

observable:addressOfEntryPoint
	a owl:DatatypeProperty ;
	rdfs:label "addressOfEntryPoint"@en ;
	rdfs:comment "Specifies the address of the entry point relative to the image base when the executable is loaded into memory."@en ;
	rdfs:range xsd:unsignedInt ;
	.

observable:addressValue
	a owl:DatatypeProperty ;
	rdfs:label "addressValue"@en ;
	rdfs:comment "The value of an address."@en ;
	rdfs:range xsd:string ;
	.

observable:allocationStatus
	a owl:DatatypeProperty ;
	rdfs:label "allocationStatus"@en ;
	rdfs:comment "The allocation status of a file."@en ;
	rdfs:range xsd:string ;
	.

observable:alternateDataStreams
	a owl:ObjectProperty ;
	rdfs:label "alternateDataStreams"@en ;
	rdfs:range observable:AlternateDataStream ;
	.

observable:application
	a owl:ObjectProperty ;
	rdfs:label "application"@en ;
	rdfs:comment "The application associated with this object."@en ;
	rdfs:range observable:ObservableObject ;
	.

observable:applicationFileName
	a owl:DatatypeProperty ;
	rdfs:label "applicationFileName"@en ;
	rdfs:comment "Name of the executable of the prefetch file."@en ;
	rdfs:range xsd:string ;
	.

observable:applicationIdentifier
	a owl:DatatypeProperty ;
	rdfs:label "applicationIdentifier"@en ;
	rdfs:range xsd:string ;
	.

observable:archiveType
	a owl:DatatypeProperty ;
	rdfs:label "archiveType"@en ;
	rdfs:comment "The type of a file archive, e.g. ZIP, GZIP or RAR."@en ;
	rdfs:range xsd:string ;
	.

observable:arguments
	a owl:DatatypeProperty ;
	rdfs:label "arguments"@en ;
	rdfs:comment "A list of arguments utilized in initiating the process."@en ;
	rdfs:range xsd:string ;
	.

observable:asHandle
	a owl:DatatypeProperty ;
	rdfs:label "asHandle"@en ;
	rdfs:range xsd:string ;
	.

observable:aslrEnabled
	a owl:DatatypeProperty ;
	rdfs:label "aslrEnabled"@en ;
	rdfs:range xsd:boolean ;
	.

observable:attendant
	a owl:ObjectProperty ;
	rdfs:label "attendant"@en ;
	rdfs:comment "The attendants of the event."@en ;
	rdfs:range identity:Identity ;
	.

observable:audioType
	a owl:DatatypeProperty ;
	rdfs:label "audioType"@en ;
	rdfs:comment "The type of a audio. For example: music or speech."@en ;
	rdfs:range xsd:string ;
	.

observable:authorityKeyIdentifier
	a owl:DatatypeProperty ;
	rdfs:label "authorityKeyIdentifier"@en ;
	rdfs:range xsd:string ;
	.

observable:availableRam
	a owl:DatatypeProperty ;
	rdfs:label "availableRam"@en ;
	rdfs:comment "Specifies the amount of physical memory available on the system, in bytes."@en ;
	rdfs:range xsd:integer ;
	.

observable:baseOfCode
	a owl:DatatypeProperty ;
	rdfs:label "baseOfCode"@en ;
	rdfs:comment "Specifies the address that is relative to the image base of the beginning-of-code section when it is loaded into memory."@en ;
	rdfs:range xsd:unsignedInt ;
	.

observable:baseStation
	a owl:DatatypeProperty ;
	rdfs:label "baseStation"@en ;
	rdfs:comment "The base station."@en ;
	rdfs:range xsd:string ;
	.

observable:basicConstraints
	a owl:DatatypeProperty ;
	rdfs:label "basicConstraints"@en ;
	rdfs:range xsd:string ;
	.

observable:bcc
	a owl:ObjectProperty ;
	rdfs:label "bcc"@en ;
	rdfs:range observable:ObservableObject ;
	.

observable:binary
	a owl:ObjectProperty ;
	rdfs:label "binary"@en ;
	rdfs:range observable:ObservableObject ;
	.

observable:biosDate
	a owl:DatatypeProperty ;
	rdfs:label "biosDate"@en ;
	rdfs:comment "Specifies the date of the BIOS (e.g. the datestamp of the BIOS revision)."@en ;
	rdfs:range xsd:dateTime ;
	.

observable:biosManufacturer
	a owl:DatatypeProperty ;
	rdfs:label "biosManufacturer"@en ;
	rdfs:comment "Specifies the manufacturer of the BIOS."@en ;
	rdfs:range xsd:string ;
	.

observable:biosReleaseDate
	a owl:DatatypeProperty ;
	rdfs:label "biosReleaseDate"@en ;
	rdfs:comment "Specifies the date the BIOS was released."@en ;
	rdfs:range xsd:dateTime ;
	.

observable:biosSerialNumber
	a owl:DatatypeProperty ;
	rdfs:label "biosSerialNumber"@en ;
	rdfs:comment "Specifies the serial number of the BIOS."@en ;
	rdfs:range xsd:string ;
	.

observable:biosVersion
	a owl:DatatypeProperty ;
	rdfs:label "biosVersion"@en ;
	rdfs:comment "Specifies the version of the BIOS."@en ;
	rdfs:range xsd:string ;
	.

observable:bitRate
	a owl:DatatypeProperty ;
	rdfs:label "bitRate"@en ;
	rdfs:comment "The bitrate of the audio in bits per second."@en ;
	rdfs:range xsd:integer ;
	.

observable:bitness
	a owl:DatatypeProperty ;
	rdfs:label "bitness"@en ;
	rdfs:comment "Specifies the bitness of the operating system (i.e. 32 or 64). Note that this is potentially different from the word size of the underlying hardware or CPU. A 32-bit operating system can be installed on a machine running a 64-bit processor."@en ;
	rdfs:range xsd:string ;
	.

observable:bitsPerPixel
	a owl:DatatypeProperty ;
	rdfs:label "bitsPerPixel"@en ;
	rdfs:range xsd:integer ;
	.

observable:blockType
	a owl:DatatypeProperty ;
	rdfs:label "blockType"@en ;
	rdfs:comment "The blockType property specifies the block type of a particular memory object."@en ;
	rdfs:range vocabulary:MemoryBlockTypeVocab ;
	.

observable:bluetoothDeviceName
	a owl:DatatypeProperty ;
	rdfs:label "bluetoothDeviceName"@en ;
	rdfs:comment "Name configured withing Bluetooth settings on a device."@en ;
	rdfs:range xsd:string ;
	.

observable:body
	a owl:DatatypeProperty ;
	rdfs:label "body"@en ;
	rdfs:range xsd:string ;
	.

observable:bodyMultipart
	a owl:ObjectProperty ;
	rdfs:label "bodyMultipart"@en ;
	rdfs:comment "A list of the MIME parts that make up the email body. This field MAY only be used if isMultipart is true."@en ;
	rdfs:range observable:MimePartType ;
	.

observable:bodyRaw
	a owl:ObjectProperty ;
	rdfs:label "bodyRaw"@en ;
	rdfs:range observable:ObservableObject ;
	.

observable:bookmarkPath
	a owl:DatatypeProperty ;
	rdfs:label "bookmarkPath"@en ;
	rdfs:comment "The folder containing the bookmark."@en ;
	rdfs:range xsd:string ;
	.

observable:browserInformation
	a owl:ObjectProperty ;
	rdfs:label "Browser Information"@en ;
	rdfs:comment "Specifies information about the particular Web Browser."@en ;
	rdfs:range observable:ObservableObject ;
	.

observable:browserUserProfile
	a owl:DatatypeProperty ;
	rdfs:label "Browser User Profile"@en ;
	rdfs:comment "Specifies the web browser user profile for which the URL history entry was created."@en ;
	rdfs:range xsd:string ;
	.

observable:byteOrder
	a owl:DatatypeProperty ;
	rdfs:label "byteOrder"@en ;
	rdfs:range vocabulary:EndiannessTypeVocab ;
	.

observable:byteStringValue
	a owl:DatatypeProperty ;
	rdfs:label "byteStringValue"@en ;
	rdfs:comment "Specifies the raw, byte-string representation of the extracted string."@en ;
	.

observable:callType
	a owl:DatatypeProperty ;
	rdfs:label "callType"@en ;
	rdfs:comment "The type of a phone call,for example incoming, outgoing, missed."@en ;
	rdfs:range xsd:string ;
	.

observable:camera
	a owl:ObjectProperty ;
	rdfs:label "camera"@en ;
	rdfs:comment "The name/make of the camera that was used for taking the picture."@en ;
	rdfs:range observable:ObservableObject ;
	.

observable:canEscalatePrivs
	a owl:DatatypeProperty ;
	rdfs:label "canEscalatePrivs"@en ;
	rdfs:range xsd:boolean ;
	.

observable:carrier
	a owl:ObjectProperty ;
	rdfs:label "carrier"@en ;
	rdfs:comment "Telecommunications service provider that sold the SIM card."@en ;
	rdfs:range identity:Identity ;
	.

observable:categories
	a owl:DatatypeProperty ;
	rdfs:label "categories"@en ;
	rdfs:comment "Categories applied to the object."@en ;
	rdfs:range xsd:string ;
	.

observable:cc
	a owl:ObjectProperty ;
	rdfs:label "cc"@en ;
	rdfs:range observable:ObservableObject ;
	.

observable:certificateIssuer
	a owl:ObjectProperty ;
	rdfs:label "certificateIssuer"@en ;
	rdfs:range identity:Identity ;
	.

observable:certificatePolicies
	a owl:DatatypeProperty ;
	rdfs:label "certificatePolicies"@en ;
	rdfs:range xsd:string ;
	.

observable:certificateSubject
	a owl:ObjectProperty ;
	rdfs:label "certificateSubject"@en ;
	rdfs:range <https://unifiedcyberontology.org/ontology/uco/core#UcoObject> ;
	.

observable:characteristics
	a owl:DatatypeProperty ;
	rdfs:label "characteristics"@en ;
	rdfs:comment "Specifies the flags that indicate the files characteristics."@en ;
	rdfs:range xsd:unsignedShort ;
	.

observable:checksum
	a owl:DatatypeProperty ;
	rdfs:label "checksum"@en ;
	rdfs:comment "Specifies the checksum of the PE binary."@en ;
	rdfs:range xsd:unsignedInt ;
	.

observable:clockSetting
	a owl:DatatypeProperty ;
	rdfs:label "clockSetting"@en ;
	rdfs:comment "The generalizedTime value on the mobile device when it was processed."@en ;
	rdfs:range xsd:string ;
	.

observable:clusterSize
	a owl:DatatypeProperty ;
	rdfs:label "clusterSize"@en ;
	rdfs:comment "The size of cluster allocation units in a file system."@en ;
	rdfs:range xsd:integer ;
	.

observable:columnName
	a owl:DatatypeProperty ;
	rdfs:label "columnName"@en ;
	rdfs:range xsd:string ;
	.

observable:comClassID
	a owl:DatatypeProperty ;
	rdfs:label "comClassID"@en ;
	rdfs:comment "Specifies the ID of the COM action. See also: http://msdn.microsoft.com/en-us/library/windows/desktop/aa380613(v=vs.85).aspx."@en ;
	rdfs:range xsd:string ;
	.

observable:comData
	a owl:DatatypeProperty ;
	rdfs:label "comData"@en ;
	rdfs:comment "Specifies the data associated with the COM handler. See also: http://msdn.microsoft.com/en-us/library/windows/desktop/aa380613(v=vs.85).aspx."@en ;
	rdfs:range xsd:string ;
	.

observable:comment
	a owl:DatatypeProperty ;
	rdfs:label "comment"@en ;
	rdfs:range xsd:string ;
	.

observable:compressionMethod
	a owl:DatatypeProperty ;
	rdfs:label "compressionMethod"@en ;
	rdfs:comment "The algorithm used to compress the data."@en ;
	rdfs:range xsd:string ;
	.

observable:compressionRatio
	a owl:DatatypeProperty ;
	rdfs:label "compressionRatio"@en ;
	rdfs:comment "The compression ratio of the compressed data."@en ;
	rdfs:range xsd:double ;
	.

observable:computerName
	a owl:DatatypeProperty ;
	rdfs:label "computerName"@en ;
	rdfs:comment "A name of the computer on which the log entry was created."@en ;
	rdfs:range xsd:string ;
	.

observable:contact
	a owl:ObjectProperty ;
	rdfs:label "contact"@en ;
	rdfs:comment "Contact specifies information characterizing contact details for a single entity."@en ;
	rdfs:range observable:ObservableObject ;
	.

observable:contactAddress
	a owl:ObjectProperty ;
	rdfs:label "contactAddress"@en ;
	rdfs:comment "Contact address specifies information characterizing a geolocation address of a contact entity."@en ;
	rdfs:range observable:ContactAddress ;
	.

observable:contactAddressScope
	a owl:DatatypeProperty ;
	rdfs:label "contactAddressScope"@en ;
	rdfs:comment "Contact address scope specifies the relevant scope (home, work, school, etc) for a geolocation address of a contact entity."@en ;
	rdfs:range [
		a rdfs:Datatype ;
		owl:unionOf (
			xsd:string
			vocabulary:ContactAddressScopeVocab
		) ;
	] ;
	.

observable:contactAffiliation
	a owl:ObjectProperty ;
	rdfs:label "contactAffiliation"@en ;
	rdfs:comment "Contact affiliation specifies information characterizing details of an organizational affiliation for a single contact entity."@en ;
	rdfs:range observable:ContactAffiliation ;
	.

observable:contactEmail
	a owl:ObjectProperty ;
	rdfs:label "contactEmail"@en ;
	rdfs:comment "Contact email specifies information characterizing details for contacting a contact entity by email."@en ;
	rdfs:range observable:ContactEmail ;
	.

observable:contactEmailScope
	a owl:DatatypeProperty ;
	rdfs:label "contactEmailScope"@en ;
	rdfs:comment "Contact email scope specifies the relevant scope (home, work, school, etc) of details for contacting a contact entity by email."@en ;
	rdfs:range [
		a rdfs:Datatype ;
		owl:unionOf (
			xsd:string
			vocabulary:ContactEmailScopeVocab
		) ;
	] ;
	.

observable:contactGroup
	a owl:DatatypeProperty ;
	rdfs:label "contactGroup"@en ;
	rdfs:comment "Contact group specifies the name/tag of a particular named/tagged grouping of contacts."@en ;
	rdfs:range xsd:string ;
	.

observable:contactID
	a owl:DatatypeProperty ;
	rdfs:label "contactID"@en ;
	rdfs:comment "Specifies an ID for the contact."@en ;
	rdfs:range xsd:string ;
	.

observable:contactMessaging
	a owl:ObjectProperty ;
	rdfs:label "contactMessaging"@en ;
	rdfs:comment "Contact messaging specifies information characterizing details for contacting a contact entity by digital messaging."@en ;
	rdfs:range observable:ContactMessaging ;
	.

observable:contactMessagingPlatform
	a owl:ObjectProperty ;
	rdfs:label "contactMessagingPlatform"@en ;
	rdfs:comment "A contact messaging platform specifies a digital messaging platform associated with a contact."@en ;
	rdfs:range observable:ObservableObject ;
	.

observable:contactNote
	a owl:DatatypeProperty ;
	rdfs:label "contactNote"@en ;
	rdfs:comment "Contact note specifies a comment/note associated with a given contact."@en ;
	rdfs:range xsd:string ;
	.

observable:contactOrganization
	a owl:ObjectProperty ;
	rdfs:label "contactOrganization"@en ;
	rdfs:comment "The name of the organization a contact works for or is assocciated with."@en ;
	rdfs:range identity:Organization ;
	.

observable:contactPhone
	a owl:ObjectProperty ;
	rdfs:label "contactPhone"@en ;
	rdfs:comment "Contact phone specifies information characterizing details for contacting a contact entity by telephone."@en ;
	rdfs:range observable:ContactPhone ;
	.

observable:contactPhoneNumber
	a owl:ObjectProperty ;
	rdfs:label "contactPhoneNumber"@en ;
	rdfs:comment "Contact phone number specifies a telephone service account number for contacting a contact entity by telephone."@en ;
	rdfs:range observable:ObservableObject ;
	.

observable:contactPhoneScope
	a owl:DatatypeProperty ;
	rdfs:label "contactPhoneScope"@en ;
	rdfs:comment "Contact phone scope specifies the relevant scope (home, work, school, etc) of details for contacting a contact entity by telephone."@en ;
	rdfs:range [
		a rdfs:Datatype ;
		owl:unionOf (
			xsd:string
			vocabulary:ContactPhoneScopeVocab
		) ;
	] ;
	.

observable:contactProfile
	a owl:ObjectProperty ;
	rdfs:label "contactProfile"@en ;
	rdfs:comment "Contact profile specifies information characterizing details for contacting a contact entity by online service."@en ;
	rdfs:range observable:ContactProfile ;
	.

observable:contactProfilePlatform
	a owl:ObjectProperty ;
	rdfs:label "contactProfilePlatform"@en ;
	rdfs:comment "A contact profile platform specifies an online service platform associated with a contact."@en ;
	rdfs:range observable:ObservableObject ;
	.

observable:contactSIP
	a owl:ObjectProperty ;
	rdfs:label "contactSIP"@en ;
	rdfs:comment "Contact SIP specifies information characterizing details for contacting a contact entity by Session Initiation Protocol (SIP)."@en ;
	rdfs:range observable:ContactSIP ;
	.

observable:contactSIPScope
	a owl:DatatypeProperty ;
	rdfs:label "contactSIPScope"@en ;
	rdfs:comment "Contact SIP scope specifies the relevant scope (home, work, school, etc) of details for contacting a contact entity by Session Initiation Protocol (SIP)."@en ;
	rdfs:range [
		a rdfs:Datatype ;
		owl:unionOf (
			xsd:string
			vocabulary:ContactSIPScopeVocab
		) ;
	] ;
	.

observable:contactURL
	a owl:ObjectProperty ;
	rdfs:label "contactURL"@en ;
	rdfs:comment "Contact URL specifies information characterizing details for contacting a contact entity by Uniform Resource Locator (URL)."@en ;
	rdfs:range observable:ContactURL ;
	.

observable:contactURLScope
	a owl:DatatypeProperty ;
	rdfs:label "contactURLScope"@en ;
	rdfs:comment "Contact url scope specifies the relevant scope (homepage, home, work, school, etc) of details for contacting a contact entity by Uniform Resource Locator (URL)."@en ;
	rdfs:range [
		a rdfs:Datatype ;
		owl:unionOf (
			xsd:string
			vocabulary:ContactURLScopeVocab
		) ;
	] ;
	.

observable:contentDisposition
	a owl:DatatypeProperty ;
	rdfs:label "contentDisposition"@en ;
	rdfs:range xsd:string ;
	.

observable:contentType
	a owl:DatatypeProperty ;
	rdfs:label "contentType"@en ;
	rdfs:range xsd:string ;
	.

observable:context
	a owl:DatatypeProperty ;
	rdfs:label "context"@en ;
	rdfs:range xsd:string ;
	.

observable:controlCode
	a owl:DatatypeProperty ;
	rdfs:label "controlCode"@en ;
	rdfs:comment "Specifies the actual control code that was sent to the observable object."@en ;
	rdfs:range xsd:string ;
	.

observable:cookieDomain
	a owl:ObjectProperty ;
	rdfs:label "cookieDomain"@en ;
	rdfs:comment "The domain for which the cookie is stored, for example nfi.minjus.nl."@en ;
	rdfs:range observable:ObservableObject ;
	.

observable:cookieName
	a owl:DatatypeProperty ;
	rdfs:label "cookieName"@en ;
	rdfs:comment "The name of the cookie."@en ;
	rdfs:range xsd:string ;
	.

observable:cookiePath
	a owl:DatatypeProperty ;
	rdfs:label "cookiePath"@en ;
	rdfs:comment "String representation of the path of the cookie."@en ;
	rdfs:range xsd:string ;
	.

observable:cpeid
	a owl:DatatypeProperty ;
	rdfs:label "cpeid"@en ;
	rdfs:comment "Specifies the Common Platform Enumeration identifier for the software."@en ;
	rdfs:range xsd:string ;
	.

observable:cpu
	a owl:DatatypeProperty ;
	rdfs:label "cpu"@en ;
	rdfs:comment "Specifies the name of the CPU used by the system."@en ;
	rdfs:range xsd:string ;
	.

observable:cpuFamily
	a owl:DatatypeProperty ;
	rdfs:label "cpuFamily"@en ;
	rdfs:comment "Specifies the name of the CPU family used by the system."@en ;
	rdfs:range xsd:string ;
	.

observable:creationDate
	a owl:DatatypeProperty ;
	rdfs:label "creationDate"@en ;
	rdfs:comment "Specifies the date in which the registered domain was created."@en ;
	rdfs:range xsd:dateTime ;
	.

observable:creationFlags
	a owl:DatatypeProperty ;
	rdfs:label "creationFlags"@en ;
	rdfs:range xsd:unsignedInt ;
	.

observable:creationTime
	a owl:DatatypeProperty ;
	rdfs:label "creationTime"@en ;
	rdfs:range xsd:dateTime ;
	.

observable:creator
	a owl:ObjectProperty ;
	rdfs:label "creator"@en ;
	rdfs:comment "Specifies the name of the creator of the registry key."@en ;
	rdfs:range observable:ObservableObject ;
	.

observable:creatorUser
	a owl:ObjectProperty ;
	rdfs:label "creatorUser"@en ;
	rdfs:comment "The user that created/owns the process."@en ;
	rdfs:range observable:ObservableObject ;
	.

observable:crlDistributionPoints
	a owl:DatatypeProperty ;
	rdfs:label "crlDistributionPoints"@en ;
	rdfs:range xsd:string ;
	.

observable:currentSystemDate
	a owl:DatatypeProperty ;
	rdfs:label "currentSystemDate"@en ;
	rdfs:comment "Specifies the current date on the system."@en ;
	rdfs:range xsd:dateTime ;
	.

observable:currentWorkingDirectory
	a owl:DatatypeProperty ;
	rdfs:label "currentWorkingDirectory"@en ;
	rdfs:range xsd:string ;
	.

observable:cyberAction
	a owl:ObjectProperty ;
	rdfs:label "cyberAction"@en ;
	rdfs:comment "The action taken in response to the event."@en ;
	rdfs:range observable:ObservableAction ;
	.

observable:data
	a owl:DatatypeProperty ;
	rdfs:label "data"@en ;
	rdfs:range xsd:string ;
	.

observable:dataPayload
	a owl:DatatypeProperty ;
	rdfs:label "dataPayload"@en ;
	rdfs:range xsd:string ;
	.

observable:dataPayloadReferenceURL
	a owl:ObjectProperty ;
	rdfs:label "dataPayloadReferenceURL"@en ;
	rdfs:range observable:ObservableObject ;
	.

observable:dataType
	a owl:DatatypeProperty ;
	rdfs:label "dataType"@en ;
	rdfs:range xsd:string ;
	.

observable:depEnabled
	a owl:DatatypeProperty ;
	rdfs:label "depEnabled"@en ;
	rdfs:range xsd:boolean ;
	.

observable:descriptions
	a owl:DatatypeProperty ;
	rdfs:label "descriptions"@en ;
	rdfs:range xsd:string ;
	.

observable:destination
	a owl:DatatypeProperty ;
	rdfs:label "destination"@en ;
	rdfs:comment "The destination of a global flag. See also: http://msdn.microsoft.com/en-us/library/windows/hardware/ff549646(v=vs.85).aspx."@en ;
	rdfs:range xsd:string ;
	.

observable:destinationFlags
	a owl:DatatypeProperty ;
	rdfs:label "destinationFlags"@en ;
	rdfs:comment """Specifies the destination TCP flags.
          """@en ;
	.

observable:destinationPort
	a owl:DatatypeProperty ;
	rdfs:label "destinationPort"@en ;
	rdfs:comment "Specifies the destination port used in the connection, as an integer in the range of 0 - 65535."@en ;
	rdfs:range xsd:integer ;
	.

observable:deviceType
	a owl:DatatypeProperty ;
	rdfs:label "deviceType"@en ;
	rdfs:range xsd:string ;
	.

observable:dhcpLeaseExpires
	a owl:DatatypeProperty ;
	rdfs:label "dhcpLeaseExpires"@en ;
	rdfs:comment "Specifies the date/time that the DHCP lease obtained on the network interface expires."@en ;
	rdfs:range xsd:dateTime ;
	.

observable:dhcpLeaseObtained
	a owl:DatatypeProperty ;
	rdfs:label "dhcpLeaseObtained"@en ;
	rdfs:comment "Specifies the date/time that the DHCP lease was obtained on the network interface."@en ;
	rdfs:range xsd:dateTime ;
	.

observable:dhcpServer
	a owl:ObjectProperty ;
	rdfs:label "dhcpServer"@en ;
	rdfs:comment "Specifies the list of DHCP server IP Addresses used by the network interface."@en ;
	rdfs:range observable:ObservableObject ;
	.

observable:diskPartitionType
	a owl:DatatypeProperty ;
	rdfs:label "diskPartitionType"@en ;
	rdfs:comment "Specifies the type of partition being characterized."@en ;
	rdfs:range xsd:string ;
	.

observable:diskSize
	a owl:DatatypeProperty ;
	rdfs:label "diskSize"@en ;
	rdfs:comment "The size of the disk, in bytes."@en ;
	rdfs:range xsd:integer ;
	.

observable:diskType
	a owl:DatatypeProperty ;
	rdfs:label "diskType"@en ;
	rdfs:comment "The type of disk being characterized, e.g., removable."@en ;
	rdfs:range xsd:string ;
	.

observable:displayName
	a owl:DatatypeProperty ;
	rdfs:label "displayName"@en ;
	rdfs:comment "Display name specifies the name to display for some entity within a user interface."@en ;
	rdfs:range xsd:string ;
	.

observable:dllCharacteristics
	a owl:DatatypeProperty ;
	rdfs:label "dllCharacteristics"@en ;
	rdfs:comment "Specifies the flags that characterize the PE binary."@en ;
	rdfs:range xsd:unsignedShort ;
	.

observable:dnssec
	a owl:DatatypeProperty ;
	rdfs:label "dnssec"@en ;
	rdfs:comment "Specifies the DNSSEC property associated with a Whois entry. Acceptable values are: 'Signed' or 'Unsigned'."@en ;
	rdfs:range vocabulary:WhoisDNSSECTypeVocab ;
	.

observable:documentInformationDictionary
	a owl:ObjectProperty ;
	rdfs:label "documentInformationDictionary"@en ;
	rdfs:range <https://unifiedcyberontology.org/ontology/uco/types#ControlledDictionary> ;
	.

observable:domain
	a owl:DatatypeProperty ;
	rdfs:label "domain"@en ;
	rdfs:comment "The domain(s) that the system belongs to."@en ;
	rdfs:range xsd:string ;
	.

observable:domainID
	a owl:DatatypeProperty ;
	rdfs:label "domainID"@en ;
	rdfs:comment "Specifies the domain id for the domain associated with a Whois entry."@en ;
	rdfs:range xsd:string ;
	.

observable:domainName
	a owl:ObjectProperty ;
	rdfs:label "domainName"@en ;
	rdfs:comment "Specifies the corresponding domain name for a whois entry."@en ;
	rdfs:range observable:ObservableObject ;
	.

observable:driveLetter
	a owl:DatatypeProperty ;
	rdfs:label "driveLetter"@en ;
	rdfs:comment "Specifies the drive letter of a windows volume."@en ;
	rdfs:range xsd:string ;
	.

observable:driveType
	a owl:DatatypeProperty ;
	rdfs:label "driveType"@en ;
	rdfs:comment "Specifies the drive type of a windows volume."@en ;
	rdfs:range vocabulary:WindowsDriveTypeVocab ;
	.

observable:dst
	a owl:ObjectProperty ;
	rdfs:label "dst"@en ;
	rdfs:comment "Specifies the destination(s) of the network connection."@en ;
	rdfs:range observable:ObservableObject ;
	.

observable:dstBytes
	a owl:DatatypeProperty ;
	rdfs:label "dstBytes"@en ;
	rdfs:range xsd:integer ;
	.

observable:dstPackets
	a owl:DatatypeProperty ;
	rdfs:label "dstPackets"@en ;
	rdfs:range xsd:integer ;
	.

observable:dstPayload
	a owl:ObjectProperty ;
	rdfs:label "dstPayload"@en ;
	rdfs:range observable:ObservableObject ;
	.

observable:duration
	a owl:DatatypeProperty ;
	rdfs:label "duration"@en ;
	rdfs:comment "The duration of the phone call in seconds."@en ;
	rdfs:range xsd:integer ;
	.

observable:effectiveGroup
	a owl:DatatypeProperty ;
	rdfs:label "effectiveGroup"@en ;
	rdfs:comment "Specifies the name of the effective group used in the user session."@en ;
	rdfs:range xsd:string ;
	.

observable:effectiveGroupID
	a owl:DatatypeProperty ;
	rdfs:label "effectiveGroupID"@en ;
	rdfs:comment "Specifies the effective group ID of the group used in the user session."@en ;
	rdfs:range xsd:string ;
	.

observable:effectiveUser
	a owl:ObjectProperty ;
	rdfs:label "effectiveUser"@en ;
	rdfs:comment "Specifies the effective user details used in the user session."@en ;
	rdfs:range observable:ObservableObject ;
	.

observable:emailAddress
	a owl:ObjectProperty ;
	rdfs:label "emailAddress"@en ;
	rdfs:comment "An email address."@en ;
	rdfs:range observable:ObservableObject ;
	.

observable:encoding
	a owl:DatatypeProperty ;
	rdfs:label "Encoding"@en ;
	rdfs:comment "The encoding method used for the extracted string."@en ;
	rdfs:range xsd:string ;
	.

observable:encodingMethod
	a owl:DatatypeProperty ;
	rdfs:label "encodingMethod"@en ;
	rdfs:range xsd:string ;
	.

observable:encryptionIV
	a owl:DatatypeProperty ;
	rdfs:label "encryptionIV"@en ;
	rdfs:range xsd:string ;
	.

observable:encryptionKey
	a owl:DatatypeProperty ;
	rdfs:label "encryptionKey"@en ;
	rdfs:range xsd:string ;
	.

observable:encryptionMethod
	a owl:DatatypeProperty ;
	rdfs:label "encryptionMethod"@en ;
	rdfs:range xsd:string ;
	.

observable:encryptionMode
	a owl:DatatypeProperty ;
	rdfs:label "encryptionMode"@en ;
	rdfs:range xsd:string ;
	.

observable:endTime
	a owl:DatatypeProperty ;
	rdfs:label "endTime"@en ;
	rdfs:range xsd:dateTime ;
	.

observable:englishTranslation
	a owl:DatatypeProperty ;
	rdfs:label "englishTranslation"@en ;
	rdfs:comment "Specifies the English translation of the string, if it is not written in English."@en ;
	rdfs:range xsd:string ;
	.

observable:entropy
	a owl:DatatypeProperty ;
	rdfs:label "entropy"@en ;
	rdfs:comment "Shannon entropy (a measure of randomness) of the data."@en ;
	rdfs:range xsd:double ;
	.

observable:entryID
	a owl:DatatypeProperty ;
	rdfs:label "entryID"@en ;
	rdfs:comment "A unique identifier for the file within the filesystem."@en ;
	rdfs:range xsd:integer ;
	.

observable:environmentVariables
	a owl:ObjectProperty ;
	rdfs:label "environmentVariables"@en ;
	rdfs:comment "A list of environment variables associated with the process. "@en ;
	rdfs:range <https://unifiedcyberontology.org/ontology/uco/types#Dictionary> ;
	.

observable:eventID
	a owl:DatatypeProperty ;
	rdfs:label "eventID"@en ;
	rdfs:comment "The identifier of the event."@en ;
	rdfs:range xsd:string ;
	.

observable:eventStatus
	a owl:DatatypeProperty ;
	rdfs:label "eventStatus"@en ;
	rdfs:comment "The status of the event, for instance accepted, pending or cancelled."@en ;
	rdfs:range xsd:string ;
	.

observable:eventText
	a owl:DatatypeProperty ;
	rdfs:label "eventText"@en ;
	rdfs:comment "The textual representation of the event."@en ;
	rdfs:range xsd:string ;
	.

observable:eventType
	a owl:DatatypeProperty ;
	rdfs:label "eventType"@en ;
	rdfs:comment "The type of the event, for example 'information', 'warning' or 'error'."@en ;
	rdfs:range xsd:string ;
	.

observable:execArguments
	a owl:DatatypeProperty ;
	rdfs:label "execArguments"@en ;
	rdfs:comment "Specifies the arguments associated with the command-line operation launched by the action. See also: http://msdn.microsoft.com/en-us/library/windows/desktop/aa380715(v=vs.85).aspx."@en ;
	rdfs:range xsd:string ;
	.

observable:execProgramHashes
	a owl:ObjectProperty ;
	rdfs:label "execProgramHashes"@en ;
	rdfs:comment "Specifies the hashes of the executable file launched by the action."@en ;
	rdfs:range <https://unifiedcyberontology.org/ontology/uco/types#Hash> ;
	.

observable:execProgramPath
	a owl:DatatypeProperty ;
	rdfs:label "execProgramPath"@en ;
	rdfs:comment "Specifies the path to the executable file launched by the action. See also: http://msdn.microsoft.com/en-us/library/windows/desktop/aa380715(v=vs.85).aspx."@en ;
	rdfs:range xsd:string ;
	.

observable:execWorkingDirectory
	a owl:DatatypeProperty ;
	rdfs:label "execWorkingDirectory"@en ;
	rdfs:comment "Specifies the directory that contains either the executable file or the files that are used by the executable file launched by the action. See also: http://msdn.microsoft.com/en-us/library/windows/desktop/aa380715(v=vs.85).aspx."@en ;
	rdfs:range xsd:string ;
	.

observable:exifData
	a owl:ObjectProperty ;
	rdfs:label "exifData"@en ;
	rdfs:range <https://unifiedcyberontology.org/ontology/uco/types#ControlledDictionary> ;
	.

observable:exitCode
	a owl:DatatypeProperty ;
	rdfs:label "exitCode"@en ;
	rdfs:comment "Specifies the last exit code of the scheduled task. See also: http://msdn.microsoft.com/en-us/library/windows/desktop/aa381245(v=vs.85).aspx."@en ;
	rdfs:range xsd:integer ;
	.

observable:exitStatus
	a owl:DatatypeProperty ;
	rdfs:label "exitStatus"@en ;
	rdfs:comment "A small number passed from the process to the parent process when it has finished executing. In general, 0 indicates successful termination, any other number indicates a failure."@en ;
	rdfs:range xsd:integer ;
	.

observable:exitTime
	a owl:DatatypeProperty ;
	rdfs:label "exitTime"@en ;
	rdfs:comment "The time at which the process exited."@en ;
	rdfs:range xsd:dateTime ;
	.

observable:expirationDate
	a owl:DatatypeProperty ;
	rdfs:label "expirationDate"@en ;
	rdfs:comment "Specifies the date in which the registered domain will expire."@en ;
	rdfs:range xsd:dateTime ;
	.

observable:expirationTime
	a owl:DatatypeProperty ;
	rdfs:label "expirationTime"@en ;
	rdfs:comment "The date and time at which the validity of the object expires."@en ;
	rdfs:range xsd:dateTime ;
	.

observable:extDeletionTime
	a owl:DatatypeProperty ;
	rdfs:label "extDeletionTime"@en ;
	rdfs:comment "Specifies the time at which the file represented by an Inode was 'deleted'."@en ;
	rdfs:range xsd:dateTime ;
	.

observable:extFileType
	a owl:DatatypeProperty ;
	rdfs:label "extFileType"@en ;
	rdfs:comment "Specifies the EXT file type (FIFO, Directory, Regular file, Symbolic link, etc) for the Inode."@en ;
	rdfs:range xsd:integer ;
	.

observable:extFlags
	a owl:DatatypeProperty ;
	rdfs:label "extFlags"@en ;
	rdfs:comment "Specifies user flags to further protect (limit its use and modification) the file represented by an Inode."@en ;
	rdfs:range xsd:integer ;
	.

observable:extHardLinkCount
	a owl:DatatypeProperty ;
	rdfs:label "extHardLinkCount"@en ;
	rdfs:comment "Specifies a count of how many hard links point to an Inode."@en ;
	rdfs:range xsd:integer ;
	.

observable:extInodeChangeTime
	a owl:DatatypeProperty ;
	rdfs:label "extInodeChangeTime"@en ;
	rdfs:comment "The date and time at which the file Inode metadata was last modified."@en ;
	rdfs:range xsd:dateTime ;
	.

observable:extInodeID
	a owl:DatatypeProperty ;
	rdfs:label "extInodeID"@en ;
	rdfs:comment "Specifies a single Inode identifier."@en ;
	rdfs:range xsd:integer ;
	.

observable:extPermissions
	a owl:DatatypeProperty ;
	rdfs:label "extPermissions"@en ;
	rdfs:comment "Specifies the read/write/execute permissions for the file represented by an EXT Inode."@en ;
	rdfs:range xsd:integer ;
	.

observable:extSGID
	a owl:DatatypeProperty ;
	rdfs:label "extSGID"@en ;
	rdfs:comment "Specifies the group ID for the file represented by an Inode."@en ;
	rdfs:range xsd:integer ;
	.

observable:extSUID
	a owl:DatatypeProperty ;
	rdfs:label "extSUID"@en ;
	rdfs:comment "Specifies the user ID that 'owns' the file represented by an Inode."@en ;
	rdfs:range xsd:integer ;
	.

observable:extendedKeyUsage
	a owl:DatatypeProperty ;
	rdfs:label "extendedKeyUsage"@en ;
	rdfs:range xsd:string ;
	.

observable:extension
	a owl:DatatypeProperty ;
	rdfs:label "extension"@en ;
	rdfs:comment "The file name extension: everything after the last dot. Not present if the file has no dot in its name."@en ;
	rdfs:range xsd:string ;
	.

observable:favoritesCount
	a owl:DatatypeProperty ;
	rdfs:label "Favorites Count"@en-US ;
	rdfs:comment "Specifies the number of times that this profile has favorited a tweet."@en-US ;
	rdfs:range xsd:nonNegativeInteger ;
	.

observable:faxNumber
	a owl:ObjectProperty ;
	rdfs:label "faxNumber"@en ;
	rdfs:comment "A phone number(account) of a fax."@en ;
	rdfs:range observable:ObservableObject ;
	.

observable:fileAlignment
	a owl:DatatypeProperty ;
	rdfs:label "fileAlignment"@en ;
	rdfs:comment "Specifies the factor (in bytes) that is used to align the raw data of sections in the image file."@en ;
	rdfs:range xsd:unsignedInt ;
	.

observable:fileHeaderHashes
	a owl:ObjectProperty ;
	rdfs:label "fileHeaderHashes"@en ;
	rdfs:comment "Specifies any hashes that were computed for the file header."@en ;
	rdfs:range <https://unifiedcyberontology.org/ontology/uco/types#Hash> ;
	.

observable:fileName
	a owl:DatatypeProperty ;
	rdfs:label "fileName"@en ;
	rdfs:comment "Specifies the name associated with a file in a file system."@en ;
	rdfs:range xsd:string ;
	.

observable:filePath
	a owl:DatatypeProperty ;
	rdfs:label "filePath"@en ;
	rdfs:comment "Specifies the file path for the location of a file within a filesystem."@en ;
	rdfs:range xsd:string ;
	.

observable:fileSystemType
	a owl:DatatypeProperty ;
	rdfs:label "fileSystemType"@en ;
	rdfs:comment "The specific type of a file system."@en ;
	rdfs:range xsd:string ;
	.

observable:firstLoginTime
	a owl:DatatypeProperty ;
	rdfs:label "firstLoginTime"@en ;
	rdfs:comment "The date and time of the first login of the account."@en ;
	rdfs:range xsd:dateTime ;
	.

observable:firstName
	a owl:DatatypeProperty ;
	rdfs:label "firstName"@en ;
	rdfs:comment "The first name of a person."@en ;
	rdfs:range xsd:string ;
	.

observable:firstRun
	a owl:DatatypeProperty ;
	rdfs:label "firstRun"@en ;
	rdfs:comment "Timestamp of when the prefetch application was first run."@en ;
	rdfs:range xsd:dateTime ;
	.

observable:firstVisit
	a owl:DatatypeProperty ;
	rdfs:label "First Visit Time"@en ;
	rdfs:comment "Specifies the date/time that the URL referred to by the URL field was first visited."@en-US ;
	rdfs:range xsd:dateTime ;
	.

observable:flags
	a owl:DatatypeProperty ;
	rdfs:label "flags"@en ;
	rdfs:comment "Specifies any flags that modify the behavior of the scheduled task. See also: http://msdn.microsoft.com/en-us/library/windows/desktop/aa381248(v=vs.85).aspx."@en ;
	rdfs:range vocabulary:TaskFlagVocab ;
	.

observable:followersCount
	a owl:DatatypeProperty ;
	rdfs:label "Followers Count"@en-US ;
	rdfs:comment "Specifies the followers count associated with the twitter profile."@en-US ;
	rdfs:range xsd:nonNegativeInteger ;
	.

observable:format
	a owl:DatatypeProperty ;
	rdfs:label "format"@en ;
	rdfs:comment "The format of the audio. For example: mp3 or flac."@en ;
	rdfs:range xsd:string ;
	.

observable:fragment
	a owl:DatatypeProperty ;
	rdfs:label "fragment"@en ;
	rdfs:comment "Fragment pointing to a specific part in the resource."@en ;
	rdfs:range xsd:string ;
	.

observable:fragmentIndex
	a owl:DatatypeProperty ;
	rdfs:label "fragmentIndex"@en ;
	rdfs:range xsd:integer ;
	.

observable:freeSpace
	a owl:DatatypeProperty ;
	rdfs:label "freeSpace"@en ;
	rdfs:comment "The amount of free space on the disk, in bytes."@en ;
	rdfs:range xsd:integer ;
	.

observable:friendsCount
	a owl:DatatypeProperty ;
	rdfs:label "Friends Count"@en-US ;
	rdfs:comment "Specifies the friends count associated with the twitter profile."@en-US ;
	rdfs:range xsd:nonNegativeInteger ;
	.

observable:from
	a owl:ObjectProperty ;
	rdfs:label "from"@en ;
	rdfs:comment "The phone number of the initiating party."@en ;
	rdfs:range observable:ObservableObject ;
	.

observable:fromURLVisit
	a owl:ObjectProperty ;
	rdfs:label "From URL Visit"@en ;
	rdfs:comment "Specifies the URL visit origination point (i.e., URL) of the URL captured in the URL history entry, if applicable."@en ;
	rdfs:range observable:ObservableObject ;
	.

observable:fullValue
	a owl:DatatypeProperty ;
	rdfs:label "fullValue"@en ;
	rdfs:comment "The full string value of the URL."@en ;
	rdfs:range xsd:string ;
	.

observable:geoLocationEntry
	a owl:ObjectProperty ;
	rdfs:label "geoLocationEntry"@en ;
	rdfs:range observable:ObservableObject ;
	.

observable:geolocationAddress
	a owl:ObjectProperty ;
	rdfs:label "geolocationAddress"@en ;
	rdfs:comment "An administrative address for a particular geolocation."@en ;
	rdfs:range <https://unifiedcyberontology.org/ontology/uco/location#Location> ;
	.

observable:gid
	a owl:DatatypeProperty ;
	rdfs:label "gid"@en ;
	rdfs:range xsd:integer ;
	.

observable:globalFlagList
	a owl:ObjectProperty ;
	rdfs:label "globalFlagList"@en ;
	rdfs:comment "A list of global flags. See also: http://msdn.microsoft.com/en-us/library/windows/hardware/ff549557(v=vs.85).aspx."@en ;
	rdfs:range observable:GlobalFlagType ;
	.

observable:gpu
	a owl:DatatypeProperty ;
	rdfs:label "gpu"@en ;
	rdfs:comment "Specifies the name of the GPU used by the system."@en ;
	rdfs:range xsd:string ;
	.

observable:gpuFamily
	a owl:DatatypeProperty ;
	rdfs:label "gpuFamily"@en ;
	rdfs:comment "Specifies the name of the GPU family used by the system."@en ;
	rdfs:range xsd:string ;
	.

observable:groupName
	a owl:DatatypeProperty ;
	rdfs:label "groupName"@en ;
	rdfs:range xsd:string ;
	.

observable:groups
	a owl:DatatypeProperty ;
	rdfs:label "groups"@en ;
	rdfs:range xsd:string ;
	.

observable:hasChanged
	a owl:DatatypeProperty ;
	rdfs:label "hasChanged"@en ;
	rdfs:range xsd:boolean ;
	.

observable:hash
	a owl:ObjectProperty ;
	rdfs:label "hash"@en ;
	rdfs:comment "Hash values of the data."@en ;
	rdfs:range <https://unifiedcyberontology.org/ontology/uco/types#Hash> ;
	.

observable:hashes
	a owl:ObjectProperty ;
	rdfs:label "hashes"@en ;
	rdfs:comment "Specifies any hashes computed over the section."@en ;
	rdfs:range <https://unifiedcyberontology.org/ontology/uco/types#Hash> ;
	.

observable:headerRaw
	a owl:ObjectProperty ;
	rdfs:label "headerRaw"@en ;
	rdfs:range observable:ObservableObject ;
	.

observable:hexadecimalValue
	a owl:DatatypeProperty ;
	rdfs:label "hexadecimalValue"@en ;
	rdfs:comment "The hexadecimal value of a global flag. See also: http://msdn.microsoft.com/en-us/library/windows/hardware/ff549646(v=vs.85).aspx."@en ;
	rdfs:range xsd:hexBinary ;
	.

observable:hiveType
	a owl:DatatypeProperty ;
	rdfs:label "hiveType"@en ;
	rdfs:comment "The type of a registry hive."@en ;
	rdfs:range xsd:string ;
	.

observable:homeDirectory
	a owl:DatatypeProperty ;
	rdfs:label "homeDirectory"@en ;
	rdfs:range xsd:string ;
	.

observable:host
	a owl:ObjectProperty ;
	rdfs:label "host"@en ;
	rdfs:comment "Domain name or IP address where the resource is located."@en ;
	rdfs:range observable:ObservableObject ;
	.

observable:hostname
	a owl:DatatypeProperty ;
	rdfs:label "hostname"@en ;
	rdfs:comment "Specifies the hostname of the system."@en ;
	rdfs:range xsd:string ;
	.

observable:httpMesageBodyLength
	a owl:DatatypeProperty ;
	rdfs:label "httpMesageBodyLength"@en ;
	rdfs:comment "Specifies the length of an HTTP message body in bytes."@en ;
	rdfs:range xsd:integer ;
	.

observable:httpMessageBodyData
	a owl:ObjectProperty ;
	rdfs:label "httpMessageBodyData"@en ;
	rdfs:comment "Specifies the data contained in an HTTP message body."@en ;
	rdfs:range observable:ObservableObject ;
	.

observable:httpRequestHeader
	a owl:ObjectProperty ;
	rdfs:label "httpRequestHeader"@en ;
	rdfs:comment "Specifies all of the HTTP header fields that may be found in the HTTP client request"@en ;
	rdfs:range <https://unifiedcyberontology.org/ontology/uco/types#Dictionary> ;
	.

observable:iComHandlerAction
	a owl:ObjectProperty ;
	rdfs:label "iComHandlerAction"@en ;
	rdfs:comment "Specifies the data associated with the task action-fired COM handler."@en ;
	rdfs:range observable:IComHandlerActionType ;
	.

observable:iEmailAction
	a owl:ObjectProperty ;
	rdfs:label "iEmailAction"@en ;
	rdfs:comment "Specifies an action that sends an e-mail, which in this context refers to actual email message sent. See also: http://msdn.microsoft.com/en-us/library/windows/desktop/aa380693(v=vs.85).aspx."@en ;
	rdfs:range observable:ObservableObject ;
	.

observable:iExecAction
	a owl:ObjectProperty ;
	rdfs:label "iExecAction"@en ;
	rdfs:comment "Specifies an action that executes a command-line operation. See also: http://msdn.microsoft.com/en-us/library/windows/desktop/aa380715(v=vs.85).aspx."@en ;
	rdfs:range observable:IExecActionType ;
	.

observable:iShowMessageAction
	a owl:ObjectProperty ;
	rdfs:label "iShowMessageAction"@en ;
	rdfs:comment "Specifies an action that shows a message box when a task is activated. See also: http://msdn.microsoft.com/en-us/library/windows/desktop/aa381302(v=vs.85).aspx."@en ;
	rdfs:range observable:IShowMessageActionType ;
	.

observable:icmpCode
	a owl:DatatypeProperty ;
	rdfs:label "icmpCode"@en ;
	rdfs:comment "Specifies the ICMP code byte."@en ;
	rdfs:range xsd:hexBinary ;
	.

observable:icmpType
	a owl:DatatypeProperty ;
	rdfs:label "icmpType"@en ;
	rdfs:comment "Specifies the ICMP type byte."@en ;
	rdfs:range xsd:hexBinary ;
	.

observable:imageBase
	a owl:DatatypeProperty ;
	rdfs:label "imageBase"@en ;
	rdfs:comment "Specifies the address that is relative to the image base of the beginning-of-data section when it is loaded into memory."@en ;
	rdfs:range xsd:unsignedInt ;
	.

observable:imageCompressionMethod
	a owl:DatatypeProperty ;
	rdfs:label "imageCompressionMethod"@en ;
	rdfs:range xsd:string ;
	.

observable:imageName
	a owl:DatatypeProperty ;
	rdfs:label "imageName"@en ;
	rdfs:comment "Specifies the image name for the task."@en ;
	rdfs:range xsd:string ;
	.

observable:imageType
	a owl:DatatypeProperty ;
	rdfs:label "imageType"@en ;
	rdfs:comment "The type of the image, e.g. EnCase, RAW or LocalFolder."@en ;
	rdfs:range xsd:string ;
	.

observable:impHash
	a owl:DatatypeProperty ;
	rdfs:label "impHash"@en ;
	rdfs:comment "Specifies the special import hash, or imphash, calculated for the PE Binary based on its imported libraries and functions. "@en ;
	rdfs:range xsd:string ;
	.

observable:inReplyTo
	a owl:ObjectProperty ;
	rdfs:label "inReplyTo"@en ;
	rdfs:comment "One of more unique identifiers for identifying the email(s) this email is a reply to."@en ;
	rdfs:range observable:ObservableObject ;
	.

observable:inetLocation
	a owl:ObjectProperty ;
	rdfs:label "Internet Location"@en-US ;
	rdfs:comment "Specifies a location on the Internet."@en-US ;
	rdfs:range observable:ObservableObject ;
	.

observable:inhibitAnyPolicy
	a owl:DatatypeProperty ;
	rdfs:label "inhibitAnyPolicy"@en ;
	rdfs:range xsd:string ;
	.

observable:installDate
	a owl:DatatypeProperty ;
	rdfs:label "installDate"@en ;
	rdfs:comment "Specifies the date the operating system was installed."@en ;
	rdfs:range xsd:dateTime ;
	.

observable:ip
	a owl:ObjectProperty ;
	rdfs:label "ip"@en ;
	rdfs:comment "Specifies the list of IP addresses used by the network interface."@en ;
	rdfs:range observable:ObservableObject ;
	.

observable:ipAddress
	a owl:ObjectProperty ;
	rdfs:label "ipAddress"@en ;
	rdfs:comment "Specifies the corresponding ip address for a whois entry. Usually corresponds to a nameserver lookup."@en ;
	rdfs:range observable:ObservableObject ;
	.

observable:ipGateway
	a owl:ObjectProperty ;
	rdfs:label "ipGateway"@en ;
	rdfs:comment "Specifies the list of IP Gateway IP Addresses used by the network interface."@en ;
	rdfs:range observable:ObservableObject ;
	.

observable:ipfix
	a owl:ObjectProperty ;
	rdfs:label "ipfix"@en ;
	rdfs:comment "Specifies any IP Flow Information Export (IPFIX) data for the network traffic flow."@en ;
	rdfs:range <https://unifiedcyberontology.org/ontology/uco/types#Dictionary> ;
	.

observable:isActive
	a owl:DatatypeProperty ;
	rdfs:label "isActive"@en ;
	rdfs:comment "Indicates whether the network connection is still active."@en ;
	rdfs:range xsd:boolean ;
	.

observable:isDirectory
	a owl:DatatypeProperty ;
	rdfs:label "isDirectory"@en ;
	rdfs:comment "Specifies whether a file entry represents a directory."@en ;
	rdfs:range xsd:boolean ;
	.

observable:isDisabled
	a owl:DatatypeProperty ;
	rdfs:label "isDisabled"@en ;
	rdfs:comment "Is the digital account disabled?"@en ;
	rdfs:range xsd:boolean ;
	.

observable:isEnabled
	a owl:DatatypeProperty ;
	rdfs:label "isEnabled"@en ;
	rdfs:comment "Specifies whether the trigger is enabled."@en ;
	rdfs:range xsd:boolean ;
	.

observable:isEncrypted
	a owl:DatatypeProperty ;
	rdfs:label "isEncrypted"@en ;
	rdfs:range xsd:boolean ;
	.

observable:isHidden
	a owl:DatatypeProperty ;
	rdfs:label "isHidden"@en ;
	rdfs:comment """The isHidden property specifies whether the process is hidden or not.
          """@en ;
	rdfs:range xsd:boolean ;
	.

observable:isInjected
	a owl:DatatypeProperty ;
	rdfs:label "isInjected"@en ;
	rdfs:comment "The isInjected property specifies whether or not the particular memory object has had data/code injected into it by another process."@en ;
	rdfs:range xsd:boolean ;
	.

observable:isMapped
	a owl:DatatypeProperty ;
	rdfs:label "isMapped"@en ;
	rdfs:comment "The isMapped property specifies whether or not the particular memory object has been assigned a byte-for-byte correlation with some portion of a file or file-like resource."@en ;
	rdfs:range xsd:boolean ;
	.

observable:isMimeEncoded
	a owl:DatatypeProperty ;
	rdfs:label "isMimeEncoded"@en ;
	rdfs:range xsd:boolean ;
	.

observable:isMultipart
	a owl:DatatypeProperty ;
	rdfs:label "isMultipart"@en ;
	rdfs:range xsd:boolean ;
	.

observable:isNamed
	a owl:DatatypeProperty ;
	rdfs:label "isNamed"@en ;
	rdfs:range xsd:boolean ;
	.

observable:isOptimized
	a owl:DatatypeProperty ;
	rdfs:label "isOptimized"@en ;
	rdfs:range xsd:boolean ;
	.

observable:isPrivate
	a owl:DatatypeProperty ;
	rdfs:label "isPrivate"@en ;
	rdfs:comment "Is the event marked as private?"@en ;
	rdfs:range xsd:boolean ;
	.

observable:isPrivileged
	a owl:DatatypeProperty ;
	rdfs:label "isPrivileged"@en ;
	rdfs:range xsd:boolean ;
	.

observable:isProtected
	a owl:DatatypeProperty ;
	rdfs:label "isProtected"@en ;
	rdfs:comment "The isProtected property specifies whether or not the particular memory object is protected (read/write only from the process that allocated it)."@en ;
	rdfs:range xsd:boolean ;
	.

observable:isRead
	a owl:DatatypeProperty ;
	rdfs:label "isRead"@en ;
	rdfs:range xsd:boolean ;
	.

observable:isSecure
	a owl:DatatypeProperty ;
	rdfs:label "isSecure"@en ;
	rdfs:comment "Is the cookie secure? If the cookie is secure it cannot be delivered over an unencrypted session such as http."@en ;
	rdfs:range xsd:boolean ;
	.

observable:isSelfSigned
	a owl:DatatypeProperty ;
	rdfs:label "isSelfSigned"@en ;
	rdfs:range xsd:boolean ;
	.

observable:isServiceAccount
	a owl:DatatypeProperty ;
	rdfs:label "isServiceAccount"@en ;
	rdfs:range xsd:boolean ;
	.

observable:isTLD
	a owl:DatatypeProperty ;
	rdfs:label "isTLD"@en ;
	rdfs:range xsd:boolean ;
	.

observable:isVolatile
	a owl:DatatypeProperty ;
	rdfs:label "isVolatile"@en ;
	rdfs:comment "The isVolatile property specifies whether or not the particular memory object is volatile."@en ;
	rdfs:range xsd:boolean ;
	.

observable:issuer
	a owl:DatatypeProperty ;
	rdfs:label "issuer"@en ;
	rdfs:range xsd:string ;
	.

observable:issuerAlternativeName
	a owl:DatatypeProperty ;
	rdfs:label "issuerAlternativeName"@en ;
	rdfs:range xsd:string ;
	.

observable:issuerHash
	a owl:ObjectProperty ;
	rdfs:label "issuerHash"@en ;
	rdfs:comment "A hash calculated on the certificate issuer name."@en ;
	rdfs:range <https://unifiedcyberontology.org/ontology/uco/types#Hash> ;
	.

observable:key
	a owl:DatatypeProperty ;
	rdfs:label "key"@en ;
	rdfs:range xsd:string ;
	.

observable:keyUsage
	a owl:DatatypeProperty ;
	rdfs:label "keyUsage"@en ;
	rdfs:range xsd:string ;
	.

observable:keypadUnlockCode
	a owl:DatatypeProperty ;
	rdfs:label "keypadUnlockCode"@en ;
	rdfs:comment "A code or password set on a device for security that must be entered to gain access to the device."@en ;
	rdfs:range xsd:string ;
	.

observable:keywordSearchTerm
	a owl:DatatypeProperty ;
	rdfs:label "Keyword Search Term"@en ;
	rdfs:comment "Specifies a string representing a keyword search term contained within the URL field."@en ;
	rdfs:range xsd:string ;
	.

observable:labels
	a owl:DatatypeProperty ;
	rdfs:label "labels"@en ;
	rdfs:comment "Named and colored label."@en ;
	rdfs:range xsd:string ;
	.

observable:language
	a owl:DatatypeProperty ;
	rdfs:label "language"@en ;
	rdfs:comment """Specifies the language the string is written in, e.g. English.
          For consistency, it is strongly recommended to use the ISO 639-2 language code, if available. Please see http://www.loc.gov/standards/iso639-2/php/code_list.php for a list of ISO 639-2 codes."""@en ;
	rdfs:range xsd:string ;
	.

observable:lastLoginTime
	a owl:DatatypeProperty ;
	rdfs:label "lastLoginTime"@en ;
	rdfs:comment "The date and time of the last login of the account."@en ;
	rdfs:range xsd:dateTime ;
	.

observable:lastName
	a owl:DatatypeProperty ;
	rdfs:label "lastName"@en ;
	rdfs:comment "The last name of a person."@en ;
	rdfs:range xsd:string ;
	.

observable:lastRun
	a owl:DatatypeProperty ;
	rdfs:label "lastRun"@en ;
	rdfs:comment "Timestamp of when the prefetch application was last run."@en ;
	rdfs:range xsd:dateTime ;
	.

observable:lastTimeContacted
	a owl:DatatypeProperty ;
	rdfs:label "lastTimeContacted"@en ;
	rdfs:comment "Last time contacted specifies the date and time that a particular contact was last contacted."@en ;
	.

observable:lastVisit
	a owl:DatatypeProperty ;
	rdfs:label "Last Visit Time"@en ;
	rdfs:comment "Specifies the date/time that the URL referred to by the URL field was last visited."@en ;
	rdfs:range xsd:dateTime ;
	.

observable:length
	a owl:DatatypeProperty ;
	rdfs:label "length"@en ;
	rdfs:comment "Specifies the length, in characters, of the extracted string."@en ;
	rdfs:range xsd:integer ;
	.

observable:libraryType
	a owl:DatatypeProperty ;
	rdfs:label "libraryType"@en ;
	rdfs:comment "Specifies the type of library being characterized."@en ;
	rdfs:range xsd:string ;
	.

observable:loaderFlags
	a owl:DatatypeProperty ;
	rdfs:label "loaderFlags"@en ;
	rdfs:comment "Specifies the reserved loader flags"@en ;
	rdfs:range xsd:unsignedInt ;
	.

observable:localTime
	a owl:DatatypeProperty ;
	rdfs:label "localTime"@en ;
	rdfs:comment "Specifies the local time on the system."@en ;
	rdfs:range xsd:dateTime ;
	.

observable:location
	a owl:ObjectProperty ;
	rdfs:label "location"@en ;
	rdfs:comment "An associated location."@en ;
	rdfs:range <https://unifiedcyberontology.org/ontology/uco/location#Location> ;
	.

observable:loginTime
	a owl:DatatypeProperty ;
	rdfs:label "loginTime"@en ;
	rdfs:comment "Specifies the date/time of the login for the user session."@en ;
	rdfs:range xsd:dateTime ;
	.

observable:logoutTime
	a owl:DatatypeProperty ;
	rdfs:label "logoutTime"@en ;
	rdfs:comment "Specifies the date/time of the logout for the user session."@en ;
	rdfs:range xsd:dateTime ;
	.

observable:lookupDate
	a owl:DatatypeProperty ;
	rdfs:label "lookupDate"@en ;
	rdfs:comment "Specifies the date and time that the Whois record was queried."@en ;
	rdfs:range xsd:dateTime ;
	.

observable:macAddress
	a owl:ObjectProperty ;
	rdfs:label "macAddress"@en ;
	rdfs:comment "Specifies the MAC or hardware address of the physical network card. "@en ;
	rdfs:range observable:ObservableObject ;
	.

observable:machine
	a owl:DatatypeProperty ;
	rdfs:label "machine"@en ;
	rdfs:comment "Specifies the type of target machine."@en ;
	rdfs:range xsd:string ;
	.

observable:magic
	a owl:DatatypeProperty ;
	rdfs:label "magic"@en ;
	rdfs:comment "Specifies the value that indicates the type of the PE binary."@en ;
	rdfs:range xsd:unsignedShort ;
	.

observable:magicNumber
	a owl:DatatypeProperty ;
	rdfs:label "magicNumber"@en ;
	rdfs:range xsd:string ;
	.

observable:majorImageVersion
	a owl:DatatypeProperty ;
	rdfs:label "majorImageVersion"@en ;
	rdfs:comment "Specifies the major version number of the image."@en ;
	rdfs:range xsd:unsignedShort ;
	.

observable:majorLinkerVersion
	a owl:DatatypeProperty ;
	rdfs:label "majorLinkerVersion"@en ;
	rdfs:comment "Specifies the linker major version number."@en ;
	rdfs:range xsd:byte ;
	.

observable:majorOSVersion
	a owl:DatatypeProperty ;
	rdfs:label "majorOSVersion"@en ;
	rdfs:comment "Specifies the major version number of the required operating system."@en ;
	rdfs:range xsd:unsignedShort ;
	.

observable:majorSubsystemVersion
	a owl:DatatypeProperty ;
	rdfs:label "majorSubsystemVersion"@en ;
	rdfs:comment "Specifies the major version number of the subsystem."@en ;
	rdfs:range xsd:unsignedShort ;
	.

observable:manuallyEnteredCount
	a owl:DatatypeProperty ;
	rdfs:label "Manually-Entered Count"@en ;
	rdfs:comment "Specifies the number of times the URL referred to by the URL field was manually entered into the browser's address field by the user. This field is only applicable for URL history entries generated by Google's Chrome browser."@en ;
	rdfs:range xsd:nonNegativeInteger ;
	.

observable:manufacturer
	a owl:DatatypeProperty ;
	rdfs:label "manufacturer"@en ;
	rdfs:range xsd:string ;
	.

observable:maxRunTime
	a owl:DatatypeProperty ;
	rdfs:label "maxRunTime"@en ;
	rdfs:comment "Specifies the maximum run time of the scheduled task before terminating, in milliseconds. See also: http://msdn.microsoft.com/en-us/library/windows/desktop/aa381874(v=vs.85).aspx."@en ;
	rdfs:range xsd:integer ;
	.

observable:message
	a owl:ObjectProperty ;
	rdfs:label "message"@en ;
	rdfs:range observable:ObservableObject ;
	.

observable:messageID
	a owl:DatatypeProperty ;
	rdfs:label "messageID"@en ;
	rdfs:comment "An unique identifier for the message."@en ;
	rdfs:range xsd:string ;
	.

observable:messageText
	a owl:DatatypeProperty ;
	rdfs:label "messageText"@en ;
	rdfs:comment "The contents of the message."@en ;
	rdfs:range xsd:string ;
	.

observable:messageType
	a owl:DatatypeProperty ;
	rdfs:label "messageType"@en ;
	rdfs:comment "Message type specifies what sort of message (email, chat, SMS, etc) a Message is."@en ;
	rdfs:range xsd:string ;
	.

observable:messagingAddress
	a owl:ObjectProperty ;
	rdfs:label "messagingAddress"@en ;
	rdfs:comment "A messaging address specifies details of an identifier for digital messsaging communication."@en ;
	rdfs:range observable:ObservableObject ;
	.

observable:metadataChangeTime
	a owl:DatatypeProperty ;
	rdfs:label "metadataChangeTime"@en ;
	rdfs:comment "The date and time at which the file metadata was last modified."@en ;
	rdfs:range xsd:dateTime ;
	.

observable:mftFileID
	a owl:DatatypeProperty ;
	rdfs:label "mftFileID"@en ;
	rdfs:comment "Specifies the record number for the file within an NTFS Master File Table."@en ;
	rdfs:range xsd:integer ;
	.

observable:mftFileNameAccessedTime
	a owl:DatatypeProperty ;
	rdfs:label "mftFileNameAccessedTime"@en ;
	rdfs:comment "The access date and time recorded in an MFT entry $File_Name attribute."@en ;
	rdfs:range xsd:dateTime ;
	.

observable:mftFileNameCreatedTime
	a owl:DatatypeProperty ;
	rdfs:label "mftFileNameCreatedTime"@en ;
	rdfs:comment "The creation date and time recorded in an MFT entry $File_Name attribute."@en ;
	rdfs:range xsd:dateTime ;
	.

observable:mftFileNameLength
	a owl:DatatypeProperty ;
	rdfs:label "mftFileNameLength"@en ;
	rdfs:comment " Specifies the length of an NTFS file name, in unicode characters."@en ;
	rdfs:range xsd:integer ;
	.

observable:mftFileNameModifiedTime
	a owl:DatatypeProperty ;
	rdfs:label "mftFileNameModifiedTime"@en ;
	rdfs:comment "The modification date and time recorded in an MFT entry $File_Name attribute."@en ;
	rdfs:range xsd:dateTime ;
	.

observable:mftFileNameRecordChangeTime
	a owl:DatatypeProperty ;
	rdfs:label "mftFileNameRecordChangeTime"@en ;
	rdfs:comment "The metadata modification date and time recorded in an MFT entry $File_Name attribute."@en ;
	rdfs:range xsd:dateTime ;
	.

observable:mftFlags
	a owl:DatatypeProperty ;
	rdfs:label "mftFlags"@en ;
	rdfs:comment "Specifies basic permissions for the file (Read-Only, Hidden, Archive, Compressed, etc.)."@en ;
	rdfs:range xsd:integer ;
	.

observable:mftParentID
	a owl:DatatypeProperty ;
	rdfs:label "mftParentID"@en ;
	rdfs:comment "Specifies the record number within an NTFS Master File Table for parent directory of the file."@en ;
	rdfs:range xsd:integer ;
	.

observable:mftRecordChangeTime
	a owl:DatatypeProperty ;
	rdfs:label "mftRecordChangeTime"@en ;
	rdfs:comment "The date and time at which an NTFS file metadata was last modified."@en ;
	rdfs:range xsd:dateTime ;
	.

observable:middleName
	a owl:DatatypeProperty ;
	rdfs:label "middleName"@en ;
	rdfs:comment "The middle name of a person."@en ;
	rdfs:range xsd:string ;
	.

observable:mimeClass
	a owl:DatatypeProperty ;
	rdfs:label "mimeClass"@en ;
	rdfs:range xsd:string ;
	.

observable:mimeType
	a owl:DatatypeProperty ;
	rdfs:label "mimeType"@en ;
	rdfs:comment "MIME type of the data. For example 'text/html' or 'audio/mp3'."@en ;
	rdfs:range xsd:string ;
	.

observable:minorImageVersion
	a owl:DatatypeProperty ;
	rdfs:label "minorImageVersion"@en ;
	rdfs:comment "Specifies the minor version number of the image."@en ;
	rdfs:range xsd:unsignedShort ;
	.

observable:minorLinkerVersion
	a owl:DatatypeProperty ;
	rdfs:label "minorLinkerVersion"@en ;
	rdfs:comment "Specifies the linker minor version number."@en ;
	rdfs:range xsd:byte ;
	.

observable:minorOSVersion
	a owl:DatatypeProperty ;
	rdfs:label "minorOSVersion"@en ;
	rdfs:comment "Specifies the minor version number of the required operating system."@en ;
	rdfs:range xsd:unsignedShort ;
	.

observable:minorSubsystemVersion
	a owl:DatatypeProperty ;
	rdfs:label "minorSubsystemVersion"@en ;
	rdfs:comment """Specifies the minor version number of the subsystem.
          """@en ;
	rdfs:range xsd:unsignedShort ;
	.

observable:mockLocationsAllowed
	a owl:DatatypeProperty ;
	rdfs:label "mockLocationsAllowed"@en ;
	rdfs:comment "???."@en ;
	rdfs:range xsd:boolean ;
	.

observable:model
	a owl:DatatypeProperty ;
	rdfs:label "model"@en ;
	rdfs:range xsd:string ;
	.

observable:modifiedTime
	a owl:DatatypeProperty ;
	rdfs:label "modifiedTime"@en ;
	rdfs:comment "The date and time at which the Object was last modified."@en ;
	rdfs:range xsd:dateTime ;
	.

observable:mostRecentRunTime
	a owl:DatatypeProperty ;
	rdfs:label "mostRecentRunTime"@en ;
	rdfs:comment "Specifies the most recent run date/time of this scheduled task. See also: http://msdn.microsoft.com/en-us/library/windows/desktop/aa381254(v=vs.85).aspx."@en ;
	rdfs:range xsd:dateTime ;
	.

observable:mountPoint
	a owl:DatatypeProperty ;
	rdfs:label "mountPoint"@en ;
	rdfs:comment "Specifies the mount point of the partition."@en ;
	rdfs:range xsd:string ;
	.

observable:msProductID
	a owl:DatatypeProperty ;
	rdfs:label "msProductID"@en ;
	rdfs:comment "The Microsoft Product ID. See also: http://support.microsoft.com/gp/pidwin."@en ;
	rdfs:range xsd:string ;
	.

observable:msProductName
	a owl:DatatypeProperty ;
	rdfs:label "msProductName"@en ;
	rdfs:comment "The Microsoft ProductName of the current installation of Windows. This is typically found in HKEY_LOCAL_MACHINE\\Software\\Microsoft\\Windows\\CurrentVersion!ProductName."@en ;
	rdfs:range xsd:string ;
	.

observable:nameConstraints
	a owl:DatatypeProperty ;
	rdfs:label "nameConstraints"@en ;
	rdfs:range xsd:string ;
	.

observable:namePhonetic
	a owl:DatatypeProperty ;
	rdfs:label "namePhonetic"@en ;
	rdfs:comment "Name phonetic specifies the phonetic pronunciation of the name of a person."@en ;
	rdfs:range xsd:string ;
	.

observable:namePrefix
	a owl:DatatypeProperty ;
	rdfs:label "namePrefix"@en ;
	rdfs:comment "Name prefix specifies an honorific prefix (coming ordinally before first/given name) for the name of a person."@en ;
	rdfs:range xsd:string ;
	.

observable:nameSuffix
	a owl:DatatypeProperty ;
	rdfs:label "nameSuffix"@en ;
	rdfs:comment "Name suffix specifies an suffix (coming ordinally after last/family name) for the name of a person."@en ;
	rdfs:range xsd:string ;
	.

observable:nameserver
	a owl:ObjectProperty ;
	rdfs:label "nameserver"@en ;
	rdfs:comment "Specifies a list of nameserver entries for a Whois entry."@en ;
	rdfs:range observable:ObservableObject ;
	.

observable:netBIOSName
	a owl:DatatypeProperty ;
	rdfs:label "netBIOSName"@en ;
	rdfs:comment "Specifies the NetBIOS (Network Basic Input/Output System) name of the Windows system. This is not the same as the host name."@en ;
	rdfs:range xsd:string ;
	.

observable:network
	a owl:DatatypeProperty ;
	rdfs:label "network"@en ;
	rdfs:comment "???."@en ;
	rdfs:range xsd:string ;
	.

observable:networkInterface
	a owl:ObjectProperty ;
	rdfs:label "networkInterface"@en ;
	rdfs:comment "Specifies the list of network interfaces present on the system."@en ;
	rdfs:range observable:ObservableObject ;
	.

observable:newObject
	a owl:ObjectProperty ;
	rdfs:label "newObject"@en ;
	rdfs:comment "Specifies the observable object and its properties as they are after the state change effect occurred."@en ;
	rdfs:range observable:ObservableObject ;
	.

observable:nextRunTime
	a owl:DatatypeProperty ;
	rdfs:label "nextRunTime"@en ;
	rdfs:comment "Specifies the next run date/time of the scheduled task. See also: http://msdn.microsoft.com/en-us/library/windows/desktop/aa381257(v=vs.85).aspx."@en ;
	rdfs:range xsd:dateTime ;
	.

observable:nickname
	a owl:DatatypeProperty ;
	rdfs:label "nickname"@en ;
	rdfs:comment "Nickname specifies an alternate, unofficial and typically informal name for a person independent of their official name."@en ;
	rdfs:range xsd:string ;
	.

observable:ntfsHardLinkCount
	a owl:DatatypeProperty ;
	rdfs:label "ntfsHardLinkCount"@en ;
	rdfs:comment "Specifies the number of directory entries that reference an NTFS file record."@en ;
	rdfs:range xsd:integer ;
	.

observable:ntfsOwnerID
	a owl:DatatypeProperty ;
	rdfs:label "ntfsOwnerID"@en ;
	rdfs:comment "Specifies the identifier of the file owner, from the security index."@en ;
	rdfs:range xsd:string ;
	.

observable:ntfsOwnerSID
	a owl:DatatypeProperty ;
	rdfs:label "ntfsOwnerSID"@en ;
	rdfs:comment "Specifies the security ID (key in the $SII Index and $SDS DataStream in the file $Secure) for an NTFS file."@en ;
	rdfs:range xsd:string ;
	.

observable:number
	a owl:DatatypeProperty ;
	rdfs:label "number"@en ;
	rdfs:range xsd:integer ;
	.

observable:numberOfLaunches
	a owl:DatatypeProperty ;
	rdfs:label "numberOfLaunches"@en ;
	rdfs:range xsd:integer ;
	.

observable:numberOfRVAAndSizes
	a owl:DatatypeProperty ;
	rdfs:label "numberOfRVAAndSizes"@en ;
	rdfs:comment "Specifies the number of data-directory entries in the remainder of the optional header."@en ;
	rdfs:range xsd:unsignedInt ;
	.

observable:numberOfSections
	a owl:DatatypeProperty ;
	rdfs:label "numberOfSections"@en ;
	rdfs:comment "Specifies the number of sections in the PE binary, as a non-negative integer."@en ;
	rdfs:range xsd:integer ;
	.

observable:numberOfSubkeys
	a owl:DatatypeProperty ;
	rdfs:label "numberOfSubkeys"@en ;
	rdfs:range xsd:integer ;
	.

observable:numberOfSymbols
	a owl:DatatypeProperty ;
	rdfs:label "numberOfSymbols"@en ;
	rdfs:comment "Specifies the number of entries in the symbol table of the PE binary, as a non-negative integer."@en ;
	rdfs:range xsd:integer ;
	.

observable:numberTimesContacted
	a owl:DatatypeProperty ;
	rdfs:label "numberTimesContacted"@en ;
	rdfs:comment "Number times contacted specifies the number of times a particular contact has been contacted."@en ;
	rdfs:range xsd:integer ;
	.

observable:objectGUID
	a owl:DatatypeProperty ;
	rdfs:label "objectGUID"@en ;
	rdfs:range xsd:string ;
	.

observable:observableCreatedTime
	a owl:DatatypeProperty ;
	rdfs:label "observableCreatedTime"@en ;
	rdfs:comment "The date and time at which the observable object being characterized was created. This time pertains to an intrinsic characteristic of the observable object, and would be consistent across independent characterizations or observations of the observable object."@en ;
	rdfs:range xsd:dateTime ;
	.

observable:oldObject
	a owl:ObjectProperty ;
	rdfs:label "oldObject"@en ;
	rdfs:comment "Specifies the observable object and its properties as they were before the state change effect occurred."@en ;
	rdfs:range observable:ObservableObject ;
	.

observable:openFileDescriptor
	a owl:DatatypeProperty ;
	rdfs:label "openFileDescriptor"@en ;
	rdfs:comment "Specifies a listing of the current file descriptors used by the Unix process."@en ;
	rdfs:range xsd:integer ;
	.

observable:operatingSystem
	a owl:ObjectProperty ;
	rdfs:label "operatingSystem"@en ;
	rdfs:range observable:ObservableObject ;
	.

observable:optionalHeader
	a owl:ObjectProperty ;
	rdfs:label "optionalHeader"@en ;
	rdfs:comment "Specifies the PE optional header of the PE binary."@en ;
	rdfs:range observable:WindowsPEOptionalHeader ;
	.

observable:options
	a owl:DatatypeProperty ;
	rdfs:label "options"@en ;
	rdfs:comment "Specifies any options used when mounting the volume."@en ;
	rdfs:range xsd:string ;
	.

observable:organizationDepartment
	a owl:DatatypeProperty ;
	rdfs:label "organizationDepartment"@en ;
	rdfs:comment "Specifies a particular suborganization (division, branch, office, etc.) that exists within a larger organization."@en ;
	rdfs:range xsd:string ;
	.

observable:organizationLocation
	a owl:ObjectProperty ;
	rdfs:label "organizationLocation"@en ;
	rdfs:comment "Specifies a geolocation address of an organization."@en ;
	rdfs:range observable:ContactAddress ;
	.

observable:organizationPosition
	a owl:DatatypeProperty ;
	rdfs:label "organizationPosition"@en ;
	rdfs:comment "Specifies the title or role that a person plays within an organization."@en ;
	rdfs:range xsd:string ;
	.

observable:otherHeaders
	a owl:ObjectProperty ;
	rdfs:label "otherHeaders"@en ;
	rdfs:range <https://unifiedcyberontology.org/ontology/uco/types#Dictionary> ;
	.

observable:owner
	a owl:ObjectProperty ;
	rdfs:label "owner"@en ;
	rdfs:comment
		"The owner of the file."@en ,
		"The owner of this account."@en
		;
	rdfs:range
		<https://unifiedcyberontology.org/ontology/uco/core#UcoObject> ,
		observable:ObservableObject
		;
	.

observable:ownerSID
	a owl:DatatypeProperty ;
	rdfs:label "ownerSID"@en ;
	rdfs:range xsd:string ;
	.

observable:pageTitle
	a owl:DatatypeProperty ;
	rdfs:label "Page Title"@en ;
	rdfs:comment "Specifies the title of a web page."@en ;
	rdfs:range xsd:string ;
	.

observable:parameterAddress
	a owl:DatatypeProperty ;
	rdfs:label "parameterAddress"@en ;
	rdfs:range xsd:hexBinary ;
	.

observable:parameters
	a owl:DatatypeProperty ;
	rdfs:label "parameters"@en ;
	rdfs:comment "Specifies the command line parameters used to launch the scheduled task. See also: http://msdn.microsoft.com/en-us/library/windows/desktop/aa381875(v=vs.85).aspx."@en ;
	rdfs:range xsd:string ;
	.

observable:parent
	a owl:ObjectProperty ;
	rdfs:label "parent"@en ;
	rdfs:comment "The process that created this process."@en ;
	rdfs:range observable:ObservableObject ;
	.

observable:participant
	a owl:ObjectProperty ;
	rdfs:label "participant"@en ;
	rdfs:range observable:ObservableObject ;
	.

observable:partition
	a owl:ObjectProperty ;
	rdfs:label "partition"@en ;
	rdfs:comment "The partitions that reside on the disk."@en ;
	rdfs:range observable:ObservableObject ;
	.

observable:partitionID
	a owl:DatatypeProperty ;
	rdfs:label "partitionID"@en ;
	rdfs:comment "Specifies the identifier of the partition, as provided by the containing partition table.  This identifier is the index value within the partition table, and is expected to be an incrementing alphanumeric value (numeric in most partition systems), not a GUID or UUID.  Sorting partitions by this index should first attempt to sort a numeric cast of the value."@en ;
	rdfs:range xsd:string ;
	.

observable:partitionLength
	a owl:DatatypeProperty ;
	rdfs:label "partitionLength"@en ;
	rdfs:comment "Specifies the length of the partition, in bytes."@en ;
	rdfs:range xsd:integer ;
	.

observable:partitionOffset
	a owl:DatatypeProperty ;
	rdfs:label "partitionOffset"@en ;
	rdfs:comment "Specifies the starting offset of the partition, in bytes."@en ;
	rdfs:range xsd:integer ;
	.

observable:password
	a owl:DatatypeProperty ;
	rdfs:label "password"@en ;
	rdfs:comment
		"Password used to authenticate to this resource."@en ,
		"The account authentication password."@en
		;
	rdfs:range xsd:string ;
	.

observable:passwordLastChanged
	a owl:DatatypeProperty ;
	rdfs:label "passwordLastChanged"@en ;
	rdfs:comment "The date and time that the password was last changed."@en ;
	rdfs:range xsd:dateTime ;
	.

observable:passwordType
	a owl:DatatypeProperty ;
	rdfs:label "passwordType"@en ;
	rdfs:comment "The type of password, for instance plain-text or encrypted."@en ;
	rdfs:range xsd:string ;
	.

observable:path
	a owl:DatatypeProperty ;
	rdfs:label "path"@en ;
	rdfs:comment "Specifies the location of one object within another containing object."@en ;
	rdfs:range xsd:string ;
	.

observable:pdfId0
	a owl:DatatypeProperty ;
	rdfs:label "pdfId0"@en ;
	rdfs:range xsd:string ;
	.

observable:pdfId1
	a owl:DatatypeProperty ;
	rdfs:label "pdfId1"@en ;
	rdfs:range xsd:string ;
	.

observable:peType
	a owl:DatatypeProperty ;
	rdfs:label "peType"@en ;
	rdfs:comment "Specifies the type of the PE binary."@en ;
	rdfs:range xsd:string ;
	.

observable:phoneActivationTime
	a owl:DatatypeProperty ;
	rdfs:label "phoneActivationTime"@en ;
	rdfs:comment "The date and time that a device was activated."@en ;
	rdfs:range xsd:dateTime ;
	.

observable:phoneNumber
	a owl:DatatypeProperty ;
	rdfs:label "phoneNumber"@en ;
	rdfs:comment "A phone number(account)."@en ;
	rdfs:range xsd:string ;
	.

observable:pictureHeight
	a owl:DatatypeProperty ;
	rdfs:label "pictureHeight"@en ;
	rdfs:range xsd:integer ;
	.

observable:pictureType
	a owl:DatatypeProperty ;
	rdfs:label "pictureType"@en ;
	rdfs:comment "The type of a picture, for example a thumbnail."@en ;
	rdfs:range xsd:string ;
	.

observable:pictureWidth
	a owl:DatatypeProperty ;
	rdfs:label "pictureWidth"@en ;
	rdfs:comment "The width of the picture in pixels."@en ;
	rdfs:range xsd:integer ;
	.

observable:pid
	a owl:DatatypeProperty ;
	rdfs:label "pid"@en ;
	rdfs:comment "The Process ID, or PID, of the process."@en ;
	rdfs:range xsd:integer ;
	.

observable:pointerToSymbolTable
	a owl:DatatypeProperty ;
	rdfs:label "pointerToSymbolTable"@en ;
	rdfs:comment "Specifies the file offset of the COFF symbol table."@en ;
	rdfs:range xsd:hexBinary ;
	.

observable:policyConstraints
	a owl:DatatypeProperty ;
	rdfs:label "policyConstraints"@en ;
	rdfs:range xsd:string ;
	.

observable:policyMappings
	a owl:DatatypeProperty ;
	rdfs:label "policyMappings"@en ;
	rdfs:range xsd:string ;
	.

observable:port
	a owl:DatatypeProperty ;
	rdfs:label "port"@en ;
	rdfs:comment "Port on which communication takes place."@en ;
	rdfs:range xsd:integer ;
	.

observable:prefetchHash
	a owl:DatatypeProperty ;
	rdfs:label "prefetchHash"@en ;
	rdfs:comment "An eight character hash of the location from which the application was run."@en ;
	rdfs:range xsd:string ;
	.

observable:priority
	a owl:DatatypeProperty ;
	rdfs:label "priority"@en ;
	rdfs:comment "The priority of the email."@en ;
	rdfs:range xsd:string ;
	.

observable:privateKeyUsagePeriodNotAfter
	a owl:DatatypeProperty ;
	rdfs:label "privateKeyUsagePeriodNotAfter"@en ;
	rdfs:range xsd:dateTime ;
	.

observable:privateKeyUsagePeriodNotBefore
	a owl:DatatypeProperty ;
	rdfs:label "privateKeyUsagePeriodNotBefore"@en ;
	rdfs:range xsd:dateTime ;
	.

observable:processorArchitecture
	a owl:DatatypeProperty ;
	rdfs:label "processorArchitecture"@en ;
	rdfs:comment "Specifies the specific architecture (e.g. x86) used by the CPU of the system."@en ;
	rdfs:range xsd:string ;
	.

observable:profile
	a owl:ObjectProperty ;
	rdfs:label "profile"@en ;
	rdfs:comment "A profile specifies a particular online service profile."@en ;
	rdfs:range observable:ObservableObject ;
	.

observable:profileAccount
	a owl:ObjectProperty ;
	rdfs:label "Profile Account"@en-US ;
	rdfs:comment "Specifies the online service account associated with the profile."@en-US ;
	rdfs:range observable:ObservableObject ;
	.

observable:profileBackgroundHash
	a owl:ObjectProperty ;
	rdfs:label "Profile Background Hash"@en-US ;
	rdfs:comment "Specifies hashes of the background associated with the profile."@en-US ;
	rdfs:range <https://unifiedcyberontology.org/ontology/uco/types#Hash> ;
	.

observable:profileBackgroundLocation
	a owl:ObjectProperty ;
	rdfs:label "Profile Background Location"@en-US ;
	rdfs:comment "Specifies the network location of the background associated with the profile."@en-US ;
	rdfs:range observable:ObservableObject ;
	.

observable:profileBannerHash
	a owl:ObjectProperty ;
	rdfs:label "Profile Banner Hash"@en-US ;
	rdfs:comment "Specifies hashes of the banner associated with the profile."@en-US ;
	rdfs:range <https://unifiedcyberontology.org/ontology/uco/types#Hash> ;
	.

observable:profileBannerLocation
	a owl:ObjectProperty ;
	rdfs:label "Profile Banner Location"@en-US ;
	rdfs:comment "Specifies the network location of the banner associated with the profile."@en-US ;
	rdfs:range observable:ObservableObject ;
	.

observable:profileCreated
	a owl:DatatypeProperty ;
	rdfs:label "Profile Created"@en-US ;
	rdfs:comment "Specifies the date and time the profile was created."@en-US ;
	rdfs:range xsd:dateTime ;
	.

observable:profileIdentity
	a owl:ObjectProperty ;
	rdfs:label "Profile Identity"@en-US ;
	rdfs:comment "Specifies the identity associated with the profile."@en-US ;
	rdfs:range identity:Identity ;
	.

observable:profileImageHash
	a owl:ObjectProperty ;
	rdfs:label "Profile Image Hash"@en-US ;
	rdfs:comment "Specifies hashes of the profile image associated with the profile."@en-US ;
	rdfs:range <https://unifiedcyberontology.org/ontology/uco/types#Hash> ;
	.

observable:profileImageLocation
	a owl:ObjectProperty ;
	rdfs:label "Profile Image Location"@en-US ;
	rdfs:comment "Specifies the network location of the profile image associated with the profile."@en-US ;
	rdfs:range observable:ObservableObject ;
	.

observable:profileIsProtected
	a owl:DatatypeProperty ;
	rdfs:label "Is_Protected"@en-US ;
	rdfs:comment "Specifies whether the twitter profile is protected."@en-US ;
	rdfs:range xsd:boolean ;
	.

observable:profileIsVerified
	a owl:DatatypeProperty ;
	rdfs:label "Is_Verified"@en-US ;
	rdfs:comment "Specifies whether the twitter profile is verified."@en-US ;
	rdfs:range xsd:boolean ;
	.

observable:profileService
	a owl:ObjectProperty ;
	rdfs:label "Profile Service"@en-US ;
	rdfs:comment "Specifies the online service associated with the profile."@en-US ;
	rdfs:range observable:ObservableObject ;
	.

observable:profileWebsite
	a owl:ObjectProperty ;
	rdfs:label "Profile Website"@en-US ;
	rdfs:comment "Specifies the website URL associated with the profile."@en-US ;
	rdfs:range observable:ObservableObject ;
	.

observable:profilelanguage
	a owl:DatatypeProperty ;
	rdfs:label "Profile Language"@en-US ;
	rdfs:comment "Specifies the language associated with the profile. When present, it MUST be a language code conformant to RFC 5646/BCP47."@en-US ;
	rdfs:range xsd:string ;
	.

observable:properties
	a owl:DatatypeProperty ;
	rdfs:label "properties"@en ;
	rdfs:comment "Specifies the properties that were enumerated as a result of the action on the observable object."@en ;
	rdfs:range xsd:string ;
	.

observable:propertyName
	a owl:DatatypeProperty ;
	rdfs:label "propertyName"@en ;
	rdfs:comment "Specifies the Name of the property being read."@en ;
	rdfs:range xsd:string ;
	.

observable:protocols
	a owl:ObjectProperty ;
	rdfs:label "protocols"@en ;
	rdfs:comment "Specifies the protocols involved in the network connection, along with their corresponding state. "@en ;
	rdfs:range <https://unifiedcyberontology.org/ontology/uco/types#ControlledDictionary> ;
	.

observable:query
	a owl:DatatypeProperty ;
	rdfs:label "query"@en ;
	rdfs:comment "Query passed to the resource."@en ;
	rdfs:range xsd:string ;
	.

observable:rangeOffset
	a owl:DatatypeProperty ;
	rdfs:label "rangeOffset"@en ;
	rdfs:comment "The offset at which the start of data can be found, relative to the rangeOffsetType defined."@en ;
	rdfs:range xsd:integer ;
	.

observable:rangeOffsetType
	a owl:DatatypeProperty ;
	rdfs:label "rangeOffsetType"@en ;
	rdfs:comment "The type of offset defined for the range (e.g., image, file, address)."@en ;
	rdfs:range xsd:string ;
	.

observable:rangeSize
	a owl:DatatypeProperty ;
	rdfs:label "rangeSize"@en ;
	rdfs:comment "The size of the data in bytes."@en ;
	rdfs:range xsd:integer ;
	.

observable:receivedLines
	a owl:DatatypeProperty ;
	rdfs:label "receivedLines"@en ;
	rdfs:range xsd:string ;
	.

observable:receivedTime
	a owl:DatatypeProperty ;
	rdfs:label "receivedTime"@en ;
	rdfs:comment "The date and time at which the message received. "@en ;
	rdfs:range xsd:dateTime ;
	.

observable:recurrence
	a owl:DatatypeProperty ;
	rdfs:label "recurrence"@en ;
	rdfs:comment "Recurrence of the event."@en ;
	rdfs:range xsd:string ;
	.

observable:references
	a owl:ObjectProperty ;
	rdfs:label "references"@en ;
	rdfs:comment "A list of email message identifiers this email relates to."@en ;
	rdfs:range observable:ObservableObject ;
	.

observable:referralURL
	a owl:ObjectProperty ;
	rdfs:label "referralURL"@en ;
	rdfs:comment "Specifies the corresponding referral URL for a registrar."@en ;
	rdfs:range observable:ObservableObject ;
	.

observable:referrerUrl
	a owl:ObjectProperty ;
	rdfs:label "referrerURL"@en ;
	rdfs:comment "Specifies the origination point (i.e., URL) of a URL request."@en ;
	rdfs:range observable:ObservableObject ;
	.

observable:regionEndAddress
	a owl:DatatypeProperty ;
	rdfs:label "regionEndAddress"@en ;
	rdfs:comment "The regionEndAddress property specifies the ending address of the particular memory region."@en ;
	rdfs:range xsd:hexBinary ;
	.

observable:regionSize
	a owl:DatatypeProperty ;
	rdfs:label "regionSize"@en ;
	rdfs:comment "The regionSize property specifies the size of the particular memory region, in bytes."@en ;
	rdfs:range xsd:integer ;
	.

observable:regionStartAddress
	a owl:DatatypeProperty ;
	rdfs:label "regionStartAddress"@en ;
	rdfs:comment """The regionStartAddress property specifies the starting address of the particular memory region.
          """@en ;
	rdfs:range xsd:hexBinary ;
	.

observable:regionalInternetRegistry
	a owl:DatatypeProperty ;
	rdfs:label "regionalInternetRegistry"@en ;
	rdfs:comment "specifies the name of the Regional Internet Registry (RIR) which allocated the IP address contained in a WHOIS entry."@en ;
	rdfs:range vocabulary:RegionalRegistryTypeVocab ;
	.

observable:registeredOrganization
	a owl:ObjectProperty ;
	rdfs:label "registeredOrganization"@en ;
	rdfs:comment "The organization that this copy of Windows is registered to."@en ;
	rdfs:range identity:Identity ;
	.

observable:registeredOwner
	a owl:ObjectProperty ;
	rdfs:label "registeredOwner"@en ;
	rdfs:comment "The person or organization that is the registered owner of this copy of Windows."@en ;
	rdfs:range identity:Identity ;
	.

observable:registrantContactInfo
	a owl:ObjectProperty ;
	rdfs:label "registrantContactInfo"@en ;
	rdfs:comment "Specifies contact info for the registrant of a domain within a WHOIS entity."@en ;
	rdfs:range observable:ObservableObject ;
	.

observable:registrantIDs
	a owl:DatatypeProperty ;
	rdfs:label "registrantIDs"@en ;
	rdfs:comment "Specifies the registrant IDs associated with a domain lookup."@en ;
	rdfs:range xsd:string ;
	.

observable:registrarGUID
	a owl:DatatypeProperty ;
	rdfs:label "registrarGUID"@en ;
	rdfs:comment "Specifies the Registrar GUID field of a Whois entry."@en ;
	rdfs:range xsd:string ;
	.

observable:registrarID
	a owl:DatatypeProperty ;
	rdfs:label "registrarID"@en ;
	rdfs:comment "Specifies the Registrar ID field of a Whois entry."@en ;
	rdfs:range xsd:string ;
	.

observable:registrarInfo
	a owl:ObjectProperty ;
	rdfs:label "registrarInfo"@en ;
	rdfs:comment "Specifies registrar info that would be returned from a registrar lookup."@en ;
	rdfs:range observable:WhoisRegistrarInfoType ;
	.

observable:registrarName
	a owl:DatatypeProperty ;
	rdfs:label "registrarName"@en ;
	rdfs:comment "The name of the registrar organization."@en ;
	rdfs:range xsd:string ;
	.

observable:registryValues
	a owl:ObjectProperty ;
	rdfs:label "registryValues"@en ;
	rdfs:comment "The values that were enumerated as a result of the action on the object."@en ;
	rdfs:range observable:WindowsRegistryValue ;
	.

observable:remarks
	a owl:DatatypeProperty ;
	rdfs:label "remarks"@en ;
	rdfs:comment "Specifies any remarks associated with this Whois entry."@en ;
	rdfs:range xsd:string ;
	.

observable:remindTime
	a owl:DatatypeProperty ;
	rdfs:label "remindTime"@en ;
	rdfs:range xsd:dateTime ;
	.

observable:requestMethod
	a owl:DatatypeProperty ;
	rdfs:label "requestMethod"@en ;
	rdfs:comment """Specifies the HTTP method portion of the HTTP request line, as a lowercase string.
          """@en ;
	rdfs:range xsd:string ;
	.

observable:requestValue
	a owl:DatatypeProperty ;
	rdfs:label "requestValue"@en ;
	rdfs:comment "Specifies the value (typically a resource path) portion of the HTTP request line."@en ;
	rdfs:range xsd:string ;
	.

observable:requestVersion
	a owl:DatatypeProperty ;
	rdfs:label "requestVersion"@en ;
	rdfs:comment "Specifies the HTTP version portion of the HTTP request line, as a lowercase string."@en ;
	rdfs:range xsd:string ;
	.

observable:rowCondition
	a owl:DatatypeProperty ;
	rdfs:label "rowCondition"@en ;
	rdfs:range xsd:string ;
	.

observable:rowIndex
	a owl:DatatypeProperty ;
	rdfs:label "rowIndex"@en ;
	rdfs:range xsd:positiveInteger ;
	.

observable:ruid
	a owl:DatatypeProperty ;
	rdfs:label "ruid"@en ;
	rdfs:comment "Specifies the real user ID, which represents the Unix user who created the process."@en ;
	rdfs:range xsd:nonNegativeInteger ;
	.

observable:runningStatus
	a owl:DatatypeProperty ;
	rdfs:label "runningStatus"@en ;
	rdfs:range xsd:string ;
	.

observable:scheme
	a owl:DatatypeProperty ;
	rdfs:label "scheme"@en ;
	rdfs:comment "Identifies the type of URL."@en ;
	rdfs:range xsd:string ;
	.

observable:sectionAlignment
	a owl:DatatypeProperty ;
	rdfs:label "sectionAlignment"@en ;
	rdfs:comment "Specifies the alignment (in bytes) of PE sections when they are loaded into memory."@en ;
	rdfs:range xsd:unsignedInt ;
	.

observable:sections
	a owl:ObjectProperty ;
	rdfs:label "sections"@en ;
	rdfs:comment "Specifies metadata about the sections in the PE file."@en ;
	rdfs:range observable:WindowsPESection ;
	.

observable:sectorSize
	a owl:DatatypeProperty ;
	rdfs:label "sectorSize"@en ;
	rdfs:comment "The sector size of the volume in bytes."@en ;
	rdfs:range xsd:integer ;
	.

observable:securityAttributes
	a owl:DatatypeProperty ;
	rdfs:label "securityAttributes"@en ;
	rdfs:range xsd:string ;
	.

observable:sender
	a owl:ObjectProperty ;
	rdfs:label "sender"@en ;
	rdfs:range observable:ObservableObject ;
	.

observable:sentTime
	a owl:DatatypeProperty ;
	rdfs:label "sentTime"@en ;
	rdfs:comment "The date and time at which the message sent."@en ;
	rdfs:range xsd:dateTime ;
	.

observable:serialNumber
	a owl:DatatypeProperty ;
	rdfs:label "serialNumber"@en ;
	rdfs:range xsd:string ;
	.

observable:serverName
	a owl:ObjectProperty ;
	rdfs:label "serverName"@en ;
	rdfs:comment "Specifies the corresponding server name for a whois entry. This usually corresponds to a nameserver lookup."@en ;
	rdfs:range observable:ObservableObject ;
	.

observable:serviceName
	a owl:DatatypeProperty ;
	rdfs:label "serviceName"@en ;
	rdfs:range xsd:string ;
	.

observable:serviceStatus
	a owl:DatatypeProperty ;
	rdfs:label "serviceStatus"@en ;
	rdfs:range xsd:string ;
	.

observable:serviceType
	a owl:DatatypeProperty ;
	rdfs:label "serviceType"@en ;
	rdfs:range xsd:string ;
	.

observable:sessionID
	a owl:DatatypeProperty ;
	rdfs:label "sessionID"@en ;
	rdfs:comment "An identifier for the session from which the message originates."@en ;
	rdfs:range xsd:string ;
	.

observable:shell
	a owl:DatatypeProperty ;
	rdfs:label "shell"@en ;
	rdfs:range xsd:string ;
	.

observable:showMessageBody
	a owl:DatatypeProperty ;
	rdfs:label "showMessageBody"@en ;
	rdfs:comment "Specifies the message text that is displayed in the body of the message box by the action. See also: http://msdn.microsoft.com/en-us/library/windows/desktop/aa381302(v=vs.85).aspx."@en ;
	rdfs:range xsd:string ;
	.

observable:showMessageTitle
	a owl:DatatypeProperty ;
	rdfs:label "showMessageTitle"@en ;
	rdfs:comment "Specifies the title of the message box shown by the action. See also: http://msdn.microsoft.com/en-us/library/windows/desktop/aa381302(v=vs.85).aspx."@en ;
	rdfs:range xsd:string ;
	.

observable:sid
	a owl:DatatypeProperty ;
	rdfs:label "sid"@en ;
	rdfs:range xsd:string ;
	.

observable:signature
	a owl:DatatypeProperty ;
	rdfs:label "signature"@en ;
	rdfs:comment "A"@en ;
	rdfs:range xsd:string ;
	.

observable:signatureAlgorithm
	a owl:DatatypeProperty ;
	rdfs:label "signatureAlgorithm"@en ;
	rdfs:range xsd:string ;
	.

observable:signatureDescription
	a owl:DatatypeProperty ;
	rdfs:label "signatureDescription"@en ;
	rdfs:range xsd:string ;
	.

observable:signatureExists
	a owl:DatatypeProperty ;
	rdfs:label "signatureExists"@en ;
	rdfs:range xsd:boolean ;
	.

observable:signatureVerified
	a owl:DatatypeProperty ;
	rdfs:label "signatureVerified"@en ;
	rdfs:range xsd:boolean ;
	.

observable:sipAddress
	a owl:ObjectProperty ;
	rdfs:label "sipAddress"@en ;
	rdfs:comment "A SIP address specifies Session Initiation Protocol (SIP) identifier."@en ;
	rdfs:range observable:ObservableObject ;
	.

observable:size
	a owl:DatatypeProperty ;
	rdfs:label "size"@en ;
	rdfs:comment "Specifies the size of the section, in bytes."@en ;
	rdfs:range xsd:integer ;
	.

observable:sizeInBytes
	a owl:DatatypeProperty ;
	rdfs:label "sizeInBytes"@en ;
	rdfs:comment "The size of the data in bytes."@en ;
	rdfs:range xsd:integer ;
	.

observable:sizeOfCode
	a owl:DatatypeProperty ;
	rdfs:label "sizeOfCode"@en ;
	rdfs:comment "Specifies the size of the code (text) section. If there are multiple such sections, this refers to the sum of the sizes of each section."@en ;
	rdfs:range xsd:unsignedInt ;
	.

observable:sizeOfHeaders
	a owl:DatatypeProperty ;
	rdfs:label "sizeOfHeaders"@en ;
	rdfs:comment "Specifies the combined size of the MS-DOS, PE header, and section headers, rounded up a multiple of the value specified in the file_alignment header."@en ;
	rdfs:range xsd:unsignedInt ;
	.

observable:sizeOfHeapCommit
	a owl:DatatypeProperty ;
	rdfs:label "sizeOfHeapCommit"@en ;
	rdfs:comment "Specifies the size of the local heap space to commit."@en ;
	rdfs:range xsd:unsignedInt ;
	.

observable:sizeOfHeapReserve
	a owl:DatatypeProperty ;
	rdfs:label "sizeOfHeapReserve"@en ;
	rdfs:comment "Specifies the size of the local heap space to reserve."@en ;
	rdfs:range xsd:unsignedInt ;
	.

observable:sizeOfImage
	a owl:DatatypeProperty ;
	rdfs:label "sizeOfImage"@en ;
	rdfs:comment "Specifies the size, in bytes, of the image, including all headers, as the image is loaded in memory."@en ;
	rdfs:range xsd:unsignedInt ;
	.

observable:sizeOfInitializedData
	a owl:DatatypeProperty ;
	rdfs:label "sizeOfInitializedData"@en ;
	rdfs:comment "Specifies the size of the initialized data section. If there are multiple such sections, this refers to the sum of the sizes of each section."@en ;
	rdfs:range xsd:unsignedInt ;
	.

observable:sizeOfOptionalHeader
	a owl:DatatypeProperty ;
	rdfs:label "sizeOfOptionalHeader"@en ;
	rdfs:comment "Specifies the size of the optional header of the PE binary. "@en ;
	rdfs:range xsd:integer ;
	.

observable:sizeOfStackCommit
	a owl:DatatypeProperty ;
	rdfs:label "sizeOfStackCommit"@en ;
	rdfs:comment "Specifies the size of the stack to commit."@en ;
	rdfs:range xsd:unsignedInt ;
	.

observable:sizeOfStackReserve
	a owl:DatatypeProperty ;
	rdfs:label "sizeOfStackReserve"@en ;
	rdfs:comment "Specifies the size of the stack to reserve."@en ;
	rdfs:range xsd:unsignedInt ;
	.

observable:sizeOfUninitializedData
	a owl:DatatypeProperty ;
	rdfs:label "sizeOfUninitializedData"@en ;
	rdfs:comment "Specifies the size of the uninitialized data section. If there are multiple such sections, this refers to the sum of the sizes of each section."@en ;
	rdfs:range xsd:unsignedInt ;
	.

observable:sourceApplication
	a owl:ObjectProperty ;
	rdfs:label "sourceApplication"@en ;
	rdfs:comment "Source application specifies the software application that a particular contact or contact list is associated with."@en ;
	rdfs:range observable:ObservableObject ;
	.

observable:sourceFlags
	a owl:DatatypeProperty ;
	rdfs:label "sourceFlags"@en ;
	rdfs:comment "Specifies the source TCP flags."@en ;
	rdfs:range xsd:hexBinary ;
	.

observable:sourcePort
	a owl:DatatypeProperty ;
	rdfs:label "sourcePort"@en ;
	rdfs:comment """Specifies the source port used in the connection, as an integer in the range of 0 - 65535.
          """@en ;
	rdfs:range xsd:integer ;
	.

observable:spaceLeft
	a owl:DatatypeProperty ;
	rdfs:label "spaceLeft"@en ;
	rdfs:comment "Specifies the amount of space left on the partition, in bytes."@en ;
	rdfs:range xsd:integer ;
	.

observable:spaceUsed
	a owl:DatatypeProperty ;
	rdfs:label "spaceUsed"@en ;
	rdfs:comment "Specifies the amount of space used on the partition, in bytes."@en ;
	rdfs:range xsd:integer ;
	.

observable:sponsoringRegistrar
	a owl:DatatypeProperty ;
	rdfs:label "sponsoringRegistrar"@en ;
	rdfs:comment "Specifies the name of the sponsoring registrar for a domain."@en ;
	rdfs:range xsd:string ;
	.

observable:src
	a owl:ObjectProperty ;
	rdfs:label "src"@en ;
	rdfs:comment "Specifies the source(s) of the network connection."@en ;
	rdfs:range <https://unifiedcyberontology.org/ontology/uco/core#UcoObject> ;
	.

observable:srcBytes
	a owl:DatatypeProperty ;
	rdfs:label "srcBytes"@en ;
	rdfs:range xsd:integer ;
	.

observable:srcPackets
	a owl:DatatypeProperty ;
	rdfs:label "srcPackets"@en ;
	rdfs:range xsd:integer ;
	.

observable:srcPayload
	a owl:ObjectProperty ;
	rdfs:label "srcPayload"@en ;
	rdfs:range observable:ObservableObject ;
	.

observable:ssid
	a owl:DatatypeProperty ;
	rdfs:label "ssid"@en ;
	rdfs:comment "Network identifier."@en ;
	rdfs:range xsd:string ;
	.

observable:stackSize
	a owl:DatatypeProperty ;
	rdfs:label "stackSize"@en ;
	rdfs:range xsd:nonNegativeInteger ;
	.

observable:startAddress
	a owl:DatatypeProperty ;
	rdfs:label "startAddress"@en ;
	rdfs:range xsd:hexBinary ;
	.

observable:startCommandLine
	a owl:DatatypeProperty ;
	rdfs:label "startCommandLine"@en ;
	rdfs:range xsd:string ;
	.

observable:startTime
	a owl:DatatypeProperty ;
	rdfs:label "startTime"@en ;
	rdfs:range xsd:dateTime ;
	.

observable:startType
	a owl:DatatypeProperty ;
	rdfs:label "startType"@en ;
	rdfs:range xsd:string ;
	.

observable:startupInfo
	a owl:ObjectProperty ;
	rdfs:label "startupInfo"@en ;
	rdfs:range <https://unifiedcyberontology.org/ontology/uco/types#Dictionary> ;
	.

observable:state
	a owl:DatatypeProperty ;
	rdfs:label "State"@en ;
	rdfs:range xsd:string ;
	.

observable:status
	a owl:DatatypeProperty ;
	rdfs:label "status"@en ;
	rdfs:comment "Specifies a list of statuses for a given Whois entry."@en ;
	rdfs:range vocabulary:WhoisStatusTypeVocab ;
	.

observable:statusesCount
	a owl:DatatypeProperty ;
	rdfs:label "Statuses Count"@en-US ;
	rdfs:comment "Specifies the number of tweets that this profile has issued."@en-US ;
	rdfs:range xsd:nonNegativeInteger ;
	.

observable:storageCapacityInBytes
	a owl:DatatypeProperty ;
	rdfs:label "storageCapacityInBytes"@en ;
	rdfs:comment "The number of bytes that can be stored on a SIM card."@en ;
	rdfs:range xsd:integer ;
	.

observable:stringValue
	a owl:DatatypeProperty ;
	rdfs:label "stringValue"@en ;
	rdfs:comment "Specifies the actual value of the extracted string."@en ;
	rdfs:range xsd:string ;
	.

observable:strings
	a owl:ObjectProperty ;
	rdfs:label "strings"@en ;
	rdfs:range observable:ExtractedString ;
	.

observable:subject
	a owl:DatatypeProperty ;
	rdfs:label "subject"@en ;
	rdfs:comment "The subject of the email."@en ;
	rdfs:range xsd:string ;
	.

observable:subjectAlternativeName
	a owl:DatatypeProperty ;
	rdfs:label "subjectAlternativeName"@en ;
	rdfs:range xsd:string ;
	.

observable:subjectDirectoryAttributes
	a owl:DatatypeProperty ;
	rdfs:label "subjectDirectoryAttributes"@en ;
	rdfs:range xsd:string ;
	.

observable:subjectHash
	a owl:ObjectProperty ;
	rdfs:label "subjectHash"@en ;
	rdfs:comment "A hash calculated on the certificate subject name."@en ;
	rdfs:range <https://unifiedcyberontology.org/ontology/uco/types#Hash> ;
	.

observable:subjectKeyIdentifier
	a owl:DatatypeProperty ;
	rdfs:label "subjectKeyIdentifier"@en ;
	rdfs:range xsd:string ;
	.

observable:subjectPublicKeyAlgorithm
	a owl:DatatypeProperty ;
	rdfs:label "subjectPublicKeyAlgorithm"@en ;
	rdfs:range xsd:string ;
	.

observable:subjectPublicKeyExponent
	a owl:DatatypeProperty ;
	rdfs:label "subjectPublicKeyExponent"@en ;
	rdfs:range xsd:integer ;
	.

observable:subjectPublicKeyModulus
	a owl:DatatypeProperty ;
	rdfs:label "subjectPublicKeyModulus"@en ;
	rdfs:range xsd:string ;
	.

observable:subsystem
	a owl:DatatypeProperty ;
	rdfs:label "subsystem"@en ;
	rdfs:comment "Specifies the subsystem (e.g., GUI, device driver, etc.) that is required to run this image."@en ;
	rdfs:range xsd:unsignedShort ;
	.

observable:swid
	a owl:DatatypeProperty ;
	rdfs:label "swid"@en ;
	rdfs:comment "Specifies the SWID tag for the software."@en ;
	rdfs:range xsd:string ;
	.

observable:symbolicName
	a owl:DatatypeProperty ;
	rdfs:label "symbolicName"@en ;
	rdfs:comment "The symbolic name of a global flag. See also: http://msdn.microsoft.com/en-us/library/windows/hardware/ff549646(v=vs.85).aspx."@en ;
	rdfs:range xsd:string ;
	.

observable:systemTime
	a owl:DatatypeProperty ;
	rdfs:label "systemTime"@en ;
	rdfs:range xsd:dateTime ;
	.

observable:tableName
	a owl:DatatypeProperty ;
	rdfs:label "tableName"@en ;
	rdfs:range xsd:string ;
	.

observable:targetFile
	a owl:ObjectProperty ;
	rdfs:label "targetFile"@en ;
	rdfs:comment "Specifies the file targeted by a symbolic link."@en ;
	rdfs:range observable:ObservableObject ;
	.

observable:taskComment
	a owl:DatatypeProperty ;
	rdfs:label "taskComment"@en ;
	rdfs:comment "Specifies a comment for the scheduled task. See also: http://msdn.microsoft.com/en-us/library/windows/desktop/aa381232(v=vs.85).aspx."@en ;
	rdfs:range xsd:string ;
	.

observable:taskCreator
	a owl:DatatypeProperty ;
	rdfs:label "taskCreator"@en ;
	rdfs:comment "Specifies the name of the creator of the scheduled task. See also: http://msdn.microsoft.com/en-us/library/windows/desktop/aa381235(v=vs.85).aspx."@en ;
	rdfs:range xsd:string ;
	.

observable:text
	a owl:DatatypeProperty ;
	rdfs:label "text"@en ;
	rdfs:range xsd:string ;
	.

observable:threadID
	a owl:DatatypeProperty ;
	rdfs:label "threadID"@en ;
	rdfs:range xsd:nonNegativeInteger ;
	.

observable:thumbprintHash
	a owl:ObjectProperty ;
	rdfs:label "thumbprintHash"@en ;
	rdfs:comment "A hash calculated on the entire certificate including signature."@en ;
	rdfs:range <https://unifiedcyberontology.org/ontology/uco/types#Hash> ;
	.

observable:timeDateStamp
	a owl:DatatypeProperty ;
	rdfs:label "timeDateStamp"@en ;
	rdfs:comment "Specifies the time when the PE binary was created."@en ;
	rdfs:range xsd:dateTime ;
	.

observable:timesExecuted
	a owl:DatatypeProperty ;
	rdfs:label "timesExecuted"@en ;
	rdfs:comment "The number of times the prefetch application has executed."@en ;
	rdfs:range xsd:integer ;
	.

observable:timezoneDST
	a owl:DatatypeProperty ;
	rdfs:label "timezoneDST"@en ;
	rdfs:comment "Specifies the time zone used by the system, taking daylight savings time (DST) into account."@en ;
	rdfs:range xsd:string ;
	.

observable:timezoneStandard
	a owl:DatatypeProperty ;
	rdfs:label "timezoneStandard"@en ;
	rdfs:comment "Specifies the time zone used by the system, without taking daylight savings time (DST) into account."@en ;
	rdfs:range xsd:string ;
	.

observable:to
	a owl:ObjectProperty ;
	rdfs:label "to"@en ;
	rdfs:comment "The receiver's phone number."@en ;
	rdfs:range observable:ObservableObject ;
	.

observable:totalFragments
	a owl:DatatypeProperty ;
	rdfs:label "totalFragments"@en ;
	rdfs:range xsd:integer ;
	.

observable:totalRam
	a owl:DatatypeProperty ;
	rdfs:label "totalRam"@en ;
	rdfs:comment "Specifies the total amount of physical memory present on the system, in bytes."@en ;
	rdfs:range xsd:integer ;
	.

observable:totalSpace
	a owl:DatatypeProperty ;
	rdfs:label "totalSpace"@en ;
	rdfs:comment "Specifies the total amount of space available on the partition, in bytes."@en ;
	rdfs:range xsd:integer ;
	.

observable:triggerBeginTime
	a owl:DatatypeProperty ;
	rdfs:label "triggerBeginTime"@en ;
	rdfs:comment "Specifies the date/time that the trigger is activated."@en ;
	rdfs:range xsd:dateTime ;
	.

observable:triggerDelay
	a owl:DatatypeProperty ;
	rdfs:label "triggerDelay"@en ;
	rdfs:comment "Specifies the delay that takes place between when the task is registered and when the task is started."@en ;
	rdfs:range xsd:string ;
	.

observable:triggerEndTime
	a owl:DatatypeProperty ;
	rdfs:label "triggerEndTime"@en ;
	rdfs:comment "Specifies the date/time that the trigger is deactivated."@en ;
	rdfs:range xsd:dateTime ;
	.

observable:triggerFrequency
	a owl:DatatypeProperty ;
	rdfs:label "triggerFrequency"@en ;
	rdfs:comment "Specifies the frequency at which the trigger repeats."@en ;
	rdfs:range vocabulary:TriggerFrequencyVocab ;
	.

observable:triggerList
	a owl:ObjectProperty ;
	rdfs:label "triggerList"@en ;
	rdfs:comment "Specifies a set of triggers used by the scheduled task. See also: http://msdn.microsoft.com/en-us/library/windows/desktop/aa383264(v=vs.85).aspx."@en ;
	rdfs:range observable:TriggerType ;
	.

observable:triggerMaxRunTime
	a owl:DatatypeProperty ;
	rdfs:label "triggerMaxRunTime"@en ;
	rdfs:comment "The maximum amount of time that the task launched by the trigger is allowed to run. See also: http://msdn.microsoft.com/en-us/library/windows/desktop/aa383868(v=vs.85).aspx."@en ;
	rdfs:range xsd:string ;
	.

observable:triggerSessionChangeType
	a owl:DatatypeProperty ;
	rdfs:label "triggerSessionChangeType"@en ;
	rdfs:comment "Specifies the type of Terminal Server session change that would trigger a task launch. See also: http://msdn.microsoft.com/en-us/library/windows/desktop/aa381298(v=vs.85).aspx."@en ;
	rdfs:range xsd:string ;
	.

observable:triggerType
	a owl:DatatypeProperty ;
	rdfs:label "triggerType"@en ;
	rdfs:comment "Specifies the type of the task trigger."@en ;
	rdfs:range vocabulary:TriggerTypeVocab ;
	.

observable:twitterHandle
	a owl:DatatypeProperty ;
	rdfs:label "Twitter Handle"@en-US ;
	rdfs:comment "Specifies the twitter handle associated with the profile."@en-US ;
	rdfs:range xsd:string ;
	.

observable:twitterId
	a owl:DatatypeProperty ;
	rdfs:label "Twitter ID"@en-US ;
	rdfs:comment "Specifies the twitter id associated with the profile."@en-US ;
	rdfs:range xsd:string ;
	.

observable:updatedDate
	a owl:DatatypeProperty ;
	rdfs:label "updatedDate"@en ;
	rdfs:comment "Specifies the date in which the registered domain information was last updated."@en ;
	rdfs:range xsd:dateTime ;
	.

observable:uptime
	a owl:DatatypeProperty ;
	rdfs:label "uptime"@en ;
	rdfs:comment "Specifies the duration that represents the current amount of time that the system has been up."@en ;
	rdfs:range xsd:string ;
	.

observable:url
	a owl:ObjectProperty ;
	rdfs:label "url"@en ;
	rdfs:comment "Specifies a URL associated with a particular observable object or facet."@en ;
	rdfs:range observable:ObservableObject ;
	.

observable:urlHistoryEntry
	a owl:ObjectProperty ;
	rdfs:label "URL History Entries"@en ;
	rdfs:comment "Specifies a URL history record stored in the browser's history."@en ;
	rdfs:range observable:URLHistoryEntry ;
	.

observable:urlTargeted
	a owl:DatatypeProperty ;
	rdfs:label "urlTargeted"@en ;
	rdfs:comment "The target of the bookmark."@en ;
	rdfs:range xsd:anyURI ;
	.

observable:urlTransitionType
	a owl:DatatypeProperty ;
	rdfs:label "Transition Type"@en ;
	rdfs:comment "Specifies how a browser navigated to a particular URL on a particular visit."@en ;
	rdfs:range [
		a rdfs:Datatype ;
		owl:unionOf (
			xsd:string
			vocabulary:URLTransitionTypeVocab
		) ;
	] ;
	.

observable:userLocationString
	a owl:DatatypeProperty ;
	rdfs:label "User Location String"@en-US ;
	rdfs:comment "Specifies the user-provided location string associated with the profile."@en-US ;
	rdfs:range xsd:string ;
	.

observable:userName
	a owl:ObjectProperty ;
	rdfs:label "userName"@en ;
	rdfs:comment "Username used to authenticate to this resource."@en ;
	rdfs:range observable:ObservableObject ;
	.

observable:validityNotAfter
	a owl:DatatypeProperty ;
	rdfs:label "validityNotAfter"@en ;
	rdfs:range xsd:dateTime ;
	.

observable:validityNotBefore
	a owl:DatatypeProperty ;
	rdfs:label "validityNotBefore"@en ;
	rdfs:range xsd:dateTime ;
	.

observable:value
	a owl:DatatypeProperty ;
	rdfs:label "value"@en ;
	rdfs:range xsd:string ;
	.

observable:values
	a owl:DatatypeProperty ;
	rdfs:label "values"@en ;
	rdfs:comment "The values that were enumerated as a result of the action on the object."@en ;
	rdfs:range xsd:string ;
	.

observable:version
	a owl:DatatypeProperty ;
	rdfs:label "version"@en ;
	rdfs:range xsd:string ;
	.

observable:visibility
	a owl:DatatypeProperty ;
	rdfs:label "visibility"@en ;
	rdfs:range xsd:boolean ;
	.

observable:visitCount
	a owl:DatatypeProperty ;
	rdfs:label "visitCount"@en ;
	rdfs:comment "Specifies the number of times a URL has been visited by a particular web browser."@en ;
	rdfs:range xsd:integer ;
	.

observable:visitDuration
	a owl:DatatypeProperty ;
	rdfs:label "Visit Duration"@en ;
	rdfs:comment "Specifies the duration of a specific visit of a URL within a particular browser."@en ;
	rdfs:range xsd:duration ;
	.

observable:visitTime
	a owl:DatatypeProperty ;
	rdfs:label "Visit Time"@en ;
	rdfs:comment "Specifies the date/time of a specific visit of a URL within a particular browser."@en ;
	rdfs:range xsd:dateTime ;
	.

observable:volume
	a owl:ObjectProperty ;
	rdfs:label "volume"@en ;
	rdfs:comment "The volume from which the prefetch application was run. If the applicatin was run from multiple volumes, there will be a separate prefetch file for each."@en ;
	rdfs:range observable:ObservableObject ;
	.

observable:volumeID
	a owl:DatatypeProperty ;
	rdfs:label "volumeID"@en ;
	rdfs:comment "The unique identifier of the volume."@en ;
	rdfs:range xsd:string ;
	.

observable:whoisContactType
	a owl:DatatypeProperty ;
	rdfs:label "whoisContactType"@en ;
	rdfs:comment "Specifies what type of WHOIS contact this is."@en ;
	rdfs:range [
		a rdfs:Datatype ;
		owl:unionOf (
			xsd:string
			vocabulary:WhoisContactTypeVocab
		) ;
	] ;
	.

observable:whoisServer
	a owl:ObjectProperty ;
	rdfs:label "whoisServer"@en ;
	rdfs:comment "Specifies the corresponding whois server for a registrar."@en ;
	rdfs:range observable:ObservableObject ;
	.

observable:win32VersionValue
	a owl:DatatypeProperty ;
	rdfs:label "win32VersionValue"@en ;
	rdfs:comment "Specifies the reserved win32 version value."@en ;
	rdfs:range xsd:unsignedInt ;
	.

observable:windowTitle
	a owl:DatatypeProperty ;
	rdfs:label "windowTitle"@en ;
	rdfs:range xsd:string ;
	.

observable:windowsDirectory
	a owl:ObjectProperty ;
	rdfs:label "windowsDirectory"@en ;
	rdfs:comment "The Windows_Directory field specifies the fully-qualified path to the Windows install directory."@en ;
	rdfs:range observable:ObservableObject ;
	.

observable:windowsSystemDirectory
	a owl:ObjectProperty ;
	rdfs:label "windowsSystemDirectory"@en ;
	rdfs:comment "The Windows_System_Directory field specifies the fully-qualified path to the Windows system directory."@en ;
	rdfs:range observable:ObservableObject ;
	.

observable:windowsTempDirectory
	a owl:ObjectProperty ;
	rdfs:label "windowsTempDirectory"@en ;
	rdfs:comment "The Windows_Temp_Directory field specifies the fully-qualified path to the Windows temporary files directory."@en ;
	rdfs:range observable:ObservableObject ;
	.

observable:windowsVolumeAttributes
	a owl:DatatypeProperty ;
	rdfs:label "windowsVolumeAttributes"@en ;
	rdfs:comment "Specifies the attributes of a windows volume."@en ;
	rdfs:range vocabulary:WindowsVolumeAttributeVocab ;
	.

observable:workItemData
	a owl:ObjectProperty ;
	rdfs:label "workItemData"@en ;
	rdfs:comment "Specifies application defined data associated with the scheduled task. See also: http://msdn.microsoft.com/en-us/library/windows/desktop/aa381271(v=vs.85).aspx."@en ;
	rdfs:range observable:ObservableObject ;
	.

observable:workingDirectory
	a owl:ObjectProperty ;
	rdfs:label "workingDirectory"@en ;
	rdfs:comment "Specifies the working directory for the scheduled task. See also: http://msdn.microsoft.com/en-us/library/windows/desktop/aa381878(v=vs.85).aspx."@en ;
	rdfs:range observable:ObservableObject ;
	.

observable:x509v3extensions
	a owl:ObjectProperty ;
	rdfs:label "x509V3Extensions"@en ;
	rdfs:range observable:X509V3ExtensionsFacet ;
	.

observable:xMailer
	a owl:DatatypeProperty ;
	rdfs:label "xMailer"@en ;
	rdfs:range xsd:string ;
	.

observable:xOriginatingIP
	a owl:ObjectProperty ;
	rdfs:label "xOriginatingIP"@en ;
	rdfs:range observable:ObservableObject ;
	.

